@prefix : <http://w3id.org/arto#> .
@prefix cc: <http://creativecommons.org/ns#> .
@prefix dc: <http://purl.org/dc/terms/> .
@prefix gn: <https://www.geonames.org/ontology#> .
@prefix aat: <http://vocab.getty.edu/aat/> .
@prefix crm: <http://www.cidoc-crm.org/cidoc-crm/> .
@prefix dbp: <https://dbpedia.org/property/> .
@prefix edm: <http://www.europeana.eu/schemas/edm/> .
@prefix geo: <http://www.opengis.net/ont/geosparql#> .
@prefix owl: <http://www.w3.org/2002/07/owl#> .
@prefix rdf: <http://www.w3.org/1999/02/22-rdf-syntax-ns#> .
@prefix sdo: <https://schema.org/> .
@prefix xml: <http://www.w3.org/XML/1998/namespace> .
@prefix xsd: <http://www.w3.org/2001/XMLSchema#> .
@prefix arto: <http://w3id.org/arto#> .
@prefix foaf: <http://xmlns.com/foaf/spec/> .
@prefix icon: <https://w3id.org/icon/ontology/> .
@prefix qudt: <http://qudt.org/schema/qudt/> .
@prefix rdfs: <http://www.w3.org/2000/01/rdf-schema#> .
@prefix skos: <http://www.w3.org/2004/02/skos/core#> .
@prefix vann: <http://purl.org/vocab/vann/> .
@prefix event: <https://w3id.org/MON/event.owl#> .
@prefix mfoem: <http://purl.obolibrary.org/obo/> .
@prefix ebucore: <http://www.ebu.ch/metadata/ontologies/ebucore/ebucore#> .
@base <http://w3id.org/arto#> .

<http://purl.org/dc/terms/> rdf:type owl:Ontology ;
                             owl:imports crm: ,
                                         <http://www.w3.org/2004/02/skos/core> ,
                                         <http://xmlns.com/foaf/0.1/> ,
                                         sdo: ;
                             cc:attributionURL <http://w3id.org/arto> ;
                             dc:description "The Artwork Object Ontology (ARTO) is a comprehensive ontology designed for describing and contextualising artworks. It consists of two main components: the Artwork Descriptive Model and the Artwork Contextual Model. ARTO aims to provide a structured and detailed representation of artworks, facilitating tasks such as artwork captioning and information retrieval."@en ;
                             dc:issued "2024-04-10" ;
                             dc:license <https://github.com/SocialMachineLab/ArtworkOntology/blob/main/License> ;
                             dc:modified "2025-08-05" ;
                             dc:title "Artwork Object Ontology"@en ;
                             vann:preferredNamespacePrefix "arto" ;
                             rdfs:label "Artwork Object Ontology (ARTO)"@en ;
                             owl:versionInfo "0.2" .

#################################################################
#    Annotation properties
#################################################################

###  http://creativecommons.org/ns#attributionURL
cc:attributionURL rdf:type owl:AnnotationProperty .


###  http://purl.org/dc/dcam/domainIncludes
<http://purl.org/dc/dcam/domainIncludes> rdf:type owl:AnnotationProperty .


###  http://purl.org/dc/dcam/rangeIncludes
<http://purl.org/dc/dcam/rangeIncludes> rdf:type owl:AnnotationProperty .


###  http://purl.org/dc/elements/1.1/contributor
<http://purl.org/dc/elements/1.1/contributor> rdf:type owl:AnnotationProperty .


###  http://purl.org/dc/elements/1.1/coverage
<http://purl.org/dc/elements/1.1/coverage> rdf:type owl:AnnotationProperty .


###  http://purl.org/dc/elements/1.1/creator
<http://purl.org/dc/elements/1.1/creator> rdf:type owl:AnnotationProperty .


###  http://purl.org/dc/elements/1.1/format
<http://purl.org/dc/elements/1.1/format> rdf:type owl:AnnotationProperty .


###  http://purl.org/dc/elements/1.1/identifier
<http://purl.org/dc/elements/1.1/identifier> rdf:type owl:AnnotationProperty .


###  http://purl.org/dc/elements/1.1/language
<http://purl.org/dc/elements/1.1/language> rdf:type owl:AnnotationProperty .


###  http://purl.org/dc/elements/1.1/publisher
<http://purl.org/dc/elements/1.1/publisher> rdf:type owl:AnnotationProperty .


###  http://purl.org/dc/elements/1.1/relation
<http://purl.org/dc/elements/1.1/relation> rdf:type owl:AnnotationProperty .


###  http://purl.org/dc/elements/1.1/rights
<http://purl.org/dc/elements/1.1/rights> rdf:type owl:AnnotationProperty .


###  http://purl.org/dc/elements/1.1/source
<http://purl.org/dc/elements/1.1/source> rdf:type owl:AnnotationProperty .


###  http://purl.org/dc/elements/1.1/subject
<http://purl.org/dc/elements/1.1/subject> rdf:type owl:AnnotationProperty .


###  http://purl.org/dc/elements/1.1/type
<http://purl.org/dc/elements/1.1/type> rdf:type owl:AnnotationProperty .


###  http://purl.org/dc/terms/abstract
dc:abstract rdf:type owl:AnnotationProperty ;
            rdfs:subPropertyOf <http://purl.org/dc/elements/1.1/description> ,
                               dc:description .


###  http://purl.org/dc/terms/accessRights
dc:accessRights rdf:type owl:AnnotationProperty ;
                rdfs:subPropertyOf <http://purl.org/dc/elements/1.1/rights> ,
                                   dc:rights .


###  http://purl.org/dc/terms/accrualMethod
dc:accrualMethod rdf:type owl:AnnotationProperty ;
                 rdfs:domain <http://purl.org/dc/dcmitype/Collection> .


###  http://purl.org/dc/terms/accrualPeriodicity
dc:accrualPeriodicity rdf:type owl:AnnotationProperty ;
                      rdfs:domain <http://purl.org/dc/dcmitype/Collection> .


###  http://purl.org/dc/terms/accrualPolicy
dc:accrualPolicy rdf:type owl:AnnotationProperty ;
                 rdfs:domain <http://purl.org/dc/dcmitype/Collection> .


###  http://purl.org/dc/terms/alternative
dc:alternative rdf:type owl:AnnotationProperty ;
               rdfs:subPropertyOf <http://purl.org/dc/elements/1.1/title> .


###  http://purl.org/dc/terms/audience
dc:audience rdf:type owl:AnnotationProperty .


###  http://purl.org/dc/terms/available
dc:available rdf:type owl:AnnotationProperty ;
             rdfs:subPropertyOf <http://purl.org/dc/elements/1.1/date> ;
             rdfs:range rdfs:Literal .


###  http://purl.org/dc/terms/bibliographicCitation
dc:bibliographicCitation rdf:type owl:AnnotationProperty ;
                         rdfs:subPropertyOf <http://purl.org/dc/elements/1.1/identifier> ;
                         rdfs:range rdfs:Literal .


###  http://purl.org/dc/terms/conformsTo
dc:conformsTo rdf:type owl:AnnotationProperty ;
              rdfs:subPropertyOf <http://purl.org/dc/elements/1.1/relation> ,
                                 dc:relation .


###  http://purl.org/dc/terms/contributor
dc:contributor rdfs:subPropertyOf <http://purl.org/dc/elements/1.1/contributor> .


###  http://purl.org/dc/terms/coverage
dc:coverage rdf:type owl:AnnotationProperty ;
            rdfs:subPropertyOf <http://purl.org/dc/elements/1.1/coverage> .


###  http://purl.org/dc/terms/created
dc:created rdf:type owl:AnnotationProperty ;
           rdfs:subPropertyOf <http://purl.org/dc/elements/1.1/date> ;
           rdfs:range rdfs:Literal .


###  http://purl.org/dc/terms/creator
dc:creator rdfs:subPropertyOf <http://purl.org/dc/elements/1.1/creator> ,
                              dc:contributor .


###  http://purl.org/dc/terms/date
dc:date rdf:type owl:AnnotationProperty ;
        rdfs:subPropertyOf <http://purl.org/dc/elements/1.1/date> ;
        rdfs:range rdfs:Literal .


###  http://purl.org/dc/terms/dateAccepted
dc:dateAccepted rdf:type owl:AnnotationProperty ;
                rdfs:subPropertyOf <http://purl.org/dc/elements/1.1/date> ;
                rdfs:range rdfs:Literal .


###  http://purl.org/dc/terms/dateCopyrighted
dc:dateCopyrighted rdf:type owl:AnnotationProperty ;
                   rdfs:subPropertyOf <http://purl.org/dc/elements/1.1/date> ;
                   rdfs:range rdfs:Literal .


###  http://purl.org/dc/terms/dateSubmitted
dc:dateSubmitted rdf:type owl:AnnotationProperty ;
                 rdfs:subPropertyOf <http://purl.org/dc/elements/1.1/date> ;
                 rdfs:range rdfs:Literal .


###  http://purl.org/dc/terms/description
dc:description rdfs:subPropertyOf <http://purl.org/dc/elements/1.1/description> .


###  http://purl.org/dc/terms/educationLevel
dc:educationLevel rdf:type owl:AnnotationProperty ;
                  rdfs:subPropertyOf dc:audience .


###  http://purl.org/dc/terms/extent
dc:extent rdf:type owl:AnnotationProperty ;
          rdfs:subPropertyOf <http://purl.org/dc/elements/1.1/format> ,
                             dc:format .


###  http://purl.org/dc/terms/format
dc:format rdf:type owl:AnnotationProperty ;
          rdfs:subPropertyOf <http://purl.org/dc/elements/1.1/format> .


###  http://purl.org/dc/terms/hasFormat
dc:hasFormat rdf:type owl:AnnotationProperty ;
             rdfs:subPropertyOf <http://purl.org/dc/elements/1.1/relation> ,
                                dc:relation .


###  http://purl.org/dc/terms/hasPart
dc:hasPart rdf:type owl:AnnotationProperty ;
           rdfs:subPropertyOf <http://purl.org/dc/elements/1.1/relation> ,
                              dc:relation .


###  http://purl.org/dc/terms/hasVersion
dc:hasVersion rdf:type owl:AnnotationProperty ;
              rdfs:subPropertyOf <http://purl.org/dc/elements/1.1/relation> ,
                                 dc:relation .


###  http://purl.org/dc/terms/identifier
dc:identifier rdf:type owl:AnnotationProperty ;
              rdfs:subPropertyOf <http://purl.org/dc/elements/1.1/identifier> ;
              rdfs:range rdfs:Literal .


###  http://purl.org/dc/terms/isFormatOf
dc:isFormatOf rdf:type owl:AnnotationProperty ;
              rdfs:subPropertyOf <http://purl.org/dc/elements/1.1/relation> ,
                                 dc:relation .


###  http://purl.org/dc/terms/isPartOf
dc:isPartOf rdf:type owl:AnnotationProperty ;
            rdfs:subPropertyOf <http://purl.org/dc/elements/1.1/relation> ,
                               dc:relation .


###  http://purl.org/dc/terms/isReferencedBy
dc:isReferencedBy rdf:type owl:AnnotationProperty ;
                  rdfs:subPropertyOf <http://purl.org/dc/elements/1.1/relation> ,
                                     dc:relation .


###  http://purl.org/dc/terms/isReplacedBy
dc:isReplacedBy rdf:type owl:AnnotationProperty ;
                rdfs:subPropertyOf <http://purl.org/dc/elements/1.1/relation> ,
                                   dc:relation .


###  http://purl.org/dc/terms/isRequiredBy
dc:isRequiredBy rdf:type owl:AnnotationProperty ;
                rdfs:subPropertyOf <http://purl.org/dc/elements/1.1/relation> ,
                                   dc:relation .


###  http://purl.org/dc/terms/isVersionOf
dc:isVersionOf rdf:type owl:AnnotationProperty ;
               rdfs:subPropertyOf <http://purl.org/dc/elements/1.1/relation> ,
                                  dc:relation .


###  http://purl.org/dc/terms/issued
dc:issued rdf:type owl:AnnotationProperty ;
          rdfs:subPropertyOf <http://purl.org/dc/elements/1.1/date> ;
          rdfs:range rdfs:Literal .


###  http://purl.org/dc/terms/language
dc:language rdf:type owl:AnnotationProperty ;
            rdfs:subPropertyOf <http://purl.org/dc/elements/1.1/language> .


###  http://purl.org/dc/terms/license
dc:license rdf:type owl:AnnotationProperty ;
           rdfs:subPropertyOf <http://purl.org/dc/elements/1.1/rights> ,
                              dc:rights .


###  http://purl.org/dc/terms/mediator
dc:mediator rdf:type owl:AnnotationProperty ;
            rdfs:subPropertyOf dc:audience .


###  http://purl.org/dc/terms/medium
dc:medium rdf:type owl:AnnotationProperty ;
          rdfs:subPropertyOf <http://purl.org/dc/elements/1.1/format> ,
                             dc:format .


###  http://purl.org/dc/terms/modified
dc:modified rdf:type owl:AnnotationProperty ;
            rdfs:subPropertyOf <http://purl.org/dc/elements/1.1/date> ;
            rdfs:range rdfs:Literal .


###  http://purl.org/dc/terms/publisher
dc:publisher rdf:type owl:AnnotationProperty ;
             rdfs:subPropertyOf <http://purl.org/dc/elements/1.1/publisher> .


###  http://purl.org/dc/terms/references
dc:references rdf:type owl:AnnotationProperty ;
              rdfs:subPropertyOf <http://purl.org/dc/elements/1.1/relation> ,
                                 dc:relation .


###  http://purl.org/dc/terms/relation
dc:relation rdf:type owl:AnnotationProperty ;
            rdfs:subPropertyOf <http://purl.org/dc/elements/1.1/relation> .


###  http://purl.org/dc/terms/replaces
dc:replaces rdf:type owl:AnnotationProperty ;
            rdfs:subPropertyOf <http://purl.org/dc/elements/1.1/relation> ,
                               dc:relation .


###  http://purl.org/dc/terms/requires
dc:requires rdf:type owl:AnnotationProperty ;
            rdfs:subPropertyOf <http://purl.org/dc/elements/1.1/relation> ,
                               dc:relation .


###  http://purl.org/dc/terms/rights
dc:rights rdf:type owl:AnnotationProperty ;
          rdfs:subPropertyOf <http://purl.org/dc/elements/1.1/rights> .


###  http://purl.org/dc/terms/source
dc:source rdf:type owl:AnnotationProperty ;
          rdfs:subPropertyOf <http://purl.org/dc/elements/1.1/source> ,
                             dc:relation .


###  http://purl.org/dc/terms/spatial
dc:spatial rdf:type owl:AnnotationProperty ;
           rdfs:subPropertyOf <http://purl.org/dc/elements/1.1/coverage> ,
                              dc:coverage .


###  http://purl.org/dc/terms/subject
dc:subject rdf:type owl:AnnotationProperty ;
           rdfs:subPropertyOf <http://purl.org/dc/elements/1.1/subject> .


###  http://purl.org/dc/terms/tableOfContents
dc:tableOfContents rdf:type owl:AnnotationProperty ;
                   rdfs:subPropertyOf <http://purl.org/dc/elements/1.1/description> ,
                                      dc:description .


###  http://purl.org/dc/terms/temporal
dc:temporal rdf:type owl:AnnotationProperty ;
            rdfs:subPropertyOf <http://purl.org/dc/elements/1.1/coverage> ,
                               dc:coverage .


###  http://purl.org/dc/terms/title
dc:title rdf:type owl:AnnotationProperty ;
         rdfs:subPropertyOf <http://purl.org/dc/elements/1.1/title> ;
         rdfs:range rdfs:Literal .


###  http://purl.org/dc/terms/type
dc:type rdf:type owl:AnnotationProperty ;
        rdfs:subPropertyOf <http://purl.org/dc/elements/1.1/type> .


###  http://purl.org/dc/terms/valid
dc:valid rdf:type owl:AnnotationProperty ;
         rdfs:subPropertyOf <http://purl.org/dc/elements/1.1/date> ;
         rdfs:range rdfs:Literal .


###  http://purl.org/vocab/vann/preferredNamespacePrefix
vann:preferredNamespacePrefix rdf:type owl:AnnotationProperty .


###  http://www.w3.org/2002/07/owl#cardinality
owl:cardinality rdf:type owl:AnnotationProperty .


###  http://www.w3.org/2002/07/owl#maxCardinality
owl:maxCardinality rdf:type owl:AnnotationProperty .


###  http://www.w3.org/2002/07/owl#maxQualifiedCardinality
owl:maxQualifiedCardinality rdf:type owl:AnnotationProperty .


###  http://www.w3.org/2002/07/owl#minCardinality
owl:minCardinality rdf:type owl:AnnotationProperty .


###  http://www.w3.org/2002/07/owl#qualifiedCardinality
owl:qualifiedCardinality rdf:type owl:AnnotationProperty .


#################################################################
#    Datatypes
#################################################################

###  http://purl.org/dc/terms/Box
dc:Box rdf:type rdfs:Datatype .


###  http://purl.org/dc/terms/ISO3166
dc:ISO3166 rdf:type rdfs:Datatype .


###  http://purl.org/dc/terms/ISO639-2
dc:ISO639-2 rdf:type rdfs:Datatype .


###  http://purl.org/dc/terms/ISO639-3
dc:ISO639-3 rdf:type rdfs:Datatype .


###  http://purl.org/dc/terms/Period
dc:Period rdf:type rdfs:Datatype .


###  http://purl.org/dc/terms/Point
dc:Point rdf:type rdfs:Datatype .


###  http://purl.org/dc/terms/RFC1766
dc:RFC1766 rdf:type rdfs:Datatype .


###  http://purl.org/dc/terms/RFC3066
dc:RFC3066 rdf:type rdfs:Datatype .


###  http://purl.org/dc/terms/RFC4646
dc:RFC4646 rdf:type rdfs:Datatype .


###  http://purl.org/dc/terms/RFC5646
dc:RFC5646 rdf:type rdfs:Datatype .


###  http://purl.org/dc/terms/URI
dc:URI rdf:type rdfs:Datatype .


###  http://purl.org/dc/terms/W3CDTF
dc:W3CDTF rdf:type rdfs:Datatype .


###  http://www.w3.org/2001/XMLSchema#date
xsd:date rdf:type rdfs:Datatype .


#################################################################
#    Object Properties
#################################################################

###  http://qudt.org/schema/qudt/vector
qudt:vector rdf:type owl:ObjectProperty .


###  http://w3id.org/arto#containsElement
arto:containsElement rdf:type owl:ObjectProperty ;
                     rdfs:domain [ rdf:type owl:Class ;
                                   owl:unionOf ( arto:Object
                                                 arto:Scene
                                               )
                                 ] ;
                     rdfs:range arto:VisualElement ;
                     rdfs:comment "Specifies the visual elements (such as colour, line, composition) contained within an object in the artwork." ;
                     rdfs:label "containsElement" ;
                     skos:example """
                      - colour elements: :sky_object arto:containsElement :blue_gradient_colour
                      - Line elements: :mountain_object arto:containsElement :diagonal_line
                      - Compositional elements: :tree_object arto:containsElement :vertical_composition""" .


###  http://w3id.org/arto#containsObject
arto:containsObject rdf:type owl:ObjectProperty ;
                    owl:inverseOf arto:isObjectOf ;
                    rdfs:domain arto:Scene ;
                    rdfs:range arto:Object ;
                    rdfs:comment "Indicates specific objects that are present within a scene of an artwork." ;
                    rdfs:label "containsObject" ;
                    skos:example """
                      - Landscape scene: :garden_scene arto:containsObject :fountain, :bench, :flowers
                      - Portrait scene: :interior_scene arto:containsObject :chair, :table, :book
                      - Still life scene: :table_scene arto:containsObject :fruit_bowl, :wine_glass, :cloth""" .


###  http://w3id.org/arto#containsScene
arto:containsScene rdf:type owl:ObjectProperty ;
                   owl:inverseOf arto:isSceneOf ;
                   rdfs:domain [ rdf:type owl:Class ;
                                 owl:unionOf ( arto:Artwork
                                               arto:Scene
                                             )
                               ] ;
                   rdfs:range arto:Scene ;
                   rdfs:comment "Identifies distinct scenes within an artwork or within another scene, allowing for hierarchical scene composition." ;
                   rdfs:label "containsScene" ;
                   skos:example """
                      - Nested scenes: :market_scene arto:containsScene :vendor_scene, :customer_scene
                      - Background scenes: :landscape_painting arto:containsScene :mountain_scene, :valley_scene""" .


###  http://w3id.org/arto#currentLocation
arto:currentLocation rdf:type owl:ObjectProperty ;
                     rdfs:subPropertyOf edm:currentLocation ;
                     rdfs:domain arto:Artwork ;
                     rdfs:range arto:Location ;
                     rdfs:comment "Specifies the present physical location where an artwork is housed, displayed, or stored. This property extends EDM's currentLocation with art-specific constraints ensuring single location assignment while supporting location change tracking. Essential for provenance research, exhibition planning, and artwork accessibility, this property maintains connections to institutional and geographical data through the Location class." ;
                     rdfs:label "currentLocation" ;
                     owl:cardinality 1 ;
                     skos:example """
                      - Museum location: :mona_lisa arto:currentLocation :louvre_museum
                      - Gallery location: :starry_night arto:currentLocation :moma_gallery_room_24
                      """ .


###  http://w3id.org/arto#expresses
arto:expresses rdf:type owl:ObjectProperty ;
               rdfs:domain arto:Emotion ;
               rdfs:range mfoem:MFOEM_000001 ;
               rdfs:comment "Relates arto:Emotion to a specific emotion concept defined in the Mental Functioning Ontology Emotion Module (MFOEM). This property is used to link local emotion representations to controlled vocabulary terms (e.g., joy, sadness, anger, fear) from MFOEM, ensuring consistent and interoperable emotion classification across datasets. In the context of artworks, this enables precise and standardised description of emotions expressed within artistic content." ;
               rdfs:label "expresses" ;
               skos:example """
              - :joy_emotion arto:expresses mfoem:MFOEM_000034 ; 
              - :sadness_emotion arto:expresses mfoem:MFOEM_000056 ; 
              - :anger_emotion arto:expresses mfoem:MFOEM_000009 ; 
              - :fear_emotion arto:expresses mfoem:MFOEM_000026 ; 
              """ .


###  http://w3id.org/arto#genre
arto:genre rdf:type owl:ObjectProperty ;
           rdfs:domain arto:Artwork ;
           rdfs:range arto:GenreType ;
           rdfs:comment "Genre classification is fundamental to art analysis, which connects artworks to established genre categories from Getty AAT vocabulary while supporting custom genre definitions." ;
           rdfs:label "genre" ;
           skos:example """
               - Traditional genres: :mona_lisa arto:genre aat:portrait_paintings
               - Landscape genre: :starry_night arto:genre aat:landscape_paintings  
               - Religious genre: :last_supper arto:genre aat:religious_paintings
               - Still life genre: :sunflowers arto:genre aat:still_life_paintings
               - Abstract genre: :composition_vii arto:genre aat:abstract_paintings
               """ .


###  http://w3id.org/arto#hasColourTerm
arto:hasColourTerm rdf:type owl:ObjectProperty ;
                   rdfs:domain arto:Colour ;
                   rdfs:range arto:ColourTerm ;
                   rdfs:comment "Links a colour to its corresponding standardised term from controlled vocabularies, establishing semantic connections that enable consistent colour identification, hierarchical classification, and cross-institutional interoperability for cultural heritage documentation and research." ;
                   skos:example """
                    :colour1 a arto:Colour ;
                      arto:hasColourTerm aat:red .

                    :colour2 a arto:Colour ;
                      arto:hasColourTerm aat:vermillion .

                    :colour3 a arto:Colour ;
                      arto:hasColourTerm aat:imperial_yellow .

                    """ ;
                   rdfs:label "hasColourTerm" .


###  http://w3id.org/arto#hasColourValue
arto:hasColourValue rdf:type owl:ObjectProperty ;
                    rdfs:domain arto:Colour ;
                    rdfs:range arto:ColourValue ;
                    rdfs:comment "Associates a colour with its value, allowing for flexible representation of colour information in artworks. This property supports different colour spaces for example RGB and HSV formats, enabling detailed colour analysis and representation." ;
                    skos:example """
                      - RGB value:
                        :c_vermilion a arto:Colour ;
                          arto:hasColourValue [
                            a arto:ColourValue ;
                            arto:colourSpace "RGB" ;
                            qudt:vector (227 66 52)      # R,G,B in 0–255
                          ] .

                      - HSV value:
                        :c_skyBlue a arto:Colour ;
                          arto:hasColourValue [
                            a arto:ColourValue ;
                            arto:colourSpace "HSV" ;
                            qudt:vector (197 0.76 1.00)  # H in degrees; S,V in 0–1
                          ] .

                      - CMYK value:
                        :c_cadmiumYellow a arto:Colour ;
                          arto:hasColourValue [
                            a arto:ColourValue ;
                            arto:colourSpace "CMYK" ;
                            qudt:vector (0.00 0.09 0.90 0.00)  # C,M,Y,K in 0–1
                          ] .

                      - CIE Lab value with white point:
                        :c_ultramarine a arto:Colour ;
                          arto:hasColourValue [
                            a arto:ColourValue ;
                            arto:colourSpace "Lab" ;
                            qudt:vector (32.4 14.8 -38.1) ;
                            arto:whitePoint arto:D65
                          ] .
                      """ ;
                    rdfs:label "hasColourValue" .


###  http://w3id.org/arto#hasConnotation
arto:hasConnotation rdf:type owl:ObjectProperty ;
                    owl:inverseOf arto:isConnotationOf ;
                    rdfs:domain [ rdf:type owl:Class ;
                                  owl:unionOf ( arto:Artwork
                                                arto:Object
                                                arto:Scene
                                                arto:VisualElement
                                              )
                                ] ;
                    rdfs:range arto:Connotation ;
                    rdfs:comment "Links visual elements, objects, scenes, or artworks to their symbolic meanings or emotional connotations.The relationship enables multiple interpretation levels while maintaining clear connections between visible elements and their cultural, symbolic, or emotional significance. Similar to ICON's recognizedConcept but with broader domain coverage." ;
                    rdfs:label "hasConnotation" ;
                    skos:example """
              - Emotional expression: :red_colour arto:hasConnotation :anger_emotion
              - Symbolic meaning: :dove_object arto:hasConnotation :peace_meaning
              - Scene mood: :storm_scene arto:hasConnotation :turbulence_emotion
              - Artwork meaning: :guernica arto:hasConnotation :anti_war_theme""" .


###  http://w3id.org/arto#hasCoordinates
arto:hasCoordinates rdf:type owl:ObjectProperty ;
                    rdfs:domain [ rdf:type owl:Class ;
                                  owl:unionOf ( arto:Object
                                                arto:Scene
                                              )
                                ] ;
                    rdfs:range qudt:Vector ;
                    rdfs:comment "Specifies the spatial location of objects and scenes within the artwork's coordinate system. This property supports spatial analysis, object relationship studies, compositional balance analysis, and digital humanities research requiring precise object localisation." ;
                    rdfs:label "hasCoordinates" ;
                    skos:example """
                        - Digital image coordinates: :main_figure arto:hasCoordinates qudt_Vector_250_300
                    qudt_Vector_250_300 rdf:type qudt:Vector ;
                        - 3D artwork coordinates: :sculpture_detail arto:hasCoordinates qudt_Vector_15_20_5
                    qudt_Vector_15_20_5 rdf:type qudt:Vector ;
                    """ .


###  http://w3id.org/arto#hasLocation
arto:hasLocation rdf:type owl:ObjectProperty ;
                 owl:inverseOf arto:isLocationOf ;
                 rdfs:domain [ rdf:type owl:Class ;
                               owl:unionOf ( arto:Agent
                                             arto:Event
                                           )
                             ] ;
                 rdfs:range arto:Location ;
                 rdfs:comment "Specifies the physical location of an agent or event related to the artwork." ;
                 rdfs:label "hasLocation" ;
                 skos:example """
                - Museum address: :metropolitan_museum arto:hasLocation :met_nyc_location
                - Gallery location: :tate_modern arto:hasLocation :london_bankside                 
                - Exhibition event: :venice_biennale_2024 arto:hasLocation :venice_giardini""" .


###  http://w3id.org/arto#hasMetric
arto:hasMetric rdf:type owl:ObjectProperty ;
               owl:inverseOf arto:isMetricOf ;
               rdfs:domain [ rdf:type owl:Class ;
                             owl:unionOf ( arto:Connotation
                                           arto:Object
                                           arto:Scene
                                           arto:VisualElement
                                         )
                           ] ;
               rdfs:range arto:Metric ;
               rdfs:comment "Associates artwork components with quantifiable measurements supporting computational analysis and comparative studies. This property enables integration of statistical colour analysis, compositional balance metrics, emotional intensity measures, and other quantitative assessments with qualitative art historical analysis. The relationship supports both automated artwork analysis and structured comparison studies while maintaining connection to interpretive content." ;
               rdfs:label "hasMetric" ;
               skos:example """
                - Colour metrics: :sky_area arto:hasMetric :blue_intensity_75_percent
                - Composition balance: :landscape_scene arto:hasMetric :symmetry_score_0.8
                - Emotional intensity: :expression_scene arto:hasMetric :fear_intensity_high""" .


###  http://w3id.org/arto#hasTime
arto:hasTime rdf:type owl:ObjectProperty ;
             owl:inverseOf arto:isTimeOf ;
             rdfs:domain arto:Event ;
             rdfs:range arto:Time ;
              rdfs:comment "Links an event to its temporal specification. The time entity may represent a specific date, a period (e.g., season, decade), or a cultural-historical era, allowing precise or approximate temporal anchoring of events." ;
             rdfs:label "hasTime" ;
             skos:example """
               # Specific date
               :exhibition2024 arto:hasTime :date_2024_05_12

               # Period/season
               :venice_biennale2022 arto:hasTime :summer2022

               # Historical era
               :napoleon_coronation arto:hasTime :early19thCentury
              """ .


###  http://w3id.org/arto#isConnotationOf
arto:isConnotationOf rdf:type owl:ObjectProperty ;
                     rdfs:domain arto:Connotation ;
                     rdfs:range [ rdf:type owl:Class ;
                                  owl:unionOf ( arto:Artwork
                                                arto:Object
                                                arto:Scene
                                                arto:VisualElement
                                              )
                                ] ;
                     rdfs:comment "Associates a connotation with the visual elements, objects, scenes or artwork that express it." ;
                     rdfs:label "isConnotationOf" ;
                     skos:example """
                    - Emotional expression: :anger_emotion arto:isConnotationOf :red_colour
                    - Symbolic meaning: :peace_meaning arto:isConnotationOf :dove_object
                    - Scene mood: :turbulence_emotion arto:isConnotationOf :storm_scene
                    - Artwork meaning: :anti_war_theme arto:isConnotationOf :guernica""" .


###  http://w3id.org/arto#isElementOf
arto:isElementOf rdf:type owl:ObjectProperty ;
                 rdfs:domain arto:VisualElement ;
                 rdfs:range [ rdf:type owl:Class ;
                              owl:unionOf ( arto:Object
                                            arto:Scene
                                          )
                            ] ;
                 rdfs:comment "Specifies the object or scene that contains the visual element in the artwork." ;
                 rdfs:label "isElementOf" ;
                 skos:example """
                  - colour elements: :blue_gradient_colour arto:isElementOf :sky_object
                  - Line elements: :diagonal_line arto:isElementOf :mountain_object
                  - Compositional elements: :vertical_composition arto:isElementOf :tree_object""" .


###  http://w3id.org/arto#isEventOf
arto:isEventOf rdf:type owl:ObjectProperty ;
               owl:inverseOf arto:relatedToEvent ;
               rdfs:domain arto:Event ;
               rdfs:range [ rdf:type owl:Class ;
                            owl:unionOf ( arto:Artwork
                                          arto:Scene
                                        )
                          ] ;
               rdfs:comment "Associates an event with the artwork or scene that it is related to." ;
               rdfs:label "isEventOf" ;
               skos:example """
                - Historical event: :french_revolution_1830 arto:isEventOf :liberty_leading_the_people
                - Biblical event: :biblical_last_supper arto:isEventOf :last_supper
                """ .


###  http://w3id.org/arto#isLocationOf
arto:isLocationOf rdf:type owl:ObjectProperty ;
                  rdfs:domain arto:Location ;
                  rdfs:range [ rdf:type owl:Class ;
                               owl:unionOf ( arto:Agent
                                             arto:Event
                                           )
                             ] ;
                  rdfs:comment "Associates a location with the agent or event that it is related to." ;
                  rdfs:label "isLocationOf" ;
                  skos:example """
                - Museum address: :met_nyc_location arto:isLocationOf :metropolitan_museum
                - Gallery location: :london_bankside arto:isLocationOf :tate_modern
                - Studio location: :manhattan_location arto:isLocationOf :warhol_factory
                - Exhibition event: :venice_giardini arto:isLocationOf :venice_biennale_2024""" .


###  http://w3id.org/arto#isMetricOf
arto:isMetricOf rdf:type owl:ObjectProperty ;
                rdfs:domain arto:Metric ;
                rdfs:range [ rdf:type owl:Class ;
                             owl:unionOf ( arto:Connotation
                                           arto:Object
                                           arto:Scene
                                           arto:VisualElement
                                         )
                           ] ;
                rdfs:comment "Associates a metric with the component of an artwork that it is related to." ;
                rdfs:label "isMetricOf" ;
                skos:example """
                - Colour metrics: :blue_intensity_75_percent arto:isMetricOf :sky_area
                - Composition balance: :symmetry_score_0.8 arto:isMetricOf :landscape_scene
                - Emotional intensity: :fear_intensity_high arto:isMetricOf :expression_scene""" .


###  http://w3id.org/arto#isObjectOf
arto:isObjectOf rdf:type owl:ObjectProperty ;
                rdfs:domain arto:Object ;
                rdfs:range arto:Scene ;
                rdfs:comment "Indicates the scene that contains the object in the artwork." ;
                rdfs:label "isObjectOf" ;
                skos:example """
                - Landscape scene: :fountain arto:isObjectOf :garden_scene
                - Portrait scene: :chair arto:isObjectOf :interior_scene
                - Still life scene: :fruit_bowl arto:isObjectOf :table_scene""" .


###  http://w3id.org/arto#isSceneOf
arto:isSceneOf rdf:type owl:ObjectProperty ;
               rdfs:domain arto:Scene ;
               rdfs:range [ rdf:type owl:Class ;
                            owl:unionOf ( arto:Artwork
                                          arto:Scene
                                        )
                          ] ;
               rdfs:comment "Specifies the artwork or scene that contains the scene in the artwork." ;
               rdfs:label "isSceneOf" ;
               skos:example """
                - Nested scenes: :vendor_scene arto:isSceneOf :market_scene
                - Background scenes: :mountain_scene arto:isSceneOf :landscape_painting""" .


###  http://w3id.org/arto#isTimeOf
arto:isTimeOf rdf:type owl:ObjectProperty ;
              rdfs:domain arto:Time ;
              rdfs:range arto:Event ;
              rdfs:comment "Associates a time entity with the event that it is related to. The time entity may represent a specific date, a period (e.g., season, decade), or a cultural-historical era, allowing precise or approximate temporal anchoring of events or locations." ;
              rdfs:label "isTimeOf" ;
              skos:example """
              - Event timing: :spring2024 arto:isTimeOf :exhibition2024
              - Location historical period: :belle_epoque arto:isTimeOf :paris_studio
              """ .


###  http://w3id.org/arto#knows
arto:knows rdf:type owl:ObjectProperty ;
           rdfs:domain arto:Person ;
           rdfs:range arto:Person ;
           rdfs:comment "The person knows persons. This property, equivalent to foaf:knows, enables study of artistic movements, teacher-student relationships, collaborative networks, and cultural exchange patterns essential for understanding art historical development and cross-cultural artistic influence." ;
           rdfs:label "knows" ;
           skos:example """
            - Artist relationships: :vincent_van_gogh arto:knows :paul_gauguin
            - Teacher-student: :gustav_klimt arto:knows :egon_schiele
            - Collaborative artists: :pablo_picasso arto:knows :georges_braque""" .


###  http://w3id.org/arto#material
arto:material rdf:type owl:ObjectProperty ;
              rdfs:domain arto:Object ;
              rdfs:range arto:MaterialType ;
              rdfs:comment "The material of the Object. It connect to the Getty AAT's material hierarchy, allowing for both standardised and custom material definitions. Not for the artwork's physical medium." ;
              skos:example """
                :glass_vase_obj     a arto:Object ; arto:material aat:glass .
                :pewter_plate_obj   a arto:Object ; arto:material aat:pewter .
                :walnut_table_obj   a arto:Object ; arto:material aat:walnut_wood . 
                """ ;
              rdfs:label "material" .


###  http://w3id.org/arto#medium
arto:medium rdf:type owl:ObjectProperty ;
            rdfs:domain arto:Artwork ;
            rdfs:range arto:MediumType ;
            rdfs:comment "Specifies the physical medium of the artwork itself (e.g., oil on canvas, tempera on panel, bronze sculpture). This property aligns with Getty AAT's medium hierarchy, ensuring standardised description of artistic medium." ;
            skos:example """
              :painting_001 a arto:Artwork ;
                arto:medium aat:oil_on_canvas .

              :wall_painting_001 a arto:Artwork ;
                arto:medium aat:fresco .

              :bronze_statue_001 a arto:Artwork ;
                arto:medium aat:bronze .
              """ ;
            rdfs:label "medium" .


###  http://w3id.org/arto#relatedTo
arto:relatedTo rdf:type owl:ObjectProperty ;
               rdfs:domain arto:Object ;
               rdfs:range arto:Object ;
               rdfs:comment "Describes spatial or conceptual relationships between objects within artworks. This extensible property enables specific relationship types (behind, holds, above) through subproperty mechanisms, supporting detailed spatial analysis while maintaining semantic clarity." ;
               rdfs:label "relatedTo" ;
               skos:example """
                - Spatial relation: :cup_object arto:rests_on :table_object ;
                  arto:rests_on rdfs:subPropertyOf arto:relatedTo;
                - Interaction: :mother_figure arto:holds :child_figure ;
                  arto:holds rdfs:subPropertyOf arto:relatedTo;
                - Position: :cloud_object arto:above :mountain_object ;
                  arto:above rdfs:subPropertyOf arto:relatedTo ;
                - Position: :tree_object arto:behind :house_object ;
                  arto:behind rdfs:subPropertyOf arto:relatedTo ;""" .


###  http://w3id.org/arto#relatedToConnotation
arto:relatedToConnotation rdf:type owl:ObjectProperty ;
                          rdfs:domain arto:Event ;
                          rdfs:range arto:Connotation ;
                          rdfs:comment "Indicates that an event related to some connotations." ;
                          rdfs:label "relatedToConnotation" ;
                          skos:example """
                  ex:NoahDoveEvent rdf:type arto:Event ;
                  arto:relatedToConnotation ex:PeaceSymbolism ;
                """ .


###  http://w3id.org/arto#relatedToEvent
arto:relatedToEvent rdf:type owl:ObjectProperty ;
                    rdfs:domain [ rdf:type owl:Class ;
                                  owl:unionOf ( arto:Artwork
                                                arto:Scene
                                              )
                                ] ;
                    rdfs:range arto:Event ;
                    rdfs:comment "Connects an artwork or its scene to historical, mythological, or contemporary events depicted or referenced in the work." ;
                    rdfs:label "relatedToEvent" ;
                    skos:example """
                      - Historical event: :liberty_leading_the_people arto:relatedToEvent :french_revolution_1830
                      - Biblical event: :last_supper arto:relatedToEvent :biblical_last_supper
                      """ .


###  http://w3id.org/arto#relatedToScene
arto:relatedToScene rdf:type owl:ObjectProperty ;
                    rdfs:domain arto:Object ;
                    rdfs:range arto:Scene ;
                    rdfs:comment "Links objects to the scenes they appear in or are associated with." ;
                    rdfs:label "relatedToScene" ;
                    skos:example """
                      - Object context: :bread_loaf arto:relatedToScene :market_scene """ .


###  http://w3id.org/arto#state
arto:state rdf:type owl:ObjectProperty ;
           rdfs:domain arto:Object ;
           rdfs:range skos:Concept ;
           rdfs:comment "Describes the condition, position, or status of objects within artworks, capturing both physical states (damaged, intact) and depicted conditions (motion, rest, emotional states of figures)." ;
           rdfs:label "state" ;
           skos:example """
               - Physical conditions: :broken_amphora arto:state :damaged_state ;
                 :marble_statue arto:state :weathered_state
               - Motion states: :running_horse arto:state :galloping_state ;
                 :falling_figure arto:state :in_motion_state
               - Positional states: :seated_figure arto:state :sitting_state ;
                 :reclining_venus arto:state :lying_state
               - Emotional states: :weeping_magdalene arto:state :grieving_state ;
                 :laughing_child arto:state :joyful_state
               - Temporal states: :blooming_flower arto:state :spring_state ;
                 :withered_leaves arto:state :autumn_state
               - Functional states: :open_book arto:state :readable_state ;
                 :lit_candle arto:state :burning_state
               """ .


###  http://w3id.org/arto#style
arto:style rdf:type owl:ObjectProperty ;
           rdfs:domain arto:Artwork ;
           rdfs:range arto:StyleType ;
           rdfs:comment "Indicates the artistic style or movement of an artwork, such as Impressionism, Cubism, or Baroque. This property links to Getty AAT's style and period classifications, while also allowing for the inclusion of custom style definitions when necessary." ;
           skos:example """
              :water_lilies a arto:Artwork ;
                arto:style aat:impressionism .

              :guernica a arto:Artwork ;
                arto:style aat:cubism .

              :baroque_altarpiece a arto:Artwork ;
                arto:style aat:baroque .
              """ ;
           rdfs:label "style" .


###  http://w3id.org/arto#technique
arto:technique rdf:type owl:ObjectProperty ;
               rdfs:domain arto:Artwork ;
               rdfs:range arto:TechniqueType ;
               rdfs:comment "Specifies the artistic methods or processes applied in the creation of the artwork (e.g., fresco, engraving, pointillism). This property connects to Getty AAT’s technique hierarchy, while also supporting the definition of custom techniques not covered by AAT." ;
               skos:example """
                :sistine_ceiling a arto:Artwork ;
                  arto:technique aat:fresco .

                :rembrandt_print a arto:Artwork ;
                  arto:technique aat:etching .

                :seurat_painting a arto:Artwork ;
                  arto:technique aat:pointillism .

                :bronze_sculpture a arto:Artwork ;
                  arto:technique aat:lost_wax_casting .
                """ ;
               rdfs:label "technique" .


###  http://www.europeana.eu/schemas/edm/currentLocation
edm:currentLocation rdf:type owl:ObjectProperty .


###  http://www.opengis.net/ont/geosparql#asWKT
geo:asWKT rdf:type owl:ObjectProperty .


###  https://dbpedia.org/property/residence
dbp:residence rdf:type owl:ObjectProperty .


###  https://schema.org/height
sdo:height rdf:type owl:ObjectProperty .


###  https://schema.org/width
sdo:width rdf:type owl:ObjectProperty .


###  https://w3id.org/MON/event.owl#agent
event:agent rdf:type owl:ObjectProperty .


#################################################################
#    Data properties
#################################################################

###  http://purl.org/dc/terms/alternative
dc:alternative rdf:type owl:DatatypeProperty ;
               rdfs:subPropertyOf dc:title ;
               rdfs:range rdfs:Literal .


###  http://purl.org/dc/terms/available
dc:available rdf:type owl:DatatypeProperty ;
             rdfs:subPropertyOf dc:date ;
             rdfs:range rdfs:Literal .


###  http://purl.org/dc/terms/bibliographicCitation
dc:bibliographicCitation rdf:type owl:DatatypeProperty ;
                         rdfs:subPropertyOf dc:identifier ;
                         rdfs:range rdfs:Literal .


###  http://purl.org/dc/terms/created
dc:created rdf:type owl:DatatypeProperty ;
           rdfs:subPropertyOf dc:date ;
           rdfs:range rdfs:Literal .


###  http://purl.org/dc/terms/date
dc:date rdf:type owl:DatatypeProperty ;
        rdfs:range rdfs:Literal .


###  http://purl.org/dc/terms/dateAccepted
dc:dateAccepted rdf:type owl:DatatypeProperty ;
                rdfs:subPropertyOf dc:date ;
                rdfs:range rdfs:Literal .


###  http://purl.org/dc/terms/dateCopyrighted
dc:dateCopyrighted rdf:type owl:DatatypeProperty ;
                   rdfs:subPropertyOf dc:date ;
                   rdfs:range rdfs:Literal .


###  http://purl.org/dc/terms/dateSubmitted
dc:dateSubmitted rdf:type owl:DatatypeProperty ;
                 rdfs:subPropertyOf dc:date ;
                 rdfs:range rdfs:Literal .


###  http://purl.org/dc/terms/identifier
dc:identifier rdf:type owl:DatatypeProperty ;
              rdfs:range rdfs:Literal .


###  http://purl.org/dc/terms/issued
dc:issued rdf:type owl:DatatypeProperty ;
          rdfs:subPropertyOf dc:date ;
          rdfs:range rdfs:Literal .


###  http://purl.org/dc/terms/modified
dc:modified rdf:type owl:DatatypeProperty ;
            rdfs:subPropertyOf dc:date ;
            rdfs:range rdfs:Literal .


###  http://purl.org/dc/terms/title
dc:title rdf:type owl:DatatypeProperty ;
         rdfs:range rdfs:Literal .


###  http://purl.org/dc/terms/valid
dc:valid rdf:type owl:DatatypeProperty ;
         rdfs:subPropertyOf dc:date ;
         rdfs:range rdfs:Literal .


###  http://w3id.org/arto#colourSpace
arto:colourSpace rdf:type owl:DatatypeProperty .


###  http://w3id.org/arto#colourSystem
arto:colourSystem rdf:type owl:DatatypeProperty ;
                  rdfs:domain arto:ColourValue ;
                  rdfs:range [ rdf:type rdfs:Datatype ;
                               owl:oneOf [ rdf:type rdf:List ;
                                           rdf:first "CMYK" ;
                                           rdf:rest [ rdf:type rdf:List ;
                                                      rdf:first "Greyscale" ;
                                                      rdf:rest [ rdf:type rdf:List ;
                                                                 rdf:first "HSV" ;
                                                                 rdf:rest [ rdf:type rdf:List ;
                                                                            rdf:first "Lab" ;
                                                                            rdf:rest [ rdf:type rdf:List ;
                                                                                       rdf:first "RGB" ;
                                                                                       rdf:rest [ rdf:type rdf:List ;
                                                                                                  rdf:first "XYZ" ;
                                                                                                  rdf:rest rdf:nil
                                                                                                ]
                                                                                     ]
                                                                          ]
                                                               ]
                                                    ]
                                         ]
                             ] ;
                  rdfs:comment "The colour system of the ColourValue, indicating the model used for its representation. This property supports various colour models such as RGB, HSV, Lab, and CMYK, allowing for flexible colour representation and analysis in artworks. The use of a restricted set of values ensures consistency and interoperability across different systems and applications." ;
                  rdfs:label "colourSystem" .


###  http://w3id.org/arto#descriptor
arto:descriptor rdf:type owl:DatatypeProperty ;
                rdfs:domain [ rdf:type owl:Class ;
                              owl:unionOf ( arto:Object
                                            arto:Scene
                                          )
                            ] ;
                rdfs:range xsd:string ;
                rdfs:comment "Provides extensible descriptive framework for capturing object and scene characteristics not covered by specific properties, enabling domain-specific extensions through subproperties. This design addresses the infinite variety of artistic content while maintaining semantic structure. Examples include clothing descriptions for figures, or environmental conditions for scene." ;
                rdfs:label "descriptor" ;
                skos:example """
                Portrait1 :clothing :RedDress ;
                :clothing rdfs:subPropertyOf arto:descriptor""" .


###  http://w3id.org/arto#direction
arto:direction rdf:type owl:DatatypeProperty ;
               rdfs:domain arto:Line ;
               rdfs:range xsd:string ;
               rdfs:comment "Describes the orientation of linear elements in an artwork." ;
               rdfs:label "direction" .


###  http://w3id.org/arto#emotionPerspective
arto:emotionPerspective rdf:type owl:DatatypeProperty ;
                        rdfs:domain arto:Emotion ;
                        rdfs:range [ rdf:type rdfs:Datatype ;
                                     owl:oneOf [ rdf:type rdf:List ;
                                                 rdf:first "Artist" ;
                                                 rdf:rest [ rdf:type rdf:List ;
                                                            rdf:first "Artwork" ;
                                                            rdf:rest [ rdf:type rdf:List ;
                                                                       rdf:first "Viewer" ;
                                                                       rdf:rest rdf:nil
                                                                     ]
                                                          ]
                                               ]
                                   ] ;
                        rdfs:comment "Specifies the perspective or viewpoint from which an emotion is interpreted in relation to an artwork. This property distinguishes between emotions intended by the artist, emotions expressed by the artwork itself, emotions experienced by viewers. Values are restricted to: 'artist' (artist's intended emotion), 'artwork' (emotion expressed by the artwork's formal elements), and 'viewer' (viewer's emotional response)." ;
                        rdfs:label "emotionPerspective"@en ;
                        skos:example """
                          ex:melancholy_emotion arto:emotionPerspective \"artist\"^^xsd:string ;
                          ex:serenity_emotion arto:emotionPerspective \"artwork\"^^xsd:string ;
                          ex:excitement_emotion arto:emotionPerspective \"viewer\"^^xsd:string .
                          """ .


###  http://w3id.org/arto#length
arto:length rdf:type owl:DatatypeProperty ;
            rdfs:domain arto:Line ;
            rdfs:range xsd:float ;
            rdfs:comment "The length of the line." ;
            rdfs:label "length" .


###  http://w3id.org/arto#size
arto:size rdf:type owl:DatatypeProperty ;
          rdfs:domain [ rdf:type owl:Class ;
                        owl:unionOf ( arto:Object
                                      arto:Scene
                                    )
                      ] ;
          rdfs:range xsd:string ;
          rdfs:comment "Indicates the relative or absolute dimensions of objects and scenes within artwork composition. Size often correlate with narrative importance, symbolic significance, or perspectival organisation in artistic composition." ;
          rdfs:label "size" .


###  http://w3id.org/arto#source
arto:source rdf:type owl:DatatypeProperty ;
            rdfs:domain arto:Symbolism ;
            rdfs:range xsd:string ;
            rdfs:comment "Identifies the cultural, historical, or textual origins of symbolic meanings, enabling traceability of iconographic interpretations and cross-cultural symbolic analysis. Sources can include mythological traditions, religious texts, historical events, literary works, or folk traditions that inform symbolic interpretation." ;
            rdfs:label "source" .


###  http://w3id.org/arto#width
arto:width rdf:type owl:DatatypeProperty ;
            rdfs:domain arto:Line ;
            rdfs:range xsd:float ;
            rdfs:comment "The width of the line." ;
            rdfs:label "width" .


###  http://www.europeana.eu/schemas/edm/isShownBy
edm:isShownBy rdf:type owl:DatatypeProperty .


###  https://schema.org/endDate
sdo:endDate rdf:type owl:DatatypeProperty .


###  https://schema.org/startDate
sdo:startDate rdf:type owl:DatatypeProperty .


#################################################################
#    Classes
#################################################################

###  http://purl.obolibrary.org/obo/MFOEM_000001
mfoem:MFOEM_000001 rdf:type owl:Class .


###  http://purl.org/dc/dcam/VocabularyEncodingScheme
<http://purl.org/dc/dcam/VocabularyEncodingScheme> rdf:type owl:Class .


###  http://purl.org/dc/terms/Agent
dc:Agent rdf:type owl:Class .


###  http://purl.org/dc/terms/AgentClass
dc:AgentClass rdf:type owl:Class ;
              rdfs:subClassOf rdfs:Class .


###  http://purl.org/dc/terms/BibliographicResource
dc:BibliographicResource rdf:type owl:Class .


###  http://purl.org/dc/terms/FileFormat
dc:FileFormat rdf:type owl:Class ;
              rdfs:subClassOf dc:MediaType .


###  http://purl.org/dc/terms/Frequency
dc:Frequency rdf:type owl:Class .


###  http://purl.org/dc/terms/Jurisdiction
dc:Jurisdiction rdf:type owl:Class ;
                rdfs:subClassOf dc:LocationPeriodOrJurisdiction .


###  http://purl.org/dc/terms/LicenseDocument
dc:LicenseDocument rdf:type owl:Class ;
                   rdfs:subClassOf dc:RightsStatement .


###  http://purl.org/dc/terms/LinguisticSystem
dc:LinguisticSystem rdf:type owl:Class .


###  http://purl.org/dc/terms/Location
dc:Location rdf:type owl:Class ;
            rdfs:subClassOf dc:LocationPeriodOrJurisdiction .


###  http://purl.org/dc/terms/LocationPeriodOrJurisdiction
dc:LocationPeriodOrJurisdiction rdf:type owl:Class .


###  http://purl.org/dc/terms/MediaType
dc:MediaType rdf:type owl:Class ;
             rdfs:subClassOf dc:MediaTypeOrExtent .


###  http://purl.org/dc/terms/MediaTypeOrExtent
dc:MediaTypeOrExtent rdf:type owl:Class .


###  http://purl.org/dc/terms/MethodOfAccrual
dc:MethodOfAccrual rdf:type owl:Class .


###  http://purl.org/dc/terms/MethodOfInstruction
dc:MethodOfInstruction rdf:type owl:Class .


###  http://purl.org/dc/terms/PeriodOfTime
dc:PeriodOfTime rdf:type owl:Class ;
                rdfs:subClassOf dc:LocationPeriodOrJurisdiction .


###  http://purl.org/dc/terms/PhysicalMedium
dc:PhysicalMedium rdf:type owl:Class ;
                  rdfs:subClassOf dc:MediaType .


###  http://purl.org/dc/terms/PhysicalResource
dc:PhysicalResource rdf:type owl:Class .


###  http://purl.org/dc/terms/Policy
dc:Policy rdf:type owl:Class .


###  http://purl.org/dc/terms/ProvenanceStatement
dc:ProvenanceStatement rdf:type owl:Class .


###  http://purl.org/dc/terms/RightsStatement
dc:RightsStatement rdf:type owl:Class .


###  http://purl.org/dc/terms/SizeOrDuration
dc:SizeOrDuration rdf:type owl:Class ;
                  rdfs:subClassOf dc:MediaTypeOrExtent .


###  http://purl.org/dc/terms/Standard
dc:Standard rdf:type owl:Class .


###  http://qudt.org/schema/qudt/Vector
qudt:Vector rdf:type owl:Class .


###  http://vocab.getty.edu/aat/300163343
<http://vocab.getty.edu/aat/300163343> rdf:type owl:Class .


###  http://w3id.org/arto#Agent
arto:Agent rdf:type owl:Class ;
           rdfs:subClassOf foaf:Agent ,
                           [ rdf:type owl:Restriction ;
                             owl:onProperty arto:hasLocation ;
                             owl:allValuesFrom arto:Location
                           ] ;
           rdfs:comment "Represents individuals or organisations involved in artwork creation, curation, or related activities. This class extends foaf:Agent with art-specific roles and relationships. Agents can be artists, curators, collectors, institutions, or other entities. " ;
           rdfs:label "Agent" .


###  http://w3id.org/arto#Artist
arto:Artist rdf:type owl:Class ;
            rdfs:subClassOf arto:Person ;
            rdfs:comment "The person or group who create or contribute the artwork." ;
            rdfs:label "Artist" .


###  http://w3id.org/arto#Artwork
arto:Artwork rdf:type owl:Class ;
             rdfs:subClassOf sdo:CreativeWork ,
                             [ rdf:type owl:Restriction ;
                               owl:onProperty dc:contributor ;
                               owl:allValuesFrom arto:Agent
                             ] ,
                             [ rdf:type owl:Restriction ;
                               owl:onProperty dc:creator ;
                               owl:allValuesFrom arto:Artist
                             ] ,
                             [ rdf:type owl:Restriction ;
                               owl:onProperty dc:isPartOf ;
                               owl:allValuesFrom arto:Series
                             ] ,
                             [ rdf:type owl:Restriction ;
                               owl:onProperty arto:containsScene ;
                               owl:allValuesFrom arto:Scene
                             ] ,
                             [ rdf:type owl:Restriction ;
                               owl:onProperty arto:genre ;
                               owl:allValuesFrom arto:GenreType
                             ] ,
                             [ rdf:type owl:Restriction ;
                               owl:onProperty arto:hasConnotation ;
                               owl:allValuesFrom arto:Connotation
                             ] ,
                             [ rdf:type owl:Restriction ;
                               owl:onProperty arto:medium ;
                               owl:allValuesFrom arto:MediumType
                             ] ,
                             [ rdf:type owl:Restriction ;
                               owl:onProperty arto:relatedToEvent ;
                               owl:allValuesFrom arto:Event
                             ] ,
                             [ rdf:type owl:Restriction ;
                               owl:onProperty arto:style ;
                               owl:allValuesFrom arto:StyleType
                             ] ,
                             [ rdf:type owl:Restriction ;
                               owl:onProperty arto:technique ;
                               owl:allValuesFrom arto:TechniqueType
                             ] ,
                             [ rdf:type owl:Restriction ;
                               owl:onProperty arto:currentLocation ;
                               owl:maxQualifiedCardinality "1"^^xsd:nonNegativeInteger ;
                               owl:onClass arto:Location
                             ] ,
                             [ rdf:type owl:Restriction ;
                               owl:onProperty sdo:height ;
                               owl:maxQualifiedCardinality "1"^^xsd:nonNegativeInteger ;
                               owl:onClass sdo:QuantitativeValue
                             ] ,
                             [ rdf:type owl:Restriction ;
                               owl:onProperty sdo:width ;
                               owl:maxQualifiedCardinality "1"^^xsd:nonNegativeInteger ;
                               owl:onClass sdo:QuantitativeValue
                             ] ,
                             [ rdf:type owl:Restriction ;
                               owl:onProperty dc:description ;
                               owl:allValuesFrom xsd:string
                             ] ,
                             [ rdf:type owl:Restriction ;
                               owl:onProperty dc:title ;
                               owl:allValuesFrom xsd:string
                             ] ,
                             [ rdf:type owl:Restriction ;
                               owl:onProperty edm:isShownBy ;
                               owl:maxQualifiedCardinality "1"^^xsd:nonNegativeInteger ;
                               owl:onDataRange xsd:anyURI
                             ] ;
             rdfs:comment "Represents a created object intended to be aesthetically pleasing or convey artistic meaning. This class encompasses various art forms including paintings, sculptures, photographs, and digital art. Unlike CIDOC-CRM's E22_Human-Made_Object which covers all manufactured items, arto:Artwork specifically focuses on objects created with artistic intent. The class inherits essential properties from schema:CreativeWork (creator, dateCreated, description) while adding art-specific constraints such as mandatory visual representation (edm:isShownBy) and current location tracking. Each artwork must contain at least one scene and have defined dimensions, supporting both traditional and contemporary art analysis." ;
             rdfs:label "Artwork" .


###  http://w3id.org/arto#BalanceOfComposition
arto:BalanceOfComposition rdf:type owl:Class ;
                          rdfs:subClassOf arto:Metric ;
                          rdfs:comment "Used to assess and describe the visual equilibrium of an artwork's composition. This metric captures how elements are arranged in terms of symmetry, asymmetry, and spatial distribution of visual weight. It can be applied in qualitative analysis (e.g., identifying harmonious vs. dynamic arrangements) or in quantitative evaluation when assigning a balance score to artworks." ;
                          rdfs:label "BalanceOfComposition" .


###  http://w3id.org/arto#Character
arto:Character rdf:type owl:Class ;
               rdfs:subClassOf arto:Person ;
               rdfs:comment "Represents persons, figures, or beings depicted within an artwork." ;
               rdfs:label "Character" .


###  http://w3id.org/arto#Colour
arto:Colour rdf:type owl:Class ;
            rdfs:subClassOf arto:VisualElement ,
                            [ rdf:type owl:Restriction ;
                              owl:onProperty arto:hasColourTerm ;
                              owl:allValuesFrom arto:ColourTerm
                            ] ,
                            [ rdf:type owl:Restriction ;
                              owl:onProperty arto:hasColourValue ;
                              owl:allValuesFrom arto:ColourValue
                            ] ;
            rdfs:comment "Represents colour usage in artworks with precise technical specifications and art historical context. This class provides both computational colour analysis (RGB, HSV values) and art theoretical foundations, aligning with Getty AAT's colour concepts while maintaining specific properties for digital analysis. Colour instances can express symbolic meanings and emotional content, supporting both technical image processing and interpretive art analysis." ;
            skos:example """
            :c_vermilion a arto:Colour ;
              arto:hasColourTerm <http://vocab.getty.edu/aat/300266400> ;  # vermilion
              arto:hasColourValue [
                a arto:ColourValue ;
                arto:colourSpace "RGB" ;
                qudt:vector (227,66,52)  ] .


            :c_bluePeace a arto:Colour ;
              arto:hasColourTerm <http://vocab.getty.edu/aat/300129361> ;  # blue
              arto:hasColourValue [
                a arto:ColourValue ;
                arto:colourSpace "HSV" ;
                qudt:vector (197,76,100)
              ] ;
            """ ;
            rdfs:label "Colour" .


###  http://w3id.org/arto#ColourHistogram
arto:ColourHistogram rdf:type owl:Class ;
                     rdfs:subClassOf arto:Metric ;
                     rdfs:comment "A metric that captures the distribution of colours within an artwork. It represents how frequently each colour or colour range occurs, typically in the form of a histogram or similar quantitative structure. This metric can be used for tasks such as palette analysis, artwork comparison" ;
                     rdfs:label "ColourHistogram" .


###  http://w3id.org/arto#ColourTerm
arto:ColourTerm rdf:type owl:Class ;
                rdfs:subClassOf [ rdf:type owl:Class ;
                                  owl:unionOf ( skos:Concept
                                                [ rdf:type owl:Restriction ;
                                                  owl:onProperty skos:broaderTransitive ;
                                                  owl:hasValue <http://vocab.getty.edu/aat/300131647>
                                                ]
                                              )
                                ] ;
                rdfs:comment "Represents standardised colour terminology from controlled vocabularies, art historical literature, and established colour naming systems. This class provides semantic interoperability by linking colour instances to authoritative colour classifications, enabling consistent colour identification across institutions and research projects. Colour terms encompass basic colour names, specific pigment designations, cultural colour concepts, and technical colour classifications. The class primarily aligns with Getty AAT's colour hierarchy while supporting additional colour vocabularies and historical colour terminology." ;
                rdfs:label "ColourTerm" ;
                skos:example """
                   - Basic colour terms: aat:red, aat:blue, aat:yellow, aat:green
                     # Fundamental colour categories from Getty AAT
                   - Specific pigment terms: aat:ultramarine_blue, aat:vermillion, aat:cadmium_yellow
                     # Historical and contemporary pigment names
                   - Cultural colour terms: aat:royal_purple, aat:imperial_yellow, aat:sacred_red
                     # Colours with cultural or symbolic significance
                   - Technical colour terms: aat:primary_colours, aat:complementary_colours, aat:earth_tones
                     # Colour theory and technical classifications
                   - Historical colour terms: aat:tyrian_purple, aat:lapis_lazuli_blue, aat:gold_leaf
                     # Historically significant colourants and materials
                   - Descriptive colour terms: aat:warm_colours, aat:cool_colours, aat:neutral_tones
                     # Colour temperature and mood classifications
                   """ .


###  http://w3id.org/arto#ColourValue
arto:ColourValue rdf:type owl:Class ;
                 rdfs:subClassOf [ rdf:type owl:Restriction ;
                                   owl:onProperty qudt:vector ;
                                   owl:allValuesFrom qudt:Vector
                                 ] ,
                                 [ rdf:type owl:Restriction ;
                                   owl:onProperty arto:colourSpace ;
                                   owl:allValuesFrom [ rdf:type rdfs:Datatype ;
                                                       owl:oneOf [ rdf:type rdf:List ;
                                                                   rdf:first "CMYK" ;
                                                                   rdf:rest [ rdf:type rdf:List ;
                                                                              rdf:first "Greyscale" ;
                                                                              rdf:rest [ rdf:type rdf:List ;
                                                                                         rdf:first "HSV" ;
                                                                                         rdf:rest [ rdf:type rdf:List ;
                                                                                                    rdf:first "Lab" ;
                                                                                                    rdf:rest [ rdf:type rdf:List ;
                                                                                                               rdf:first "RGB" ;
                                                                                                               rdf:rest [ rdf:type rdf:List ;
                                                                                                                          rdf:first "XYZ" ;
                                                                                                                          rdf:rest rdf:nil
                                                                                                                        ]
                                                                                                             ]
                                                                                                  ]
                                                                                       ]
                                                                            ]
                                                                 ]
                                                     ]
                                 ] ;
                 rdfs:comment "Represents the precise numeric specification of colours using various colour models and measurement systems. This class captures quantitative colour data for digital analysis, colour matching and reproduction studies. Colour values enable objective colour comparison, automated colour analysis, and integration with digital image processing workflows. The class supports multiple colour spaces to accommodate different analytical needs and technical requirements." ;
                 rdfs:label "colourValue" ;
                 skos:example """
                    - RGB specification: :red_primary rdf:type arto:ColourValue ;
                      arto:colourSpace \"RGB\" ; qudt:vector (255,0,0) ;
                    - HSV specification: :golden_yellow rdf:type arto:ColourValue ;
                      arto:colourSpace \"HSV\" ; qudt:vector (45,85,95) ;
                    - CMYK print colours: :prussian_blue rdf:type arto:ColourValue ;
                      arto:colourSpace \"CMYK\" ; qudt:vector (100,85,0,25) ;
                    - LAB colour measurement: :skin_tone rdf:type arto:ColourValue ;
                        arto:colourSpace \"Lab\" ; qudt:vector (75,8,15) ;
                    """ .


###  http://w3id.org/arto#Composition
arto:Composition rdf:type owl:Class ;
                 rdfs:subClassOf arto:VisualElement ,
                                 [ rdf:type owl:Restriction ;
                                   owl:onProperty dc:type ;
                                   owl:allValuesFrom xsd:string
                                 ] ;
                 rdfs:comment """Represents the arrangement and organisation of visual elements within artworks, fundamental to art historical analysis and aesthetic evaluation. This class captures compositional strategies, balance, and spatial relationships that structure artistic meaning.
                 Currently ARTO includes common compositions types: symmetry, asymmetry, radial balance, rule of thirds, golden ratio, and dynamic composition.
                 """ ;
                 rdfs:label "Composition" .


###  http://w3id.org/arto#Connotation
arto:Connotation rdf:type owl:Class ;
                 rdfs:subClassOf crm:E28_Conceptual_Object ,
                                 [ rdf:type owl:Restriction ;
                                   owl:onProperty arto:hasMetric ;
                                   owl:allValuesFrom arto:Metric
                                 ] ;
                 rdfs:comment """Represents the implied meanings of artwork, includeing themes, symbolic meanings, and
      emotions conveyed by an artwork.""" ;
                 rdfs:label "Connotation" ;
                 skos:example """
                     - Symbolic meaning: :dove_symbolism rdf:type arto:Symbolism .
                     - Emotional content: :melancholy_mood rdf:type arto:Emotion ; arto:emotionPerspective \"artwork\"
                     - Historical reference: :revolution_allegory rdf:type arto:Connotation ;
                       dc:description \"French Revolution political symbolism\"
                     """ .


###  http://w3id.org/arto#Emotion
arto:Emotion rdf:type owl:Class ;
             rdfs:subClassOf arto:Connotation ,
                             [ rdf:type owl:Restriction ;
                               owl:onProperty arto:expresses ;
                               owl:allValuesFrom mfoem:MFOEM_000001
                             ] ,
                             [ rdf:type owl:Restriction ;
                               owl:onProperty arto:emotionPerspective ;
                               owl:allValuesFrom [ rdf:type rdfs:Datatype ;
                                                   owl:oneOf [ rdf:type rdf:List ;
                                                               rdf:first "artist" ;
                                                               rdf:rest [ rdf:type rdf:List ;
                                                                          rdf:first "artwork" ;
                                                                          rdf:rest [ rdf:type rdf:List ;
                                                                                     rdf:first "viewer" ;
                                                                                     rdf:rest rdf:nil
                                                                                   ]
                                                                        ]
                                                             ]
                                                 ]
                             ] ;
             rdfs:comment """Represents emotional content or affective responses in artworks.
             Uses MFOEM emotion ontology types and the emotionPerspective property to distinguish 
             between artist's intended emotion, artwork's emotional expression, and viewer's response.
             Emotions are expressed using standardised MFOEM emotion types including basic emotions (happiness, sadness, anger, fear, surprise, disgust) and complex emotions (love, anxiety, hope, despair, serenity). """ ;
             rdfs:label "Emotion" ;
             skos:example """
# Artist's intended emotion
:guernica_antiwar_anger  arto:Emotion ;
    arto:expresses mfoem:MFOEM_000009 ;
    arto:emotionPerspective \"artist\" ;
    dc:description \"Picasso's anger against the brutality of war\" .

# Artwork's emotional expression  
:starry_night_turbulence rdf:type arto:Emotion ;
    arto:expresses mfoem:MFOEM_000028 ;
    arto:emotionPerspective \"artwork\" ;
    dc:description \"Anxiety expressed through swirling brushstrokes and dynamic composition\" .

# Viewer's emotional response
:mona_lisa_mystery rdf:type  arto:Emotion ;
    arto:expresses mfoem:MFOEM_000167 ;
    arto:emotionPerspective \"viewer\" ;
    dc:description \"Viewer's curiosity evoked by the enigmatic smile\" .
""" .


###  http://w3id.org/arto#EmotionIntensity
arto:EmotionIntensity rdf:type owl:Class ;
                      rdfs:subClassOf arto:Metric ;
                       rdfs:comment """Represents the measured strength of an emotional response evoked by an artwork. 
Values may be expressed on different scales, for example:
- Categorical levels such as low / medium / high
- Numeric ranges (e.g., 0-1, 1-5, or 1-10)
This flexibility allows projects to choose the scale best suited to their analytical or interpretive framework.""" ;
                      rdfs:label "EmotionIntensity" .


###  http://w3id.org/arto#Event
arto:Event rdf:type owl:Class ;
           rdfs:subClassOf event:Event ,
                           [ rdf:type owl:Restriction ;
                             owl:onProperty arto:hasLocation ;
                             owl:someValuesFrom arto:Location
                           ] ,
                           [ rdf:type owl:Restriction ;
                             owl:onProperty arto:hasTime ;
                             owl:someValuesFrom arto:Time
                           ] ,
                           [ rdf:type owl:Restriction ;
                             owl:onProperty event:agent ;
                             owl:someValuesFrom arto:Agent
                           ] ,
                           [ rdf:type owl:Restriction ;
                             owl:onProperty arto:relatedToConnotation ;
                             owl:allValuesFrom arto:Connotation
                           ] ,
                           [ rdf:type owl:Restriction ;
                             owl:onProperty dc:type ;
                             owl:allValuesFrom xsd:string
                           ] ;
           rdfs:comment """
Represents a temporally and spatially situated occurrence involving agents and locations.
This class extends the Event Ontology and aligns conceptually with CIDOC CRM’s E5_Event,
supporting cultural heritage interoperability. Event instances may cover artistic activities
(creation, sketching, exhibition), artist life events (residence changes, collaborations),
as well as historical or mythological occurrences referenced in artworks. Event categories
can be expressed using rdf:type (e.g., Creation, Exhibition, ResidenceMove).
""" ;
      skos:example """
          << :Guernica arto:sketchedBy :Picasso >> a arto:Event ;
              arto:hasTime :t_1937_Spring ; arto:hasLocation :ParisStudio ;
              dc:type "Sketching".

          << :Guernica dcterms:creator :Picasso >> a arto:Event ;
              arto:hasTime :t_1937 ; arto:hasLocation :ParisStudio ;
              dc:type "Creation".
          << :Georgia_OKeeffe arto:movedResidenceTo :Abiquiu_Home >> a arto:Event ;
            arto:hasTime :t_1949 ; arto:hasLocation :Abiquiu_NewMexico ;
            dc:type "ResidenceMove".
          """ ;
           rdfs:label "Event" .


###  http://w3id.org/arto#GenreType
arto:GenreType rdf:type owl:Class ;
               rdfs:subClassOf [ rdf:type owl:Class ;
                                 owl:unionOf ( skos:Concept
                                               [ rdf:type owl:Restriction ;
                                                 owl:onProperty skos:broaderTransitive ;
                                                 owl:hasValue <http://vocab.getty.edu/aat/300056444>
                                               ]
                                             )
                               ] ;
               rdfs:comment "Represents the genre of an artwork, such as portrait, landscape, still life, etc. This class allows for the classification of artworks based on their thematic or stylistic content." ;
               rdfs:label "GenreType" .


###  http://w3id.org/arto#Line
arto:Line rdf:type owl:Class ;
          rdfs:subClassOf arto:VisualElement ,
                          [ rdf:type owl:Restriction ;
                            owl:onProperty dc:type ;
                            owl:allValuesFrom xsd:string
                          ] ,
                          [ rdf:type owl:Restriction ;
                            owl:onProperty arto:direction ;
                            owl:allValuesFrom xsd:string
                          ] ,
                          [ rdf:type owl:Restriction ;
                            owl:onProperty arto:length ;
                            owl:allValuesFrom xsd:float
                          ] ,
                          [ rdf:type owl:Restriction ;
                            owl:onProperty arto:width ;
                            owl:allValuesFrom xsd:float
                          ] ;
          rdfs:comment "Represents linear visual elements in artworks. Typical line types may include straight, curved, broken, contour, gestural, structural, implied, and hatching or cross-hatching. These categories are indicative and may be aligned with controlled vocabularies such as Getty AAT where applicable." ;
          rdfs:label "Line" .


###  http://w3id.org/arto#Location
arto:Location rdf:type owl:Class ;
              rdfs:subClassOf crm:E53_Place ,
                              [ rdf:type owl:Restriction ;
                                owl:onProperty geo:asWKT ;
                                owl:allValuesFrom geo:wktLiteral
                              ] ,
                              [ rdf:type owl:Restriction ;
                                owl:onProperty dc:type ;
                                owl:allValuesFrom xsd:string
                              ] ;
              rdfs:comment "Represents physical or conceptual places associated with artwork creation, display, storage, or depicted content, supporting both precise geographical coordinates and general names. This class addresses the complex relationship between location and time in historical contexts, where political boundaries and place names evolve over centuries. The class integrates GeoSPARQL coordinates with flexible place type classifications, supporting the artwork's historical geographical analysis." ;
              rdfs:label "Location" .


###  http://w3id.org/arto#MainColour
arto:MainColour rdf:type owl:Class ;
                rdfs:subClassOf arto:Metric ;
                rdfs:comment """Represents the dominant or most prominent colour in an artwork, which can be
      determined through visual analysis or colour quantisation techniques.""" ;
                rdfs:label "MainColour" .


###  http://w3id.org/arto#MaterialType
arto:MaterialType rdf:type owl:Class ;
                  rdfs:subClassOf [ rdf:type owl:Class ;
                                    owl:unionOf ( skos:Concept
                                                  [ rdf:type owl:Restriction ;
                                                    owl:onProperty skos:broaderTransitive ;
                                                    owl:hasValue <http://vocab.getty.edu/aat/300264091>
                                                  ]
                                                )
                                  ] ;
                  rdfs:comment """Represents the material type of an object, such as wood,
      metal, glass, or fabric. This class allows for the classification of objects based on the
      materials used in their construction or representation.""" ;
                  rdfs:label "MaterialType" ;
                  skos:example """
                  - :wood_material rdf:type arto:  .
                  - :metal_material rdf:type arto:MaterialType .
                  - :glass_material rdf:type arto:MaterialType .
                      """ .


###  http://w3id.org/arto#MediumType
arto:MediumType rdf:type owl:Class ;
                rdfs:subClassOf [ rdf:type owl:Class ;
                                  owl:unionOf ( skos:Concept
                                                [ rdf:type owl:Restriction ;
                                                  owl:onProperty skos:broader ;
                                                  owl:someValuesFrom <http://vocab.getty.edu/aat/300163343>
                                                ]
                                              )
                                ] ;
                rdfs:comment "Represents the medium of an artwork, such as oil on canvas, watercolour, etc. This class allows for the classification of artworks based on the materials and techniques used in their creation." ;
                rdfs:label "MediumType" .


###  http://w3id.org/arto#Metric
arto:Metric rdf:type owl:Class ;
            rdfs:comment """Represents a quantifiable measurement or characteristic of an artwork,
      encompassing statistical information about basic elements such as colour statistics, emotion
      intensity, balance of composition, and other visual elements, to facilitate structural
      analysis
      and comparison of artworks.""" ;
            rdfs:label "Metric" .


###  http://w3id.org/arto#Object
arto:Object rdf:type owl:Class ;
            rdfs:subClassOf [ rdf:type owl:Restriction ;
                              owl:onProperty arto:hasConnotation ;
                              owl:someValuesFrom arto:Connotation
                            ] ,
                            [ rdf:type owl:Restriction ;
                              owl:onProperty arto:hasCoordinates ;
                              owl:allValuesFrom qudt:Vector
                            ] ,
                            [ rdf:type owl:Restriction ;
                              owl:onProperty arto:hasMetric ;
                              owl:allValuesFrom arto:Metric
                            ] ,
                            [ rdf:type owl:Restriction ;
                              owl:onProperty arto:material ;
                              owl:allValuesFrom arto:MaterialType
                            ] ,
                            [ rdf:type owl:Restriction ;
                              owl:onProperty arto:relatedTo ;
                              owl:allValuesFrom arto:Object
                            ] ,
                            [ rdf:type owl:Restriction ;
                              owl:onProperty arto:relatedToScene ;
                              owl:allValuesFrom arto:Scene
                            ] ,
                            [ rdf:type owl:Restriction ;
                              owl:onProperty arto:state ;
                              owl:allValuesFrom skos:Concept
                            ] ,
                            [ rdf:type owl:Restriction ;
                              owl:onProperty arto:descriptor ;
                              owl:allValuesFrom xsd:string
                            ] ,
                            [ rdf:type owl:Restriction ;
                              owl:onProperty arto:size ;
                              owl:allValuesFrom xsd:string
                            ] ;
            rdfs:comment "Represents identifiable and meaningful entities depicted within artworks, composed of various visual elements. Objects serve as the primary content units for artwork analysis, with properties describing their physical state, material composition, and spatial relationships" ;
            rdfs:label "Object" .


###  http://w3id.org/arto#Organisation
arto:Organisation rdf:type owl:Class ;
                  rdfs:subClassOf arto:Agent ,
                                  foaf:Organization ;
                  owl:disjointWith arto:Person ;
                  rdfs:comment "Represents institutional entities involved in artwork creation, curation, preservation, or display, including museums, galleries, art schools, cultural institutions, commercial art enterprises, etc." ;
                  rdfs:label "Organisation" .


###  http://w3id.org/arto#Painting
arto:Painting rdf:type owl:Class ;
              rdfs:subClassOf arto:Artwork ;
              rdfs:comment "A specific type of artwork created using paint or similar media. " ;
              rdfs:label "Painting" .


###  http://w3id.org/arto#Person
arto:Person rdf:type owl:Class ;
            rdfs:subClassOf arto:Agent ,
                            foaf:Person ,
                            [ rdf:type owl:Restriction ;
                              owl:onProperty arto:knows ;
                              owl:allValuesFrom arto:Person
                            ] ;
            rdfs:comment "Individual human beings involved with artwork may include artists, curators, critics, collectors, conservators, researchers, and other roles." ;
            rdfs:label "Person" .


###  http://w3id.org/arto#Photograph
arto:Photograph rdf:type owl:Class ;
                rdfs:subClassOf arto:Artwork ;
                rdfs:comment "A specific type of artwork created using photography or similar media. " ;
                rdfs:label "Photograph" .


###  http://w3id.org/arto#Relevance
arto:Relevance rdf:type owl:Class ;
               rdfs:subClassOf arto:Metric ;
               rdfs:comment """Measures and describes the significance or importance of elements within an artwork, including:
                  - Thematic relevance
                  - Visual importance
                  - Symbolic significance
                  - Narrative relevance
                  - Historical relevance
                  - Compositional importance""" ;
               rdfs:label "Relevance" .


###  http://w3id.org/arto#Scene
arto:Scene rdf:type owl:Class ;
           rdfs:subClassOf [ rdf:type owl:Restriction ;
                             owl:onProperty arto:containsObject ;
                             owl:allValuesFrom arto:Object
                           ] ,
                           [ rdf:type owl:Restriction ;
                             owl:onProperty arto:containsScene ;
                             owl:allValuesFrom arto:Scene
                           ] ,
                           [ rdf:type owl:Restriction ;
                             owl:onProperty arto:hasConnotation ;
                             owl:allValuesFrom arto:Connotation
                           ] ,
                           [ rdf:type owl:Restriction ;
                             owl:onProperty arto:hasCoordinates ;
                             owl:allValuesFrom qudt:Vector
                           ] ,
                           [ rdf:type owl:Restriction ;
                             owl:onProperty arto:hasMetric ;
                             owl:allValuesFrom arto:Metric
                           ] ,
                           [ rdf:type owl:Restriction ;
                             owl:onProperty arto:relatedToEvent ;
                             owl:allValuesFrom arto:Event
                           ] ,
                           [ rdf:type owl:Restriction ;
                             owl:onProperty arto:descriptor ;
                             owl:allValuesFrom xsd:string
                           ] ,
                           [ rdf:type owl:Restriction ;
                             owl:onProperty arto:size ;
                             owl:allValuesFrom xsd:string
                           ] ;
           rdfs:comment "Represents a coherent visual or narrative unit within an artwork that conveys specific meaning or sentiment. A scene aggregates objects and visual elements into meaningful compositions, supporting hierarchical structures where complex artworks contain multiple interconnected scenes. It's similar to ICON's image representations but with explicit support for scene nesting and relationships. Scenes can reference historical, mythological, or fictional events through relatedToEvent, enabling contextual artwork analysis." ;
           rdfs:label "Scene" .


###  http://w3id.org/arto#Sculpture
arto:Sculpture rdf:type owl:Class ;
               rdfs:subClassOf arto:Artwork ;
               rdfs:comment """A specific type of artwork created using sculptural techniques, such as carving,
      modelling, or casting.""" ;
               rdfs:label "Sculpture" .


###  http://w3id.org/arto#Series
arto:Series rdf:type owl:Class ;
            rdfs:subClassOf sdo:CreativeWorkSeries ,
                            [ rdf:type owl:Restriction ;
                              owl:onProperty dc:creator ;
                              owl:allValuesFrom arto:Agent
                            ] ;
            rdfs:comment """A collection of related artworks that share common characteristics, themes, or purposes, including:
                - Thematic series
                - Chronological series
                - Technique-based series
                - Subject-based series
                - Experimental series
                - Documentary series""" ;
            rdfs:label "Series" .


###  http://w3id.org/arto#Space
arto:Space rdf:type owl:Class ;
           rdfs:subClassOf arto:VisualElement ,
                           [ rdf:type owl:Restriction ;
                             owl:onProperty dc:type ;
                             owl:allValuesFrom xsd:string
                           ] ;
           rdfs:comment "Captures the representation of depth, and spatial organisation within artworks. " ;
           rdfs:label "Space" .


###  http://w3id.org/arto#Sponsor
arto:Sponsor rdf:type owl:Class ;
             rdfs:subClassOf arto:Person ;
             rdfs:comment "The person or group who sponsor the artwork." ;
             rdfs:label "Sponsor" .


###  http://w3id.org/arto#StyleType
arto:StyleType rdf:type owl:Class ;
               rdfs:subClassOf [ rdf:type owl:Class ;
                                 owl:unionOf ( skos:Concept
                                               [ rdf:type owl:Restriction ;
                                                 owl:onProperty skos:broaderTransitive ;
                                                 owl:hasValue <http://vocab.getty.edu/aat/300264088>
                                               ]
                                             )
                               ] ;
               rdfs:comment "Represents the style of an artwork, such as Impressionism, Cubism, etc. This class allows for the classification of artworks based on their stylistic characteristics." ;
               rdfs:label "StyleType" .


###  http://w3id.org/arto#Symbolism
arto:Symbolism rdf:type owl:Class ;
               rdfs:subClassOf arto:Connotation ,
                               [ rdf:type owl:Restriction ;
                                 owl:onProperty arto:source ;
                                 owl:allValuesFrom xsd:string
                               ] ;
               rdfs:comment "Captures the symbolic meanings and iconographic content embedded in artwork elements. It connects to ICON ontology's symbolic framework while providing source property for symbolic interpretations. Symbolism instances can relate to mythological, religious, cultural, or personal symbolic systems, enabling systematic iconographic analysis and cross-cultural symbolic comparison." ;
               rdfs:label "Symbolism" ;
               skos:example """
    # Religious symbolism
    :dove_peace_symbolism rdf:type arto:Symbolism ;
        dc:description \"The dove as a symbol of peace and the Holy Spirit\" ;
        arto:source \"Christian tradition and Biblical references\" ;
        arto:isConnotationOf :dove_object .
        
    # Mythological symbolism
    :apple_temptation_symbolism rdf:type arto:Symbolism ;
        dc:description \"Apple as symbol of temptation and forbidden knowledge\" ;
        arto:source \"Biblical Genesis and Christian iconographic tradition\" ;
        arto:isConnotationOf :apple_object .
        
    # Cultural symbolism  
    :lotus_purity_symbolism rdf:type arto:Symbolism ;
        dc:description \"Lotus flower symbolising purity and spiritual awakening\" ;
        arto:source \"Buddhist and Hindu religious traditions\" ;
        arto:isConnotationOf :lotus_flower_object .
        
    # Historical symbolism
    :laurel_wreath_victory_symbolism rdf:type arto:Symbolism ;
        dc:description \"Laurel wreath as symbol of victory and honor\" ;
        arto:source \"Ancient Greek and Roman ceremonial traditions\" ;
        arto:isConnotationOf :laurel_crown_object .
""" .


###  http://w3id.org/arto#TechniqueType
arto:TechniqueType rdf:type owl:Class ;
                   rdfs:subClassOf [ rdf:type owl:Class ;
                                     owl:unionOf ( skos:Concept
                                                   [ rdf:type owl:Restriction ;
                                                     owl:onProperty skos:broaderTransitive ;
                                                     owl:hasValue <http://vocab.getty.edu/aat/300053001>
                                                   ]
                                                 )
                                   ] ;
                   rdfs:comment "Represents the specific artistic techniques used in creating artwork, drawing from Getty AAT's technique hierarchy while supporting custom undefined techniques." ;
                   rdfs:label "TechniqueType" .


###  http://w3id.org/arto#Theme
arto:Theme rdf:type owl:Class ;
           rdfs:subClassOf arto:Connotation ;
           rdfs:comment "Represents a central idea, subject, or concept explored in an artwork, which can be explicit or implicit, and may reflect broader cultural, social, or political issues." ;
           rdfs:label "Theme" .


###  http://w3id.org/arto#Time
arto:Time rdf:type owl:Class ;
          owl:equivalentClass <http://www.w3.org/2006/time#TemporalEntity> ;
          rdfs:subClassOf [ rdf:type owl:Restriction ;
                            owl:onProperty dc:type ;
                            owl:allValuesFrom xsd:string
                          ] ,
                          [ rdf:type owl:Restriction ;
                            owl:onProperty sdo:endDate ;
                            owl:allValuesFrom xsd:dateTime
                          ] ,
                          [ rdf:type owl:Restriction ;
                            owl:onProperty sdo:startDate ;
                            owl:allValuesFrom xsd:dateTime
                          ] ;
          rdfs:comment """Represents temporal aspects related to artwork, including:
            - Creation periods
            - Historical periods
            - Exhibition periods
            - Conservation periods
            - Depicted time periods
            - Time-based elements
            """ ;
          rdfs:label "Time" ;
          skos:example """
            - :renaissance_period rdf:type arto:Time ;
                sdo:startDate \"1400\" ;
                sdo:endDate \"1600\" .
                
            """ .


###  http://w3id.org/arto#VisualElement
arto:VisualElement rdf:type owl:Class ;
                   rdfs:subClassOf [ rdf:type owl:Restriction ;
                                     owl:onProperty arto:hasConnotation ;
                                     owl:allValuesFrom arto:Connotation
                                   ] ,
                                   [ rdf:type owl:Restriction ;
                                     owl:onProperty arto:hasMetric ;
                                     owl:allValuesFrom arto:Metric
                                   ] ;
                   rdfs:comment "Represents the fundamental visual components of an artwork, including: lines and shapes, colours and textures, forms and patterns, space and perspective, light and shadow, etc." ,
                                "Represents the fundamental visual components of artworks, including colours, lines, shapes, textures, and compositional structures. This abstract class serves as the foundation for systematic visual analysis, bridging computational image processing with art historical methodology. Visual elements can express connotations and have measurable properties, supporting both quantitative analysis (colour histograms, line density) and qualitative interpretation (symbolic colour use, expressive line quality). " ;
                   rdfs:label "VisualElement" .


###  http://www.cidoc-crm.org/cidoc-crm/E28_Conceptual_Object
crm:E28_Conceptual_Object rdf:type owl:Class .


###  http://www.opengis.net/ont/geosparql#wktLiteral
geo:wktLiteral rdf:type owl:Class .


###  http://www.w3.org/2006/time#TemporalEntity
<http://www.w3.org/2006/time#TemporalEntity> rdf:type owl:Class .


###  http://xmlns.com/foaf/spec/Agent
foaf:Agent rdf:type owl:Class .


###  http://xmlns.com/foaf/spec/Organization
foaf:Organization rdf:type owl:Class .


###  http://xmlns.com/foaf/spec/Person
foaf:Person rdf:type owl:Class .


###  https://schema.org/CreativeWork
sdo:CreativeWork rdf:type owl:Class .


###  https://schema.org/CreativeWorkSeries
sdo:CreativeWorkSeries rdf:type owl:Class .


###  https://schema.org/QuantitativeValue
sdo:QuantitativeValue rdf:type owl:Class .


###  https://w3id.org/MON/event.owl#Event
event:Event rdf:type owl:Class .


#################################################################
#    Individuals
#################################################################

###  http://purl.org/dc/terms/
<http://purl.org/dc/terms/> rdf:type owl:NamedIndividual ;
                            dc:modified "2012-06-14"^^xsd:date ;
                            dc:title "DCMI Metadata Terms - other"@en ;
                            dc:publisher <http://purl.org/dc/aboutdcmi#DCMI> .


###  http://purl.org/dc/terms/Agent
dc:Agent rdf:type owl:NamedIndividual ,
                  dc:AgentClass ;
         dc:issued "2008-01-14"^^xsd:date .


###  http://purl.org/dc/terms/AgentClass
dc:AgentClass rdf:type owl:NamedIndividual ;
              dc:issued "2008-01-14"^^xsd:date .


###  http://purl.org/dc/terms/BibliographicResource
dc:BibliographicResource rdf:type owl:NamedIndividual ;
                         dc:issued "2008-01-14"^^xsd:date .


###  http://purl.org/dc/terms/Box
dc:Box rdf:type owl:NamedIndividual ;
       dc:issued "2000-07-11"^^xsd:date .


###  http://purl.org/dc/terms/DCMIType
dc:DCMIType rdf:type owl:NamedIndividual ,
                     <http://purl.org/dc/dcam/VocabularyEncodingScheme> ;
            dc:issued "2000-07-11"^^xsd:date ;
            rdfs:comment "The set of classes specified by the DCMI Type Vocabulary, used to categorise the nature or genre of the resource."@en ,
                         "The set of classes specified by the DCMI Type Vocabulary, used to categorize the nature or genre of the resource."@en ;
            rdfs:isDefinedBy <http://purl.org/dc/terms/> ;
            rdfs:label "DCMI Type Vocabulary"@en ;
            rdfs:seeAlso <http://purl.org/dc/dcmitype/> .


###  http://purl.org/dc/terms/DDC
dc:DDC rdf:type owl:NamedIndividual ,
                <http://purl.org/dc/dcam/VocabularyEncodingScheme> ;
       dc:issued "2000-07-11"^^xsd:date ;
       rdfs:comment "The set of conceptual resources specified by the Dewey Decimal Classification."@en ;
       rdfs:isDefinedBy <http://purl.org/dc/terms/> ;
       rdfs:label "DDC"@en ;
       rdfs:seeAlso <http://www.oclc.org/dewey/> .


###  http://purl.org/dc/terms/FileFormat
dc:FileFormat rdf:type owl:NamedIndividual ;
              dc:issued "2008-01-14"^^xsd:date .


###  http://purl.org/dc/terms/Frequency
dc:Frequency rdf:type owl:NamedIndividual ;
             dc:issued "2008-01-14"^^xsd:date .


###  http://purl.org/dc/terms/IMT
dc:IMT rdf:type owl:NamedIndividual ,
                <http://purl.org/dc/dcam/VocabularyEncodingScheme> ;
       dc:issued "2000-07-11"^^xsd:date ;
       rdfs:comment "The set of media types specified by the Internet Assigned Numbers Authority."@en ;
       rdfs:isDefinedBy <http://purl.org/dc/terms/> ;
       rdfs:label "IMT"@en ;
       rdfs:seeAlso <http://www.iana.org/assignments/media-types/> .


###  http://purl.org/dc/terms/ISO3166
dc:ISO3166 rdf:type owl:NamedIndividual ;
           dc:issued "2000-07-11"^^xsd:date .


###  http://purl.org/dc/terms/ISO639-2
dc:ISO639-2 rdf:type owl:NamedIndividual ;
            dc:issued "2000-07-11"^^xsd:date .


###  http://purl.org/dc/terms/ISO639-3
dc:ISO639-3 rdf:type owl:NamedIndividual ;
            dc:issued "2008-01-14"^^xsd:date .


###  http://purl.org/dc/terms/Jurisdiction
dc:Jurisdiction rdf:type owl:NamedIndividual ;
                dc:issued "2008-01-14"^^xsd:date .


###  http://purl.org/dc/terms/LCC
dc:LCC rdf:type owl:NamedIndividual ,
                <http://purl.org/dc/dcam/VocabularyEncodingScheme> ;
       dc:issued "2000-07-11"^^xsd:date ;
       rdfs:comment "The set of conceptual resources specified by the Library of Congress Classification."@en ;
       rdfs:isDefinedBy <http://purl.org/dc/terms/> ;
       rdfs:label "LCC"@en ;
       rdfs:seeAlso <http://lcweb.loc.gov/catdir/cpso/lcco/lcco.html> .


###  http://purl.org/dc/terms/LCSH
dc:LCSH rdf:type owl:NamedIndividual ,
                 <http://purl.org/dc/dcam/VocabularyEncodingScheme> ;
        dc:issued "2000-07-11"^^xsd:date ;
        rdfs:comment "The set of labeled concepts specified by the Library of Congress Subject Headings."@en ;
        rdfs:isDefinedBy <http://purl.org/dc/terms/> ;
        rdfs:label "LCSH"@en .


###  http://purl.org/dc/terms/LicenseDocument
dc:LicenseDocument rdf:type owl:NamedIndividual ;
                   dc:issued "2008-01-14"^^xsd:date .


###  http://purl.org/dc/terms/LinguisticSystem
dc:LinguisticSystem rdf:type owl:NamedIndividual ;
                    dc:issued "2008-01-14"^^xsd:date .


###  http://purl.org/dc/terms/Location
dc:Location rdf:type owl:NamedIndividual ;
            dc:issued "2008-01-14"^^xsd:date .


###  http://purl.org/dc/terms/LocationPeriodOrJurisdiction
dc:LocationPeriodOrJurisdiction rdf:type owl:NamedIndividual ;
                                dc:issued "2008-01-14"^^xsd:date .


###  http://purl.org/dc/terms/MESH
dc:MESH rdf:type owl:NamedIndividual ,
                 <http://purl.org/dc/dcam/VocabularyEncodingScheme> ;
        dc:issued "2000-07-11"^^xsd:date ;
        rdfs:comment "The set of labeled concepts specified by the Medical Subject Headings."@en ;
        rdfs:isDefinedBy <http://purl.org/dc/terms/> ;
        rdfs:label "MeSH"@en ;
        rdfs:seeAlso <http://www.nlm.nih.gov/mesh/meshhome.html> .


###  http://purl.org/dc/terms/MediaType
dc:MediaType rdf:type owl:NamedIndividual ;
             dc:issued "2008-01-14"^^xsd:date .


###  http://purl.org/dc/terms/MediaTypeOrExtent
dc:MediaTypeOrExtent rdf:type owl:NamedIndividual ;
                     dc:issued "2008-01-14"^^xsd:date .


###  http://purl.org/dc/terms/MethodOfAccrual
dc:MethodOfAccrual rdf:type owl:NamedIndividual ;
                   dc:issued "2008-01-14"^^xsd:date .


###  http://purl.org/dc/terms/MethodOfInstruction
dc:MethodOfInstruction rdf:type owl:NamedIndividual ;
                       dc:issued "2008-01-14"^^xsd:date .


###  http://purl.org/dc/terms/NLM
dc:NLM rdf:type owl:NamedIndividual ,
                <http://purl.org/dc/dcam/VocabularyEncodingScheme> ;
       dc:issued "2005-06-13"^^xsd:date ;
       rdfs:comment "The set of conceptual resources specified by the National Library of Medicine Classification."@en ;
       rdfs:isDefinedBy <http://purl.org/dc/terms/> ;
       rdfs:label "NLM"@en ;
       rdfs:seeAlso <http://wwwcf.nlm.nih.gov/class/> .


###  http://purl.org/dc/terms/Period
dc:Period rdf:type owl:NamedIndividual ;
          dc:issued "2000-07-11"^^xsd:date .


###  http://purl.org/dc/terms/PeriodOfTime
dc:PeriodOfTime rdf:type owl:NamedIndividual ;
                dc:issued "2008-01-14"^^xsd:date .


###  http://purl.org/dc/terms/PhysicalMedium
dc:PhysicalMedium rdf:type owl:NamedIndividual ;
                  dc:issued "2008-01-14"^^xsd:date .


###  http://purl.org/dc/terms/PhysicalResource
dc:PhysicalResource rdf:type owl:NamedIndividual ;
                    dc:issued "2008-01-14"^^xsd:date .


###  http://purl.org/dc/terms/Point
dc:Point rdf:type owl:NamedIndividual ;
         dc:issued "2000-07-11"^^xsd:date .


###  http://purl.org/dc/terms/Policy
dc:Policy rdf:type owl:NamedIndividual ;
          dc:issued "2008-01-14"^^xsd:date .


###  http://purl.org/dc/terms/ProvenanceStatement
dc:ProvenanceStatement rdf:type owl:NamedIndividual ;
                       dc:issued "2008-01-14"^^xsd:date .


###  http://purl.org/dc/terms/RFC1766
dc:RFC1766 rdf:type owl:NamedIndividual ;
           dc:issued "2000-07-11"^^xsd:date .


###  http://purl.org/dc/terms/RFC3066
dc:RFC3066 rdf:type owl:NamedIndividual ;
           dc:issued "2002-07-13"^^xsd:date .


###  http://purl.org/dc/terms/RFC4646
dc:RFC4646 rdf:type owl:NamedIndividual ;
           dc:issued "2008-01-14"^^xsd:date .


###  http://purl.org/dc/terms/RFC5646
dc:RFC5646 rdf:type owl:NamedIndividual ;
           dc:issued "2010-10-11"^^xsd:date .


###  http://purl.org/dc/terms/RightsStatement
dc:RightsStatement rdf:type owl:NamedIndividual ;
                   dc:issued "2008-01-14"^^xsd:date .


###  http://purl.org/dc/terms/SizeOrDuration
dc:SizeOrDuration rdf:type owl:NamedIndividual ;
                  dc:issued "2008-01-14"^^xsd:date .


###  http://purl.org/dc/terms/Standard
dc:Standard rdf:type owl:NamedIndividual ;
            dc:issued "2008-01-14"^^xsd:date .


###  http://purl.org/dc/terms/TGN
dc:TGN rdf:type owl:NamedIndividual ,
                <http://purl.org/dc/dcam/VocabularyEncodingScheme> ;
       dc:issued "2000-07-11"^^xsd:date ;
       rdfs:comment "The set of places specified by the Getty Thesaurus of Geographic Names."@en ;
       rdfs:isDefinedBy <http://purl.org/dc/terms/> ;
       rdfs:label "TGN"@en ;
       rdfs:seeAlso <http://www.getty.edu/research/tools/vocabulary/tgn/index.html> .


###  http://purl.org/dc/terms/UDC
dc:UDC rdf:type owl:NamedIndividual ,
                <http://purl.org/dc/dcam/VocabularyEncodingScheme> ;
       dc:issued "2000-07-11"^^xsd:date ;
       rdfs:comment "The set of conceptual resources specified by the Universal Decimal Classification."@en ;
       rdfs:isDefinedBy <http://purl.org/dc/terms/> ;
       rdfs:label "UDC"@en ;
       rdfs:seeAlso <http://www.udcc.org/> .


###  http://purl.org/dc/terms/URI
dc:URI rdf:type owl:NamedIndividual ;
       dc:issued "2000-07-11"^^xsd:date .


###  http://purl.org/dc/terms/W3CDTF
dc:W3CDTF rdf:type owl:NamedIndividual ;
          dc:issued "2000-07-11"^^xsd:date .


###  http://purl.org/dc/terms/abstract
dc:abstract rdf:type owl:NamedIndividual ;
            dc:issued "2000-07-11"^^xsd:date .


###  http://purl.org/dc/terms/accessRights
dc:accessRights rdf:type owl:NamedIndividual ;
                dc:issued "2003-02-15"^^xsd:date .


###  http://purl.org/dc/terms/accrualMethod
dc:accrualMethod rdf:type owl:NamedIndividual ;
                 dc:issued "2005-06-13"^^xsd:date .


###  http://purl.org/dc/terms/accrualPeriodicity
dc:accrualPeriodicity rdf:type owl:NamedIndividual ;
                      dc:issued "2005-06-13"^^xsd:date .


###  http://purl.org/dc/terms/accrualPolicy
dc:accrualPolicy rdf:type owl:NamedIndividual ;
                 dc:issued "2005-06-13"^^xsd:date .


###  http://purl.org/dc/terms/alternative
dc:alternative rdf:type owl:NamedIndividual ;
               dc:issued "2000-07-11"^^xsd:date .


###  http://purl.org/dc/terms/audience
dc:audience rdf:type owl:NamedIndividual ;
            dc:issued "2001-05-21"^^xsd:date .


###  http://purl.org/dc/terms/available
dc:available rdf:type owl:NamedIndividual ;
             dc:issued "2000-07-11"^^xsd:date .


###  http://purl.org/dc/terms/bibliographicCitation
dc:bibliographicCitation rdf:type owl:NamedIndividual ;
                         dc:issued "2003-02-15"^^xsd:date .


###  http://purl.org/dc/terms/conformsTo
dc:conformsTo rdf:type owl:NamedIndividual ;
              dc:issued "2001-05-21"^^xsd:date .


###  http://purl.org/dc/terms/contributor
dc:contributor rdf:type owl:NamedIndividual ;
               dc:issued "2008-01-14"^^xsd:date .


###  http://purl.org/dc/terms/coverage
dc:coverage rdf:type owl:NamedIndividual ;
            dc:issued "2008-01-14"^^xsd:date .


###  http://purl.org/dc/terms/created
dc:created rdf:type owl:NamedIndividual ;
           dc:issued "2000-07-11"^^xsd:date .


###  http://purl.org/dc/terms/creator
dc:creator rdf:type owl:NamedIndividual ;
           dc:issued "2008-01-14"^^xsd:date .


###  http://purl.org/dc/terms/date
dc:date rdf:type owl:NamedIndividual ;
        dc:issued "2008-01-14"^^xsd:date .


###  http://purl.org/dc/terms/dateAccepted
dc:dateAccepted rdf:type owl:NamedIndividual ;
                dc:issued "2002-07-13"^^xsd:date .


###  http://purl.org/dc/terms/dateCopyrighted
dc:dateCopyrighted rdf:type owl:NamedIndividual ;
                   dc:issued "2002-07-13"^^xsd:date .


###  http://purl.org/dc/terms/dateSubmitted
dc:dateSubmitted rdf:type owl:NamedIndividual ;
                 dc:issued "2002-07-13"^^xsd:date .


###  http://purl.org/dc/terms/description
dc:description rdf:type owl:NamedIndividual ;
               dc:issued "2008-01-14"^^xsd:date .


###  http://purl.org/dc/terms/educationLevel
dc:educationLevel rdf:type owl:NamedIndividual ;
                  dc:issued "2002-07-13"^^xsd:date .


###  http://purl.org/dc/terms/extent
dc:extent rdf:type owl:NamedIndividual ;
          dc:issued "2000-07-11"^^xsd:date .


###  http://purl.org/dc/terms/format
dc:format rdf:type owl:NamedIndividual ;
          dc:issued "2008-01-14"^^xsd:date .


###  http://purl.org/dc/terms/hasFormat
dc:hasFormat rdf:type owl:NamedIndividual ;
             dc:issued "2000-07-11"^^xsd:date .


###  http://purl.org/dc/terms/hasPart
dc:hasPart rdf:type owl:NamedIndividual ;
           dc:issued "2000-07-11"^^xsd:date .


###  http://purl.org/dc/terms/hasVersion
dc:hasVersion rdf:type owl:NamedIndividual ;
              dc:issued "2000-07-11"^^xsd:date .


###  http://purl.org/dc/terms/identifier
dc:identifier rdf:type owl:NamedIndividual ;
              dc:issued "2008-01-14"^^xsd:date .


###  http://purl.org/dc/terms/instructionalMethod
dc:instructionalMethod rdf:type owl:NamedIndividual ;
                       dc:issued "2005-06-13"^^xsd:date ;
                       <http://purl.org/dc/dcam/rangeIncludes> dc:MethodOfInstruction ;
                       dc:description "Instructional Method typically includes ways of presenting instructional materials or conducting instructional activities, patterns of learner-to-learner and learner-to-instructor interactions, and mechanisms by which group and individual levels of learning are measured.  Instructional methods include all aspects of the instruction and learning processes from planning and implementation through evaluation and feedback."@en ;
                       rdfs:comment "A process, used to engender knowledge, attitudes and skills, that the described resource is designed to support."@en ;
                       rdfs:isDefinedBy <http://purl.org/dc/terms/> ;
                       rdfs:label "Instructional Method"@en .


###  http://purl.org/dc/terms/isFormatOf
dc:isFormatOf rdf:type owl:NamedIndividual ;
              dc:issued "2000-07-11"^^xsd:date .


###  http://purl.org/dc/terms/isPartOf
dc:isPartOf rdf:type owl:NamedIndividual ;
            dc:issued "2000-07-11"^^xsd:date .


###  http://purl.org/dc/terms/isReferencedBy
dc:isReferencedBy rdf:type owl:NamedIndividual ;
                  dc:issued "2000-07-11"^^xsd:date .


###  http://purl.org/dc/terms/isReplacedBy
dc:isReplacedBy rdf:type owl:NamedIndividual ;
                dc:issued "2000-07-11"^^xsd:date .


###  http://purl.org/dc/terms/isRequiredBy
dc:isRequiredBy rdf:type owl:NamedIndividual ;
                dc:issued "2000-07-11"^^xsd:date .


###  http://purl.org/dc/terms/isVersionOf
dc:isVersionOf rdf:type owl:NamedIndividual ;
               dc:issued "2000-07-11"^^xsd:date .


###  http://purl.org/dc/terms/issued
dc:issued rdf:type owl:NamedIndividual ;
          dc:issued "2000-07-11"^^xsd:date .


###  http://purl.org/dc/terms/language
dc:language rdf:type owl:NamedIndividual ;
            dc:issued "2008-01-14"^^xsd:date .


###  http://purl.org/dc/terms/license
dc:license rdf:type owl:NamedIndividual ;
           dc:issued "2004-06-14"^^xsd:date .


###  http://purl.org/dc/terms/mediator
dc:mediator rdf:type owl:NamedIndividual ;
            dc:issued "2001-05-21"^^xsd:date .


###  http://purl.org/dc/terms/medium
dc:medium rdf:type owl:NamedIndividual ;
          dc:issued "2000-07-11"^^xsd:date .


###  http://purl.org/dc/terms/modified
dc:modified rdf:type owl:NamedIndividual ;
            dc:issued "2000-07-11"^^xsd:date .


###  http://purl.org/dc/terms/provenance
dc:provenance rdf:type owl:NamedIndividual ;
              dc:issued "2004-09-20"^^xsd:date ;
              <http://purl.org/dc/dcam/rangeIncludes> dc:ProvenanceStatement ;
              dc:description "The statement may include a description of any changes successive custodians made to the resource."@en ;
              rdfs:comment "A statement of any changes in ownership and custody of the resource since its creation that are significant for its authenticity, integrity, and interpretation."@en ;
              rdfs:isDefinedBy <http://purl.org/dc/terms/> ;
              rdfs:label "Provenance"@en .


###  http://purl.org/dc/terms/publisher
dc:publisher rdf:type owl:NamedIndividual ;
             dc:issued "2008-01-14"^^xsd:date .


###  http://purl.org/dc/terms/references
dc:references rdf:type owl:NamedIndividual ;
              dc:issued "2000-07-11"^^xsd:date .


###  http://purl.org/dc/terms/relation
dc:relation rdf:type owl:NamedIndividual ;
            dc:issued "2008-01-14"^^xsd:date .


###  http://purl.org/dc/terms/replaces
dc:replaces rdf:type owl:NamedIndividual ;
            dc:issued "2000-07-11"^^xsd:date .


###  http://purl.org/dc/terms/requires
dc:requires rdf:type owl:NamedIndividual ;
            dc:issued "2000-07-11"^^xsd:date .


###  http://purl.org/dc/terms/rights
dc:rights rdf:type owl:NamedIndividual ;
          dc:issued "2008-01-14"^^xsd:date .


###  http://purl.org/dc/terms/rightsHolder
dc:rightsHolder rdf:type owl:NamedIndividual ;
                dc:issued "2004-06-14"^^xsd:date ;
                <http://purl.org/dc/dcam/rangeIncludes> dc:Agent ;
                dc:description "Recommended practice is to refer to the rights holder with a URI. If this is not possible or feasible, a literal value that identifies the rights holder may be provided."@en ;
                rdfs:comment "A person or organisation owning or managing rights over the resource."@en ,
                             "A person or organization owning or managing rights over the resource."@en ;
                rdfs:isDefinedBy <http://purl.org/dc/terms/> ;
                rdfs:label "Rights Holder"@en .


###  http://purl.org/dc/terms/source
dc:source rdf:type owl:NamedIndividual ;
          dc:issued "2008-01-14"^^xsd:date .


###  http://purl.org/dc/terms/spatial
dc:spatial rdf:type owl:NamedIndividual ;
           dc:issued "2000-07-11"^^xsd:date .


###  http://purl.org/dc/terms/subject
dc:subject rdf:type owl:NamedIndividual ;
           dc:issued "2008-01-14"^^xsd:date .


###  http://purl.org/dc/terms/tableOfContents
dc:tableOfContents rdf:type owl:NamedIndividual ;
                   dc:issued "2000-07-11"^^xsd:date .


###  http://purl.org/dc/terms/temporal
dc:temporal rdf:type owl:NamedIndividual ;
            dc:issued "2000-07-11"^^xsd:date .


###  http://purl.org/dc/terms/title
dc:title rdf:type owl:NamedIndividual ;
         dc:issued "2008-01-14"^^xsd:date .


###  http://purl.org/dc/terms/type
dc:type rdf:type owl:NamedIndividual ;
        dc:issued "2008-01-14"^^xsd:date .


###  http://purl.org/dc/terms/valid
dc:valid rdf:type owl:NamedIndividual ;
         dc:issued "2000-07-11"^^xsd:date .


###  http://vocab.getty.edu/aat/300053001
<http://vocab.getty.edu/aat/300053001> rdf:type owl:NamedIndividual .


###  http://vocab.getty.edu/aat/300056444
<http://vocab.getty.edu/aat/300056444> rdf:type owl:NamedIndividual .


###  http://vocab.getty.edu/aat/300131647
<http://vocab.getty.edu/aat/300131647> rdf:type owl:NamedIndividual .


###  http://vocab.getty.edu/aat/300264088
<http://vocab.getty.edu/aat/300264088> rdf:type owl:NamedIndividual .


###  http://vocab.getty.edu/aat/300264091
<http://vocab.getty.edu/aat/300264091> rdf:type owl:NamedIndividual .


[ owl:minCardinality "1"^^xsd:nonNegativeInteger
] .

[ owl:minCardinality "1"^^xsd:nonNegativeInteger
 ] .

[ owl:cardinality "1"^^xsd:nonNegativeInteger
 ] .

[ owl:cardinality "1"^^xsd:nonNegativeInteger
 ] .

[ owl:cardinality "1"^^xsd:nonNegativeInteger
 ] .

[ owl:minCardinality "0"^^xsd:nonNegativeInteger
 ] .

[ owl:cardinality "1"^^xsd:nonNegativeInteger
 ] .

[ owl:cardinality "1"^^xsd:nonNegativeInteger
 ] .

[ owl:cardinality "1"^^xsd:nonNegativeInteger
 ] .

[ owl:minCardinality "1"^^xsd:nonNegativeInteger
 ] .

[ owl:cardinality "1"^^xsd:nonNegativeInteger
 ] .

[ owl:minCardinality "1"^^xsd:nonNegativeInteger
 ] .

[ owl:cardinality "1"^^xsd:nonNegativeInteger
 ] .

[ owl:minCardinality "0"^^xsd:nonNegativeInteger
 ] .

[ owl:minCardinality "1"^^xsd:nonNegativeInteger
 ] .

[ owl:cardinality "1"^^xsd:nonNegativeInteger
 ] .

[ owl:cardinality "1"^^xsd:nonNegativeInteger
 ] .

[ owl:cardinality "1"^^xsd:nonNegativeInteger
 ] .

[ owl:minCardinality "1"^^xsd:nonNegativeInteger
 ] .

[ owl:cardinality "1"^^xsd:nonNegativeInteger
 ] .

[ owl:minCardinality "1"^^xsd:nonNegativeInteger
 ] .

[ owl:minCardinality "1"^^xsd:nonNegativeInteger
 ] .

[ owl:cardinality "1"^^xsd:nonNegativeInteger
 ] .

[ owl:cardinality "1"^^xsd:nonNegativeInteger
 ] .

[ owl:cardinality "1"^^xsd:nonNegativeInteger
 ] .

[ owl:minCardinality "1"^^xsd:nonNegativeInteger
 ] .

[ owl:minCardinality "1"^^xsd:nonNegativeInteger
 ] .

[ owl:maxCardinality "1"^^xsd:nonNegativeInteger
 ] .

[ owl:minCardinality "0"^^xsd:nonNegativeInteger
 ] .

[ owl:minCardinality "1"^^xsd:nonNegativeInteger
 ] .

[ owl:cardinality "1"^^xsd:nonNegativeInteger
 ] .

[ owl:cardinality "1"^^xsd:nonNegativeInteger
 ] .

[ owl:minCardinality "1"^^xsd:nonNegativeInteger
 ] .

[ owl:maxCardinality "1"^^xsd:nonNegativeInteger
 ] .

[ owl:cardinality "1"^^xsd:nonNegativeInteger
 ] .

[ owl:cardinality "1"^^xsd:nonNegativeInteger
 ] .

[ owl:cardinality "1"^^xsd:nonNegativeInteger
 ] .

[ owl:cardinality "1"^^xsd:nonNegativeInteger
 ] .

[ owl:cardinality "1"^^xsd:nonNegativeInteger
 ] .

[ owl:cardinality "1"^^xsd:nonNegativeInteger
 ] .

[ owl:cardinality "1"^^xsd:nonNegativeInteger
 ] .

[ owl:cardinality "1"^^xsd:nonNegativeInteger
 ] .

[ owl:cardinality "1"^^xsd:nonNegativeInteger
 ] .

[ owl:maxQualifiedCardinality "1"^^xsd:nonNegativeInteger
 ] .

[ owl:minCardinality "1"^^xsd:nonNegativeInteger
 ] .

[ owl:cardinality "1"^^xsd:nonNegativeInteger
 ] .

[ owl:cardinality "1"^^xsd:nonNegativeInteger
 ] .

[ owl:cardinality "1"^^xsd:nonNegativeInteger
 ] .

[ owl:cardinality "1"^^xsd:nonNegativeInteger
 ] .

[ owl:qualifiedCardinality "1"^^xsd:nonNegativeInteger
 ] .

#################################################################
#    Annotations
#################################################################

dc:Agent dc:issued "2008-01-14"^^xsd:date ;
          rdfs:comment "A resource that acts or has the power to act."@en ;
          rdfs:isDefinedBy <http://purl.org/dc/terms/> ;
          rdfs:label "Agent"@en .


dc:AgentClass dc:issued "2008-01-14"^^xsd:date ;
              rdfs:comment "A group of agents."@en ;
              rdfs:isDefinedBy <http://purl.org/dc/terms/> ;
              rdfs:label "Agent Class"@en .


dc:BibliographicResource dc:issued "2008-01-14"^^xsd:date ;
                         rdfs:comment "A book, article, or other documentary resource."@en ;
                         rdfs:isDefinedBy <http://purl.org/dc/terms/> ;
                         rdfs:label "Bibliographic Resource"@en .


dc:Box dc:issued "2000-07-11"^^xsd:date ;
       rdfs:comment "The set of regions in space defined by their geographic coordinates according to the DCMI Box Encoding Scheme."@en ;
       rdfs:isDefinedBy <http://purl.org/dc/terms/> ;
       rdfs:label "DCMI Box"@en ;
       rdfs:seeAlso <https://www.dublincore.org/specifications/dublin-core/dcmi-box/> .


dc:FileFormat dc:issued "2008-01-14"^^xsd:date ;
              rdfs:comment "A digital resource format."@en ;
              rdfs:isDefinedBy <http://purl.org/dc/terms/> ;
              rdfs:label "File Format"@en .


dc:Frequency dc:issued "2008-01-14"^^xsd:date ;
             rdfs:comment "A rate at which something recurs."@en ;
             rdfs:isDefinedBy <http://purl.org/dc/terms/> ;
             rdfs:label "Frequency"@en .


dc:ISO3166 dc:issued "2000-07-11"^^xsd:date ;
           rdfs:comment "The set of codes listed in ISO 3166-1 for the representation of names of countries."@en ;
           rdfs:isDefinedBy <http://purl.org/dc/terms/> ;
           rdfs:label "ISO 3166"@en ;
           rdfs:seeAlso <https://www.iso.org/obp/ui/#search> .


dc:ISO639-2 dc:issued "2000-07-11"^^xsd:date ;
            rdfs:comment "The three-letter alphabetic codes listed in ISO639-2 for the representation of names of languages."@en ;
            rdfs:isDefinedBy <http://purl.org/dc/terms/> ;
            rdfs:label "ISO 639-2"@en ;
            rdfs:seeAlso <http://lcweb.loc.gov/standards/iso639-2/langhome.html> .


dc:ISO639-3 dc:issued "2008-01-14"^^xsd:date ;
            rdfs:comment "The set of three-letter codes listed in ISO 639-3 for the representation of names of languages."@en ;
            rdfs:isDefinedBy <http://purl.org/dc/terms/> ;
            rdfs:label "ISO 639-3"@en ;
            rdfs:seeAlso <http://www.sil.org/iso639-3/> .


dc:Jurisdiction dc:issued "2008-01-14"^^xsd:date ;
                rdfs:comment "The extent or range of judicial, law enforcement, or other authority."@en ;
                rdfs:isDefinedBy <http://purl.org/dc/terms/> ;
                rdfs:label "Jurisdiction"@en .


dc:LicenseDocument dc:issued "2008-01-14"^^xsd:date ;
                   rdfs:comment "A legal document giving official permission to do something with a resource."@en ;
                   rdfs:isDefinedBy <http://purl.org/dc/terms/> ;
                   rdfs:label "License Document"@en .


dc:LinguisticSystem dc:description "Written, spoken, sign, and computer languages are linguistic systems."@en ;
                    dc:issued "2008-01-14"^^xsd:date ;
                    rdfs:comment "A system of signs, symbols, sounds, gestures, or rules used in communication."@en ;
                    rdfs:isDefinedBy <http://purl.org/dc/terms/> ;
                    rdfs:label "Linguistic System"@en .


dc:Location dc:issued "2008-01-14"^^xsd:date ;
            rdfs:comment "A spatial region or named place."@en ;
            rdfs:isDefinedBy <http://purl.org/dc/terms/> ;
            rdfs:label "Location"@en .


dc:LocationPeriodOrJurisdiction dc:issued "2008-01-14"^^xsd:date ;
                                rdfs:comment "A location, period of time, or jurisdiction."@en ;
                                rdfs:isDefinedBy <http://purl.org/dc/terms/> ;
                                rdfs:label "Location, Period, or Jurisdiction"@en .


dc:MediaType dc:issued "2008-01-14"^^xsd:date ;
             rdfs:comment "A file format or physical medium."@en ;
             rdfs:isDefinedBy <http://purl.org/dc/terms/> ;
             rdfs:label "Media Type"@en .


dc:MediaTypeOrExtent dc:issued "2008-01-14"^^xsd:date ;
                     rdfs:comment "A media type or extent."@en ;
                     rdfs:isDefinedBy <http://purl.org/dc/terms/> ;
                     rdfs:label "Media Type or Extent"@en .


dc:MethodOfAccrual dc:issued "2008-01-14"^^xsd:date ;
                   rdfs:comment "A method by which resources are added to a collection."@en ;
                   rdfs:isDefinedBy <http://purl.org/dc/terms/> ;
                   rdfs:label "Method of Accrual"@en .


dc:MethodOfInstruction dc:issued "2008-01-14"^^xsd:date ;
                       rdfs:comment "A process that is used to engender knowledge, attitudes, and skills."@en ;
                       rdfs:isDefinedBy <http://purl.org/dc/terms/> ;
                       rdfs:label "Method of Instruction"@en .


dc:Period dc:issued "2000-07-11"^^xsd:date ;
          rdfs:comment "The set of time intervals defined by their limits according to the DCMI Period Encoding Scheme."@en ;
          rdfs:isDefinedBy <http://purl.org/dc/terms/> ;
          rdfs:label "DCMI Period"@en ;
          rdfs:seeAlso <https://www.dublincore.org/specifications/dublin-core/dcmi-period/> .


dc:PeriodOfTime dc:issued "2008-01-14"^^xsd:date ;
                rdfs:comment "An interval of time that is named or defined by its start and end dates."@en ;
                rdfs:isDefinedBy <http://purl.org/dc/terms/> ;
                rdfs:label "Period of Time"@en .


dc:PhysicalMedium dc:description "Examples include paper, canvas, or DVD."@en ;
                  dc:issued "2008-01-14"^^xsd:date ;
                  rdfs:comment "A physical material or carrier."@en ;
                  rdfs:isDefinedBy <http://purl.org/dc/terms/> ;
                  rdfs:label "Physical Medium"@en .


dc:PhysicalResource dc:issued "2008-01-14"^^xsd:date ;
                    rdfs:comment "A material thing."@en ;
                    rdfs:isDefinedBy <http://purl.org/dc/terms/> ;
                    rdfs:label "Physical Resource"@en .


dc:Point dc:issued "2000-07-11"^^xsd:date ;
         rdfs:comment "The set of points in space defined by their geographic coordinates according to the DCMI Point Encoding Scheme."@en ;
         rdfs:isDefinedBy <http://purl.org/dc/terms/> ;
         rdfs:label "DCMI Point"@en ;
         rdfs:seeAlso <https://www.dublincore.org/specifications/dublin-core/dcmi-point/> .


dc:Policy dc:issued "2008-01-14"^^xsd:date ;
          rdfs:comment "A plan or course of action by an authority, intended to influence and determine decisions, actions, and other matters."@en ;
          rdfs:isDefinedBy <http://purl.org/dc/terms/> ;
          rdfs:label "Policy"@en .


dc:ProvenanceStatement dc:issued "2008-01-14"^^xsd:date ;
                       rdfs:comment "Any changes in ownership and custody of a resource since its creation that are significant for its authenticity, integrity, and interpretation."@en ;
                       rdfs:isDefinedBy <http://purl.org/dc/terms/> ;
                       rdfs:label "Provenance Statement"@en .


dc:RFC1766 dc:issued "2000-07-11"^^xsd:date ;
           rdfs:comment "The set of tags, constructed according to RFC 1766, for the identification of languages."@en ;
           rdfs:isDefinedBy <http://purl.org/dc/terms/> ;
           rdfs:label "RFC 1766"@en ;
           rdfs:seeAlso <http://www.ietf.org/rfc/rfc1766.txt> .


dc:RFC3066 dc:description "RFC 3066 has been obsoleted by RFC 4646."@en ;
           dc:issued "2002-07-13"^^xsd:date ;
           rdfs:comment "The set of tags constructed according to RFC 3066 for the identification of languages."@en ;
           rdfs:isDefinedBy <http://purl.org/dc/terms/> ;
           rdfs:label "RFC 3066"@en ;
           rdfs:seeAlso <http://www.ietf.org/rfc/rfc3066.txt> .


dc:RFC4646 dc:description "RFC 4646 obsoletes RFC 3066."@en ;
           dc:issued "2008-01-14"^^xsd:date ;
           rdfs:comment "The set of tags constructed according to RFC 4646 for the identification of languages."@en ;
           rdfs:isDefinedBy <http://purl.org/dc/terms/> ;
           rdfs:label "RFC 4646"@en ;
           rdfs:seeAlso <http://www.ietf.org/rfc/rfc4646.txt> .


dc:RFC5646 dc:description "RFC 5646 obsoletes RFC 4646."@en ;
           dc:issued "2010-10-11"^^xsd:date ;
           rdfs:comment "The set of tags constructed according to RFC 5646 for the identification of languages."@en ;
           rdfs:isDefinedBy <http://purl.org/dc/terms/> ;
           rdfs:label "RFC 5646"@en ;
           rdfs:seeAlso <http://www.ietf.org/rfc/rfc5646.txt> .


dc:RightsStatement dc:issued "2008-01-14"^^xsd:date ;
                   rdfs:comment "A statement about the intellectual property rights (IPR) held in or over a resource, a legal document giving official permission to do something with a resource, or a statement about access rights."@en ;
                   rdfs:isDefinedBy <http://purl.org/dc/terms/> ;
                   rdfs:label "Rights Statement"@en .


dc:SizeOrDuration dc:description "Examples include a number of pages, a specification of length, width, and breadth, or a period in hours, minutes, and seconds."@en ;
                  dc:issued "2008-01-14"^^xsd:date ;
                  rdfs:comment "A dimension or extent, or a time taken to play or execute."@en ;
                  rdfs:isDefinedBy <http://purl.org/dc/terms/> ;
                  rdfs:label "Size or Duration"@en .


dc:Standard dc:issued "2008-01-14"^^xsd:date ;
            rdfs:comment "A reference point against which other things can be evaluated or compared."@en ;
            rdfs:isDefinedBy <http://purl.org/dc/terms/> ;
            rdfs:label "Standard"@en .


dc:URI dc:issued "2000-07-11"^^xsd:date ;
       rdfs:comment "The set of identifiers constructed according to the generic syntax for Uniform Resource Identifiers as specified by the Internet Engineering Task Force."@en ;
       rdfs:isDefinedBy <http://purl.org/dc/terms/> ;
       rdfs:label "URI"@en ;
       rdfs:seeAlso <http://www.ietf.org/rfc/rfc3986.txt> .


dc:W3CDTF dc:issued "2000-07-11"^^xsd:date ;
          rdfs:comment "The set of dates and times constructed according to the W3C Date and Time Formats Specification."@en ;
          rdfs:isDefinedBy <http://purl.org/dc/terms/> ;
          rdfs:label "W3C-DTF"@en ;
          rdfs:seeAlso <http://www.w3.org/TR/NOTE-datetime> .


dc:abstract dc:issued "2000-07-11"^^xsd:date ;
            rdfs:comment "A summary of the resource."@en ;
            rdfs:isDefinedBy <http://purl.org/dc/terms/> ;
            rdfs:label "Abstract"@en .


dc:accessRights <http://purl.org/dc/dcam/rangeIncludes> dc:RightsStatement ;
                dc:description "Access Rights may include information regarding access or restrictions based on privacy, security, or other policies."@en ;
                dc:issued "2003-02-15"^^xsd:date ;
                rdfs:comment "Information about who access the resource or an indication of its security status."@en ;
                rdfs:isDefinedBy <http://purl.org/dc/terms/> ;
                rdfs:label "Access Rights"@en .


dc:accrualMethod <http://purl.org/dc/dcam/rangeIncludes> dc:MethodOfAccrual ;
                 dc:description "Recommended practice is to use a value from the Collection Description Accrual Method Vocabulary [[DCMI-ACCRUALMETHOD](https://dublincore.org/groups/collections/accrual-method/)]."@en ;
                 dc:issued "2005-06-13"^^xsd:date ;
                 rdfs:comment "The method by which items are added to a collection."@en ;
                 rdfs:isDefinedBy <http://purl.org/dc/terms/> ;
                 rdfs:label "Accrual Method"@en .


dc:accrualPeriodicity <http://purl.org/dc/dcam/rangeIncludes> dc:Frequency ;
                      dc:description "Recommended practice is to use a value from the Collection Description Frequency Vocabulary [[DCMI-COLLFREQ](https://dublincore.org/groups/collections/frequency/)]."@en ;
                      dc:issued "2005-06-13"^^xsd:date ;
                      rdfs:comment "The frequency with which items are added to a collection."@en ;
                      rdfs:isDefinedBy <http://purl.org/dc/terms/> ;
                      rdfs:label "Accrual Periodicity"@en .


dc:accrualPolicy <http://purl.org/dc/dcam/rangeIncludes> dc:Policy ;
                 dc:description "Recommended practice is to use a value from the Collection Description Accrual Policy Vocabulary [[DCMI-ACCRUALPOLICY](https://dublincore.org/groups/collections/accrual-policy/)]."@en ;
                 dc:issued "2005-06-13"^^xsd:date ;
                 rdfs:comment "The policy governing the addition of items to a collection."@en ;
                 rdfs:isDefinedBy <http://purl.org/dc/terms/> ;
                 rdfs:label "Accrual Policy"@en .


dc:alternative dc:description "The distinction between titles and alternative titles is application-specific."@en ;
               dc:issued "2000-07-11"^^xsd:date ;
               rdfs:comment "An alternative name for the resource."@en ;
               rdfs:isDefinedBy <http://purl.org/dc/terms/> ;
               rdfs:label "Alternative Title"@en .


dc:audience <http://purl.org/dc/dcam/rangeIncludes> dc:AgentClass ;
            dc:description "Recommended practice is to use this property with non-literal values from a vocabulary of audience types."@en ;
            dc:issued "2001-05-21"^^xsd:date ;
            rdfs:comment "A class of agents for whom the resource is intended or useful."@en ;
            rdfs:isDefinedBy <http://purl.org/dc/terms/> ;
            rdfs:label "Audience"@en .


dc:available dc:description "Recommended practice is to describe the date, date/time, or period of time as recommended for the property Date, of which this is a subproperty."@en ;
             dc:issued "2000-07-11"^^xsd:date ;
             rdfs:comment "Date that the resource became or will become available."@en ;
             rdfs:isDefinedBy <http://purl.org/dc/terms/> ;
             rdfs:label "Date Available"@en .


dc:bibliographicCitation dc:description "Recommended practice is to include sufficient bibliographic detail to identify the resource as unambiguously as possible."@en ;
                         dc:issued "2003-02-15"^^xsd:date ;
                         rdfs:comment "A bibliographic reference for the resource."@en ;
                         rdfs:isDefinedBy <http://purl.org/dc/terms/> ;
                         rdfs:label "Bibliographic Citation"@en .


dc:conformsTo <http://purl.org/dc/dcam/rangeIncludes> dc:Standard ;
              dc:issued "2001-05-21"^^xsd:date ;
              rdfs:comment "An established standard to which the described resource conforms."@en ;
              rdfs:isDefinedBy <http://purl.org/dc/terms/> ;
              rdfs:label "Conforms To"@en .


dc:contributor <http://purl.org/dc/dcam/rangeIncludes> dc:Agent ;
               dc:description "The guidelines for using names of persons or organisations as creators apply to contributors."@en ,
                              "The guidelines for using names of persons or organizations as creators apply to contributors."@en ;
               dc:issued "2008-01-14"^^xsd:date ;
               rdfs:comment "An entity responsible for making contributions to the resource."@en ;
               rdfs:isDefinedBy <http://purl.org/dc/terms/> ;
               rdfs:label "Contributor"@en .


dc:coverage <http://purl.org/dc/dcam/rangeIncludes> dc:Jurisdiction ,
                                                    dc:Location ,
                                                    dc:Period ;
            dc:description "Spatial topic and spatial applicability may be a named place or a location specified by its geographic coordinates. Temporal topic may be a named period, date, or date range. A jurisdiction may be a named administrative entity or a geographic place to which the resource applies. Recommended practice is to use a controlled vocabulary such as the Getty Thesaurus of Geographic Names [[TGN](https://www.getty.edu/research/tools/vocabulary/tgn/index.html)]. Where appropriate, named places or time periods may be used in preference to numeric identifiers such as sets of coordinates or date ranges.  Because coverage is so broadly defined, it is preferable to use the more specific subproperties Temporal Coverage and Spatial Coverage."@en ;
            dc:issued "2008-01-14"^^xsd:date ;
            rdfs:comment "The spatial or temporal topic of the resource, spatial applicability of the resource, or jurisdiction under which the resource is relevant."@en ;
            rdfs:isDefinedBy <http://purl.org/dc/terms/> ;
            rdfs:label "Coverage"@en .


dc:created dc:description "Recommended practice is to describe the date, date/time, or period of time as recommended for the property Date, of which this is a subproperty."@en ;
           dc:issued "2000-07-11"^^xsd:date ;
           rdfs:comment "Date of creation of the resource."@en ;
           rdfs:isDefinedBy <http://purl.org/dc/terms/> ;
           rdfs:label "Date Created"@en .


dc:creator <http://purl.org/dc/dcam/rangeIncludes> dc:Agent ;
           dc:description "Recommended practice is to identify the creator with a URI.  If this is not possible or feasible, a literal value that identifies the creator may be provided."@en ;
           dc:issued "2008-01-14"^^xsd:date ;
           rdfs:comment "An entity responsible for making the resource."@en ;
           rdfs:isDefinedBy <http://purl.org/dc/terms/> ;
           rdfs:label "Creator"@en .


dc:date dc:description "Date may be used to express temporal information at any level of granularity.  Recommended practice is to express the date, date/time, or period of time according to ISO 8601-1 [[ISO 8601-1](https://www.iso.org/iso-8601-date-and-time-format.html)] or a published profile of the ISO standard, such as the W3C Note on Date and Time Formats [[W3CDTF](https://www.w3.org/TR/NOTE-datetime)] or the Extended Date/Time Format Specification [[EDTF](http://www.loc.gov/standards/datetime/)].  If the full date is unknown, month and year (YYYY-MM) or just year (YYYY) may be used. Date ranges may be specified using ISO 8601 period of time specification in which start and end dates are separated by a '/' (slash) character.  Either the start or end date may be missing."@en ;
        dc:issued "2008-01-14"^^xsd:date ;
        rdfs:comment "A point or period of time associated with an event in the lifecycle of the resource."@en ;
        rdfs:isDefinedBy <http://purl.org/dc/terms/> ;
        rdfs:label "Date"@en .


dc:dateAccepted dc:description "Recommended practice is to describe the date, date/time, or period of time as recommended for the property Date, of which this is a subproperty.  Examples of resources to which a date of acceptance may be relevant are a thesis (accepted by a university department) or an article (accepted by a journal)."@en ;
                dc:issued "2002-07-13"^^xsd:date ;
                rdfs:comment "Date of acceptance of the resource."@en ;
                rdfs:isDefinedBy <http://purl.org/dc/terms/> ;
                rdfs:label "Date Accepted"@en .


dc:dateCopyrighted dc:description "Typically a year.  Recommended practice is to describe the date, date/time, or period of time as recommended for the property Date, of which this is a subproperty."@en ;
                   dc:issued "2002-07-13"^^xsd:date ;
                   rdfs:comment "Date of copyright of the resource."@en ;
                   rdfs:isDefinedBy <http://purl.org/dc/terms/> ;
                   rdfs:label "Date Copyrighted"@en .


dc:dateSubmitted dc:description "Recommended practice is to describe the date, date/time, or period of time as recommended for the property Date, of which this is a subproperty.  Examples of resources to which a 'Date Submitted' may be relevant include a thesis (submitted to a university department) or an article (submitted to a journal)."@en ;
                 dc:issued "2002-07-13"^^xsd:date ;
                 rdfs:comment "Date of submission of the resource."@en ;
                 rdfs:isDefinedBy <http://purl.org/dc/terms/> ;
                 rdfs:label "Date Submitted"@en .


dc:description dc:description "Description may include but is not limited to: an abstract, a table of contents, a graphical representation, or a free-text account of the resource."@en ;
               dc:issued "2008-01-14"^^xsd:date ;
               rdfs:comment "An account of the resource."@en ;
               rdfs:isDefinedBy <http://purl.org/dc/terms/> ;
               rdfs:label "Description"@en .


dc:educationLevel <http://purl.org/dc/dcam/rangeIncludes> dc:AgentClass ;
                  dc:issued "2002-07-13"^^xsd:date ;
                  rdfs:comment "A class of agents, defined in terms of progression through an educational or training context, for which the described resource is intended."@en ;
                  rdfs:isDefinedBy <http://purl.org/dc/terms/> ;
                  rdfs:label "Audience Education Level"@en .


dc:extent <http://purl.org/dc/dcam/rangeIncludes> dc:SizeOrDuration ;
          dc:description "Recommended practice is to specify the file size in megabytes and duration in ISO 8601 format."@en ;
          dc:issued "2000-07-11"^^xsd:date ;
          rdfs:comment "The size or duration of the resource."@en ;
          rdfs:isDefinedBy <http://purl.org/dc/terms/> ;
          rdfs:label "Extent"@en .


dc:format <http://purl.org/dc/dcam/rangeIncludes> dc:Extent ,
                                                  dc:MediaType ;
          dc:description "Recommended practice is to use a controlled vocabulary where available. For example, for file formats one could use the list of Internet Media Types [[MIME](https://www.iana.org/assignments/media-types/media-types.xhtml)].  Examples of dimensions include size and duration."@en ;
          dc:issued "2008-01-14"^^xsd:date ;
          rdfs:comment "The file format, physical medium, or dimensions of the resource."@en ;
          rdfs:isDefinedBy <http://purl.org/dc/terms/> ;
          rdfs:label "Format"@en .


dc:hasFormat dc:description "This property is intended to be used with non-literal values. This property is an inverse property of Is Format Of."@en ;
             dc:issued "2000-07-11"^^xsd:date ;
             rdfs:comment "A related resource that is substantially the same as the pre-existing described resource, but in another format."@en ;
             rdfs:isDefinedBy <http://purl.org/dc/terms/> ;
             rdfs:label "Has Format"@en .


dc:hasPart dc:description "This property is intended to be used with non-literal values. This property is an inverse property of Is Part Of."@en ;
           dc:issued "2000-07-11"^^xsd:date ;
           rdfs:comment "A related resource that is included either physically or logically in the described resource."@en ;
           rdfs:isDefinedBy <http://purl.org/dc/terms/> ;
           rdfs:label "Has Part"@en .


dc:hasVersion dc:description "Changes in version imply substantive changes in content rather than differences in format. This property is intended to be used with non-literal values. This property is an inverse property of Is Version Of."@en ;
              dc:issued "2000-07-11"^^xsd:date ;
              rdfs:comment "A related resource that is a version, edition, or adaptation of the described resource."@en ;
              rdfs:isDefinedBy <http://purl.org/dc/terms/> ;
              rdfs:label "Has Version"@en .


dc:identifier dc:description "Recommended practice is to identify the resource by means of a string conforming to an identification system. Examples include International Standard Book Number (ISBN), Digital Object Identifier (DOI), and Uniform Resource Name (URN).  Persistent identifiers should be provided as HTTP URIs."@en ;
              dc:issued "2008-01-14"^^xsd:date ;
              rdfs:comment "An unambiguous reference to the resource within a given context."@en ;
              rdfs:isDefinedBy <http://purl.org/dc/terms/> ;
              rdfs:label "Identifier"@en .


dc:isFormatOf dc:description "This property is intended to be used with non-literal values. This property is an inverse property of Has Format."@en ;
              dc:issued "2000-07-11"^^xsd:date ;
              rdfs:comment "A pre-existing related resource that is substantially the same as the described resource, but in another format."@en ;
              rdfs:isDefinedBy <http://purl.org/dc/terms/> ;
              rdfs:label "Is Format Of"@en .


dc:isPartOf dc:description "This property is intended to be used with non-literal values. This property is an inverse property of Has Part."@en ;
            dc:issued "2000-07-11"^^xsd:date ;
            rdfs:comment "A related resource in which the described resource is physically or logically included."@en ;
            rdfs:isDefinedBy <http://purl.org/dc/terms/> ;
            rdfs:label "Is Part Of"@en .


dc:isReferencedBy dc:description "This property is intended to be used with non-literal values. This property is an inverse property of References."@en ;
                  dc:issued "2000-07-11"^^xsd:date ;
                  rdfs:comment "A related resource that references, cites, or otherwise points to the described resource."@en ;
                  rdfs:isDefinedBy <http://purl.org/dc/terms/> ;
                  rdfs:label "Is Referenced By"@en .


dc:isReplacedBy dc:description "This property is intended to be used with non-literal values. This property is an inverse property of Replaces."@en ;
                dc:issued "2000-07-11"^^xsd:date ;
                rdfs:comment "A related resource that supplants, displaces, or supersedes the described resource."@en ;
                rdfs:isDefinedBy <http://purl.org/dc/terms/> ;
                rdfs:label "Is Replaced By"@en .


dc:isRequiredBy dc:description "This property is intended to be used with non-literal values. This property is an inverse property of Requires."@en ;
                dc:issued "2000-07-11"^^xsd:date ;
                rdfs:comment "A related resource that requires the described resource to support its function, delivery, or coherence."@en ;
                rdfs:isDefinedBy <http://purl.org/dc/terms/> ;
                rdfs:label "Is Required By"@en .


dc:isVersionOf dc:description "Changes in version imply substantive changes in content rather than differences in format. This property is intended to be used with non-literal values. This property is an inverse property of Has Version."@en ;
               dc:issued "2000-07-11"^^xsd:date ;
               rdfs:comment "A related resource of which the described resource is a version, edition, or adaptation."@en ;
               rdfs:isDefinedBy <http://purl.org/dc/terms/> ;
               rdfs:label "Is Version Of"@en .


dc:issued dc:description "Recommended practice is to describe the date, date/time, or period of time as recommended for the property Date, of which this is a subproperty."@en ;
          dc:issued "2000-07-11"^^xsd:date ;
          rdfs:comment "Date of formal issuance of the resource."@en ;
          rdfs:isDefinedBy <http://purl.org/dc/terms/> ;
          rdfs:label "Date Issued"@en .


dc:language <http://purl.org/dc/dcam/rangeIncludes> dc:LinguisticSystem ;
            dc:description "Recommended practice is to use either a non-literal value representing a language from a controlled vocabulary such as ISO 639-2 or ISO 639-3, or a literal value consisting of an IETF Best Current Practice 47 [[IETF-BCP47](https://tools.ietf.org/html/bcp47)] language tag."@en ;
            dc:issued "2008-01-14"^^xsd:date ;
            rdfs:comment "A language of the resource."@en ;
            rdfs:isDefinedBy <http://purl.org/dc/terms/> ;
            rdfs:label "Language"@en .


dc:license <http://purl.org/dc/dcam/rangeIncludes> dc:LicenseDocument ;
           dc:description "Recommended practice is to identify the license document with a URI. If this is not possible or feasible, a literal value that identifies the license may be provided."@en ;
           dc:issued "2004-06-14"^^xsd:date ;
           rdfs:comment "A legal document giving official permission to do something with the resource."@en ;
           rdfs:isDefinedBy <http://purl.org/dc/terms/> ;
           rdfs:label "License"@en .


dc:mediator <http://purl.org/dc/dcam/rangeIncludes> dc:AgentClass ;
            dc:description "In an educational context, a mediator might be a parent, teacher, teaching assistant, or care-giver."@en ;
            dc:issued "2001-05-21"^^xsd:date ;
            rdfs:comment "An entity that mediates access to the resource."@en ;
            rdfs:isDefinedBy <http://purl.org/dc/terms/> ;
            rdfs:label "Mediator"@en .


dc:medium <http://purl.org/dc/dcam/domainIncludes> dc:PhysicalResource ;
          <http://purl.org/dc/dcam/rangeIncludes> dc:PhysicalMedium ;
          dc:issued "2000-07-11"^^xsd:date ;
          rdfs:comment "The material or physical carrier of the resource."@en ;
          rdfs:isDefinedBy <http://purl.org/dc/terms/> ;
          rdfs:label "Medium"@en .


dc:modified dc:description "Recommended practice is to describe the date, date/time, or period of time as recommended for the property Date, of which this is a subproperty."@en ;
            dc:issued "2000-07-11"^^xsd:date ;
            rdfs:comment "Date on which the resource was changed."@en ;
            rdfs:isDefinedBy <http://purl.org/dc/terms/> ;
            rdfs:label "Date Modified"@en .


dc:publisher <http://purl.org/dc/dcam/rangeIncludes> dc:Agent ;
             dc:issued "2008-01-14"^^xsd:date ;
             rdfs:comment "An entity responsible for making the resource available."@en ;
             rdfs:isDefinedBy <http://purl.org/dc/terms/> ;
             rdfs:label "Publisher"@en .


dc:references dc:description "This property is intended to be used with non-literal values. This property is an inverse property of Is Referenced By."@en ;
              dc:issued "2000-07-11"^^xsd:date ;
              rdfs:comment "A related resource that is referenced, cited, or otherwise pointed to by the described resource."@en ;
              rdfs:isDefinedBy <http://purl.org/dc/terms/> ;
              rdfs:label "References"@en .


dc:relation dc:description "Recommended practice is to identify the related resource by means of a URI.  If this is not possible or feasible, a string conforming to a formal identification system may be provided."@en ;
            dc:issued "2008-01-14"^^xsd:date ;
            rdfs:comment "A related resource."@en ;
            rdfs:isDefinedBy <http://purl.org/dc/terms/> ;
            rdfs:label "Relation"@en .


dc:replaces dc:description "This property is intended to be used with non-literal values. This property is an inverse property of Is Replaced By."@en ;
            dc:issued "2000-07-11"^^xsd:date ;
            rdfs:comment "A related resource that is supplanted, displaced, or superseded by the described resource."@en ;
            rdfs:isDefinedBy <http://purl.org/dc/terms/> ;
            rdfs:label "Replaces"@en .


dc:requires dc:description "This property is intended to be used with non-literal values. This property is an inverse property of Is Required By."@en ;
            dc:issued "2000-07-11"^^xsd:date ;
            rdfs:comment "A related resource that is required by the described resource to support its function, delivery, or coherence."@en ;
            rdfs:isDefinedBy <http://purl.org/dc/terms/> ;
            rdfs:label "Requires"@en .


dc:rights <http://purl.org/dc/dcam/rangeIncludes> dc:RightsStatement ;
          dc:description "Typically, rights information includes a statement about various property rights associated with the resource, including intellectual property rights.  Recommended practice is to refer to a rights statement with a URI.  If this is not possible or feasible, a literal value (name, label, or short text) may be provided."@en ;
          dc:issued "2008-01-14"^^xsd:date ;
          rdfs:comment "Information about rights held in and over the resource."@en ;
          rdfs:isDefinedBy <http://purl.org/dc/terms/> ;
          rdfs:label "Rights"@en .


dc:source dc:description "This property is intended to be used with non-literal values. The described resource may be derived from the related resource in whole or in part. Best practice is to identify the related resource by means of a URI or a string conforming to a formal identification system."@en ;
          dc:issued "2008-01-14"^^xsd:date ;
          rdfs:comment "A related resource from which the described resource is derived."@en ;
          rdfs:isDefinedBy <http://purl.org/dc/terms/> ;
          rdfs:label "Source"@en .


dc:spatial <http://purl.org/dc/dcam/rangeIncludes> dc:Location ;
           dc:issued "2000-07-11"^^xsd:date ;
           rdfs:comment "Spatial characteristics of the resource."@en ;
           rdfs:isDefinedBy <http://purl.org/dc/terms/> ;
           rdfs:label "Spatial Coverage"@en .


dc:subject dc:description "Recommended practice is to refer to the subject with a URI. If this is not possible or feasible, a literal value that identifies the subject may be provided. Both should preferably refer to a subject in a controlled vocabulary."@en ;
           dc:issued "2008-01-14"^^xsd:date ;
           rdfs:comment "A topic of the resource."@en ;
           rdfs:isDefinedBy <http://purl.org/dc/terms/> ;
           rdfs:label "Subject"@en .


dc:tableOfContents dc:issued "2000-07-11"^^xsd:date ;
                   rdfs:comment "A list of subunits of the resource."@en ;
                   rdfs:isDefinedBy <http://purl.org/dc/terms/> ;
                   rdfs:label "Table Of Contents"@en .


dc:temporal <http://purl.org/dc/dcam/rangeIncludes> dc:PeriodOfTime ;
            dc:issued "2000-07-11"^^xsd:date ;
            rdfs:comment "Temporal characteristics of the resource."@en ;
            rdfs:isDefinedBy <http://purl.org/dc/terms/> ;
            rdfs:label "Temporal Coverage"@en .


dc:title dc:issued "2008-01-14"^^xsd:date ;
         rdfs:comment "A name given to the resource."@en ;
         rdfs:isDefinedBy <http://purl.org/dc/terms/> ;
         rdfs:label "Title"@en .


dc:type dc:description "Recommended practice is to use a controlled vocabulary such as the DCMI Type Vocabulary [[DCMI-TYPE](http://dublincore.org/documents/dcmi-type-vocabulary/)]. To describe the file format, physical medium, or dimensions of the resource, use the property Format."@en ;
        dc:issued "2008-01-14"^^xsd:date ;
        rdfs:comment "The nature or genre of the resource."@en ;
        rdfs:isDefinedBy <http://purl.org/dc/terms/> ;
        rdfs:label "Type"@en .


dc:valid dc:description "Recommended practice is to describe the date, date/time, or period of time as recommended for the property Date, of which this is a subproperty."@en ;
         dc:issued "2000-07-11"^^xsd:date ;
         rdfs:comment "Date (often a range) of validity of a resource."@en ;
         rdfs:isDefinedBy <http://purl.org/dc/terms/> ;
         rdfs:label "Date Valid"@en .


###  Generated by the OWL API (version 4.5.25.2023-02-15T19:15:49Z) https://github.com/owlcs/owlapi
