<rdf:RDF
    xmlns:qudt="http://qudt.org/schema/qudt/"
    xmlns:rdf="http://www.w3.org/1999/02/22-rdf-syntax-ns#"
    xmlns:sdo="https://schema.org/"
    xmlns:aat="http://vocab.getty.edu/aat/"
    xmlns:gn="https://www.geonames.org/ontology#"
    xmlns:crm="http://www.cidoc-crm.org/cidoc-crm/"
    xmlns:event="https://w3id.org/MON/event.owl#"
    xmlns:foaf="http://xmlns.com/foaf/spec/"
    xmlns:edm="http://www.europeana.eu/schemas/edm/"
    xmlns:rdfs="http://www.w3.org/2000/01/rdf-schema#"
    xmlns:dc="http://purl.org/dc/terms/"
    xmlns:ebucore="http://www.ebu.ch/metadata/ontologies/ebucore/ebucore#"
    xmlns:mfoem="http://purl.obolibrary.org/obo/"
    xmlns:owl="http://www.w3.org/2002/07/owl#"
    xmlns:skos="http://www.w3.org/2004/02/skos/core#"
    xmlns:dbp="https://dbpedia.org/property/"
    xmlns:j.0="http://purl.org/dc/dcam/"
    xmlns:geo="http://www.opengis.net/ont/geosparql#"
    xmlns:vann="http://purl.org/vocab/vann/"
    xmlns:cc="http://creativecommons.org/ns#"
    xmlns:arto="http://w3id.org/arto#"
    xmlns:xsd="http://www.w3.org/2001/XMLSchema#"
    xmlns:icon="https://w3id.org/icon/ontology/" > 
  <rdf:Description rdf:nodeID="A0">
    <owl:cardinality rdf:datatype="http://www.w3.org/2001/XMLSchema#nonNegativeInteger">1</owl:cardinality>
  </rdf:Description>
  <rdf:Description rdf:about="http://purl.org/dc/terms/W3CDTF">
    <rdfs:seeAlso rdf:resource="http://www.w3.org/TR/NOTE-datetime"/>
    <rdfs:label xml:lang="en">W3C-DTF</rdfs:label>
    <rdfs:isDefinedBy rdf:resource="http://purl.org/dc/terms/"/>
    <rdfs:comment xml:lang="en">The set of dates and times constructed according to the W3C Date and Time Formats Specification.</rdfs:comment>
    <dc:issued rdf:datatype="http://www.w3.org/2001/XMLSchema#date">2000-07-11</dc:issued>
    <rdf:type rdf:resource="http://www.w3.org/2002/07/owl#NamedIndividual"/>
    <rdf:type rdf:resource="http://www.w3.org/2000/01/rdf-schema#Datatype"/>
  </rdf:Description>
  <rdf:Description rdf:nodeID="A1">
    <rdf:rest rdf:nodeID="A2"/>
    <rdf:first rdf:resource="http://www.w3.org/2004/02/skos/core#Concept"/>
  </rdf:Description>
  <rdf:Description rdf:nodeID="A3">
    <rdf:rest rdf:resource="http://www.w3.org/1999/02/22-rdf-syntax-ns#nil"/>
    <rdf:first rdf:resource="http://w3id.org/arto#VisualElement"/>
  </rdf:Description>
  <rdf:Description rdf:nodeID="A4">
    <rdf:rest rdf:nodeID="A5"/>
    <rdf:first rdf:resource="http://w3id.org/arto#Artwork"/>
  </rdf:Description>
  <rdf:Description rdf:about="http://purl.org/dc/terms/tableOfContents">
    <rdfs:label xml:lang="en">Table Of Contents</rdfs:label>
    <rdfs:isDefinedBy rdf:resource="http://purl.org/dc/terms/"/>
    <rdfs:comment xml:lang="en">A list of subunits of the resource.</rdfs:comment>
    <dc:issued rdf:datatype="http://www.w3.org/2001/XMLSchema#date">2000-07-11</dc:issued>
    <rdf:type rdf:resource="http://www.w3.org/2002/07/owl#NamedIndividual"/>
    <rdfs:subPropertyOf rdf:resource="http://purl.org/dc/terms/description"/>
    <rdfs:subPropertyOf rdf:resource="http://purl.org/dc/elements/1.1/description"/>
    <rdf:type rdf:resource="http://www.w3.org/2002/07/owl#AnnotationProperty"/>
  </rdf:Description>
  <rdf:Description rdf:about="http://purl.org/dc/terms/extent">
    <rdfs:label xml:lang="en">Extent</rdfs:label>
    <rdfs:isDefinedBy rdf:resource="http://purl.org/dc/terms/"/>
    <rdfs:comment xml:lang="en">The size or duration of the resource.</rdfs:comment>
    <dc:description xml:lang="en">Recommended practice is to specify the file size in megabytes and duration in ISO 8601 format.</dc:description>
    <j.0:rangeIncludes rdf:resource="http://purl.org/dc/terms/SizeOrDuration"/>
    <dc:issued rdf:datatype="http://www.w3.org/2001/XMLSchema#date">2000-07-11</dc:issued>
    <rdf:type rdf:resource="http://www.w3.org/2002/07/owl#NamedIndividual"/>
    <rdfs:subPropertyOf rdf:resource="http://purl.org/dc/terms/format"/>
    <rdfs:subPropertyOf rdf:resource="http://purl.org/dc/elements/1.1/format"/>
    <rdf:type rdf:resource="http://www.w3.org/2002/07/owl#AnnotationProperty"/>
  </rdf:Description>
  <rdf:Description rdf:about="https://schema.org/endDate">
    <rdf:type rdf:resource="http://www.w3.org/2002/07/owl#DatatypeProperty"/>
  </rdf:Description>
  <rdf:Description rdf:nodeID="A6">
    <owl:onClass rdf:resource="http://w3id.org/arto#Location"/>
    <owl:maxQualifiedCardinality rdf:datatype="http://www.w3.org/2001/XMLSchema#nonNegativeInteger">1</owl:maxQualifiedCardinality>
    <owl:onProperty rdf:resource="http://w3id.org/arto#currentLocation"/>
    <rdf:type rdf:resource="http://www.w3.org/2002/07/owl#Restriction"/>
  </rdf:Description>
  <rdf:Description rdf:about="http://creativecommons.org/ns#attributionURL">
    <rdf:type rdf:resource="http://www.w3.org/2002/07/owl#AnnotationProperty"/>
  </rdf:Description>
  <rdf:Description rdf:about="http://w3id.org/arto#Artist">
    <rdfs:label>Artist</rdfs:label>
    <rdfs:comment>The person or group who create or contribute the artwork.</rdfs:comment>
    <rdfs:subClassOf rdf:resource="http://w3id.org/arto#Person"/>
    <rdf:type rdf:resource="http://www.w3.org/2002/07/owl#Class"/>
  </rdf:Description>
  <rdf:Description rdf:nodeID="A7">
    <owl:someValuesFrom rdf:resource="http://w3id.org/arto#Location"/>
    <owl:onProperty rdf:resource="http://w3id.org/arto#hasLocation"/>
    <rdf:type rdf:resource="http://www.w3.org/2002/07/owl#Restriction"/>
  </rdf:Description>
  <rdf:Description rdf:about="http://purl.org/dc/terms/abstract">
    <rdfs:label xml:lang="en">Abstract</rdfs:label>
    <rdfs:isDefinedBy rdf:resource="http://purl.org/dc/terms/"/>
    <rdfs:comment xml:lang="en">A summary of the resource.</rdfs:comment>
    <dc:issued rdf:datatype="http://www.w3.org/2001/XMLSchema#date">2000-07-11</dc:issued>
    <rdf:type rdf:resource="http://www.w3.org/2002/07/owl#NamedIndividual"/>
    <rdfs:subPropertyOf rdf:resource="http://purl.org/dc/terms/description"/>
    <rdfs:subPropertyOf rdf:resource="http://purl.org/dc/elements/1.1/description"/>
    <rdf:type rdf:resource="http://www.w3.org/2002/07/owl#AnnotationProperty"/>
  </rdf:Description>
  <rdf:Description rdf:about="http://vocab.getty.edu/aat/300053001">
    <rdf:type rdf:resource="http://www.w3.org/2002/07/owl#NamedIndividual"/>
  </rdf:Description>
  <rdf:Description rdf:about="http://w3id.org/arto#relatedToEvent">
    <skos:example>
                      - Historical event: :liberty_leading_the_people arto:relatedToEvent :french_revolution_1830
                      - Biblical event: :last_supper arto:relatedToEvent :biblical_last_supper
                      </skos:example>
    <rdfs:label>relatedToEvent</rdfs:label>
    <rdfs:comment>Connects an artwork or its scene to historical, mythological, or contemporary events depicted or referenced in the work.</rdfs:comment>
    <rdfs:range rdf:resource="http://w3id.org/arto#Event"/>
    <rdfs:domain rdf:nodeID="A8"/>
    <rdf:type rdf:resource="http://www.w3.org/2002/07/owl#ObjectProperty"/>
  </rdf:Description>
  <rdf:Description rdf:about="http://w3id.org/arto#relatedTo">
    <skos:example>
                - Spatial relation: :cup_object arto:rests_on :table_object ;
                  arto:rests_on rdfs:subPropertyOf arto:relatedTo;
                - Interaction: :mother_figure arto:holds :child_figure ;
                  arto:holds rdfs:subPropertyOf arto:relatedTo;
                - Position: :cloud_object arto:above :mountain_object ;
                  arto:above rdfs:subPropertyOf arto:relatedTo ;
                - Position: :tree_object arto:behind :house_object ;
                  arto:behind rdfs:subPropertyOf arto:relatedTo ;</skos:example>
    <rdfs:label>relatedTo</rdfs:label>
    <rdfs:comment>Describes spatial or conceptual relationships between objects within artworks. This extensible property enables specific relationship types (behind, holds, above) through subproperty mechanisms, supporting detailed spatial analysis while maintaining semantic clarity.</rdfs:comment>
    <rdfs:range rdf:resource="http://w3id.org/arto#Object"/>
    <rdfs:domain rdf:resource="http://w3id.org/arto#Object"/>
    <rdf:type rdf:resource="http://www.w3.org/2002/07/owl#ObjectProperty"/>
  </rdf:Description>
  <rdf:Description rdf:about="http://w3id.org/arto#Symbolism">
    <skos:example>
    # Religious symbolism
    :dove_peace_symbolism rdf:type arto:Symbolism ;
        dc:description "The dove as a symbol of peace and the Holy Spirit" ;
        arto:source "Christian tradition and Biblical references" ;
        arto:isConnotationOf :dove_object .
        
    # Mythological symbolism
    :apple_temptation_symbolism rdf:type arto:Symbolism ;
        dc:description "Apple as symbol of temptation and forbidden knowledge" ;
        arto:source "Biblical Genesis and Christian iconographic tradition" ;
        arto:isConnotationOf :apple_object .
        
    # Cultural symbolism  
    :lotus_purity_symbolism rdf:type arto:Symbolism ;
        dc:description "Lotus flower symbolising purity and spiritual awakening" ;
        arto:source "Buddhist and Hindu religious traditions" ;
        arto:isConnotationOf :lotus_flower_object .
        
    # Historical symbolism
    :laurel_wreath_victory_symbolism rdf:type arto:Symbolism ;
        dc:description "Laurel wreath as symbol of victory and honour" ;
        arto:source "Ancient Greek and Roman ceremonial traditions" ;
        arto:isConnotationOf :laurel_crown_object .
</skos:example>
    <rdfs:label>Symbolism</rdfs:label>
    <rdfs:comment>Captures the symbolic meanings and iconographic content embedded in artwork elements. It connects to ICON ontology's symbolic framework while providing source property for symbolic interpretations. Symbolism instances can relate to mythological, religious, cultural, or personal symbolic systems, enabling systematic iconographic analysis and cross-cultural symbolic comparison.</rdfs:comment>
    <rdfs:subClassOf rdf:nodeID="A9"/>
    <rdfs:subClassOf rdf:resource="http://w3id.org/arto#Connotation"/>
    <rdf:type rdf:resource="http://www.w3.org/2002/07/owl#Class"/>
  </rdf:Description>
  <rdf:Description rdf:nodeID="A10">
    <owl:hasValue rdf:resource="http://vocab.getty.edu/aat/300056444"/>
    <owl:onProperty rdf:resource="http://www.w3.org/2004/02/skos/core#broaderTransitive"/>
    <rdf:type rdf:resource="http://www.w3.org/2002/07/owl#Restriction"/>
  </rdf:Description>
  <rdf:Description rdf:about="http://w3id.org/arto#ColourHistogram">
    <rdfs:label>ColourHistogram</rdfs:label>
    <rdfs:comment>A metric that captures the distribution of colours within an artwork. It represents how frequently each colour or colour range occurs, typically in the form of a histogram or similar quantitative structure. This metric can be used for tasks such as palette analysis, artwork comparison</rdfs:comment>
    <rdfs:subClassOf rdf:resource="http://w3id.org/arto#Metric"/>
    <rdf:type rdf:resource="http://www.w3.org/2002/07/owl#Class"/>
  </rdf:Description>
  <rdf:Description rdf:about="http://purl.org/dc/terms/instructionalMethod">
    <rdfs:label xml:lang="en">Instructional Method</rdfs:label>
    <rdfs:isDefinedBy rdf:resource="http://purl.org/dc/terms/"/>
    <rdfs:comment xml:lang="en">A process, used to engender knowledge, attitudes and skills, that the described resource is designed to support.</rdfs:comment>
    <dc:description xml:lang="en">Instructional Method typically includes ways of presenting instructional materials or conducting instructional activities, patterns of learner-to-learner and learner-to-instructor interactions, and mechanisms by which group and individual levels of learning are measured.  Instructional methods include all aspects of the instruction and learning processes from planning and implementation through evaluation and feedback.</dc:description>
    <j.0:rangeIncludes rdf:resource="http://purl.org/dc/terms/MethodOfInstruction"/>
    <dc:issued rdf:datatype="http://www.w3.org/2001/XMLSchema#date">2005-06-13</dc:issued>
    <rdf:type rdf:resource="http://www.w3.org/2002/07/owl#NamedIndividual"/>
  </rdf:Description>
  <rdf:Description rdf:nodeID="A11">
    <rdf:rest rdf:resource="http://www.w3.org/1999/02/22-rdf-syntax-ns#nil"/>
    <rdf:first rdf:nodeID="A12"/>
  </rdf:Description>
  <rdf:Description rdf:about="http://w3id.org/arto#Painting">
    <rdfs:label>Painting</rdfs:label>
    <rdfs:comment>A specific type of artwork created using paint or similar media. </rdfs:comment>
    <rdfs:subClassOf rdf:resource="http://w3id.org/arto#Artwork"/>
    <rdf:type rdf:resource="http://www.w3.org/2002/07/owl#Class"/>
  </rdf:Description>
  <rdf:Description rdf:nodeID="A13">
    <owl:cardinality rdf:datatype="http://www.w3.org/2001/XMLSchema#nonNegativeInteger">1</owl:cardinality>
  </rdf:Description>
  <rdf:Description rdf:about="http://purl.org/dc/terms/valid">
    <rdfs:label xml:lang="en">Date Valid</rdfs:label>
    <rdfs:isDefinedBy rdf:resource="http://purl.org/dc/terms/"/>
    <rdfs:comment xml:lang="en">Date (often a range) of validity of a resource.</rdfs:comment>
    <dc:description xml:lang="en">Recommended practice is to describe the date, date/time, or period of time as recommended for the property Date, of which this is a subproperty.</dc:description>
    <dc:issued rdf:datatype="http://www.w3.org/2001/XMLSchema#date">2000-07-11</dc:issued>
    <rdf:type rdf:resource="http://www.w3.org/2002/07/owl#NamedIndividual"/>
    <rdfs:subPropertyOf rdf:resource="http://purl.org/dc/terms/date"/>
    <rdf:type rdf:resource="http://www.w3.org/2002/07/owl#DatatypeProperty"/>
    <rdfs:range rdf:resource="http://www.w3.org/2000/01/rdf-schema#Literal"/>
    <rdfs:subPropertyOf rdf:resource="http://purl.org/dc/elements/1.1/date"/>
    <rdf:type rdf:resource="http://www.w3.org/2002/07/owl#AnnotationProperty"/>
  </rdf:Description>
  <rdf:Description rdf:about="http://purl.org/dc/terms/Standard">
    <rdfs:label xml:lang="en">Standard</rdfs:label>
    <rdfs:isDefinedBy rdf:resource="http://purl.org/dc/terms/"/>
    <rdfs:comment xml:lang="en">A reference point against which other things can be evaluated or compared.</rdfs:comment>
    <dc:issued rdf:datatype="http://www.w3.org/2001/XMLSchema#date">2008-01-14</dc:issued>
    <rdf:type rdf:resource="http://www.w3.org/2002/07/owl#NamedIndividual"/>
    <rdf:type rdf:resource="http://www.w3.org/2002/07/owl#Class"/>
  </rdf:Description>
  <rdf:Description rdf:about="http://w3id.org/arto#width">
    <rdfs:label>width</rdfs:label>
    <rdfs:comment>The width of the line.</rdfs:comment>
    <rdfs:range rdf:resource="http://www.w3.org/2001/XMLSchema#float"/>
    <rdfs:domain rdf:resource="http://w3id.org/arto#Line"/>
    <rdf:type rdf:resource="http://www.w3.org/2002/07/owl#DatatypeProperty"/>
  </rdf:Description>
  <rdf:Description rdf:nodeID="A14">
    <rdf:rest rdf:nodeID="A15"/>
    <rdf:first>Lab</rdf:first>
    <rdf:type rdf:resource="http://www.w3.org/1999/02/22-rdf-syntax-ns#List"/>
  </rdf:Description>
  <rdf:Description rdf:about="http://purl.org/dc/terms/format">
    <rdfs:label xml:lang="en">Format</rdfs:label>
    <rdfs:isDefinedBy rdf:resource="http://purl.org/dc/terms/"/>
    <rdfs:comment xml:lang="en">The file format, physical medium, or dimensions of the resource.</rdfs:comment>
    <dc:description xml:lang="en">Recommended practice is to use a controlled vocabulary where available. For example, for file formats one could use the list of Internet Media Types [[MIME](https://www.iana.org/assignments/media-types/media-types.xhtml)].  Examples of dimensions include size and duration.</dc:description>
    <j.0:rangeIncludes rdf:resource="http://purl.org/dc/terms/MediaType"/>
    <j.0:rangeIncludes rdf:resource="http://purl.org/dc/terms/Extent"/>
    <dc:issued rdf:datatype="http://www.w3.org/2001/XMLSchema#date">2008-01-14</dc:issued>
    <rdf:type rdf:resource="http://www.w3.org/2002/07/owl#NamedIndividual"/>
    <rdfs:subPropertyOf rdf:resource="http://purl.org/dc/elements/1.1/format"/>
    <rdf:type rdf:resource="http://www.w3.org/2002/07/owl#AnnotationProperty"/>
  </rdf:Description>
  <rdf:Description rdf:about="http://www.w3.org/2002/07/owl#cardinality">
    <rdf:type rdf:resource="http://www.w3.org/2002/07/owl#AnnotationProperty"/>
  </rdf:Description>
  <rdf:Description rdf:about="http://w3id.org/arto#Agent">
    <rdfs:label>Agent</rdfs:label>
    <rdfs:comment>Represents individuals or organisations involved in artwork creation, curation, or related activities. This class extends foaf:Agent with art-specific roles and relationships. Agents can be artists, curators, collectors, institutions, or other entities. </rdfs:comment>
    <rdfs:subClassOf rdf:nodeID="A16"/>
    <rdfs:subClassOf rdf:resource="http://xmlns.com/foaf/spec/Agent"/>
    <rdf:type rdf:resource="http://www.w3.org/2002/07/owl#Class"/>
  </rdf:Description>
  <rdf:Description rdf:nodeID="A15">
    <rdf:rest rdf:nodeID="A17"/>
    <rdf:first>RGB</rdf:first>
    <rdf:type rdf:resource="http://www.w3.org/1999/02/22-rdf-syntax-ns#List"/>
  </rdf:Description>
  <rdf:Description rdf:nodeID="A18">
    <owl:cardinality rdf:datatype="http://www.w3.org/2001/XMLSchema#nonNegativeInteger">1</owl:cardinality>
  </rdf:Description>
  <rdf:Description rdf:about="http://w3id.org/arto#hasMetric">
    <skos:example>
                - Colour metrics: :sky_area arto:hasMetric :blue_intensity_75_percent
                - Composition balance: :landscape_scene arto:hasMetric :symmetry_score_0.8
                - Emotional intensity: :expression_scene arto:hasMetric :fear_intensity_high</skos:example>
    <rdfs:label>hasMetric</rdfs:label>
    <rdfs:comment>Associates artwork components with quantifiable measurements supporting computational analysis and comparative studies. This property enables integration of statistical colour analysis, compositional balance metrics, emotional intensity measures, and other quantitative assessments with qualitative art historical analysis. The relationship supports both automated artwork analysis and structured comparison studies while maintaining connection to interpretive content.</rdfs:comment>
    <rdfs:range rdf:resource="http://w3id.org/arto#Metric"/>
    <rdfs:domain rdf:nodeID="A19"/>
    <owl:inverseOf rdf:resource="http://w3id.org/arto#isMetricOf"/>
    <rdf:type rdf:resource="http://www.w3.org/2002/07/owl#ObjectProperty"/>
  </rdf:Description>
  <rdf:Description rdf:nodeID="A20">
    <rdf:rest rdf:nodeID="A21"/>
    <rdf:first rdf:resource="http://w3id.org/arto#Artwork"/>
  </rdf:Description>
  <rdf:Description rdf:about="http://purl.org/dc/terms/PhysicalMedium">
    <rdfs:label xml:lang="en">Physical Medium</rdfs:label>
    <rdfs:isDefinedBy rdf:resource="http://purl.org/dc/terms/"/>
    <rdfs:comment xml:lang="en">A physical material or carrier.</rdfs:comment>
    <dc:description xml:lang="en">Examples include paper, canvas, or DVD.</dc:description>
    <dc:issued rdf:datatype="http://www.w3.org/2001/XMLSchema#date">2008-01-14</dc:issued>
    <rdf:type rdf:resource="http://www.w3.org/2002/07/owl#NamedIndividual"/>
    <rdfs:subClassOf rdf:resource="http://purl.org/dc/terms/MediaType"/>
    <rdf:type rdf:resource="http://www.w3.org/2002/07/owl#Class"/>
  </rdf:Description>
  <rdf:Description rdf:about="http://qudt.org/schema/qudt/Vector">
    <rdf:type rdf:resource="http://www.w3.org/2002/07/owl#Class"/>
  </rdf:Description>
  <rdf:Description rdf:about="http://w3id.org/arto#BalanceOfComposition">
    <rdfs:label>BalanceOfComposition</rdfs:label>
    <rdfs:comment>Used to assess and describe the visual equilibrium of an artwork's composition. This metric captures how elements are arranged in terms of symmetry, asymmetry, and spatial distribution of visual weight. It can be applied in qualitative analysis (e.g., identifying harmonious vs. dynamic arrangements) or in quantitative evaluation when assigning a balance score to artworks.</rdfs:comment>
    <rdfs:subClassOf rdf:resource="http://w3id.org/arto#Metric"/>
    <rdf:type rdf:resource="http://www.w3.org/2002/07/owl#Class"/>
  </rdf:Description>
  <rdf:Description rdf:nodeID="A22">
    <owl:cardinality rdf:datatype="http://www.w3.org/2001/XMLSchema#nonNegativeInteger">1</owl:cardinality>
  </rdf:Description>
  <rdf:Description rdf:nodeID="A23">
    <owl:cardinality rdf:datatype="http://www.w3.org/2001/XMLSchema#nonNegativeInteger">1</owl:cardinality>
  </rdf:Description>
  <rdf:Description rdf:about="http://purl.org/dc/terms/Period">
    <rdfs:seeAlso rdf:resource="https://www.dublincore.org/specifications/dublin-core/dcmi-period/"/>
    <rdfs:label xml:lang="en">DCMI Period</rdfs:label>
    <rdfs:isDefinedBy rdf:resource="http://purl.org/dc/terms/"/>
    <rdfs:comment xml:lang="en">The set of time intervals defined by their limits according to the DCMI Period Encoding Scheme.</rdfs:comment>
    <dc:issued rdf:datatype="http://www.w3.org/2001/XMLSchema#date">2000-07-11</dc:issued>
    <rdf:type rdf:resource="http://www.w3.org/2002/07/owl#NamedIndividual"/>
    <rdf:type rdf:resource="http://www.w3.org/2000/01/rdf-schema#Datatype"/>
  </rdf:Description>
  <rdf:Description rdf:about="http://purl.org/dc/dcam/rangeIncludes">
    <rdf:type rdf:resource="http://www.w3.org/2002/07/owl#AnnotationProperty"/>
  </rdf:Description>
  <rdf:Description rdf:about="http://w3id.org/arto#Event">
    <rdfs:label>Event</rdfs:label>
    <skos:example>
          &lt;&lt; :Guernica arto:sketchedBy :Picasso &gt;&gt; a arto:Event ;
              arto:hasTime :t_1937_Spring ; arto:hasLocation :ParisStudio ;
              dc:type "Sketching".

          &lt;&lt; :Guernica dc:creator :Picasso &gt;&gt; a arto:Event ;
              arto:hasTime :t_1937 ; arto:hasLocation :ParisStudio ;
              dc:type "Creation".
          &lt;&lt; :Georgia_OKeeffe arto:movedResidenceTo :Abiquiu_Home &gt;&gt; a arto:Event ;
            arto:hasTime :t_1949 ; arto:hasLocation :Abiquiu_NewMexico ;
            dc:type "ResidenceMove".
          </skos:example>
    <rdfs:comment>
Represents a temporally and spatially situated occurrence involving agents and locations.
This class extends the Event Ontology and aligns conceptually with CIDOC CRM’s E5_Event,
supporting cultural heritage interoperability. Event instances may cover artistic activities
(creation, sketching, exhibition), artist life events (residence changes, collaborations),
as well as historical or mythological occurrences referenced in artworks. Event categories
can be expressed using rdf:type (e.g., Creation, Exhibition, ResidenceMove).
</rdfs:comment>
    <rdfs:subClassOf rdf:nodeID="A24"/>
    <rdfs:subClassOf rdf:nodeID="A25"/>
    <rdfs:subClassOf rdf:nodeID="A26"/>
    <rdfs:subClassOf rdf:nodeID="A27"/>
    <rdfs:subClassOf rdf:nodeID="A7"/>
    <rdfs:subClassOf rdf:resource="https://w3id.org/MON/event.owl#Event"/>
    <rdf:type rdf:resource="http://www.w3.org/2002/07/owl#Class"/>
  </rdf:Description>
  <rdf:Description rdf:nodeID="A28">
    <owl:cardinality rdf:datatype="http://www.w3.org/2001/XMLSchema#nonNegativeInteger">1</owl:cardinality>
  </rdf:Description>
  <rdf:Description rdf:about="http://purl.org/dc/terms/medium">
    <rdfs:label xml:lang="en">Medium</rdfs:label>
    <rdfs:isDefinedBy rdf:resource="http://purl.org/dc/terms/"/>
    <rdfs:comment xml:lang="en">The material or physical carrier of the resource.</rdfs:comment>
    <j.0:rangeIncludes rdf:resource="http://purl.org/dc/terms/PhysicalMedium"/>
    <j.0:domainIncludes rdf:resource="http://purl.org/dc/terms/PhysicalResource"/>
    <dc:issued rdf:datatype="http://www.w3.org/2001/XMLSchema#date">2000-07-11</dc:issued>
    <rdf:type rdf:resource="http://www.w3.org/2002/07/owl#NamedIndividual"/>
    <rdfs:subPropertyOf rdf:resource="http://purl.org/dc/terms/format"/>
    <rdfs:subPropertyOf rdf:resource="http://purl.org/dc/elements/1.1/format"/>
    <rdf:type rdf:resource="http://www.w3.org/2002/07/owl#AnnotationProperty"/>
  </rdf:Description>
  <rdf:Description rdf:nodeID="A29">
    <owl:unionOf rdf:nodeID="A1"/>
    <rdf:type rdf:resource="http://www.w3.org/2002/07/owl#Class"/>
  </rdf:Description>
  <rdf:Description rdf:nodeID="A30">
    <owl:allValuesFrom rdf:resource="http://www.w3.org/2001/XMLSchema#string"/>
    <owl:onProperty rdf:resource="http://purl.org/dc/terms/type"/>
    <rdf:type rdf:resource="http://www.w3.org/2002/07/owl#Restriction"/>
  </rdf:Description>
  <rdf:Description rdf:about="http://purl.org/dc/terms/RFC4646">
    <rdfs:seeAlso rdf:resource="http://www.ietf.org/rfc/rfc4646.txt"/>
    <rdfs:label xml:lang="en">RFC 4646</rdfs:label>
    <rdfs:isDefinedBy rdf:resource="http://purl.org/dc/terms/"/>
    <rdfs:comment xml:lang="en">The set of tags constructed according to RFC 4646 for the identification of languages.</rdfs:comment>
    <dc:description xml:lang="en">RFC 4646 obsoletes RFC 3066.</dc:description>
    <dc:issued rdf:datatype="http://www.w3.org/2001/XMLSchema#date">2008-01-14</dc:issued>
    <rdf:type rdf:resource="http://www.w3.org/2002/07/owl#NamedIndividual"/>
    <rdf:type rdf:resource="http://www.w3.org/2000/01/rdf-schema#Datatype"/>
  </rdf:Description>
  <rdf:Description rdf:about="http://www.opengis.net/ont/geosparql#wktLiteral">
    <rdf:type rdf:resource="http://www.w3.org/2002/07/owl#Class"/>
  </rdf:Description>
  <rdf:Description rdf:nodeID="A31">
    <owl:allValuesFrom rdf:resource="http://www.w3.org/2001/XMLSchema#string"/>
    <owl:onProperty rdf:resource="http://w3id.org/arto#size"/>
    <rdf:type rdf:resource="http://www.w3.org/2002/07/owl#Restriction"/>
  </rdf:Description>
  <rdf:Description rdf:about="http://w3id.org/arto#containsScene">
    <skos:example>
                      - Nested scenes: :market_scene arto:containsScene :vendor_scene, :customer_scene
                      - Background scenes: :landscape_painting arto:containsScene :mountain_scene, :valley_scene</skos:example>
    <rdfs:label>containsScene</rdfs:label>
    <rdfs:comment>Identifies distinct scenes within an artwork or within another scene, allowing for hierarchical scene composition.</rdfs:comment>
    <rdfs:range rdf:resource="http://w3id.org/arto#Scene"/>
    <rdfs:domain rdf:nodeID="A32"/>
    <owl:inverseOf rdf:resource="http://w3id.org/arto#isSceneOf"/>
    <rdf:type rdf:resource="http://www.w3.org/2002/07/owl#ObjectProperty"/>
  </rdf:Description>
  <rdf:Description rdf:nodeID="A33">
    <rdf:rest rdf:resource="http://www.w3.org/1999/02/22-rdf-syntax-ns#nil"/>
    <rdf:first>XYZ</rdf:first>
    <rdf:type rdf:resource="http://www.w3.org/1999/02/22-rdf-syntax-ns#List"/>
  </rdf:Description>
  <rdf:Description rdf:nodeID="A34">
    <owl:oneOf rdf:nodeID="A35"/>
    <rdf:type rdf:resource="http://www.w3.org/2000/01/rdf-schema#Datatype"/>
  </rdf:Description>
  <rdf:Description rdf:nodeID="A36">
    <rdf:rest rdf:nodeID="A37"/>
    <rdf:first rdf:resource="http://w3id.org/arto#Agent"/>
  </rdf:Description>
  <rdf:Description rdf:about="http://www.cidoc-crm.org/cidoc-crm/E28_Conceptual_Object">
    <rdf:type rdf:resource="http://www.w3.org/2002/07/owl#Class"/>
  </rdf:Description>
  <rdf:Description rdf:about="http://w3id.org/arto#VisualElement">
    <rdfs:label>VisualElement</rdfs:label>
    <rdfs:comment>Represents the fundamental visual components of artworks, including colours, lines, shapes, textures, and compositional structures. This abstract class serves as the foundation for systematic visual analysis, bridging computational image processing with art historical methodology. Visual elements can express connotations and have measurable properties, supporting both quantitative analysis (colour histograms, line density) and qualitative interpretation (symbolic colour use, expressive line quality). </rdfs:comment>
    <rdfs:comment>Represents the fundamental visual components of an artwork, including: lines and shapes, colours and textures, forms and patterns, space and perspective, light and shadow, etc.</rdfs:comment>
    <rdfs:subClassOf rdf:nodeID="A38"/>
    <rdfs:subClassOf rdf:nodeID="A39"/>
    <rdf:type rdf:resource="http://www.w3.org/2002/07/owl#Class"/>
  </rdf:Description>
  <rdf:Description rdf:nodeID="A40">
    <owl:allValuesFrom rdf:resource="http://w3id.org/arto#Person"/>
    <owl:onProperty rdf:resource="http://w3id.org/arto#knows"/>
    <rdf:type rdf:resource="http://www.w3.org/2002/07/owl#Restriction"/>
  </rdf:Description>
  <rdf:Description rdf:nodeID="A41">
    <owl:cardinality rdf:datatype="http://www.w3.org/2001/XMLSchema#nonNegativeInteger">1</owl:cardinality>
  </rdf:Description>
  <rdf:Description rdf:nodeID="A42">
    <owl:allValuesFrom rdf:resource="http://qudt.org/schema/qudt/Vector"/>
    <owl:onProperty rdf:resource="http://w3id.org/arto#hasCoordinates"/>
    <rdf:type rdf:resource="http://www.w3.org/2002/07/owl#Restriction"/>
  </rdf:Description>
  <rdf:Description rdf:nodeID="A43">
    <owl:allValuesFrom rdf:resource="http://w3id.org/arto#Object"/>
    <owl:onProperty rdf:resource="http://w3id.org/arto#containsObject"/>
    <rdf:type rdf:resource="http://www.w3.org/2002/07/owl#Restriction"/>
  </rdf:Description>
  <rdf:Description rdf:about="http://w3id.org/arto#ColourValue">
    <skos:example>
                    - RGB specification: :red_primary rdf:type arto:ColourValue ;
                      arto:colourSpace "RGB" ; qudt:vector (255,0,0) ;
                    - HSV specification: :golden_yellow rdf:type arto:ColourValue ;
                      arto:colourSpace "HSV" ; qudt:vector (45,85,95) ;
                    - CMYK print colours: :prussian_blue rdf:type arto:ColourValue ;
                      arto:colourSpace "CMYK" ; qudt:vector (100,85,0,25) ;
                    - LAB colour measurement: :skin_tone rdf:type arto:ColourValue ;
                        arto:colourSpace "Lab" ; qudt:vector (75,8,15) ;
                    </skos:example>
    <rdfs:label>colourValue</rdfs:label>
    <rdfs:comment>Represents the precise numeric specification of colours using various colour models and measurement systems. This class captures quantitative colour data for digital analysis, colour matching and reproduction studies. Colour values enable objective colour comparison, automated colour analysis, and integration with digital image processing workflows. The class supports multiple colour spaces to accommodate different analytical needs and technical requirements.</rdfs:comment>
    <rdfs:subClassOf rdf:nodeID="A44"/>
    <rdfs:subClassOf rdf:nodeID="A45"/>
    <rdf:type rdf:resource="http://www.w3.org/2002/07/owl#Class"/>
  </rdf:Description>
  <rdf:Description rdf:about="http://w3id.org/arto#style">
    <rdfs:label>style</rdfs:label>
    <skos:example>
              :water_lilies a arto:Artwork ;
                arto:style aat:impressionism .

              :guernica a arto:Artwork ;
                arto:style aat:cubism .

              :baroque_altarpiece a arto:Artwork ;
                arto:style aat:baroque .
              </skos:example>
    <rdfs:comment>Indicates the artistic style or movement of an artwork, such as Impressionism, Cubism, or Baroque. This property links to Getty AAT's style and period classifications, while also allowing for the inclusion of custom style definitions when necessary.</rdfs:comment>
    <rdfs:range rdf:resource="http://w3id.org/arto#StyleType"/>
    <rdfs:domain rdf:resource="http://w3id.org/arto#Artwork"/>
    <rdf:type rdf:resource="http://www.w3.org/2002/07/owl#ObjectProperty"/>
  </rdf:Description>
  <rdf:Description rdf:about="http://w3id.org/arto#hasLocation">
    <skos:example>
                - Museum address: :metropolitan_museum arto:hasLocation :met_nyc_location
                - Gallery location: :tate_modern arto:hasLocation :london_bankside                 
                - Exhibition event: :venice_biennale_2024 arto:hasLocation :venice_giardini</skos:example>
    <rdfs:label>hasLocation</rdfs:label>
    <rdfs:comment>Specifies the physical location of an agent or event related to the artwork.</rdfs:comment>
    <rdfs:range rdf:resource="http://w3id.org/arto#Location"/>
    <rdfs:domain rdf:nodeID="A46"/>
    <owl:inverseOf rdf:resource="http://w3id.org/arto#isLocationOf"/>
    <rdf:type rdf:resource="http://www.w3.org/2002/07/owl#ObjectProperty"/>
  </rdf:Description>
  <rdf:Description rdf:nodeID="A47">
    <owl:onClass rdf:resource="https://schema.org/QuantitativeValue"/>
    <owl:maxQualifiedCardinality rdf:datatype="http://www.w3.org/2001/XMLSchema#nonNegativeInteger">1</owl:maxQualifiedCardinality>
    <owl:onProperty rdf:resource="https://schema.org/height"/>
    <rdf:type rdf:resource="http://www.w3.org/2002/07/owl#Restriction"/>
  </rdf:Description>
  <rdf:Description rdf:about="http://purl.org/dc/terms/">
    <dc:publisher rdf:resource="http://purl.org/dc/aboutdcmi#DCMI"/>
    <dc:title xml:lang="en">DCMI Metadata Terms - other</dc:title>
    <dc:modified rdf:datatype="http://www.w3.org/2001/XMLSchema#date">2012-06-14</dc:modified>
    <rdf:type rdf:resource="http://www.w3.org/2002/07/owl#NamedIndividual"/>
  </rdf:Description>
  <rdf:Description rdf:about="http://www.w3.org/2002/07/owl#qualifiedCardinality">
    <rdf:type rdf:resource="http://www.w3.org/2002/07/owl#AnnotationProperty"/>
  </rdf:Description>
  <rdf:Description rdf:about="http://purl.org/dc/terms/conformsTo">
    <rdfs:label xml:lang="en">Conforms To</rdfs:label>
    <rdfs:isDefinedBy rdf:resource="http://purl.org/dc/terms/"/>
    <rdfs:comment xml:lang="en">An established standard to which the described resource conforms.</rdfs:comment>
    <j.0:rangeIncludes rdf:resource="http://purl.org/dc/terms/Standard"/>
    <dc:issued rdf:datatype="http://www.w3.org/2001/XMLSchema#date">2001-05-21</dc:issued>
    <rdf:type rdf:resource="http://www.w3.org/2002/07/owl#NamedIndividual"/>
    <rdfs:subPropertyOf rdf:resource="http://purl.org/dc/terms/relation"/>
    <rdfs:subPropertyOf rdf:resource="http://purl.org/dc/elements/1.1/relation"/>
    <rdf:type rdf:resource="http://www.w3.org/2002/07/owl#AnnotationProperty"/>
  </rdf:Description>
  <rdf:Description rdf:nodeID="A48">
    <rdf:rest rdf:nodeID="A49"/>
    <rdf:first>HSV</rdf:first>
    <rdf:type rdf:resource="http://www.w3.org/1999/02/22-rdf-syntax-ns#List"/>
  </rdf:Description>
  <rdf:Description rdf:about="http://w3id.org/arto#colourSystem">
    <rdfs:label>colourSystem</rdfs:label>
    <rdfs:comment>The colour system of the ColourValue, indicating the model used for its representation. This property supports various colour models such as RGB, HSV, Lab, and CMYK, allowing for flexible colour representation and analysis in artworks. The use of a restricted set of values ensures consistency and interoperability across different systems and applications.</rdfs:comment>
    <rdfs:range rdf:nodeID="A50"/>
    <rdfs:domain rdf:resource="http://w3id.org/arto#ColourValue"/>
    <rdf:type rdf:resource="http://www.w3.org/2002/07/owl#DatatypeProperty"/>
  </rdf:Description>
  <rdf:Description rdf:nodeID="A51">
    <owl:allValuesFrom rdf:resource="http://www.opengis.net/ont/geosparql#wktLiteral"/>
    <owl:onProperty rdf:resource="http://www.opengis.net/ont/geosparql#asWKT"/>
    <rdf:type rdf:resource="http://www.w3.org/2002/07/owl#Restriction"/>
  </rdf:Description>
  <rdf:Description rdf:nodeID="A46">
    <owl:unionOf rdf:nodeID="A52"/>
    <rdf:type rdf:resource="http://www.w3.org/2002/07/owl#Class"/>
  </rdf:Description>
  <rdf:Description rdf:nodeID="A53">
    <owl:cardinality rdf:datatype="http://www.w3.org/2001/XMLSchema#nonNegativeInteger">1</owl:cardinality>
  </rdf:Description>
  <rdf:Description rdf:nodeID="A54">
    <owl:allValuesFrom rdf:resource="http://www.w3.org/2001/XMLSchema#string"/>
    <owl:onProperty rdf:resource="http://w3id.org/arto#direction"/>
    <rdf:type rdf:resource="http://www.w3.org/2002/07/owl#Restriction"/>
  </rdf:Description>
  <rdf:Description rdf:nodeID="A55">
    <owl:allValuesFrom rdf:resource="http://purl.obolibrary.org/obo/MFOEM_000001"/>
    <owl:onProperty rdf:resource="http://w3id.org/arto#expresses"/>
    <rdf:type rdf:resource="http://www.w3.org/2002/07/owl#Restriction"/>
  </rdf:Description>
  <rdf:Description rdf:about="http://w3id.org/arto#Composition">
    <rdfs:label>Composition</rdfs:label>
    <rdfs:comment>Represents the arrangement and organisation of visual elements within artworks, fundamental to art historical analysis and aesthetic evaluation. This class captures compositional strategies, balance, and spatial relationships that structure artistic meaning.
                 Currently ARTO includes common compositions types: symmetry, asymmetry, radial balance, rule of thirds, golden ratio, and dynamic composition.
                 </rdfs:comment>
    <rdfs:subClassOf rdf:nodeID="A56"/>
    <rdfs:subClassOf rdf:resource="http://w3id.org/arto#VisualElement"/>
    <rdf:type rdf:resource="http://www.w3.org/2002/07/owl#Class"/>
  </rdf:Description>
  <rdf:Description rdf:about="http://vocab.getty.edu/aat/300056444">
    <rdf:type rdf:resource="http://www.w3.org/2002/07/owl#NamedIndividual"/>
  </rdf:Description>
  <rdf:Description rdf:about="http://www.opengis.net/ont/geosparql#asWKT">
    <rdf:type rdf:resource="http://www.w3.org/2002/07/owl#ObjectProperty"/>
  </rdf:Description>
  <rdf:Description rdf:about="http://w3id.org/arto#source">
    <rdfs:label>source</rdfs:label>
    <rdfs:comment>Identifies the cultural, historical, or textual origins of symbolic meanings, enabling traceability of iconographic interpretations and cross-cultural symbolic analysis. Sources can include mythological traditions, religious texts, historical events, literary works, or folk traditions that inform symbolic interpretation.</rdfs:comment>
    <rdfs:range rdf:resource="http://www.w3.org/2001/XMLSchema#string"/>
    <rdfs:domain rdf:resource="http://w3id.org/arto#Symbolism"/>
    <rdf:type rdf:resource="http://www.w3.org/2002/07/owl#DatatypeProperty"/>
  </rdf:Description>
  <rdf:Description rdf:about="http://purl.org/dc/terms/hasPart">
    <rdfs:label xml:lang="en">Has Part</rdfs:label>
    <rdfs:isDefinedBy rdf:resource="http://purl.org/dc/terms/"/>
    <rdfs:comment xml:lang="en">A related resource that is included either physically or logically in the described resource.</rdfs:comment>
    <dc:description xml:lang="en">This property is intended to be used with non-literal values. This property is an inverse property of Is Part Of.</dc:description>
    <dc:issued rdf:datatype="http://www.w3.org/2001/XMLSchema#date">2000-07-11</dc:issued>
    <rdf:type rdf:resource="http://www.w3.org/2002/07/owl#NamedIndividual"/>
    <rdfs:subPropertyOf rdf:resource="http://purl.org/dc/terms/relation"/>
    <rdfs:subPropertyOf rdf:resource="http://purl.org/dc/elements/1.1/relation"/>
    <rdf:type rdf:resource="http://www.w3.org/2002/07/owl#AnnotationProperty"/>
  </rdf:Description>
  <rdf:Description rdf:about="https://dbpedia.org/property/residence">
    <rdf:type rdf:resource="http://www.w3.org/2002/07/owl#ObjectProperty"/>
  </rdf:Description>
  <rdf:Description rdf:nodeID="A57">
    <rdf:rest rdf:nodeID="A58"/>
    <rdf:first>CMYK</rdf:first>
  </rdf:Description>
  <rdf:Description rdf:about="http://purl.org/dc/elements/1.1/subject">
    <rdf:type rdf:resource="http://www.w3.org/2002/07/owl#AnnotationProperty"/>
  </rdf:Description>
  <rdf:Description rdf:about="http://purl.org/dc/terms/contributor">
    <rdfs:label xml:lang="en">Contributor</rdfs:label>
    <rdfs:isDefinedBy rdf:resource="http://purl.org/dc/terms/"/>
    <rdfs:comment xml:lang="en">An entity responsible for making contributions to the resource.</rdfs:comment>
    <dc:description xml:lang="en">The guidelines for using names of persons or organizations as creators apply to contributors.</dc:description>
    <dc:description xml:lang="en">The guidelines for using names of persons or organisations as creators apply to contributors.</dc:description>
    <j.0:rangeIncludes rdf:resource="http://purl.org/dc/terms/Agent"/>
    <dc:issued rdf:datatype="http://www.w3.org/2001/XMLSchema#date">2008-01-14</dc:issued>
    <rdf:type rdf:resource="http://www.w3.org/2002/07/owl#NamedIndividual"/>
    <rdfs:subPropertyOf rdf:resource="http://purl.org/dc/elements/1.1/contributor"/>
  </rdf:Description>
  <rdf:Description rdf:about="http://purl.org/dc/terms/RFC5646">
    <rdfs:seeAlso rdf:resource="http://www.ietf.org/rfc/rfc5646.txt"/>
    <rdfs:label xml:lang="en">RFC 5646</rdfs:label>
    <rdfs:isDefinedBy rdf:resource="http://purl.org/dc/terms/"/>
    <rdfs:comment xml:lang="en">The set of tags constructed according to RFC 5646 for the identification of languages.</rdfs:comment>
    <dc:description xml:lang="en">RFC 5646 obsoletes RFC 4646.</dc:description>
    <dc:issued rdf:datatype="http://www.w3.org/2001/XMLSchema#date">2010-10-11</dc:issued>
    <rdf:type rdf:resource="http://www.w3.org/2002/07/owl#NamedIndividual"/>
    <rdf:type rdf:resource="http://www.w3.org/2000/01/rdf-schema#Datatype"/>
  </rdf:Description>
  <rdf:Description rdf:nodeID="A59">
    <rdf:rest rdf:resource="http://www.w3.org/1999/02/22-rdf-syntax-ns#nil"/>
    <rdf:first rdf:resource="http://w3id.org/arto#Scene"/>
  </rdf:Description>
  <rdf:Description rdf:nodeID="A60">
    <rdf:rest rdf:resource="http://www.w3.org/1999/02/22-rdf-syntax-ns#nil"/>
    <rdf:first rdf:resource="http://w3id.org/arto#VisualElement"/>
  </rdf:Description>
  <rdf:Description rdf:about="http://w3id.org/arto#Relevance">
    <rdfs:label>Relevance</rdfs:label>
    <skos:example>
                   :lastSupper_RedCloakRelevance a arto:Relevance ;
                     arto:value 0.85 .
               </skos:example>
    <rdfs:comment>Measures and describes the significance or importance of elements within an artwork. Relevance may refer to thematic, visual, symbolic, narrative, historical, or compositional importance, and can be expressed by numeric scores, categorical levels, or references to related concepts.</rdfs:comment>
    <rdfs:subClassOf rdf:resource="http://w3id.org/arto#Metric"/>
    <rdf:type rdf:resource="http://www.w3.org/2002/07/owl#Class"/>
  </rdf:Description>
  <rdf:Description rdf:nodeID="A61">
    <owl:allValuesFrom rdf:resource="http://www.w3.org/2001/XMLSchema#string"/>
    <owl:onProperty rdf:resource="http://purl.org/dc/terms/type"/>
    <rdf:type rdf:resource="http://www.w3.org/2002/07/owl#Restriction"/>
  </rdf:Description>
  <rdf:Description rdf:nodeID="A62">
    <rdf:rest rdf:nodeID="A33"/>
    <rdf:first>RGB</rdf:first>
    <rdf:type rdf:resource="http://www.w3.org/1999/02/22-rdf-syntax-ns#List"/>
  </rdf:Description>
  <rdf:Description rdf:about="http://qudt.org/schema/qudt/vector">
    <rdf:type rdf:resource="http://www.w3.org/2002/07/owl#ObjectProperty"/>
  </rdf:Description>
  <rdf:Description rdf:nodeID="A63">
    <owl:cardinality rdf:datatype="http://www.w3.org/2001/XMLSchema#nonNegativeInteger">1</owl:cardinality>
  </rdf:Description>
  <rdf:Description rdf:about="http://purl.org/dc/terms/replaces">
    <rdfs:label xml:lang="en">Replaces</rdfs:label>
    <rdfs:isDefinedBy rdf:resource="http://purl.org/dc/terms/"/>
    <rdfs:comment xml:lang="en">A related resource that is supplanted, displaced, or superseded by the described resource.</rdfs:comment>
    <dc:description xml:lang="en">This property is intended to be used with non-literal values. This property is an inverse property of Is Replaced By.</dc:description>
    <dc:issued rdf:datatype="http://www.w3.org/2001/XMLSchema#date">2000-07-11</dc:issued>
    <rdf:type rdf:resource="http://www.w3.org/2002/07/owl#NamedIndividual"/>
    <rdfs:subPropertyOf rdf:resource="http://purl.org/dc/terms/relation"/>
    <rdfs:subPropertyOf rdf:resource="http://purl.org/dc/elements/1.1/relation"/>
    <rdf:type rdf:resource="http://www.w3.org/2002/07/owl#AnnotationProperty"/>
  </rdf:Description>
  <rdf:Description rdf:about="http://purl.org/dc/terms/spatial">
    <rdfs:label xml:lang="en">Spatial Coverage</rdfs:label>
    <rdfs:isDefinedBy rdf:resource="http://purl.org/dc/terms/"/>
    <rdfs:comment xml:lang="en">Spatial characteristics of the resource.</rdfs:comment>
    <j.0:rangeIncludes rdf:resource="http://purl.org/dc/terms/Location"/>
    <dc:issued rdf:datatype="http://www.w3.org/2001/XMLSchema#date">2000-07-11</dc:issued>
    <rdf:type rdf:resource="http://www.w3.org/2002/07/owl#NamedIndividual"/>
    <rdfs:subPropertyOf rdf:resource="http://purl.org/dc/terms/coverage"/>
    <rdfs:subPropertyOf rdf:resource="http://purl.org/dc/elements/1.1/coverage"/>
    <rdf:type rdf:resource="http://www.w3.org/2002/07/owl#AnnotationProperty"/>
  </rdf:Description>
  <rdf:Description rdf:about="http://purl.org/dc/terms/available">
    <rdfs:label xml:lang="en">Date Available</rdfs:label>
    <rdfs:isDefinedBy rdf:resource="http://purl.org/dc/terms/"/>
    <rdfs:comment xml:lang="en">Date that the resource became or will become available.</rdfs:comment>
    <dc:description xml:lang="en">Recommended practice is to describe the date, date/time, or period of time as recommended for the property Date, of which this is a subproperty.</dc:description>
    <dc:issued rdf:datatype="http://www.w3.org/2001/XMLSchema#date">2000-07-11</dc:issued>
    <rdf:type rdf:resource="http://www.w3.org/2002/07/owl#NamedIndividual"/>
    <rdfs:subPropertyOf rdf:resource="http://purl.org/dc/terms/date"/>
    <rdf:type rdf:resource="http://www.w3.org/2002/07/owl#DatatypeProperty"/>
    <rdfs:range rdf:resource="http://www.w3.org/2000/01/rdf-schema#Literal"/>
    <rdfs:subPropertyOf rdf:resource="http://purl.org/dc/elements/1.1/date"/>
    <rdf:type rdf:resource="http://www.w3.org/2002/07/owl#AnnotationProperty"/>
  </rdf:Description>
  <rdf:Description rdf:nodeID="A64">
    <owl:allValuesFrom rdf:resource="http://www.w3.org/2001/XMLSchema#dateTime"/>
    <owl:onProperty rdf:resource="https://schema.org/endDate"/>
    <rdf:type rdf:resource="http://www.w3.org/2002/07/owl#Restriction"/>
  </rdf:Description>
  <rdf:Description rdf:about="http://w3id.org/arto#Colour">
    <rdfs:label>Colour</rdfs:label>
    <skos:example>
            :c_vermilion a arto:Colour ;
              arto:hasColourTerm &lt;http://vocab.getty.edu/aat/300266400&gt; ;  # vermilion
              arto:hasColourValue [
                a arto:ColourValue ;
                arto:colourSpace "RGB" ;
                qudt:vector (227,66,52)  ] .


            :c_bluePeace a arto:Colour ;
              arto:hasColourTerm &lt;http://vocab.getty.edu/aat/300129361&gt; ;  # blue
              arto:hasColourValue [
                a arto:ColourValue ;
                arto:colourSpace "HSV" ;
                qudt:vector (197,76,100)
              ] ;
            </skos:example>
    <rdfs:comment>Represents colour usage in artworks with precise technical specifications and art historical context. This class provides both computational colour analysis (RGB, HSV values) and art theoretical foundations, aligning with Getty AAT's colour concepts while maintaining specific properties for digital analysis. Colour instances can express symbolic meanings and emotional content, supporting both technical image processing and interpretive art analysis.</rdfs:comment>
    <rdfs:subClassOf rdf:nodeID="A65"/>
    <rdfs:subClassOf rdf:nodeID="A66"/>
    <rdfs:subClassOf rdf:resource="http://w3id.org/arto#VisualElement"/>
    <rdf:type rdf:resource="http://www.w3.org/2002/07/owl#Class"/>
  </rdf:Description>
  <rdf:Description rdf:about="http://w3id.org/arto#GenreType">
    <rdfs:label>GenreType</rdfs:label>
    <rdfs:comment>Represents the genre of an artwork, such as portrait, landscape, still life, etc. This class allows for the classification of artworks based on their thematic or stylistic content.</rdfs:comment>
    <rdfs:subClassOf rdf:nodeID="A67"/>
    <rdf:type rdf:resource="http://www.w3.org/2002/07/owl#Class"/>
  </rdf:Description>
  <rdf:Description rdf:nodeID="A68">
    <owl:cardinality rdf:datatype="http://www.w3.org/2001/XMLSchema#nonNegativeInteger">1</owl:cardinality>
  </rdf:Description>
  <rdf:Description rdf:about="http://w3id.org/arto#descriptor">
    <skos:example>
                Portrait1 :clothing :RedDress ;
                :clothing rdfs:subPropertyOf arto:descriptor</skos:example>
    <rdfs:label>descriptor</rdfs:label>
    <rdfs:comment>Provides extensible descriptive framework for capturing object and scene characteristics not covered by specific properties, enabling domain-specific extensions through subproperties. This design addresses the infinite variety of artistic content while maintaining semantic structure. Examples include clothing descriptions for figures, or environmental conditions for scene.</rdfs:comment>
    <rdfs:range rdf:resource="http://www.w3.org/2001/XMLSchema#string"/>
    <rdfs:domain rdf:nodeID="A69"/>
    <rdf:type rdf:resource="http://www.w3.org/2002/07/owl#DatatypeProperty"/>
  </rdf:Description>
  <rdf:Description rdf:nodeID="A70">
    <owl:unionOf rdf:nodeID="A71"/>
    <rdf:type rdf:resource="http://www.w3.org/2002/07/owl#Class"/>
  </rdf:Description>
  <rdf:Description rdf:nodeID="A72">
    <owl:unionOf rdf:nodeID="A73"/>
    <rdf:type rdf:resource="http://www.w3.org/2002/07/owl#Class"/>
  </rdf:Description>
  <rdf:Description rdf:nodeID="A74">
    <rdf:rest rdf:nodeID="A75"/>
    <rdf:first rdf:resource="http://w3id.org/arto#Scene"/>
  </rdf:Description>
  <rdf:Description rdf:nodeID="A76">
    <rdf:rest rdf:nodeID="A77"/>
    <rdf:first rdf:resource="http://w3id.org/arto#Object"/>
  </rdf:Description>
  <rdf:Description rdf:nodeID="A78">
    <owl:allValuesFrom rdf:resource="http://w3id.org/arto#GenreType"/>
    <owl:onProperty rdf:resource="http://w3id.org/arto#genre"/>
    <rdf:type rdf:resource="http://www.w3.org/2002/07/owl#Restriction"/>
  </rdf:Description>
  <rdf:Description rdf:nodeID="A79">
    <owl:allValuesFrom rdf:resource="http://www.w3.org/2001/XMLSchema#string"/>
    <owl:onProperty rdf:resource="http://purl.org/dc/terms/type"/>
    <rdf:type rdf:resource="http://www.w3.org/2002/07/owl#Restriction"/>
  </rdf:Description>
  <rdf:Description rdf:nodeID="A80">
    <rdf:rest rdf:nodeID="A81"/>
    <rdf:first>CMYK</rdf:first>
    <rdf:type rdf:resource="http://www.w3.org/1999/02/22-rdf-syntax-ns#List"/>
  </rdf:Description>
  <rdf:Description rdf:about="http://purl.org/dc/terms/Frequency">
    <rdfs:label xml:lang="en">Frequency</rdfs:label>
    <rdfs:isDefinedBy rdf:resource="http://purl.org/dc/terms/"/>
    <rdfs:comment xml:lang="en">A rate at which something recurs.</rdfs:comment>
    <dc:issued rdf:datatype="http://www.w3.org/2001/XMLSchema#date">2008-01-14</dc:issued>
    <rdf:type rdf:resource="http://www.w3.org/2002/07/owl#NamedIndividual"/>
    <rdf:type rdf:resource="http://www.w3.org/2002/07/owl#Class"/>
  </rdf:Description>
  <rdf:Description rdf:about="http://www.w3.org/2006/time#TemporalEntity">
    <rdf:type rdf:resource="http://www.w3.org/2002/07/owl#Class"/>
  </rdf:Description>
  <rdf:Description rdf:nodeID="A82">
    <owl:minCardinality rdf:datatype="http://www.w3.org/2001/XMLSchema#nonNegativeInteger">0</owl:minCardinality>
  </rdf:Description>
  <rdf:Description rdf:about="http://purl.org/dc/terms/issued">
    <rdfs:label xml:lang="en">Date Issued</rdfs:label>
    <rdfs:isDefinedBy rdf:resource="http://purl.org/dc/terms/"/>
    <rdfs:comment xml:lang="en">Date of formal issuance of the resource.</rdfs:comment>
    <dc:description xml:lang="en">Recommended practice is to describe the date, date/time, or period of time as recommended for the property Date, of which this is a subproperty.</dc:description>
    <dc:issued rdf:datatype="http://www.w3.org/2001/XMLSchema#date">2000-07-11</dc:issued>
    <rdf:type rdf:resource="http://www.w3.org/2002/07/owl#NamedIndividual"/>
    <rdfs:subPropertyOf rdf:resource="http://purl.org/dc/terms/date"/>
    <rdf:type rdf:resource="http://www.w3.org/2002/07/owl#DatatypeProperty"/>
    <rdfs:range rdf:resource="http://www.w3.org/2000/01/rdf-schema#Literal"/>
    <rdfs:subPropertyOf rdf:resource="http://purl.org/dc/elements/1.1/date"/>
    <rdf:type rdf:resource="http://www.w3.org/2002/07/owl#AnnotationProperty"/>
  </rdf:Description>
  <rdf:Description rdf:nodeID="A44">
    <owl:allValuesFrom rdf:nodeID="A83"/>
    <owl:onProperty rdf:resource="http://w3id.org/arto#colourSpace"/>
    <rdf:type rdf:resource="http://www.w3.org/2002/07/owl#Restriction"/>
  </rdf:Description>
  <rdf:Description rdf:about="http://w3id.org/arto#length">
    <rdfs:label>length</rdfs:label>
    <rdfs:comment>The length of the line.</rdfs:comment>
    <rdfs:range rdf:resource="http://www.w3.org/2001/XMLSchema#float"/>
    <rdfs:domain rdf:resource="http://w3id.org/arto#Line"/>
    <rdf:type rdf:resource="http://www.w3.org/2002/07/owl#DatatypeProperty"/>
  </rdf:Description>
  <rdf:Description rdf:about="http://purl.org/dc/terms/Jurisdiction">
    <rdfs:label xml:lang="en">Jurisdiction</rdfs:label>
    <rdfs:isDefinedBy rdf:resource="http://purl.org/dc/terms/"/>
    <rdfs:comment xml:lang="en">The extent or range of judicial, law enforcement, or other authority.</rdfs:comment>
    <dc:issued rdf:datatype="http://www.w3.org/2001/XMLSchema#date">2008-01-14</dc:issued>
    <rdf:type rdf:resource="http://www.w3.org/2002/07/owl#NamedIndividual"/>
    <rdfs:subClassOf rdf:resource="http://purl.org/dc/terms/LocationPeriodOrJurisdiction"/>
    <rdf:type rdf:resource="http://www.w3.org/2002/07/owl#Class"/>
  </rdf:Description>
  <rdf:Description rdf:nodeID="A84">
    <rdf:rest rdf:resource="http://www.w3.org/1999/02/22-rdf-syntax-ns#nil"/>
    <rdf:first rdf:resource="http://w3id.org/arto#Scene"/>
  </rdf:Description>
  <rdf:Description rdf:nodeID="A85">
    <owl:cardinality rdf:datatype="http://www.w3.org/2001/XMLSchema#nonNegativeInteger">1</owl:cardinality>
  </rdf:Description>
  <rdf:Description rdf:about="http://w3id.org/arto#genre">
    <skos:example>
               - Traditional genres: :mona_lisa arto:genre aat:portrait_paintings
               - Landscape genre: :starry_night arto:genre aat:landscape_paintings  
               - Religious genre: :last_supper arto:genre aat:religious_paintings
               - Still life genre: :sunflowers arto:genre aat:still_life_paintings
               - Abstract genre: :composition_vii arto:genre aat:abstract_paintings
               </skos:example>
    <rdfs:label>genre</rdfs:label>
    <rdfs:comment>Genre classification is fundamental to art analysis, which connects artworks to established genre categories from Getty AAT vocabulary while supporting custom genre definitions.</rdfs:comment>
    <rdfs:range rdf:resource="http://w3id.org/arto#GenreType"/>
    <rdfs:domain rdf:resource="http://w3id.org/arto#Artwork"/>
    <rdf:type rdf:resource="http://www.w3.org/2002/07/owl#ObjectProperty"/>
  </rdf:Description>
  <rdf:Description rdf:about="http://purl.org/dc/terms/DDC">
    <rdfs:seeAlso rdf:resource="http://www.oclc.org/dewey/"/>
    <rdfs:label xml:lang="en">DDC</rdfs:label>
    <rdfs:isDefinedBy rdf:resource="http://purl.org/dc/terms/"/>
    <rdfs:comment xml:lang="en">The set of conceptual resources specified by the Dewey Decimal Classification.</rdfs:comment>
    <dc:issued rdf:datatype="http://www.w3.org/2001/XMLSchema#date">2000-07-11</dc:issued>
    <rdf:type rdf:resource="http://purl.org/dc/dcam/VocabularyEncodingScheme"/>
    <rdf:type rdf:resource="http://www.w3.org/2002/07/owl#NamedIndividual"/>
  </rdf:Description>
  <rdf:Description rdf:nodeID="A39">
    <owl:allValuesFrom rdf:resource="http://w3id.org/arto#Connotation"/>
    <owl:onProperty rdf:resource="http://w3id.org/arto#hasConnotation"/>
    <rdf:type rdf:resource="http://www.w3.org/2002/07/owl#Restriction"/>
  </rdf:Description>
  <rdf:Description rdf:about="http://w3id.org/arto#isSceneOf">
    <skos:example>
                - Nested scenes: :vendor_scene arto:isSceneOf :market_scene
                - Background scenes: :mountain_scene arto:isSceneOf :landscape_painting</skos:example>
    <rdfs:label>isSceneOf</rdfs:label>
    <rdfs:comment>Specifies the artwork or scene that contains the scene in the artwork.</rdfs:comment>
    <rdfs:range rdf:nodeID="A86"/>
    <rdfs:domain rdf:resource="http://w3id.org/arto#Scene"/>
    <rdf:type rdf:resource="http://www.w3.org/2002/07/owl#ObjectProperty"/>
  </rdf:Description>
  <rdf:Description rdf:about="http://purl.org/dc/terms/LocationPeriodOrJurisdiction">
    <rdfs:label xml:lang="en">Location, Period, or Jurisdiction</rdfs:label>
    <rdfs:isDefinedBy rdf:resource="http://purl.org/dc/terms/"/>
    <rdfs:comment xml:lang="en">A location, period of time, or jurisdiction.</rdfs:comment>
    <dc:issued rdf:datatype="http://www.w3.org/2001/XMLSchema#date">2008-01-14</dc:issued>
    <rdf:type rdf:resource="http://www.w3.org/2002/07/owl#NamedIndividual"/>
    <rdf:type rdf:resource="http://www.w3.org/2002/07/owl#Class"/>
  </rdf:Description>
  <rdf:Description rdf:about="http://www.europeana.eu/schemas/edm/isShownBy">
    <rdf:type rdf:resource="http://www.w3.org/2002/07/owl#DatatypeProperty"/>
  </rdf:Description>
  <rdf:Description rdf:nodeID="A87">
    <owl:minCardinality rdf:datatype="http://www.w3.org/2001/XMLSchema#nonNegativeInteger">1</owl:minCardinality>
  </rdf:Description>
  <rdf:Description rdf:about="http://purl.org/dc/terms/isPartOf">
    <rdfs:label xml:lang="en">Is Part Of</rdfs:label>
    <rdfs:isDefinedBy rdf:resource="http://purl.org/dc/terms/"/>
    <rdfs:comment xml:lang="en">A related resource in which the described resource is physically or logically included.</rdfs:comment>
    <dc:description xml:lang="en">This property is intended to be used with non-literal values. This property is an inverse property of Has Part.</dc:description>
    <dc:issued rdf:datatype="http://www.w3.org/2001/XMLSchema#date">2000-07-11</dc:issued>
    <rdf:type rdf:resource="http://www.w3.org/2002/07/owl#NamedIndividual"/>
    <rdfs:subPropertyOf rdf:resource="http://purl.org/dc/terms/relation"/>
    <rdfs:subPropertyOf rdf:resource="http://purl.org/dc/elements/1.1/relation"/>
    <rdf:type rdf:resource="http://www.w3.org/2002/07/owl#AnnotationProperty"/>
  </rdf:Description>
  <rdf:Description rdf:nodeID="A88">
    <owl:cardinality rdf:datatype="http://www.w3.org/2001/XMLSchema#nonNegativeInteger">1</owl:cardinality>
  </rdf:Description>
  <rdf:Description rdf:about="http://purl.org/dc/terms/MediaType">
    <rdfs:label xml:lang="en">Media Type</rdfs:label>
    <rdfs:isDefinedBy rdf:resource="http://purl.org/dc/terms/"/>
    <rdfs:comment xml:lang="en">A file format or physical medium.</rdfs:comment>
    <dc:issued rdf:datatype="http://www.w3.org/2001/XMLSchema#date">2008-01-14</dc:issued>
    <rdf:type rdf:resource="http://www.w3.org/2002/07/owl#NamedIndividual"/>
    <rdfs:subClassOf rdf:resource="http://purl.org/dc/terms/MediaTypeOrExtent"/>
    <rdf:type rdf:resource="http://www.w3.org/2002/07/owl#Class"/>
  </rdf:Description>
  <rdf:Description rdf:about="http://purl.org/dc/dcam/VocabularyEncodingScheme">
    <rdf:type rdf:resource="http://www.w3.org/2002/07/owl#Class"/>
  </rdf:Description>
  <rdf:Description rdf:about="http://purl.org/dc/terms/temporal">
    <rdfs:label xml:lang="en">Temporal Coverage</rdfs:label>
    <rdfs:isDefinedBy rdf:resource="http://purl.org/dc/terms/"/>
    <rdfs:comment xml:lang="en">Temporal characteristics of the resource.</rdfs:comment>
    <j.0:rangeIncludes rdf:resource="http://purl.org/dc/terms/PeriodOfTime"/>
    <dc:issued rdf:datatype="http://www.w3.org/2001/XMLSchema#date">2000-07-11</dc:issued>
    <rdf:type rdf:resource="http://www.w3.org/2002/07/owl#NamedIndividual"/>
    <rdfs:subPropertyOf rdf:resource="http://purl.org/dc/terms/coverage"/>
    <rdfs:subPropertyOf rdf:resource="http://purl.org/dc/elements/1.1/coverage"/>
    <rdf:type rdf:resource="http://www.w3.org/2002/07/owl#AnnotationProperty"/>
  </rdf:Description>
  <rdf:Description rdf:about="http://xmlns.com/foaf/spec/Person">
    <rdf:type rdf:resource="http://www.w3.org/2002/07/owl#Class"/>
  </rdf:Description>
  <rdf:Description rdf:nodeID="A89">
    <owl:cardinality rdf:datatype="http://www.w3.org/2001/XMLSchema#nonNegativeInteger">1</owl:cardinality>
  </rdf:Description>
  <rdf:Description rdf:about="http://purl.org/dc/terms/Point">
    <rdfs:seeAlso rdf:resource="https://www.dublincore.org/specifications/dublin-core/dcmi-point/"/>
    <rdfs:label xml:lang="en">DCMI Point</rdfs:label>
    <rdfs:isDefinedBy rdf:resource="http://purl.org/dc/terms/"/>
    <rdfs:comment xml:lang="en">The set of points in space defined by their geographic coordinates according to the DCMI Point Encoding Scheme.</rdfs:comment>
    <dc:issued rdf:datatype="http://www.w3.org/2001/XMLSchema#date">2000-07-11</dc:issued>
    <rdf:type rdf:resource="http://www.w3.org/2002/07/owl#NamedIndividual"/>
    <rdf:type rdf:resource="http://www.w3.org/2000/01/rdf-schema#Datatype"/>
  </rdf:Description>
  <rdf:Description rdf:about="http://w3id.org/arto#EmotionIntensity">
    <rdfs:label>EmotionIntensity</rdfs:label>
    <rdfs:comment>Represents the measured strength of an emotional response evoked by an artwork. 
Values may be expressed on different scales, for example:
- Categorical levels such as low / medium / high
- Numeric ranges (e.g., 0-1, 1-5, or 1-10)
This flexibility allows projects to choose the scale best suited to their analytical or interpretive framework.</rdfs:comment>
    <rdfs:subClassOf rdf:resource="http://w3id.org/arto#Metric"/>
    <rdf:type rdf:resource="http://www.w3.org/2002/07/owl#Class"/>
  </rdf:Description>
  <rdf:Description rdf:nodeID="A90">
    <rdf:rest rdf:nodeID="A14"/>
    <rdf:first>HSV</rdf:first>
    <rdf:type rdf:resource="http://www.w3.org/1999/02/22-rdf-syntax-ns#List"/>
  </rdf:Description>
  <rdf:Description rdf:about="http://purl.org/dc/terms/BibliographicResource">
    <rdfs:label xml:lang="en">Bibliographic Resource</rdfs:label>
    <rdfs:isDefinedBy rdf:resource="http://purl.org/dc/terms/"/>
    <rdfs:comment xml:lang="en">A book, article, or other documentary resource.</rdfs:comment>
    <dc:issued rdf:datatype="http://www.w3.org/2001/XMLSchema#date">2008-01-14</dc:issued>
    <rdf:type rdf:resource="http://www.w3.org/2002/07/owl#NamedIndividual"/>
    <rdf:type rdf:resource="http://www.w3.org/2002/07/owl#Class"/>
  </rdf:Description>
  <rdf:Description rdf:about="http://purl.org/dc/terms/publisher">
    <rdfs:label xml:lang="en">Publisher</rdfs:label>
    <rdfs:isDefinedBy rdf:resource="http://purl.org/dc/terms/"/>
    <rdfs:comment xml:lang="en">An entity responsible for making the resource available.</rdfs:comment>
    <j.0:rangeIncludes rdf:resource="http://purl.org/dc/terms/Agent"/>
    <dc:issued rdf:datatype="http://www.w3.org/2001/XMLSchema#date">2008-01-14</dc:issued>
    <rdf:type rdf:resource="http://www.w3.org/2002/07/owl#NamedIndividual"/>
    <rdfs:subPropertyOf rdf:resource="http://purl.org/dc/elements/1.1/publisher"/>
    <rdf:type rdf:resource="http://www.w3.org/2002/07/owl#AnnotationProperty"/>
  </rdf:Description>
  <rdf:Description rdf:about="http://w3id.org/arto#hasColourTerm">
    <rdfs:label>hasColourTerm</rdfs:label>
    <skos:example>
                    :colour1 a arto:Colour ;
                      arto:hasColourTerm aat:red .

                    :colour2 a arto:Colour ;
                      arto:hasColourTerm aat:vermillion .

                    :colour3 a arto:Colour ;
                      arto:hasColourTerm aat:imperial_yellow .

                    </skos:example>
    <rdfs:comment>Links a colour to its corresponding standardised term from controlled vocabularies, establishing semantic connections that enable consistent colour identification, hierarchical classification, and cross-institutional interoperability for cultural heritage documentation and research.</rdfs:comment>
    <rdfs:range rdf:resource="http://w3id.org/arto#ColourTerm"/>
    <rdfs:domain rdf:resource="http://w3id.org/arto#Colour"/>
    <rdf:type rdf:resource="http://www.w3.org/2002/07/owl#ObjectProperty"/>
  </rdf:Description>
  <rdf:Description rdf:about="http://purl.org/dc/terms/IMT">
    <rdfs:seeAlso rdf:resource="http://www.iana.org/assignments/media-types/"/>
    <rdfs:label xml:lang="en">IMT</rdfs:label>
    <rdfs:isDefinedBy rdf:resource="http://purl.org/dc/terms/"/>
    <rdfs:comment xml:lang="en">The set of media types specified by the Internet Assigned Numbers Authority.</rdfs:comment>
    <dc:issued rdf:datatype="http://www.w3.org/2001/XMLSchema#date">2000-07-11</dc:issued>
    <rdf:type rdf:resource="http://purl.org/dc/dcam/VocabularyEncodingScheme"/>
    <rdf:type rdf:resource="http://www.w3.org/2002/07/owl#NamedIndividual"/>
  </rdf:Description>
  <rdf:Description rdf:nodeID="A91">
    <owl:allValuesFrom rdf:resource="http://w3id.org/arto#Connotation"/>
    <owl:onProperty rdf:resource="http://w3id.org/arto#hasConnotation"/>
    <rdf:type rdf:resource="http://www.w3.org/2002/07/owl#Restriction"/>
  </rdf:Description>
  <rdf:Description rdf:nodeID="A73">
    <rdf:rest rdf:nodeID="A92"/>
    <rdf:first rdf:resource="http://www.w3.org/2004/02/skos/core#Concept"/>
  </rdf:Description>
  <rdf:Description rdf:about="http://purl.org/dc/terms/UDC">
    <rdfs:seeAlso rdf:resource="http://www.udcc.org/"/>
    <rdfs:label xml:lang="en">UDC</rdfs:label>
    <rdfs:isDefinedBy rdf:resource="http://purl.org/dc/terms/"/>
    <rdfs:comment xml:lang="en">The set of conceptual resources specified by the Universal Decimal Classification.</rdfs:comment>
    <dc:issued rdf:datatype="http://www.w3.org/2001/XMLSchema#date">2000-07-11</dc:issued>
    <rdf:type rdf:resource="http://purl.org/dc/dcam/VocabularyEncodingScheme"/>
    <rdf:type rdf:resource="http://www.w3.org/2002/07/owl#NamedIndividual"/>
  </rdf:Description>
  <rdf:Description rdf:nodeID="A93">
    <rdf:rest rdf:nodeID="A57"/>
    <rdf:first>Lab</rdf:first>
  </rdf:Description>
  <rdf:Description rdf:about="http://w3id.org/arto#Series">
    <rdfs:label>Series</rdfs:label>
    <rdfs:comment>A collection of related artworks that share common characteristics, themes, or purposes, including:
                - Thematic series
                - Chronological series
                - Technique-based series
                - Subject-based series
                - Experimental series
                - Documentary series</rdfs:comment>
    <rdfs:subClassOf rdf:nodeID="A94"/>
    <rdfs:subClassOf rdf:resource="https://schema.org/CreativeWorkSeries"/>
    <rdf:type rdf:resource="http://www.w3.org/2002/07/owl#Class"/>
  </rdf:Description>
  <rdf:Description rdf:about="http://purl.org/dc/terms/RFC1766">
    <rdfs:seeAlso rdf:resource="http://www.ietf.org/rfc/rfc1766.txt"/>
    <rdfs:label xml:lang="en">RFC 1766</rdfs:label>
    <rdfs:isDefinedBy rdf:resource="http://purl.org/dc/terms/"/>
    <rdfs:comment xml:lang="en">The set of tags, constructed according to RFC 1766, for the identification of languages.</rdfs:comment>
    <dc:issued rdf:datatype="http://www.w3.org/2001/XMLSchema#date">2000-07-11</dc:issued>
    <rdf:type rdf:resource="http://www.w3.org/2002/07/owl#NamedIndividual"/>
    <rdf:type rdf:resource="http://www.w3.org/2000/01/rdf-schema#Datatype"/>
  </rdf:Description>
  <rdf:Description rdf:nodeID="A50">
    <owl:oneOf rdf:nodeID="A95"/>
    <rdf:type rdf:resource="http://www.w3.org/2000/01/rdf-schema#Datatype"/>
  </rdf:Description>
  <rdf:Description rdf:nodeID="A96">
    <owl:unionOf rdf:nodeID="A97"/>
    <rdf:type rdf:resource="http://www.w3.org/2002/07/owl#Class"/>
  </rdf:Description>
  <rdf:Description rdf:about="http://purl.org/dc/terms/hasVersion">
    <rdfs:label xml:lang="en">Has Version</rdfs:label>
    <rdfs:isDefinedBy rdf:resource="http://purl.org/dc/terms/"/>
    <rdfs:comment xml:lang="en">A related resource that is a version, edition, or adaptation of the described resource.</rdfs:comment>
    <dc:description xml:lang="en">Changes in version imply substantive changes in content rather than differences in format. This property is intended to be used with non-literal values. This property is an inverse property of Is Version Of.</dc:description>
    <dc:issued rdf:datatype="http://www.w3.org/2001/XMLSchema#date">2000-07-11</dc:issued>
    <rdf:type rdf:resource="http://www.w3.org/2002/07/owl#NamedIndividual"/>
    <rdfs:subPropertyOf rdf:resource="http://purl.org/dc/terms/relation"/>
    <rdfs:subPropertyOf rdf:resource="http://purl.org/dc/elements/1.1/relation"/>
    <rdf:type rdf:resource="http://www.w3.org/2002/07/owl#AnnotationProperty"/>
  </rdf:Description>
  <rdf:Description rdf:nodeID="A98">
    <owl:hasValue rdf:resource="http://vocab.getty.edu/aat/300053001"/>
    <owl:onProperty rdf:resource="http://www.w3.org/2004/02/skos/core#broaderTransitive"/>
    <rdf:type rdf:resource="http://www.w3.org/2002/07/owl#Restriction"/>
  </rdf:Description>
  <rdf:Description rdf:about="http://purl.org/dc/terms/ProvenanceStatement">
    <rdfs:label xml:lang="en">Provenance Statement</rdfs:label>
    <rdfs:isDefinedBy rdf:resource="http://purl.org/dc/terms/"/>
    <rdfs:comment xml:lang="en">Any changes in ownership and custody of a resource since its creation that are significant for its authenticity, integrity, and interpretation.</rdfs:comment>
    <dc:issued rdf:datatype="http://www.w3.org/2001/XMLSchema#date">2008-01-14</dc:issued>
    <rdf:type rdf:resource="http://www.w3.org/2002/07/owl#NamedIndividual"/>
    <rdf:type rdf:resource="http://www.w3.org/2002/07/owl#Class"/>
  </rdf:Description>
  <rdf:Description rdf:nodeID="A99">
    <rdf:rest rdf:nodeID="A100"/>
    <rdf:first rdf:resource="http://w3id.org/arto#Object"/>
  </rdf:Description>
  <rdf:Description rdf:nodeID="A101">
    <rdf:rest rdf:nodeID="A102"/>
    <rdf:first>artwork</rdf:first>
    <rdf:type rdf:resource="http://www.w3.org/1999/02/22-rdf-syntax-ns#List"/>
  </rdf:Description>
  <rdf:Description rdf:about="http://purl.org/dc/terms/Policy">
    <rdfs:label xml:lang="en">Policy</rdfs:label>
    <rdfs:isDefinedBy rdf:resource="http://purl.org/dc/terms/"/>
    <rdfs:comment xml:lang="en">A plan or course of action by an authority, intended to influence and determine decisions, actions, and other matters.</rdfs:comment>
    <dc:issued rdf:datatype="http://www.w3.org/2001/XMLSchema#date">2008-01-14</dc:issued>
    <rdf:type rdf:resource="http://www.w3.org/2002/07/owl#NamedIndividual"/>
    <rdf:type rdf:resource="http://www.w3.org/2002/07/owl#Class"/>
  </rdf:Description>
  <rdf:Description rdf:about="http://purl.org/dc/terms/description">
    <rdfs:label xml:lang="en">Description</rdfs:label>
    <rdfs:isDefinedBy rdf:resource="http://purl.org/dc/terms/"/>
    <rdfs:comment xml:lang="en">An account of the resource.</rdfs:comment>
    <dc:description xml:lang="en">Description may include but is not limited to: an abstract, a table of contents, a graphical representation, or a free-text account of the resource.</dc:description>
    <dc:issued rdf:datatype="http://www.w3.org/2001/XMLSchema#date">2008-01-14</dc:issued>
    <rdf:type rdf:resource="http://www.w3.org/2002/07/owl#NamedIndividual"/>
    <rdfs:subPropertyOf rdf:resource="http://purl.org/dc/elements/1.1/description"/>
  </rdf:Description>
  <rdf:Description rdf:about="http://purl.org/dc/terms/audience">
    <rdfs:label xml:lang="en">Audience</rdfs:label>
    <rdfs:isDefinedBy rdf:resource="http://purl.org/dc/terms/"/>
    <rdfs:comment xml:lang="en">A class of agents for whom the resource is intended or useful.</rdfs:comment>
    <dc:description xml:lang="en">Recommended practice is to use this property with non-literal values from a vocabulary of audience types.</dc:description>
    <j.0:rangeIncludes rdf:resource="http://purl.org/dc/terms/AgentClass"/>
    <dc:issued rdf:datatype="http://www.w3.org/2001/XMLSchema#date">2001-05-21</dc:issued>
    <rdf:type rdf:resource="http://www.w3.org/2002/07/owl#NamedIndividual"/>
    <rdf:type rdf:resource="http://www.w3.org/2002/07/owl#AnnotationProperty"/>
  </rdf:Description>
  <rdf:Description rdf:about="http://purl.org/dc/elements/1.1/creator">
    <rdf:type rdf:resource="http://www.w3.org/2002/07/owl#AnnotationProperty"/>
  </rdf:Description>
  <rdf:Description rdf:nodeID="A103">
    <owl:cardinality rdf:datatype="http://www.w3.org/2001/XMLSchema#nonNegativeInteger">1</owl:cardinality>
  </rdf:Description>
  <rdf:Description rdf:about="http://purl.org/dc/terms/accrualPolicy">
    <rdfs:label xml:lang="en">Accrual Policy</rdfs:label>
    <rdfs:isDefinedBy rdf:resource="http://purl.org/dc/terms/"/>
    <rdfs:comment xml:lang="en">The policy governing the addition of items to a collection.</rdfs:comment>
    <dc:description xml:lang="en">Recommended practice is to use a value from the Collection Description Accrual Policy Vocabulary [[DCMI-ACCRUALPOLICY](https://dublincore.org/groups/collections/accrual-policy/)].</dc:description>
    <j.0:rangeIncludes rdf:resource="http://purl.org/dc/terms/Policy"/>
    <dc:issued rdf:datatype="http://www.w3.org/2001/XMLSchema#date">2005-06-13</dc:issued>
    <rdf:type rdf:resource="http://www.w3.org/2002/07/owl#NamedIndividual"/>
    <rdfs:domain rdf:resource="http://purl.org/dc/dcmitype/Collection"/>
    <rdf:type rdf:resource="http://www.w3.org/2002/07/owl#AnnotationProperty"/>
  </rdf:Description>
  <rdf:Description rdf:nodeID="A65">
    <owl:allValuesFrom rdf:resource="http://w3id.org/arto#ColourValue"/>
    <owl:onProperty rdf:resource="http://w3id.org/arto#hasColourValue"/>
    <rdf:type rdf:resource="http://www.w3.org/2002/07/owl#Restriction"/>
  </rdf:Description>
  <rdf:Description rdf:about="http://purl.org/dc/terms/hasFormat">
    <rdfs:label xml:lang="en">Has Format</rdfs:label>
    <rdfs:isDefinedBy rdf:resource="http://purl.org/dc/terms/"/>
    <rdfs:comment xml:lang="en">A related resource that is substantially the same as the pre-existing described resource, but in another format.</rdfs:comment>
    <dc:description xml:lang="en">This property is intended to be used with non-literal values. This property is an inverse property of Is Format Of.</dc:description>
    <dc:issued rdf:datatype="http://www.w3.org/2001/XMLSchema#date">2000-07-11</dc:issued>
    <rdf:type rdf:resource="http://www.w3.org/2002/07/owl#NamedIndividual"/>
    <rdfs:subPropertyOf rdf:resource="http://purl.org/dc/terms/relation"/>
    <rdfs:subPropertyOf rdf:resource="http://purl.org/dc/elements/1.1/relation"/>
    <rdf:type rdf:resource="http://www.w3.org/2002/07/owl#AnnotationProperty"/>
  </rdf:Description>
  <rdf:Description rdf:nodeID="A104">
    <owl:minCardinality rdf:datatype="http://www.w3.org/2001/XMLSchema#nonNegativeInteger">1</owl:minCardinality>
  </rdf:Description>
  <rdf:Description rdf:nodeID="A35">
    <rdf:rest rdf:nodeID="A105"/>
    <rdf:first>RGB</rdf:first>
  </rdf:Description>
  <rdf:Description rdf:about="http://w3id.org/arto#Time">
    <skos:example>
            :picassoBirth a arto:Time ;
              dc:type "biographical" ;
              sdo:startDate "1881-10-25T00:00:00"^^xsd:dateTime ;
              sdo:endDate   "1881-10-25T23:59:59"^^xsd:dateTime .

            :impressionismPeak a arto:Time ;
              dc:type "historical-period" ;
              sdo:startDate "1890-01-01T00:00:00"^^xsd:dateTime ;
              sdo:endDate   "1899-12-31T23:59:59"^^xsd:dateTime .

            :guernicaCreationPhase a arto:Time ;
              dc:type "creation" ;
              sdo:startDate "1937-03-01T00:00:00"^^xsd:dateTime ;
              sdo:endDate   "1937-05-31T23:59:59"^^xsd:dateTime .

            :earlyModernistPeriod a arto:Time ;
              dc:type "historical-period" ;
              sdo:startDate "1895-01-01T00:00:00"^^xsd:dateTime ;
              sdo:endDate   "1905-12-31T23:59:59"^^xsd:dateTime .

            :bluePeriod a arto:Time ;
              dc:type "creation" ;
              sdo:startDate "1901-01-01T00:00:00"^^xsd:dateTime ;
              sdo:endDate   "1905-12-31T23:59:59"^^xsd:dateTime .
          </skos:example>
    <rdfs:label>Time</rdfs:label>
    <rdfs:comment>Represents temporal aspects related to artworks and related events. 
A Time instance may indicate exact dates, approximate or uncertain periods, broader intervals (decades, centuries), 
or seasonal references as they appear in historical sources. The type may classify the temporal role, 
such as creation, exhibition, depiction, historical period, or conservation.</rdfs:comment>
    <rdfs:subClassOf rdf:nodeID="A106"/>
    <rdfs:subClassOf rdf:nodeID="A64"/>
    <rdfs:subClassOf rdf:nodeID="A107"/>
    <owl:equivalentClass rdf:resource="http://www.w3.org/2006/time#TemporalEntity"/>
    <rdf:type rdf:resource="http://www.w3.org/2002/07/owl#Class"/>
  </rdf:Description>
  <rdf:Description rdf:about="http://purl.org/dc/terms/language">
    <rdfs:label xml:lang="en">Language</rdfs:label>
    <rdfs:isDefinedBy rdf:resource="http://purl.org/dc/terms/"/>
    <rdfs:comment xml:lang="en">A language of the resource.</rdfs:comment>
    <dc:description xml:lang="en">Recommended practice is to use either a non-literal value representing a language from a controlled vocabulary such as ISO 639-2 or ISO 639-3, or a literal value consisting of an IETF Best Current Practice 47 [[IETF-BCP47](https://tools.ietf.org/html/bcp47)] language tag.</dc:description>
    <j.0:rangeIncludes rdf:resource="http://purl.org/dc/terms/LinguisticSystem"/>
    <dc:issued rdf:datatype="http://www.w3.org/2001/XMLSchema#date">2008-01-14</dc:issued>
    <rdf:type rdf:resource="http://www.w3.org/2002/07/owl#NamedIndividual"/>
    <rdfs:subPropertyOf rdf:resource="http://purl.org/dc/elements/1.1/language"/>
    <rdf:type rdf:resource="http://www.w3.org/2002/07/owl#AnnotationProperty"/>
  </rdf:Description>
  <rdf:Description rdf:about="http://w3id.org/arto#MediumType">
    <rdfs:label>MediumType</rdfs:label>
    <rdfs:comment>Represents the medium of an artwork, such as oil on canvas, watercolour, etc. This class allows for the classification of artworks based on the materials and techniques used in their creation.</rdfs:comment>
    <rdfs:subClassOf rdf:nodeID="A96"/>
    <rdf:type rdf:resource="http://www.w3.org/2002/07/owl#Class"/>
  </rdf:Description>
  <rdf:Description rdf:about="http://purl.org/dc/elements/1.1/format">
    <rdf:type rdf:resource="http://www.w3.org/2002/07/owl#AnnotationProperty"/>
  </rdf:Description>
  <rdf:Description rdf:nodeID="A95">
    <rdf:rest rdf:nodeID="A108"/>
    <rdf:first>CMYK</rdf:first>
    <rdf:type rdf:resource="http://www.w3.org/1999/02/22-rdf-syntax-ns#List"/>
  </rdf:Description>
  <rdf:Description rdf:nodeID="A109">
    <owl:maxQualifiedCardinality rdf:datatype="http://www.w3.org/2001/XMLSchema#nonNegativeInteger">1</owl:maxQualifiedCardinality>
  </rdf:Description>
  <rdf:Description rdf:nodeID="A110">
    <owl:minCardinality rdf:datatype="http://www.w3.org/2001/XMLSchema#nonNegativeInteger">1</owl:minCardinality>
  </rdf:Description>
  <rdf:Description rdf:nodeID="A111">
    <owl:unionOf rdf:nodeID="A112"/>
    <rdf:type rdf:resource="http://www.w3.org/2002/07/owl#Class"/>
  </rdf:Description>
  <rdf:Description rdf:nodeID="A100">
    <rdf:rest rdf:nodeID="A60"/>
    <rdf:first rdf:resource="http://w3id.org/arto#Scene"/>
  </rdf:Description>
  <rdf:Description rdf:about="http://w3id.org/arto#Sculpture">
    <rdfs:label>Sculpture</rdfs:label>
    <rdfs:comment>A specific type of artwork created using sculptural techniques, such as carving,
      modelling, or casting.</rdfs:comment>
    <rdfs:subClassOf rdf:resource="http://w3id.org/arto#Artwork"/>
    <rdf:type rdf:resource="http://www.w3.org/2002/07/owl#Class"/>
  </rdf:Description>
  <rdf:Description rdf:nodeID="A113">
    <owl:allValuesFrom rdf:resource="http://qudt.org/schema/qudt/Vector"/>
    <owl:onProperty rdf:resource="http://w3id.org/arto#hasCoordinates"/>
    <rdf:type rdf:resource="http://www.w3.org/2002/07/owl#Restriction"/>
  </rdf:Description>
  <rdf:Description rdf:about="http://w3id.org/arto#isConnotationOf">
    <skos:example>
                    - Emotional expression: :anger_emotion arto:isConnotationOf :red_colour
                    - Symbolic meaning: :peace_meaning arto:isConnotationOf :dove_object
                    - Scene mood: :turbulence_emotion arto:isConnotationOf :storm_scene
                    - Artwork meaning: :anti_war_theme arto:isConnotationOf :guernica</skos:example>
    <rdfs:label>isConnotationOf</rdfs:label>
    <rdfs:comment>Associates a connotation with the visual elements, objects, scenes or artwork that express it.</rdfs:comment>
    <rdfs:range rdf:nodeID="A114"/>
    <rdfs:domain rdf:resource="http://w3id.org/arto#Connotation"/>
    <rdf:type rdf:resource="http://www.w3.org/2002/07/owl#ObjectProperty"/>
  </rdf:Description>
  <rdf:Description rdf:about="http://purl.org/dc/terms/license">
    <rdfs:label xml:lang="en">License</rdfs:label>
    <rdfs:isDefinedBy rdf:resource="http://purl.org/dc/terms/"/>
    <rdfs:comment xml:lang="en">A legal document giving official permission to do something with the resource.</rdfs:comment>
    <dc:description xml:lang="en">Recommended practice is to identify the license document with a URI. If this is not possible or feasible, a literal value that identifies the license may be provided.</dc:description>
    <j.0:rangeIncludes rdf:resource="http://purl.org/dc/terms/LicenseDocument"/>
    <dc:issued rdf:datatype="http://www.w3.org/2001/XMLSchema#date">2004-06-14</dc:issued>
    <rdf:type rdf:resource="http://www.w3.org/2002/07/owl#NamedIndividual"/>
    <rdfs:subPropertyOf rdf:resource="http://purl.org/dc/terms/rights"/>
    <rdfs:subPropertyOf rdf:resource="http://purl.org/dc/elements/1.1/rights"/>
    <rdf:type rdf:resource="http://www.w3.org/2002/07/owl#AnnotationProperty"/>
  </rdf:Description>
  <rdf:Description rdf:about="http://purl.org/dc/elements/1.1/publisher">
    <rdf:type rdf:resource="http://www.w3.org/2002/07/owl#AnnotationProperty"/>
  </rdf:Description>
  <rdf:Description rdf:nodeID="A114">
    <owl:unionOf rdf:nodeID="A115"/>
    <rdf:type rdf:resource="http://www.w3.org/2002/07/owl#Class"/>
  </rdf:Description>
  <rdf:Description rdf:nodeID="A83">
    <owl:oneOf rdf:nodeID="A80"/>
    <rdf:type rdf:resource="http://www.w3.org/2000/01/rdf-schema#Datatype"/>
  </rdf:Description>
  <rdf:Description rdf:about="http://purl.org/dc/terms/date">
    <rdfs:label xml:lang="en">Date</rdfs:label>
    <rdfs:isDefinedBy rdf:resource="http://purl.org/dc/terms/"/>
    <rdfs:comment xml:lang="en">A point or period of time associated with an event in the lifecycle of the resource.</rdfs:comment>
    <dc:description xml:lang="en">Date may be used to express temporal information at any level of granularity.  Recommended practice is to express the date, date/time, or period of time according to ISO 8601-1 [[ISO 8601-1](https://www.iso.org/iso-8601-date-and-time-format.html)] or a published profile of the ISO standard, such as the W3C Note on Date and Time Formats [[W3CDTF](https://www.w3.org/TR/NOTE-datetime)] or the Extended Date/Time Format Specification [[EDTF](http://www.loc.gov/standards/datetime/)].  If the full date is unknown, month and year (YYYY-MM) or just year (YYYY) may be used. Date ranges may be specified using ISO 8601 period of time specification in which start and end dates are separated by a '/' (slash) character.  Either the start or end date may be missing.</dc:description>
    <dc:issued rdf:datatype="http://www.w3.org/2001/XMLSchema#date">2008-01-14</dc:issued>
    <rdf:type rdf:resource="http://www.w3.org/2002/07/owl#NamedIndividual"/>
    <rdf:type rdf:resource="http://www.w3.org/2002/07/owl#DatatypeProperty"/>
    <rdfs:range rdf:resource="http://www.w3.org/2000/01/rdf-schema#Literal"/>
    <rdfs:subPropertyOf rdf:resource="http://purl.org/dc/elements/1.1/date"/>
    <rdf:type rdf:resource="http://www.w3.org/2002/07/owl#AnnotationProperty"/>
  </rdf:Description>
  <rdf:Description rdf:nodeID="A116">
    <owl:cardinality rdf:datatype="http://www.w3.org/2001/XMLSchema#nonNegativeInteger">1</owl:cardinality>
  </rdf:Description>
  <rdf:Description rdf:about="http://purl.org/dc/terms/subject">
    <rdfs:label xml:lang="en">Subject</rdfs:label>
    <rdfs:isDefinedBy rdf:resource="http://purl.org/dc/terms/"/>
    <rdfs:comment xml:lang="en">A topic of the resource.</rdfs:comment>
    <dc:description xml:lang="en">Recommended practice is to refer to the subject with a URI. If this is not possible or feasible, a literal value that identifies the subject may be provided. Both should preferably refer to a subject in a controlled vocabulary.</dc:description>
    <dc:issued rdf:datatype="http://www.w3.org/2001/XMLSchema#date">2008-01-14</dc:issued>
    <rdf:type rdf:resource="http://www.w3.org/2002/07/owl#NamedIndividual"/>
    <rdfs:subPropertyOf rdf:resource="http://purl.org/dc/elements/1.1/subject"/>
    <rdf:type rdf:resource="http://www.w3.org/2002/07/owl#AnnotationProperty"/>
  </rdf:Description>
  <rdf:Description rdf:nodeID="A117">
    <rdf:rest rdf:nodeID="A118"/>
    <rdf:first rdf:resource="http://w3id.org/arto#Scene"/>
  </rdf:Description>
  <rdf:Description rdf:nodeID="A119">
    <owl:cardinality rdf:datatype="http://www.w3.org/2001/XMLSchema#nonNegativeInteger">1</owl:cardinality>
  </rdf:Description>
  <rdf:Description rdf:nodeID="A45">
    <owl:allValuesFrom rdf:resource="http://qudt.org/schema/qudt/Vector"/>
    <owl:onProperty rdf:resource="http://qudt.org/schema/qudt/vector"/>
    <rdf:type rdf:resource="http://www.w3.org/2002/07/owl#Restriction"/>
  </rdf:Description>
  <rdf:Description rdf:about="http://w3id.org/arto#material">
    <rdfs:label>material</rdfs:label>
    <skos:example>
                :glass_vase_obj     a arto:Object ; arto:material aat:glass .
                :pewter_plate_obj   a arto:Object ; arto:material aat:pewter .
                :walnut_table_obj   a arto:Object ; arto:material aat:walnut_wood . 
                </skos:example>
    <rdfs:comment>The material of the Object. It connect to the Getty AAT's material hierarchy, allowing for both standardised and custom material definitions. Not for the artwork's physical medium.</rdfs:comment>
    <rdfs:range rdf:resource="http://w3id.org/arto#MaterialType"/>
    <rdfs:domain rdf:resource="http://w3id.org/arto#Object"/>
    <rdf:type rdf:resource="http://www.w3.org/2002/07/owl#ObjectProperty"/>
  </rdf:Description>
  <rdf:Description rdf:nodeID="A120">
    <owl:cardinality rdf:datatype="http://www.w3.org/2001/XMLSchema#nonNegativeInteger">1</owl:cardinality>
  </rdf:Description>
  <rdf:Description rdf:about="http://w3id.org/arto#isTimeOf">
    <skos:example>
              - Event timing: :spring2024 arto:isTimeOf :exhibition2024
              - Location historical period: :belle_epoque arto:isTimeOf :paris_studio
              </skos:example>
    <rdfs:label>isTimeOf</rdfs:label>
    <rdfs:comment>Associates a time entity with the event that it is related to. The time entity may represent a specific date, a period (e.g., season, decade), or a cultural-historical era, allowing precise or approximate temporal anchoring of events or locations.</rdfs:comment>
    <rdfs:range rdf:resource="http://w3id.org/arto#Event"/>
    <rdfs:domain rdf:resource="http://w3id.org/arto#Time"/>
    <rdf:type rdf:resource="http://www.w3.org/2002/07/owl#ObjectProperty"/>
  </rdf:Description>
  <rdf:Description rdf:about="http://purl.org/dc/terms/DCMIType">
    <rdfs:seeAlso rdf:resource="http://purl.org/dc/dcmitype/"/>
    <rdfs:label xml:lang="en">DCMI Type Vocabulary</rdfs:label>
    <rdfs:isDefinedBy rdf:resource="http://purl.org/dc/terms/"/>
    <rdfs:comment xml:lang="en">The set of classes specified by the DCMI Type Vocabulary, used to categorize the nature or genre of the resource.</rdfs:comment>
    <rdfs:comment xml:lang="en">The set of classes specified by the DCMI Type Vocabulary, used to categorise the nature or genre of the resource.</rdfs:comment>
    <dc:issued rdf:datatype="http://www.w3.org/2001/XMLSchema#date">2000-07-11</dc:issued>
    <rdf:type rdf:resource="http://purl.org/dc/dcam/VocabularyEncodingScheme"/>
    <rdf:type rdf:resource="http://www.w3.org/2002/07/owl#NamedIndividual"/>
  </rdf:Description>
  <rdf:Description rdf:nodeID="A121">
    <owl:unionOf rdf:nodeID="A122"/>
    <rdf:type rdf:resource="http://www.w3.org/2002/07/owl#Class"/>
  </rdf:Description>
  <rdf:Description rdf:nodeID="A123">
    <rdf:rest rdf:resource="http://www.w3.org/1999/02/22-rdf-syntax-ns#nil"/>
    <rdf:first rdf:resource="http://w3id.org/arto#Scene"/>
  </rdf:Description>
  <rdf:Description rdf:about="http://purl.org/dc/terms/SizeOrDuration">
    <rdfs:label xml:lang="en">Size or Duration</rdfs:label>
    <rdfs:isDefinedBy rdf:resource="http://purl.org/dc/terms/"/>
    <rdfs:comment xml:lang="en">A dimension or extent, or a time taken to play or execute.</rdfs:comment>
    <dc:issued rdf:datatype="http://www.w3.org/2001/XMLSchema#date">2008-01-14</dc:issued>
    <dc:description xml:lang="en">Examples include a number of pages, a specification of length, width, and breadth, or a period in hours, minutes, and seconds.</dc:description>
    <rdfs:subClassOf rdf:resource="http://purl.org/dc/terms/MediaTypeOrExtent"/>
    <rdf:type rdf:resource="http://www.w3.org/2002/07/owl#Class"/>
  </rdf:Description>
  <rdf:Description rdf:about="http://purl.org/dc/terms/TGN">
    <rdfs:seeAlso rdf:resource="http://www.getty.edu/research/tools/vocabulary/tgn/index.html"/>
    <rdfs:label xml:lang="en">TGN</rdfs:label>
    <rdfs:isDefinedBy rdf:resource="http://purl.org/dc/terms/"/>
    <rdfs:comment xml:lang="en">The set of places specified by the Getty Thesaurus of Geographic Names.</rdfs:comment>
    <dc:issued rdf:datatype="http://www.w3.org/2001/XMLSchema#date">2000-07-11</dc:issued>
    <rdf:type rdf:resource="http://purl.org/dc/dcam/VocabularyEncodingScheme"/>
    <rdf:type rdf:resource="http://www.w3.org/2002/07/owl#NamedIndividual"/>
  </rdf:Description>
  <rdf:Description rdf:nodeID="A124">
    <rdf:rest rdf:resource="http://www.w3.org/1999/02/22-rdf-syntax-ns#nil"/>
    <rdf:first rdf:resource="http://w3id.org/arto#Scene"/>
  </rdf:Description>
  <rdf:Description rdf:nodeID="A86">
    <owl:unionOf rdf:nodeID="A20"/>
    <rdf:type rdf:resource="http://www.w3.org/2002/07/owl#Class"/>
  </rdf:Description>
  <rdf:Description rdf:nodeID="A24">
    <owl:allValuesFrom rdf:resource="http://www.w3.org/2001/XMLSchema#string"/>
    <owl:onProperty rdf:resource="http://purl.org/dc/terms/type"/>
    <rdf:type rdf:resource="http://www.w3.org/2002/07/owl#Restriction"/>
  </rdf:Description>
  <rdf:Description rdf:about="http://w3id.org/arto#Organisation">
    <rdfs:label>Organisation</rdfs:label>
    <rdfs:comment>Represents institutional entities involved in artwork creation, curation, preservation, or display, including museums, galleries, art schools, cultural institutions, commercial art enterprises, etc.</rdfs:comment>
    <owl:disjointWith rdf:resource="http://w3id.org/arto#Person"/>
    <rdfs:subClassOf rdf:resource="http://xmlns.com/foaf/spec/Organization"/>
    <rdfs:subClassOf rdf:resource="http://w3id.org/arto#Agent"/>
    <rdf:type rdf:resource="http://www.w3.org/2002/07/owl#Class"/>
  </rdf:Description>
  <rdf:Description rdf:about="http://w3id.org/arto#state">
    <skos:example>
               - Physical conditions: :broken_amphora arto:state :damaged_state ;
                 :marble_statue arto:state :weathered_state
               - Motion states: :running_horse arto:state :galloping_state ;
                 :falling_figure arto:state :in_motion_state
               - Positional states: :seated_figure arto:state :sitting_state ;
                 :reclining_venus arto:state :lying_state
               - Emotional states: :weeping_magdalene arto:state :grieving_state ;
                 :laughing_child arto:state :joyful_state
               - Temporal states: :blooming_flower arto:state :spring_state ;
                 :withered_leaves arto:state :autumn_state
               - Functional states: :open_book arto:state :readable_state ;
                 :lit_candle arto:state :burning_state
               </skos:example>
    <rdfs:label>state</rdfs:label>
    <rdfs:comment>Describes the condition, position, or status of objects within artworks, capturing both physical states (damaged, intact) and depicted conditions (motion, rest, emotional states of figures).</rdfs:comment>
    <rdfs:range rdf:resource="http://www.w3.org/2004/02/skos/core#Concept"/>
    <rdfs:domain rdf:resource="http://w3id.org/arto#Object"/>
    <rdf:type rdf:resource="http://www.w3.org/2002/07/owl#ObjectProperty"/>
  </rdf:Description>
  <rdf:Description rdf:nodeID="A125">
    <owl:allValuesFrom rdf:resource="http://w3id.org/arto#Object"/>
    <owl:onProperty rdf:resource="http://w3id.org/arto#relatedTo"/>
    <rdf:type rdf:resource="http://www.w3.org/2002/07/owl#Restriction"/>
  </rdf:Description>
  <rdf:Description rdf:nodeID="A126">
    <owl:allValuesFrom rdf:resource="http://w3id.org/arto#MediumType"/>
    <owl:onProperty rdf:resource="http://w3id.org/arto#medium"/>
    <rdf:type rdf:resource="http://www.w3.org/2002/07/owl#Restriction"/>
  </rdf:Description>
  <rdf:Description rdf:about="http://purl.org/dc/terms/accrualPeriodicity">
    <rdfs:label xml:lang="en">Accrual Periodicity</rdfs:label>
    <rdfs:isDefinedBy rdf:resource="http://purl.org/dc/terms/"/>
    <rdfs:comment xml:lang="en">The frequency with which items are added to a collection.</rdfs:comment>
    <dc:description xml:lang="en">Recommended practice is to use a value from the Collection Description Frequency Vocabulary [[DCMI-COLLFREQ](https://dublincore.org/groups/collections/frequency/)].</dc:description>
    <j.0:rangeIncludes rdf:resource="http://purl.org/dc/terms/Frequency"/>
    <dc:issued rdf:datatype="http://www.w3.org/2001/XMLSchema#date">2005-06-13</dc:issued>
    <rdf:type rdf:resource="http://www.w3.org/2002/07/owl#NamedIndividual"/>
    <rdfs:domain rdf:resource="http://purl.org/dc/dcmitype/Collection"/>
    <rdf:type rdf:resource="http://www.w3.org/2002/07/owl#AnnotationProperty"/>
  </rdf:Description>
  <rdf:Description rdf:about="http://w3id.org/arto#containsElement">
    <skos:example>
                      - colour elements: :sky_object arto:containsElement :blue_gradient_colour
                      - Line elements: :mountain_object arto:containsElement :diagonal_line
                      - Compositional elements: :tree_object arto:containsElement :vertical_composition</skos:example>
    <rdfs:label>containsElement</rdfs:label>
    <rdfs:comment>Specifies the visual elements (such as colour, line, composition) contained within an object in the artwork.</rdfs:comment>
    <rdfs:range rdf:resource="http://w3id.org/arto#VisualElement"/>
    <rdfs:domain rdf:nodeID="A127"/>
    <owl:inverseOf rdf:resource="http://w3id.org/arto#isElementOf"/>
    <rdf:type rdf:resource="http://www.w3.org/2002/07/owl#ObjectProperty"/>
  </rdf:Description>
  <rdf:Description rdf:nodeID="A128">
    <owl:cardinality rdf:datatype="http://www.w3.org/2001/XMLSchema#nonNegativeInteger">1</owl:cardinality>
  </rdf:Description>
  <rdf:Description rdf:about="http://w3id.org/arto#Person">
    <rdfs:label>Person</rdfs:label>
    <rdfs:comment>Individual human beings involved with artwork may include artists, curators, critics, collectors, conservators, researchers, and other roles.</rdfs:comment>
    <rdfs:subClassOf rdf:nodeID="A40"/>
    <rdfs:subClassOf rdf:resource="http://xmlns.com/foaf/spec/Person"/>
    <rdfs:subClassOf rdf:resource="http://w3id.org/arto#Agent"/>
    <rdf:type rdf:resource="http://www.w3.org/2002/07/owl#Class"/>
  </rdf:Description>
  <rdf:Description rdf:about="http://purl.org/dc/terms/isRequiredBy">
    <rdfs:label xml:lang="en">Is Required By</rdfs:label>
    <rdfs:isDefinedBy rdf:resource="http://purl.org/dc/terms/"/>
    <rdfs:comment xml:lang="en">A related resource that requires the described resource to support its function, delivery, or coherence.</rdfs:comment>
    <dc:description xml:lang="en">This property is intended to be used with non-literal values. This property is an inverse property of Requires.</dc:description>
    <dc:issued rdf:datatype="http://www.w3.org/2001/XMLSchema#date">2000-07-11</dc:issued>
    <rdf:type rdf:resource="http://www.w3.org/2002/07/owl#NamedIndividual"/>
    <rdfs:subPropertyOf rdf:resource="http://purl.org/dc/terms/relation"/>
    <rdfs:subPropertyOf rdf:resource="http://purl.org/dc/elements/1.1/relation"/>
    <rdf:type rdf:resource="http://www.w3.org/2002/07/owl#AnnotationProperty"/>
  </rdf:Description>
  <rdf:Description rdf:about="http://w3id.org/arto#direction">
    <rdfs:label>direction</rdfs:label>
    <rdfs:comment>Describes the orientation of linear elements in an artwork.</rdfs:comment>
    <rdfs:range rdf:resource="http://www.w3.org/2001/XMLSchema#string"/>
    <rdfs:domain rdf:resource="http://w3id.org/arto#Line"/>
    <rdf:type rdf:resource="http://www.w3.org/2002/07/owl#DatatypeProperty"/>
  </rdf:Description>
  <rdf:Description rdf:nodeID="A9">
    <owl:allValuesFrom rdf:resource="http://www.w3.org/2001/XMLSchema#string"/>
    <owl:onProperty rdf:resource="http://w3id.org/arto#source"/>
    <rdf:type rdf:resource="http://www.w3.org/2002/07/owl#Restriction"/>
  </rdf:Description>
  <rdf:Description rdf:nodeID="A129">
    <rdf:rest rdf:nodeID="A130"/>
    <rdf:first rdf:resource="http://www.w3.org/2004/02/skos/core#Concept"/>
  </rdf:Description>
  <rdf:Description rdf:nodeID="A131">
    <owl:allValuesFrom rdf:nodeID="A132"/>
    <owl:onProperty rdf:resource="http://w3id.org/arto#emotionPerspective"/>
    <rdf:type rdf:resource="http://www.w3.org/2002/07/owl#Restriction"/>
  </rdf:Description>
  <rdf:Description rdf:about="http://w3id.org/arto#hasCoordinates">
    <skos:example>
                        - Digital image coordinates: :main_figure arto:hasCoordinates qudt_Vector_250_300
                    qudt_Vector_250_300 rdf:type qudt:Vector ;
                        - 3D artwork coordinates: :sculpture_detail arto:hasCoordinates qudt_Vector_15_20_5
                    qudt_Vector_15_20_5 rdf:type qudt:Vector ;
                    </skos:example>
    <rdfs:label>hasCoordinates</rdfs:label>
    <rdfs:comment>Specifies the spatial location of objects and scenes within the artwork's coordinate system. This property supports spatial analysis, object relationship studies, compositional balance analysis, and digital humanities research requiring precise object localisation.</rdfs:comment>
    <rdfs:range rdf:resource="http://qudt.org/schema/qudt/Vector"/>
    <rdfs:domain rdf:nodeID="A121"/>
    <rdf:type rdf:resource="http://www.w3.org/2002/07/owl#ObjectProperty"/>
  </rdf:Description>
  <rdf:Description rdf:nodeID="A133">
    <rdf:rest rdf:nodeID="A101"/>
    <rdf:first>artist</rdf:first>
    <rdf:type rdf:resource="http://www.w3.org/1999/02/22-rdf-syntax-ns#List"/>
  </rdf:Description>
  <rdf:Description rdf:about="https://schema.org/startDate">
    <rdf:type rdf:resource="http://www.w3.org/2002/07/owl#DatatypeProperty"/>
  </rdf:Description>
  <rdf:Description rdf:nodeID="A134">
    <owl:cardinality rdf:datatype="http://www.w3.org/2001/XMLSchema#nonNegativeInteger">1</owl:cardinality>
  </rdf:Description>
  <rdf:Description rdf:nodeID="A69">
    <owl:unionOf rdf:nodeID="A135"/>
    <rdf:type rdf:resource="http://www.w3.org/2002/07/owl#Class"/>
  </rdf:Description>
  <rdf:Description rdf:about="http://w3id.org/arto#currentLocation">
    <skos:example>
                      - Museum location: :mona_lisa arto:currentLocation :louvre_museum
                      - Gallery location: :starry_night arto:currentLocation :moma_gallery_room_24
                      </skos:example>
    <owl:cardinality rdf:datatype="http://www.w3.org/2001/XMLSchema#integer">1</owl:cardinality>
    <rdfs:label>currentLocation</rdfs:label>
    <rdfs:comment>Specifies the present physical location where an artwork is housed, displayed, or stored. This property extends EDM's currentLocation with art-specific constraints ensuring single location assignment while supporting location change tracking. Essential for provenance research, exhibition planning, and artwork accessibility, this property maintains connections to institutional and geographical data through the Location class.</rdfs:comment>
    <rdfs:range rdf:resource="http://w3id.org/arto#Location"/>
    <rdfs:domain rdf:resource="http://w3id.org/arto#Artwork"/>
    <rdfs:subPropertyOf rdf:resource="http://www.europeana.eu/schemas/edm/currentLocation"/>
    <rdf:type rdf:resource="http://www.w3.org/2002/07/owl#ObjectProperty"/>
  </rdf:Description>
  <rdf:Description rdf:nodeID="A21">
    <rdf:rest rdf:resource="http://www.w3.org/1999/02/22-rdf-syntax-ns#nil"/>
    <rdf:first rdf:resource="http://w3id.org/arto#Scene"/>
  </rdf:Description>
  <rdf:Description rdf:about="http://w3id.org/arto#isMetricOf">
    <skos:example>
                - Colour metrics: :blue_intensity_75_percent arto:isMetricOf :sky_area
                - Composition balance: :symmetry_score_0.8 arto:isMetricOf :landscape_scene
                - Emotional intensity: :fear_intensity_high arto:isMetricOf :expression_scene</skos:example>
    <rdfs:label>isMetricOf</rdfs:label>
    <rdfs:comment>Associates a metric with the component of an artwork that it is related to.</rdfs:comment>
    <rdfs:range rdf:nodeID="A136"/>
    <rdfs:domain rdf:resource="http://w3id.org/arto#Metric"/>
    <rdf:type rdf:resource="http://www.w3.org/2002/07/owl#ObjectProperty"/>
  </rdf:Description>
  <rdf:Description rdf:about="http://w3id.org/arto#MaterialType">
    <skos:example>
                  - :wood_material rdf:type arto:  .
                  - :metal_material rdf:type arto:MaterialType .
                  - :glass_material rdf:type arto:MaterialType .
                      </skos:example>
    <rdfs:label>MaterialType</rdfs:label>
    <rdfs:comment>Represents the material type of an object, such as wood,
      metal, glass, or fabric. This class allows for the classification of objects based on the
      materials used in their construction or representation.</rdfs:comment>
    <rdfs:subClassOf rdf:nodeID="A29"/>
    <rdf:type rdf:resource="http://www.w3.org/2002/07/owl#Class"/>
  </rdf:Description>
  <rdf:Description rdf:nodeID="A137">
    <owl:cardinality rdf:datatype="http://www.w3.org/2001/XMLSchema#nonNegativeInteger">1</owl:cardinality>
  </rdf:Description>
  <rdf:Description rdf:nodeID="A136">
    <owl:unionOf rdf:nodeID="A138"/>
    <rdf:type rdf:resource="http://www.w3.org/2002/07/owl#Class"/>
  </rdf:Description>
  <rdf:Description rdf:about="https://schema.org/height">
    <rdf:type rdf:resource="http://www.w3.org/2002/07/owl#ObjectProperty"/>
  </rdf:Description>
  <rdf:Description rdf:about="http://w3id.org/arto#isObjectOf">
    <skos:example>
                - Landscape scene: :fountain arto:isObjectOf :garden_scene
                - Portrait scene: :chair arto:isObjectOf :interior_scene
                - Still life scene: :fruit_bowl arto:isObjectOf :table_scene</skos:example>
    <rdfs:label>isObjectOf</rdfs:label>
    <rdfs:comment>Indicates the scene that contains the object in the artwork.</rdfs:comment>
    <rdfs:range rdf:resource="http://w3id.org/arto#Scene"/>
    <rdfs:domain rdf:resource="http://w3id.org/arto#Object"/>
    <rdf:type rdf:resource="http://www.w3.org/2002/07/owl#ObjectProperty"/>
  </rdf:Description>
  <rdf:Description rdf:about="http://w3id.org/arto#hasConnotation">
    <skos:example>
              - Emotional expression: :red_colour arto:hasConnotation :anger_emotion
              - Symbolic meaning: :dove_object arto:hasConnotation :peace_meaning
              - Scene mood: :storm_scene arto:hasConnotation :turbulence_emotion
              - Artwork meaning: :guernica arto:hasConnotation :anti_war_theme</skos:example>
    <rdfs:label>hasConnotation</rdfs:label>
    <rdfs:comment>Links visual elements, objects, scenes, or artworks to their symbolic meanings or emotional connotations.The relationship enables multiple interpretation levels while maintaining clear connections between visible elements and their cultural, symbolic, or emotional significance. Similar to ICON's recognizedConcept but with broader domain coverage.</rdfs:comment>
    <rdfs:range rdf:resource="http://w3id.org/arto#Connotation"/>
    <rdfs:domain rdf:nodeID="A139"/>
    <owl:inverseOf rdf:resource="http://w3id.org/arto#isConnotationOf"/>
    <rdf:type rdf:resource="http://www.w3.org/2002/07/owl#ObjectProperty"/>
  </rdf:Description>
  <rdf:Description rdf:about="http://w3id.org/arto#ColourTerm">
    <skos:example>
                   - Basic colour terms: aat:red, aat:blue, aat:yellow, aat:green
                     # Fundamental colour categories from Getty AAT
                   - Specific pigment terms: aat:ultramarine_blue, aat:vermillion, aat:cadmium_yellow
                     # Historical and contemporary pigment names
                   - Cultural colour terms: aat:royal_purple, aat:imperial_yellow, aat:sacred_red
                     # Colours with cultural or symbolic significance
                   - Technical colour terms: aat:primary_colours, aat:complementary_colours, aat:earth_tones
                     # Colour theory and technical classifications
                   - Historical colour terms: aat:tyrian_purple, aat:lapis_lazuli_blue, aat:gold_leaf
                     # Historically significant colourants and materials
                   - Descriptive colour terms: aat:warm_colours, aat:cool_colours, aat:neutral_tones
                     # Colour temperature and mood classifications
                   </skos:example>
    <rdfs:label>ColourTerm</rdfs:label>
    <rdfs:comment>Represents standardised colour terminology from controlled vocabularies, art historical literature, and established colour naming systems. This class provides semantic interoperability by linking colour instances to authoritative colour classifications, enabling consistent colour identification across institutions and research projects. Colour terms encompass basic colour names, specific pigment designations, cultural colour concepts, and technical colour classifications. The class primarily aligns with Getty AAT's colour hierarchy while supporting additional colour vocabularies and historical colour terminology.</rdfs:comment>
    <rdfs:subClassOf rdf:nodeID="A140"/>
    <rdf:type rdf:resource="http://www.w3.org/2002/07/owl#Class"/>
  </rdf:Description>
  <rdf:Description rdf:about="http://purl.org/dc/terms/provenance">
    <rdfs:label xml:lang="en">Provenance</rdfs:label>
    <rdfs:isDefinedBy rdf:resource="http://purl.org/dc/terms/"/>
    <rdfs:comment xml:lang="en">A statement of any changes in ownership and custody of the resource since its creation that are significant for its authenticity, integrity, and interpretation.</rdfs:comment>
    <dc:description xml:lang="en">The statement may include a description of any changes successive custodians made to the resource.</dc:description>
    <j.0:rangeIncludes rdf:resource="http://purl.org/dc/terms/ProvenanceStatement"/>
    <dc:issued rdf:datatype="http://www.w3.org/2001/XMLSchema#date">2004-09-20</dc:issued>
    <rdf:type rdf:resource="http://www.w3.org/2002/07/owl#NamedIndividual"/>
  </rdf:Description>
  <rdf:Description rdf:nodeID="A12">
    <owl:hasValue rdf:resource="http://vocab.getty.edu/aat/300131647"/>
    <owl:onProperty rdf:resource="http://www.w3.org/2004/02/skos/core#broaderTransitive"/>
    <rdf:type rdf:resource="http://www.w3.org/2002/07/owl#Restriction"/>
  </rdf:Description>
  <rdf:Description rdf:about="http://w3id.org/arto#expresses">
    <skos:example>
              - :joy_emotion arto:expresses mfoem:MFOEM_000034 ; 
              - :sadness_emotion arto:expresses mfoem:MFOEM_000056 ; 
              - :anger_emotion arto:expresses mfoem:MFOEM_000009 ; 
              - :fear_emotion arto:expresses mfoem:MFOEM_000026 ; 
              </skos:example>
    <rdfs:label>expresses</rdfs:label>
    <rdfs:comment>Relates arto:Emotion to a specific emotion concept defined in the Mental Functioning Ontology Emotion Module (MFOEM). This property is used to link local emotion representations to controlled vocabulary terms (e.g., joy, sadness, anger, fear) from MFOEM, ensuring consistent and interoperable emotion classification across datasets. In the context of artworks, this enables precise and standardised description of emotions expressed within artistic content.</rdfs:comment>
    <rdfs:range rdf:resource="http://purl.obolibrary.org/obo/MFOEM_000001"/>
    <rdfs:domain rdf:resource="http://w3id.org/arto#Emotion"/>
    <rdf:type rdf:resource="http://www.w3.org/2002/07/owl#ObjectProperty"/>
  </rdf:Description>
  <rdf:Description rdf:nodeID="A141">
    <owl:allValuesFrom rdf:resource="http://www.w3.org/2001/XMLSchema#float"/>
    <owl:onProperty rdf:resource="http://w3id.org/arto#length"/>
    <rdf:type rdf:resource="http://www.w3.org/2002/07/owl#Restriction"/>
  </rdf:Description>
  <rdf:Description rdf:about="http://purl.org/dc/terms/relation">
    <rdfs:label xml:lang="en">Relation</rdfs:label>
    <rdfs:isDefinedBy rdf:resource="http://purl.org/dc/terms/"/>
    <rdfs:comment xml:lang="en">A related resource.</rdfs:comment>
    <dc:description xml:lang="en">Recommended practice is to identify the related resource by means of a URI.  If this is not possible or feasible, a string conforming to a formal identification system may be provided.</dc:description>
    <dc:issued rdf:datatype="http://www.w3.org/2001/XMLSchema#date">2008-01-14</dc:issued>
    <rdf:type rdf:resource="http://www.w3.org/2002/07/owl#NamedIndividual"/>
    <rdfs:subPropertyOf rdf:resource="http://purl.org/dc/elements/1.1/relation"/>
    <rdf:type rdf:resource="http://www.w3.org/2002/07/owl#AnnotationProperty"/>
  </rdf:Description>
  <rdf:Description rdf:nodeID="A106">
    <owl:allValuesFrom rdf:resource="http://www.w3.org/2001/XMLSchema#dateTime"/>
    <owl:onProperty rdf:resource="https://schema.org/startDate"/>
    <rdf:type rdf:resource="http://www.w3.org/2002/07/owl#Restriction"/>
  </rdf:Description>
  <rdf:Description rdf:about="http://purl.org/dc/terms/type">
    <rdfs:label xml:lang="en">Type</rdfs:label>
    <rdfs:isDefinedBy rdf:resource="http://purl.org/dc/terms/"/>
    <rdfs:comment xml:lang="en">The nature or genre of the resource.</rdfs:comment>
    <dc:description xml:lang="en">Recommended practice is to use a controlled vocabulary such as the DCMI Type Vocabulary [[DCMI-TYPE](http://dublincore.org/documents/dcmi-type-vocabulary/)]. To describe the file format, physical medium, or dimensions of the resource, use the property Format.</dc:description>
    <dc:issued rdf:datatype="http://www.w3.org/2001/XMLSchema#date">2008-01-14</dc:issued>
    <rdf:type rdf:resource="http://www.w3.org/2002/07/owl#NamedIndividual"/>
    <rdfs:subPropertyOf rdf:resource="http://purl.org/dc/elements/1.1/type"/>
    <rdf:type rdf:resource="http://www.w3.org/2002/07/owl#AnnotationProperty"/>
  </rdf:Description>
  <rdf:Description rdf:about="http://purl.org/dc/terms/creator">
    <rdfs:label xml:lang="en">Creator</rdfs:label>
    <rdfs:isDefinedBy rdf:resource="http://purl.org/dc/terms/"/>
    <rdfs:comment xml:lang="en">An entity responsible for making the resource.</rdfs:comment>
    <dc:description xml:lang="en">Recommended practice is to identify the creator with a URI.  If this is not possible or feasible, a literal value that identifies the creator may be provided.</dc:description>
    <j.0:rangeIncludes rdf:resource="http://purl.org/dc/terms/Agent"/>
    <dc:issued rdf:datatype="http://www.w3.org/2001/XMLSchema#date">2008-01-14</dc:issued>
    <rdf:type rdf:resource="http://www.w3.org/2002/07/owl#NamedIndividual"/>
    <rdfs:subPropertyOf rdf:resource="http://purl.org/dc/terms/contributor"/>
    <rdfs:subPropertyOf rdf:resource="http://purl.org/dc/elements/1.1/creator"/>
  </rdf:Description>
  <rdf:Description rdf:nodeID="A142">
    <rdf:rest rdf:nodeID="A11"/>
    <rdf:first rdf:resource="http://www.w3.org/2004/02/skos/core#Concept"/>
  </rdf:Description>
  <rdf:Description rdf:nodeID="A75">
    <rdf:rest rdf:resource="http://www.w3.org/1999/02/22-rdf-syntax-ns#nil"/>
    <rdf:first rdf:resource="http://w3id.org/arto#VisualElement"/>
  </rdf:Description>
  <rdf:Description rdf:about="http://purl.org/dc/terms/requires">
    <rdfs:label xml:lang="en">Requires</rdfs:label>
    <rdfs:isDefinedBy rdf:resource="http://purl.org/dc/terms/"/>
    <rdfs:comment xml:lang="en">A related resource that is required by the described resource to support its function, delivery, or coherence.</rdfs:comment>
    <dc:description xml:lang="en">This property is intended to be used with non-literal values. This property is an inverse property of Is Required By.</dc:description>
    <dc:issued rdf:datatype="http://www.w3.org/2001/XMLSchema#date">2000-07-11</dc:issued>
    <rdf:type rdf:resource="http://www.w3.org/2002/07/owl#NamedIndividual"/>
    <rdfs:subPropertyOf rdf:resource="http://purl.org/dc/terms/relation"/>
    <rdfs:subPropertyOf rdf:resource="http://purl.org/dc/elements/1.1/relation"/>
    <rdf:type rdf:resource="http://www.w3.org/2002/07/owl#AnnotationProperty"/>
  </rdf:Description>
  <rdf:Description rdf:nodeID="A143">
    <owl:cardinality rdf:datatype="http://www.w3.org/2001/XMLSchema#nonNegativeInteger">1</owl:cardinality>
  </rdf:Description>
  <rdf:Description rdf:nodeID="A144">
    <owl:minCardinality rdf:datatype="http://www.w3.org/2001/XMLSchema#nonNegativeInteger">1</owl:minCardinality>
  </rdf:Description>
  <rdf:Description rdf:nodeID="A145">
    <owl:hasValue rdf:resource="http://vocab.getty.edu/aat/300264091"/>
    <owl:onProperty rdf:resource="http://www.w3.org/2004/02/skos/core#broaderTransitive"/>
    <rdf:type rdf:resource="http://www.w3.org/2002/07/owl#Restriction"/>
  </rdf:Description>
  <rdf:Description rdf:about="https://schema.org/CreativeWorkSeries">
    <rdf:type rdf:resource="http://www.w3.org/2002/07/owl#Class"/>
  </rdf:Description>
  <rdf:Description rdf:about="http://purl.org/dc/terms/coverage">
    <rdfs:label xml:lang="en">Coverage</rdfs:label>
    <rdfs:isDefinedBy rdf:resource="http://purl.org/dc/terms/"/>
    <rdfs:comment xml:lang="en">The spatial or temporal topic of the resource, spatial applicability of the resource, or jurisdiction under which the resource is relevant.</rdfs:comment>
    <dc:description xml:lang="en">Spatial topic and spatial applicability may be a named place or a location specified by its geographic coordinates. Temporal topic may be a named period, date, or date range. A jurisdiction may be a named administrative entity or a geographic place to which the resource applies. Recommended practice is to use a controlled vocabulary such as the Getty Thesaurus of Geographic Names [[TGN](https://www.getty.edu/research/tools/vocabulary/tgn/index.html)]. Where appropriate, named places or time periods may be used in preference to numeric identifiers such as sets of coordinates or date ranges.  Because coverage is so broadly defined, it is preferable to use the more specific subproperties Temporal Coverage and Spatial Coverage.</dc:description>
    <j.0:rangeIncludes rdf:resource="http://purl.org/dc/terms/Period"/>
    <j.0:rangeIncludes rdf:resource="http://purl.org/dc/terms/Location"/>
    <j.0:rangeIncludes rdf:resource="http://purl.org/dc/terms/Jurisdiction"/>
    <dc:issued rdf:datatype="http://www.w3.org/2001/XMLSchema#date">2008-01-14</dc:issued>
    <rdf:type rdf:resource="http://www.w3.org/2002/07/owl#NamedIndividual"/>
    <rdfs:subPropertyOf rdf:resource="http://purl.org/dc/elements/1.1/coverage"/>
    <rdf:type rdf:resource="http://www.w3.org/2002/07/owl#AnnotationProperty"/>
  </rdf:Description>
  <rdf:Description rdf:about="http://purl.org/dc/elements/1.1/identifier">
    <rdf:type rdf:resource="http://www.w3.org/2002/07/owl#AnnotationProperty"/>
  </rdf:Description>
  <rdf:Description rdf:nodeID="A146">
    <rdf:rest rdf:resource="http://www.w3.org/1999/02/22-rdf-syntax-ns#nil"/>
    <rdf:first rdf:nodeID="A147"/>
  </rdf:Description>
  <rdf:Description rdf:nodeID="A77">
    <rdf:rest rdf:resource="http://www.w3.org/1999/02/22-rdf-syntax-ns#nil"/>
    <rdf:first rdf:resource="http://w3id.org/arto#Scene"/>
  </rdf:Description>
  <rdf:Description rdf:nodeID="A148">
    <rdf:rest rdf:resource="http://www.w3.org/1999/02/22-rdf-syntax-ns#nil"/>
    <rdf:first rdf:resource="http://w3id.org/arto#Scene"/>
  </rdf:Description>
  <rdf:Description rdf:nodeID="A149">
    <rdf:rest rdf:nodeID="A150"/>
    <rdf:first rdf:resource="http://www.w3.org/2004/02/skos/core#Concept"/>
  </rdf:Description>
  <rdf:Description rdf:nodeID="A118">
    <rdf:rest rdf:resource="http://www.w3.org/1999/02/22-rdf-syntax-ns#nil"/>
    <rdf:first rdf:resource="http://w3id.org/arto#VisualElement"/>
  </rdf:Description>
  <rdf:Description rdf:about="http://purl.org/dc/terms/ISO639-2">
    <rdfs:seeAlso rdf:resource="http://lcweb.loc.gov/standards/iso639-2/langhome.html"/>
    <rdfs:label xml:lang="en">ISO 639-2</rdfs:label>
    <rdfs:isDefinedBy rdf:resource="http://purl.org/dc/terms/"/>
    <rdfs:comment xml:lang="en">The three-letter alphabetic codes listed in ISO639-2 for the representation of names of languages.</rdfs:comment>
    <dc:issued rdf:datatype="http://www.w3.org/2001/XMLSchema#date">2000-07-11</dc:issued>
    <rdf:type rdf:resource="http://www.w3.org/2002/07/owl#NamedIndividual"/>
    <rdf:type rdf:resource="http://www.w3.org/2000/01/rdf-schema#Datatype"/>
  </rdf:Description>
  <rdf:Description rdf:about="http://purl.org/dc/terms/ISO639-3">
    <rdfs:seeAlso rdf:resource="http://www.sil.org/iso639-3/"/>
    <rdfs:label xml:lang="en">ISO 639-3</rdfs:label>
    <rdfs:isDefinedBy rdf:resource="http://purl.org/dc/terms/"/>
    <rdfs:comment xml:lang="en">The set of three-letter codes listed in ISO 639-3 for the representation of names of languages.</rdfs:comment>
    <dc:issued rdf:datatype="http://www.w3.org/2001/XMLSchema#date">2008-01-14</dc:issued>
    <rdf:type rdf:resource="http://www.w3.org/2002/07/owl#NamedIndividual"/>
    <rdf:type rdf:resource="http://www.w3.org/2000/01/rdf-schema#Datatype"/>
  </rdf:Description>
  <rdf:Description rdf:nodeID="A151">
    <owl:allValuesFrom rdf:resource="http://www.w3.org/2001/XMLSchema#string"/>
    <owl:onProperty rdf:resource="http://w3id.org/arto#descriptor"/>
    <rdf:type rdf:resource="http://www.w3.org/2002/07/owl#Restriction"/>
  </rdf:Description>
  <rdf:Description rdf:about="http://w3id.org/arto#TechniqueType">
    <rdfs:label>TechniqueType</rdfs:label>
    <rdfs:comment>Represents the specific artistic techniques used in creating artwork, drawing from Getty AAT's technique hierarchy while supporting custom undefined techniques.</rdfs:comment>
    <rdfs:subClassOf rdf:nodeID="A152"/>
    <rdf:type rdf:resource="http://www.w3.org/2002/07/owl#Class"/>
  </rdf:Description>
  <rdf:Description rdf:nodeID="A153">
    <owl:allValuesFrom rdf:resource="http://w3id.org/arto#Event"/>
    <owl:onProperty rdf:resource="http://w3id.org/arto#relatedToEvent"/>
    <rdf:type rdf:resource="http://www.w3.org/2002/07/owl#Restriction"/>
  </rdf:Description>
  <rdf:Description rdf:nodeID="A154">
    <owl:cardinality rdf:datatype="http://www.w3.org/2001/XMLSchema#nonNegativeInteger">1</owl:cardinality>
  </rdf:Description>
  <rdf:Description rdf:nodeID="A155">
    <owl:minCardinality rdf:datatype="http://www.w3.org/2001/XMLSchema#nonNegativeInteger">0</owl:minCardinality>
  </rdf:Description>
  <rdf:Description rdf:about="http://purl.org/dc/terms/references">
    <rdfs:label xml:lang="en">References</rdfs:label>
    <rdfs:isDefinedBy rdf:resource="http://purl.org/dc/terms/"/>
    <rdfs:comment xml:lang="en">A related resource that is referenced, cited, or otherwise pointed to by the described resource.</rdfs:comment>
    <dc:description xml:lang="en">This property is intended to be used with non-literal values. This property is an inverse property of Is Referenced By.</dc:description>
    <dc:issued rdf:datatype="http://www.w3.org/2001/XMLSchema#date">2000-07-11</dc:issued>
    <rdf:type rdf:resource="http://www.w3.org/2002/07/owl#NamedIndividual"/>
    <rdfs:subPropertyOf rdf:resource="http://purl.org/dc/terms/relation"/>
    <rdfs:subPropertyOf rdf:resource="http://purl.org/dc/elements/1.1/relation"/>
    <rdf:type rdf:resource="http://www.w3.org/2002/07/owl#AnnotationProperty"/>
  </rdf:Description>
  <rdf:Description rdf:about="http://purl.org/dc/terms/title">
    <rdfs:label xml:lang="en">Title</rdfs:label>
    <rdfs:isDefinedBy rdf:resource="http://purl.org/dc/terms/"/>
    <rdfs:comment xml:lang="en">A name given to the resource.</rdfs:comment>
    <dc:issued rdf:datatype="http://www.w3.org/2001/XMLSchema#date">2008-01-14</dc:issued>
    <rdf:type rdf:resource="http://www.w3.org/2002/07/owl#NamedIndividual"/>
    <rdf:type rdf:resource="http://www.w3.org/2002/07/owl#DatatypeProperty"/>
    <rdfs:range rdf:resource="http://www.w3.org/2000/01/rdf-schema#Literal"/>
    <rdfs:subPropertyOf rdf:resource="http://purl.org/dc/elements/1.1/title"/>
    <rdf:type rdf:resource="http://www.w3.org/2002/07/owl#AnnotationProperty"/>
  </rdf:Description>
  <rdf:Description rdf:about="http://purl.org/dc/terms/Location">
    <rdfs:label xml:lang="en">Location</rdfs:label>
    <rdfs:isDefinedBy rdf:resource="http://purl.org/dc/terms/"/>
    <rdfs:comment xml:lang="en">A spatial region or named place.</rdfs:comment>
    <dc:issued rdf:datatype="http://www.w3.org/2001/XMLSchema#date">2008-01-14</dc:issued>
    <rdf:type rdf:resource="http://www.w3.org/2002/07/owl#NamedIndividual"/>
    <rdfs:subClassOf rdf:resource="http://purl.org/dc/terms/LocationPeriodOrJurisdiction"/>
    <rdf:type rdf:resource="http://www.w3.org/2002/07/owl#Class"/>
  </rdf:Description>
  <rdf:Description rdf:nodeID="A107">
    <owl:allValuesFrom rdf:resource="http://www.w3.org/2001/XMLSchema#string"/>
    <owl:onProperty rdf:resource="http://purl.org/dc/terms/type"/>
    <rdf:type rdf:resource="http://www.w3.org/2002/07/owl#Restriction"/>
  </rdf:Description>
  <rdf:Description rdf:about="http://purl.org/dc/terms/PeriodOfTime">
    <rdfs:label xml:lang="en">Period of Time</rdfs:label>
    <rdfs:isDefinedBy rdf:resource="http://purl.org/dc/terms/"/>
    <rdfs:comment xml:lang="en">An interval of time that is named or defined by its start and end dates.</rdfs:comment>
    <dc:issued rdf:datatype="http://www.w3.org/2001/XMLSchema#date">2008-01-14</dc:issued>
    <rdf:type rdf:resource="http://www.w3.org/2002/07/owl#NamedIndividual"/>
    <rdfs:subClassOf rdf:resource="http://purl.org/dc/terms/LocationPeriodOrJurisdiction"/>
    <rdf:type rdf:resource="http://www.w3.org/2002/07/owl#Class"/>
  </rdf:Description>
  <rdf:Description rdf:about="http://w3id.org/arto#technique">
    <rdfs:label>technique</rdfs:label>
    <skos:example>
                :sistine_ceiling a arto:Artwork ;
                  arto:technique aat:fresco .

                :rembrandt_print a arto:Artwork ;
                  arto:technique aat:etching .

                :seurat_painting a arto:Artwork ;
                  arto:technique aat:pointillism .

                :bronze_sculpture a arto:Artwork ;
                  arto:technique aat:lost_wax_casting .
                </skos:example>
    <rdfs:comment>Specifies the artistic methods or processes applied in the creation of the artwork (e.g., fresco, engraving, pointillism). This property connects to Getty AAT’s technique hierarchy, while also supporting the definition of custom techniques not covered by AAT.</rdfs:comment>
    <rdfs:range rdf:resource="http://w3id.org/arto#TechniqueType"/>
    <rdfs:domain rdf:resource="http://w3id.org/arto#Artwork"/>
    <rdf:type rdf:resource="http://www.w3.org/2002/07/owl#ObjectProperty"/>
  </rdf:Description>
  <rdf:Description rdf:about="http://w3id.org/arto#medium">
    <rdfs:label>medium</rdfs:label>
    <skos:example>
              :painting_001 a arto:Artwork ;
                arto:medium aat:oil_on_canvas .

              :wall_painting_001 a arto:Artwork ;
                arto:medium aat:fresco .

              :bronze_statue_001 a arto:Artwork ;
                arto:medium aat:bronze .
              </skos:example>
    <rdfs:comment>Specifies the physical medium of the artwork itself (e.g., oil on canvas, tempera on panel, bronze sculpture). This property aligns with Getty AAT's medium hierarchy, ensuring standardised description of artistic medium.</rdfs:comment>
    <rdfs:range rdf:resource="http://w3id.org/arto#MediumType"/>
    <rdfs:domain rdf:resource="http://w3id.org/arto#Artwork"/>
    <rdf:type rdf:resource="http://www.w3.org/2002/07/owl#ObjectProperty"/>
  </rdf:Description>
  <rdf:Description rdf:about="http://purl.org/dc/terms/isVersionOf">
    <rdfs:label xml:lang="en">Is Version Of</rdfs:label>
    <rdfs:isDefinedBy rdf:resource="http://purl.org/dc/terms/"/>
    <rdfs:comment xml:lang="en">A related resource of which the described resource is a version, edition, or adaptation.</rdfs:comment>
    <dc:description xml:lang="en">Changes in version imply substantive changes in content rather than differences in format. This property is intended to be used with non-literal values. This property is an inverse property of Has Version.</dc:description>
    <dc:issued rdf:datatype="http://www.w3.org/2001/XMLSchema#date">2000-07-11</dc:issued>
    <rdf:type rdf:resource="http://www.w3.org/2002/07/owl#NamedIndividual"/>
    <rdfs:subPropertyOf rdf:resource="http://purl.org/dc/terms/relation"/>
    <rdfs:subPropertyOf rdf:resource="http://purl.org/dc/elements/1.1/relation"/>
    <rdf:type rdf:resource="http://www.w3.org/2002/07/owl#AnnotationProperty"/>
  </rdf:Description>
  <rdf:Description rdf:nodeID="A130">
    <rdf:rest rdf:resource="http://www.w3.org/1999/02/22-rdf-syntax-ns#nil"/>
    <rdf:first rdf:nodeID="A98"/>
  </rdf:Description>
  <rdf:Description rdf:about="http://purl.org/dc/terms/accessRights">
    <rdfs:label xml:lang="en">Access Rights</rdfs:label>
    <rdfs:isDefinedBy rdf:resource="http://purl.org/dc/terms/"/>
    <rdfs:comment xml:lang="en">Information about who access the resource or an indication of its security status.</rdfs:comment>
    <dc:description xml:lang="en">Access Rights may include information regarding access or restrictions based on privacy, security, or other policies.</dc:description>
    <j.0:rangeIncludes rdf:resource="http://purl.org/dc/terms/RightsStatement"/>
    <dc:issued rdf:datatype="http://www.w3.org/2001/XMLSchema#date">2003-02-15</dc:issued>
    <rdf:type rdf:resource="http://www.w3.org/2002/07/owl#NamedIndividual"/>
    <rdfs:subPropertyOf rdf:resource="http://purl.org/dc/terms/rights"/>
    <rdfs:subPropertyOf rdf:resource="http://purl.org/dc/elements/1.1/rights"/>
    <rdf:type rdf:resource="http://www.w3.org/2002/07/owl#AnnotationProperty"/>
  </rdf:Description>
  <rdf:Description rdf:about="http://purl.org/dc/terms/accrualMethod">
    <rdfs:label xml:lang="en">Accrual Method</rdfs:label>
    <rdfs:isDefinedBy rdf:resource="http://purl.org/dc/terms/"/>
    <rdfs:comment xml:lang="en">The method by which items are added to a collection.</rdfs:comment>
    <dc:description xml:lang="en">Recommended practice is to use a value from the Collection Description Accrual Method Vocabulary [[DCMI-ACCRUALMETHOD](https://dublincore.org/groups/collections/accrual-method/)].</dc:description>
    <j.0:rangeIncludes rdf:resource="http://purl.org/dc/terms/MethodOfAccrual"/>
    <dc:issued rdf:datatype="http://www.w3.org/2001/XMLSchema#date">2005-06-13</dc:issued>
    <rdf:type rdf:resource="http://www.w3.org/2002/07/owl#NamedIndividual"/>
    <rdfs:domain rdf:resource="http://purl.org/dc/dcmitype/Collection"/>
    <rdf:type rdf:resource="http://www.w3.org/2002/07/owl#AnnotationProperty"/>
  </rdf:Description>
  <rdf:Description rdf:about="http://w3id.org/arto">
    <owl:versionInfo>0.2</owl:versionInfo>
    <rdfs:label xml:lang="en">Artwork Object Ontology (ARTO)</rdfs:label>
    <vann:preferredNamespacePrefix>arto</vann:preferredNamespacePrefix>
    <dc:title xml:lang="en">Artwork Object Ontology</dc:title>
    <dc:modified>2025-08-05</dc:modified>
    <dc:license rdf:resource="https://github.com/SocialMachineLab/ArtworkOntology/blob/main/License"/>
    <dc:issued>2024-04-10</dc:issued>
    <dc:description xml:lang="en">The Artwork Object Ontology (ARTO) is a comprehensive ontology designed for describing and contextualising artworks. It consists of two main components: the Artwork Descriptive Model and the Artwork Contextual Model. ARTO aims to provide a structured and detailed representation of artworks, facilitating tasks such as artwork captioning and information retrieval.</dc:description>
    <cc:attributionURL rdf:resource="http://w3id.org/arto"/>
    <owl:imports rdf:resource="https://schema.org/"/>
    <owl:imports rdf:resource="http://xmlns.com/foaf/spec/"/>
    <owl:imports rdf:resource="http://www.w3.org/2004/02/skos/core"/>
    <owl:imports rdf:resource="http://www.cidoc-crm.org/cidoc-crm/"/>
    <rdf:type rdf:resource="http://www.w3.org/2002/07/owl#Ontology"/>
  </rdf:Description>
  <rdf:Description rdf:nodeID="A156">
    <owl:maxCardinality rdf:datatype="http://www.w3.org/2001/XMLSchema#nonNegativeInteger">1</owl:maxCardinality>
  </rdf:Description>
  <rdf:Description rdf:about="http://w3id.org/arto#Theme">
    <rdfs:label>Theme</rdfs:label>
    <rdfs:comment>Represents a central idea, subject, or concept explored in an artwork, which can be explicit or implicit, and may reflect broader cultural, social, or political issues.</rdfs:comment>
    <rdfs:subClassOf rdf:resource="http://w3id.org/arto#Connotation"/>
    <rdf:type rdf:resource="http://www.w3.org/2002/07/owl#Class"/>
  </rdf:Description>
  <rdf:Description rdf:nodeID="A102">
    <rdf:rest rdf:resource="http://www.w3.org/1999/02/22-rdf-syntax-ns#nil"/>
    <rdf:first>viewer</rdf:first>
    <rdf:type rdf:resource="http://www.w3.org/1999/02/22-rdf-syntax-ns#List"/>
  </rdf:Description>
  <rdf:Description rdf:about="http://w3id.org/arto#Character">
    <rdfs:label>Character</rdfs:label>
    <rdfs:comment>Represents persons, figures, or beings depicted within an artwork.</rdfs:comment>
    <rdfs:subClassOf rdf:resource="http://w3id.org/arto#Person"/>
    <rdf:type rdf:resource="http://www.w3.org/2002/07/owl#Class"/>
  </rdf:Description>
  <rdf:Description rdf:nodeID="A71">
    <rdf:rest rdf:nodeID="A157"/>
    <rdf:first rdf:resource="http://w3id.org/arto#Artwork"/>
  </rdf:Description>
  <rdf:Description rdf:nodeID="A56">
    <owl:allValuesFrom rdf:resource="http://www.w3.org/2001/XMLSchema#string"/>
    <owl:onProperty rdf:resource="http://purl.org/dc/terms/type"/>
    <rdf:type rdf:resource="http://www.w3.org/2002/07/owl#Restriction"/>
  </rdf:Description>
  <rdf:Description rdf:about="http://purl.org/dc/terms/modified">
    <rdfs:label xml:lang="en">Date Modified</rdfs:label>
    <rdfs:isDefinedBy rdf:resource="http://purl.org/dc/terms/"/>
    <rdfs:comment xml:lang="en">Date on which the resource was changed.</rdfs:comment>
    <dc:description xml:lang="en">Recommended practice is to describe the date, date/time, or period of time as recommended for the property Date, of which this is a subproperty.</dc:description>
    <dc:issued rdf:datatype="http://www.w3.org/2001/XMLSchema#date">2000-07-11</dc:issued>
    <rdf:type rdf:resource="http://www.w3.org/2002/07/owl#NamedIndividual"/>
    <rdfs:subPropertyOf rdf:resource="http://purl.org/dc/terms/date"/>
    <rdf:type rdf:resource="http://www.w3.org/2002/07/owl#DatatypeProperty"/>
    <rdfs:range rdf:resource="http://www.w3.org/2000/01/rdf-schema#Literal"/>
    <rdfs:subPropertyOf rdf:resource="http://purl.org/dc/elements/1.1/date"/>
    <rdf:type rdf:resource="http://www.w3.org/2002/07/owl#AnnotationProperty"/>
  </rdf:Description>
  <rdf:Description rdf:nodeID="A58">
    <rdf:rest rdf:nodeID="A158"/>
    <rdf:first>XYZ</rdf:first>
  </rdf:Description>
  <rdf:Description rdf:nodeID="A159">
    <owl:minCardinality rdf:datatype="http://www.w3.org/2001/XMLSchema#nonNegativeInteger">1</owl:minCardinality>
  </rdf:Description>
  <rdf:Description rdf:nodeID="A160">
    <owl:allValuesFrom rdf:resource="http://w3id.org/arto#Connotation"/>
    <owl:onProperty rdf:resource="http://w3id.org/arto#hasConnotation"/>
    <rdf:type rdf:resource="http://www.w3.org/2002/07/owl#Restriction"/>
  </rdf:Description>
  <rdf:Description rdf:about="http://purl.org/dc/terms/MethodOfAccrual">
    <rdfs:label xml:lang="en">Method of Accrual</rdfs:label>
    <rdfs:isDefinedBy rdf:resource="http://purl.org/dc/terms/"/>
    <rdfs:comment xml:lang="en">A method by which resources are added to a collection.</rdfs:comment>
    <dc:issued rdf:datatype="http://www.w3.org/2001/XMLSchema#date">2008-01-14</dc:issued>
    <rdf:type rdf:resource="http://www.w3.org/2002/07/owl#NamedIndividual"/>
    <rdf:type rdf:resource="http://www.w3.org/2002/07/owl#Class"/>
  </rdf:Description>
  <rdf:Description rdf:nodeID="A161">
    <owl:allValuesFrom rdf:resource="http://www.w3.org/2001/XMLSchema#string"/>
    <owl:onProperty rdf:resource="http://purl.org/dc/terms/description"/>
    <rdf:type rdf:resource="http://www.w3.org/2002/07/owl#Restriction"/>
  </rdf:Description>
  <rdf:Description rdf:nodeID="A158">
    <rdf:rest rdf:resource="http://www.w3.org/1999/02/22-rdf-syntax-ns#nil"/>
    <rdf:first>Greyscale</rdf:first>
  </rdf:Description>
  <rdf:Description rdf:about="http://purl.org/dc/elements/1.1/coverage">
    <rdf:type rdf:resource="http://www.w3.org/2002/07/owl#AnnotationProperty"/>
  </rdf:Description>
  <rdf:Description rdf:nodeID="A162">
    <owl:allValuesFrom rdf:resource="http://w3id.org/arto#Metric"/>
    <owl:onProperty rdf:resource="http://w3id.org/arto#hasMetric"/>
    <rdf:type rdf:resource="http://www.w3.org/2002/07/owl#Restriction"/>
  </rdf:Description>
  <rdf:Description rdf:about="http://purl.org/dc/terms/Agent">
    <rdfs:label xml:lang="en">Agent</rdfs:label>
    <rdfs:isDefinedBy rdf:resource="http://purl.org/dc/terms/"/>
    <rdfs:comment xml:lang="en">A resource that acts or has the power to act.</rdfs:comment>
    <dc:issued rdf:datatype="http://www.w3.org/2001/XMLSchema#date">2008-01-14</dc:issued>
    <rdf:type rdf:resource="http://purl.org/dc/terms/AgentClass"/>
    <rdf:type rdf:resource="http://www.w3.org/2002/07/owl#NamedIndividual"/>
    <rdf:type rdf:resource="http://www.w3.org/2002/07/owl#Class"/>
  </rdf:Description>
  <rdf:Description rdf:about="http://xmlns.com/foaf/spec/Agent">
    <rdf:type rdf:resource="http://www.w3.org/2002/07/owl#Class"/>
  </rdf:Description>
  <rdf:Description rdf:about="http://www.w3.org/2002/07/owl#minCardinality">
    <rdf:type rdf:resource="http://www.w3.org/2002/07/owl#AnnotationProperty"/>
  </rdf:Description>
  <rdf:Description rdf:about="http://w3id.org/arto#isEventOf">
    <skos:example>
                - Historical event: :french_revolution_1830 arto:isEventOf :liberty_leading_the_people
                - Biblical event: :biblical_last_supper arto:isEventOf :last_supper
                </skos:example>
    <rdfs:label>isEventOf</rdfs:label>
    <rdfs:comment>Associates an event with the artwork or scene that it is related to.</rdfs:comment>
    <rdfs:range rdf:nodeID="A70"/>
    <rdfs:domain rdf:resource="http://w3id.org/arto#Event"/>
    <owl:inverseOf rdf:resource="http://w3id.org/arto#relatedToEvent"/>
    <rdf:type rdf:resource="http://www.w3.org/2002/07/owl#ObjectProperty"/>
  </rdf:Description>
  <rdf:Description rdf:nodeID="A163">
    <owl:allValuesFrom rdf:resource="http://w3id.org/arto#Scene"/>
    <owl:onProperty rdf:resource="http://w3id.org/arto#relatedToScene"/>
    <rdf:type rdf:resource="http://www.w3.org/2002/07/owl#Restriction"/>
  </rdf:Description>
  <rdf:Description rdf:nodeID="A8">
    <owl:unionOf rdf:nodeID="A4"/>
    <rdf:type rdf:resource="http://www.w3.org/2002/07/owl#Class"/>
  </rdf:Description>
  <rdf:Description rdf:about="http://purl.org/dc/elements/1.1/source">
    <rdf:type rdf:resource="http://www.w3.org/2002/07/owl#AnnotationProperty"/>
  </rdf:Description>
  <rdf:Description rdf:about="http://purl.org/dc/elements/1.1/relation">
    <rdf:type rdf:resource="http://www.w3.org/2002/07/owl#AnnotationProperty"/>
  </rdf:Description>
  <rdf:Description rdf:nodeID="A27">
    <owl:someValuesFrom rdf:resource="http://w3id.org/arto#Time"/>
    <owl:onProperty rdf:resource="http://w3id.org/arto#hasTime"/>
    <rdf:type rdf:resource="http://www.w3.org/2002/07/owl#Restriction"/>
  </rdf:Description>
  <rdf:Description rdf:about="http://purl.org/dc/terms/URI">
    <rdfs:seeAlso rdf:resource="http://www.ietf.org/rfc/rfc3986.txt"/>
    <rdfs:label xml:lang="en">URI</rdfs:label>
    <rdfs:isDefinedBy rdf:resource="http://purl.org/dc/terms/"/>
    <rdfs:comment xml:lang="en">The set of identifiers constructed according to the generic syntax for Uniform Resource Identifiers as specified by the Internet Engineering Task Force.</rdfs:comment>
    <dc:issued rdf:datatype="http://www.w3.org/2001/XMLSchema#date">2000-07-11</dc:issued>
    <rdf:type rdf:resource="http://www.w3.org/2002/07/owl#NamedIndividual"/>
    <rdf:type rdf:resource="http://www.w3.org/2000/01/rdf-schema#Datatype"/>
  </rdf:Description>
  <rdf:Description rdf:nodeID="A150">
    <rdf:rest rdf:resource="http://www.w3.org/1999/02/22-rdf-syntax-ns#nil"/>
    <rdf:first rdf:nodeID="A10"/>
  </rdf:Description>
  <rdf:Description rdf:about="https://schema.org/width">
    <rdf:type rdf:resource="http://www.w3.org/2002/07/owl#ObjectProperty"/>
  </rdf:Description>
  <rdf:Description rdf:nodeID="A94">
    <owl:allValuesFrom rdf:resource="http://w3id.org/arto#Agent"/>
    <owl:onProperty rdf:resource="http://purl.org/dc/terms/creator"/>
    <rdf:type rdf:resource="http://www.w3.org/2002/07/owl#Restriction"/>
  </rdf:Description>
  <rdf:Description rdf:nodeID="A164">
    <owl:unionOf rdf:nodeID="A36"/>
    <rdf:type rdf:resource="http://www.w3.org/2002/07/owl#Class"/>
  </rdf:Description>
  <rdf:Description rdf:nodeID="A165">
    <owl:cardinality rdf:datatype="http://www.w3.org/2001/XMLSchema#nonNegativeInteger">1</owl:cardinality>
  </rdf:Description>
  <rdf:Description rdf:nodeID="A166">
    <owl:cardinality rdf:datatype="http://www.w3.org/2001/XMLSchema#nonNegativeInteger">1</owl:cardinality>
  </rdf:Description>
  <rdf:Description rdf:nodeID="A115">
    <rdf:rest rdf:nodeID="A167"/>
    <rdf:first rdf:resource="http://w3id.org/arto#Artwork"/>
  </rdf:Description>
  <rdf:Description rdf:about="https://w3id.org/MON/event.owl#Event">
    <rdf:type rdf:resource="http://www.w3.org/2002/07/owl#Class"/>
  </rdf:Description>
  <rdf:Description rdf:nodeID="A168">
    <rdf:rest rdf:nodeID="A124"/>
    <rdf:first rdf:resource="http://w3id.org/arto#Artwork"/>
  </rdf:Description>
  <rdf:Description rdf:about="http://purl.org/dc/terms/alternative">
    <rdfs:label xml:lang="en">Alternative Title</rdfs:label>
    <rdfs:isDefinedBy rdf:resource="http://purl.org/dc/terms/"/>
    <rdfs:comment xml:lang="en">An alternative name for the resource.</rdfs:comment>
    <dc:description xml:lang="en">The distinction between titles and alternative titles is application-specific.</dc:description>
    <dc:issued rdf:datatype="http://www.w3.org/2001/XMLSchema#date">2000-07-11</dc:issued>
    <rdf:type rdf:resource="http://www.w3.org/2002/07/owl#NamedIndividual"/>
    <rdfs:range rdf:resource="http://www.w3.org/2000/01/rdf-schema#Literal"/>
    <rdfs:subPropertyOf rdf:resource="http://purl.org/dc/terms/title"/>
    <rdf:type rdf:resource="http://www.w3.org/2002/07/owl#DatatypeProperty"/>
    <rdfs:subPropertyOf rdf:resource="http://purl.org/dc/elements/1.1/title"/>
    <rdf:type rdf:resource="http://www.w3.org/2002/07/owl#AnnotationProperty"/>
  </rdf:Description>
  <rdf:Description rdf:about="http://w3id.org/arto#relatedToConnotation">
    <skos:example>
                  ex:NoahDoveEvent rdf:type arto:Event ;
                  arto:relatedToConnotation ex:PeaceSymbolism ;
                </skos:example>
    <rdfs:label>relatedToConnotation</rdfs:label>
    <rdfs:comment>Indicates that an event related to some connotations.</rdfs:comment>
    <rdfs:range rdf:resource="http://w3id.org/arto#Connotation"/>
    <rdfs:domain rdf:resource="http://w3id.org/arto#Event"/>
    <rdf:type rdf:resource="http://www.w3.org/2002/07/owl#ObjectProperty"/>
  </rdf:Description>
  <rdf:Description rdf:about="https://w3id.org/MON/event.owl#agent">
    <rdf:type rdf:resource="http://www.w3.org/2002/07/owl#ObjectProperty"/>
  </rdf:Description>
  <rdf:Description rdf:nodeID="A169">
    <rdf:rest rdf:nodeID="A170"/>
    <rdf:first>Artwork</rdf:first>
    <rdf:type rdf:resource="http://www.w3.org/1999/02/22-rdf-syntax-ns#List"/>
  </rdf:Description>
  <rdf:Description rdf:about="http://w3id.org/arto#isElementOf">
    <skos:example>
                  - colour elements: :blue_gradient_colour arto:isElementOf :sky_object
                  - Line elements: :diagonal_line arto:isElementOf :mountain_object
                  - Compositional elements: :vertical_composition arto:isElementOf :tree_object</skos:example>
    <rdfs:label>isElementOf</rdfs:label>
    <rdfs:comment>Specifies the object or scene that contains the visual element in the artwork.</rdfs:comment>
    <rdfs:range rdf:nodeID="A171"/>
    <rdfs:domain rdf:resource="http://w3id.org/arto#VisualElement"/>
    <owl:inverseOf rdf:resource="http://w3id.org/arto#containsElement"/>
    <rdf:type rdf:resource="http://www.w3.org/2002/07/owl#ObjectProperty"/>
  </rdf:Description>
  <rdf:Description rdf:nodeID="A19">
    <owl:unionOf rdf:nodeID="A172"/>
    <rdf:type rdf:resource="http://www.w3.org/2002/07/owl#Class"/>
  </rdf:Description>
  <rdf:Description rdf:about="http://www.w3.org/2002/07/owl#maxCardinality">
    <rdf:type rdf:resource="http://www.w3.org/2002/07/owl#AnnotationProperty"/>
  </rdf:Description>
  <rdf:Description rdf:nodeID="A32">
    <owl:unionOf rdf:nodeID="A168"/>
    <rdf:type rdf:resource="http://www.w3.org/2002/07/owl#Class"/>
  </rdf:Description>
  <rdf:Description rdf:nodeID="A173">
    <owl:minCardinality rdf:datatype="http://www.w3.org/2001/XMLSchema#nonNegativeInteger">1</owl:minCardinality>
  </rdf:Description>
  <rdf:Description rdf:nodeID="A81">
    <rdf:rest rdf:nodeID="A90"/>
    <rdf:first>Greyscale</rdf:first>
    <rdf:type rdf:resource="http://www.w3.org/1999/02/22-rdf-syntax-ns#List"/>
  </rdf:Description>
  <rdf:Description rdf:about="http://w3id.org/arto#colourSpace">
    <rdfs:label>colourSpace</rdfs:label>
    <rdfs:comment>Colour space used by a ColourValue. Restricted to one of: RGB, HSV, Lab, CMYK, XYZ, Greyscale.</rdfs:comment>
    <rdfs:range rdf:nodeID="A34"/>
    <rdfs:domain rdf:resource="http://w3id.org/arto#ColourValue"/>
    <rdf:type rdf:resource="http://www.w3.org/2002/07/owl#DatatypeProperty"/>
  </rdf:Description>
  <rdf:Description rdf:about="http://purl.org/dc/elements/1.1/language">
    <rdf:type rdf:resource="http://www.w3.org/2002/07/owl#AnnotationProperty"/>
  </rdf:Description>
  <rdf:Description rdf:nodeID="A140">
    <owl:unionOf rdf:nodeID="A142"/>
    <rdf:type rdf:resource="http://www.w3.org/2002/07/owl#Class"/>
  </rdf:Description>
  <rdf:Description rdf:nodeID="A174">
    <owl:allValuesFrom rdf:resource="http://www.w3.org/2001/XMLSchema#string"/>
    <owl:onProperty rdf:resource="http://w3id.org/arto#size"/>
    <rdf:type rdf:resource="http://www.w3.org/2002/07/owl#Restriction"/>
  </rdf:Description>
  <rdf:Description rdf:nodeID="A175">
    <owl:cardinality rdf:datatype="http://www.w3.org/2001/XMLSchema#nonNegativeInteger">1</owl:cardinality>
  </rdf:Description>
  <rdf:Description rdf:nodeID="A176">
    <owl:oneOf rdf:nodeID="A177"/>
    <rdf:type rdf:resource="http://www.w3.org/2000/01/rdf-schema#Datatype"/>
  </rdf:Description>
  <rdf:Description rdf:about="http://w3id.org/arto#hasTime">
    <skos:example>
               # Specific date
               :exhibition2024 arto:hasTime :date_2024_05_12

               # Period/season
               :venice_biennale2022 arto:hasTime :summer2022

               # Historical era
               :napoleon_coronation arto:hasTime :early19thCentury
              </skos:example>
    <rdfs:label>hasTime</rdfs:label>
    <rdfs:comment>Links an event to its temporal specification. The time entity may represent a specific date, a period (e.g., season, decade), or a cultural-historical era, allowing precise or approximate temporal anchoring of events.</rdfs:comment>
    <rdfs:range rdf:resource="http://w3id.org/arto#Time"/>
    <rdfs:domain rdf:resource="http://w3id.org/arto#Event"/>
    <owl:inverseOf rdf:resource="http://w3id.org/arto#isTimeOf"/>
    <rdf:type rdf:resource="http://www.w3.org/2002/07/owl#ObjectProperty"/>
  </rdf:Description>
  <rdf:Description rdf:nodeID="A178">
    <owl:onDataRange rdf:resource="http://www.w3.org/2001/XMLSchema#anyURI"/>
    <owl:maxQualifiedCardinality rdf:datatype="http://www.w3.org/2001/XMLSchema#nonNegativeInteger">1</owl:maxQualifiedCardinality>
    <owl:onProperty rdf:resource="http://www.europeana.eu/schemas/edm/isShownBy"/>
    <rdf:type rdf:resource="http://www.w3.org/2002/07/owl#Restriction"/>
  </rdf:Description>
  <rdf:Description rdf:nodeID="A179">
    <owl:allValuesFrom rdf:resource="http://w3id.org/arto#Series"/>
    <owl:onProperty rdf:resource="http://purl.org/dc/terms/isPartOf"/>
    <rdf:type rdf:resource="http://www.w3.org/2002/07/owl#Restriction"/>
  </rdf:Description>
  <rdf:Description rdf:about="http://purl.org/dc/terms/bibliographicCitation">
    <rdfs:label xml:lang="en">Bibliographic Citation</rdfs:label>
    <rdfs:isDefinedBy rdf:resource="http://purl.org/dc/terms/"/>
    <rdfs:comment xml:lang="en">A bibliographic reference for the resource.</rdfs:comment>
    <dc:description xml:lang="en">Recommended practice is to include sufficient bibliographic detail to identify the resource as unambiguously as possible.</dc:description>
    <dc:issued rdf:datatype="http://www.w3.org/2001/XMLSchema#date">2003-02-15</dc:issued>
    <rdf:type rdf:resource="http://www.w3.org/2002/07/owl#NamedIndividual"/>
    <rdfs:subPropertyOf rdf:resource="http://purl.org/dc/terms/identifier"/>
    <rdf:type rdf:resource="http://www.w3.org/2002/07/owl#DatatypeProperty"/>
    <rdfs:range rdf:resource="http://www.w3.org/2000/01/rdf-schema#Literal"/>
    <rdfs:subPropertyOf rdf:resource="http://purl.org/dc/elements/1.1/identifier"/>
    <rdf:type rdf:resource="http://www.w3.org/2002/07/owl#AnnotationProperty"/>
  </rdf:Description>
  <rdf:Description rdf:about="http://purl.org/dc/terms/dateSubmitted">
    <rdfs:label xml:lang="en">Date Submitted</rdfs:label>
    <rdfs:isDefinedBy rdf:resource="http://purl.org/dc/terms/"/>
    <rdfs:comment xml:lang="en">Date of submission of the resource.</rdfs:comment>
    <dc:description xml:lang="en">Recommended practice is to describe the date, date/time, or period of time as recommended for the property Date, of which this is a subproperty.  Examples of resources to which a 'Date Submitted' may be relevant include a thesis (submitted to a university department) or an article (submitted to a journal).</dc:description>
    <dc:issued rdf:datatype="http://www.w3.org/2001/XMLSchema#date">2002-07-13</dc:issued>
    <rdf:type rdf:resource="http://www.w3.org/2002/07/owl#NamedIndividual"/>
    <rdfs:subPropertyOf rdf:resource="http://purl.org/dc/terms/date"/>
    <rdf:type rdf:resource="http://www.w3.org/2002/07/owl#DatatypeProperty"/>
    <rdfs:range rdf:resource="http://www.w3.org/2000/01/rdf-schema#Literal"/>
    <rdfs:subPropertyOf rdf:resource="http://purl.org/dc/elements/1.1/date"/>
    <rdf:type rdf:resource="http://www.w3.org/2002/07/owl#AnnotationProperty"/>
  </rdf:Description>
  <rdf:Description rdf:nodeID="A180">
    <owl:minCardinality rdf:datatype="http://www.w3.org/2001/XMLSchema#nonNegativeInteger">0</owl:minCardinality>
  </rdf:Description>
  <rdf:Description rdf:nodeID="A171">
    <owl:unionOf rdf:nodeID="A76"/>
    <rdf:type rdf:resource="http://www.w3.org/2002/07/owl#Class"/>
  </rdf:Description>
  <rdf:Description rdf:about="http://purl.org/dc/elements/1.1/contributor">
    <rdf:type rdf:resource="http://www.w3.org/2002/07/owl#AnnotationProperty"/>
  </rdf:Description>
  <rdf:Description rdf:about="http://purl.org/dc/terms/ISO3166">
    <rdfs:seeAlso rdf:resource="https://www.iso.org/obp/ui/#search"/>
    <rdfs:label xml:lang="en">ISO 3166</rdfs:label>
    <rdfs:isDefinedBy rdf:resource="http://purl.org/dc/terms/"/>
    <rdfs:comment xml:lang="en">The set of codes listed in ISO 3166-1 for the representation of names of countries.</rdfs:comment>
    <dc:issued rdf:datatype="http://www.w3.org/2001/XMLSchema#date">2000-07-11</dc:issued>
    <rdf:type rdf:resource="http://www.w3.org/2002/07/owl#NamedIndividual"/>
    <rdf:type rdf:resource="http://www.w3.org/2000/01/rdf-schema#Datatype"/>
  </rdf:Description>
  <rdf:Description rdf:about="http://purl.org/dc/terms/identifier">
    <rdfs:label xml:lang="en">Identifier</rdfs:label>
    <rdfs:isDefinedBy rdf:resource="http://purl.org/dc/terms/"/>
    <rdfs:comment xml:lang="en">An unambiguous reference to the resource within a given context.</rdfs:comment>
    <dc:description xml:lang="en">Recommended practice is to identify the resource by means of a string conforming to an identification system. Examples include International Standard Book Number (ISBN), Digital Object Identifier (DOI), and Uniform Resource Name (URN).  Persistent identifiers should be provided as HTTP URIs.</dc:description>
    <dc:issued rdf:datatype="http://www.w3.org/2001/XMLSchema#date">2008-01-14</dc:issued>
    <rdf:type rdf:resource="http://www.w3.org/2002/07/owl#NamedIndividual"/>
    <rdf:type rdf:resource="http://www.w3.org/2002/07/owl#DatatypeProperty"/>
    <rdfs:range rdf:resource="http://www.w3.org/2000/01/rdf-schema#Literal"/>
    <rdfs:subPropertyOf rdf:resource="http://purl.org/dc/elements/1.1/identifier"/>
    <rdf:type rdf:resource="http://www.w3.org/2002/07/owl#AnnotationProperty"/>
  </rdf:Description>
  <rdf:Description rdf:nodeID="A67">
    <owl:unionOf rdf:nodeID="A149"/>
    <rdf:type rdf:resource="http://www.w3.org/2002/07/owl#Class"/>
  </rdf:Description>
  <rdf:Description rdf:about="http://w3id.org/arto#Artwork">
    <rdfs:label>Artwork</rdfs:label>
    <rdfs:comment>Represents a created object intended to be aesthetically pleasing or convey artistic meaning. This class encompasses various art forms including paintings, sculptures, photographs, and digital art. Unlike CIDOC-CRM's E22_Human-Made_Object which covers all manufactured items, arto:Artwork specifically focuses on objects created with artistic intent. The class inherits essential properties from schema:CreativeWork (creator, dateCreated, description) while adding art-specific constraints such as mandatory visual representation (edm:isShownBy) and current location tracking. Each artwork must contain at least one scene and have defined dimensions, supporting both traditional and contemporary art analysis.</rdfs:comment>
    <rdfs:subClassOf rdf:nodeID="A178"/>
    <rdfs:subClassOf rdf:nodeID="A181"/>
    <rdf:type rdf:resource="http://www.w3.org/2002/07/owl#Class"/>
    <rdfs:subClassOf rdf:resource="https://schema.org/CreativeWork"/>
    <rdfs:subClassOf rdf:nodeID="A182"/>
    <rdfs:subClassOf rdf:nodeID="A183"/>
    <rdfs:subClassOf rdf:nodeID="A179"/>
    <rdfs:subClassOf rdf:nodeID="A184"/>
    <rdfs:subClassOf rdf:nodeID="A78"/>
    <rdfs:subClassOf rdf:nodeID="A160"/>
    <rdfs:subClassOf rdf:nodeID="A126"/>
    <rdfs:subClassOf rdf:nodeID="A185"/>
    <rdfs:subClassOf rdf:nodeID="A186"/>
    <rdfs:subClassOf rdf:nodeID="A187"/>
    <rdfs:subClassOf rdf:nodeID="A6"/>
    <rdfs:subClassOf rdf:nodeID="A47"/>
    <rdfs:subClassOf rdf:nodeID="A188"/>
    <rdfs:subClassOf rdf:nodeID="A161"/>
  </rdf:Description>
  <rdf:Description rdf:nodeID="A92">
    <rdf:rest rdf:resource="http://www.w3.org/1999/02/22-rdf-syntax-ns#nil"/>
    <rdf:first rdf:nodeID="A189"/>
  </rdf:Description>
  <rdf:Description rdf:about="http://w3id.org/arto#emotionPerspective">
    <skos:example>
                          ex:melancholy_emotion arto:emotionPerspective "artist"^^xsd:string ;
                          ex:serenity_emotion arto:emotionPerspective "artwork"^^xsd:string ;
                          ex:excitement_emotion arto:emotionPerspective "viewer"^^xsd:string .
                          </skos:example>
    <rdfs:label xml:lang="en">emotionPerspective</rdfs:label>
    <rdfs:comment>Specifies the perspective or viewpoint from which an emotion is interpreted in relation to an artwork. This property distinguishes between emotions intended by the artist, emotions expressed by the artwork itself, emotions experienced by viewers. Values are restricted to: 'artist' (artist's intended emotion), 'artwork' (emotion expressed by the artwork's formal elements), and 'viewer' (viewer's emotional response).</rdfs:comment>
    <rdfs:range rdf:nodeID="A176"/>
    <rdfs:domain rdf:resource="http://w3id.org/arto#Emotion"/>
    <rdf:type rdf:resource="http://www.w3.org/2002/07/owl#DatatypeProperty"/>
  </rdf:Description>
  <rdf:Description rdf:nodeID="A52">
    <rdf:rest rdf:nodeID="A190"/>
    <rdf:first rdf:resource="http://w3id.org/arto#Agent"/>
  </rdf:Description>
  <rdf:Description rdf:about="http://purl.org/dc/terms/RFC3066">
    <rdfs:seeAlso rdf:resource="http://www.ietf.org/rfc/rfc3066.txt"/>
    <rdfs:label xml:lang="en">RFC 3066</rdfs:label>
    <rdfs:isDefinedBy rdf:resource="http://purl.org/dc/terms/"/>
    <rdfs:comment xml:lang="en">The set of tags constructed according to RFC 3066 for the identification of languages.</rdfs:comment>
    <dc:description xml:lang="en">RFC 3066 has been obsoleted by RFC 4646.</dc:description>
    <dc:issued rdf:datatype="http://www.w3.org/2001/XMLSchema#date">2002-07-13</dc:issued>
    <rdf:type rdf:resource="http://www.w3.org/2002/07/owl#NamedIndividual"/>
    <rdf:type rdf:resource="http://www.w3.org/2000/01/rdf-schema#Datatype"/>
  </rdf:Description>
  <rdf:Description rdf:about="http://w3id.org/arto#Scene">
    <rdfs:label>Scene</rdfs:label>
    <rdfs:comment>Represents a coherent visual or narrative unit within an artwork that conveys specific meaning or sentiment. A scene aggregates objects and visual elements into meaningful compositions, supporting hierarchical structures where complex artworks contain multiple interconnected scenes. It's similar to ICON's image representations but with explicit support for scene nesting and relationships. Scenes can reference historical, mythological, or fictional events through relatedToEvent, enabling contextual artwork analysis.</rdfs:comment>
    <rdfs:subClassOf rdf:nodeID="A31"/>
    <rdfs:subClassOf rdf:nodeID="A191"/>
    <rdfs:subClassOf rdf:nodeID="A153"/>
    <rdfs:subClassOf rdf:nodeID="A192"/>
    <rdfs:subClassOf rdf:nodeID="A42"/>
    <rdfs:subClassOf rdf:nodeID="A91"/>
    <rdfs:subClassOf rdf:nodeID="A193"/>
    <rdfs:subClassOf rdf:nodeID="A43"/>
    <rdf:type rdf:resource="http://www.w3.org/2002/07/owl#Class"/>
  </rdf:Description>
  <rdf:Description rdf:about="http://w3id.org/arto#Object">
    <rdfs:label>Object</rdfs:label>
    <rdfs:comment>Represents identifiable and meaningful entities depicted within artworks, composed of various visual elements. Objects serve as the primary content units for artwork analysis, with properties describing their physical state, material composition, and spatial relationships</rdfs:comment>
    <rdfs:subClassOf rdf:nodeID="A174"/>
    <rdfs:subClassOf rdf:nodeID="A151"/>
    <rdfs:subClassOf rdf:nodeID="A194"/>
    <rdfs:subClassOf rdf:nodeID="A163"/>
    <rdfs:subClassOf rdf:nodeID="A125"/>
    <rdfs:subClassOf rdf:nodeID="A195"/>
    <rdfs:subClassOf rdf:nodeID="A196"/>
    <rdfs:subClassOf rdf:nodeID="A113"/>
    <rdfs:subClassOf rdf:nodeID="A197"/>
    <rdf:type rdf:resource="http://www.w3.org/2002/07/owl#Class"/>
  </rdf:Description>
  <rdf:Description rdf:about="http://www.w3.org/2001/XMLSchema#date">
    <rdf:type rdf:resource="http://www.w3.org/2000/01/rdf-schema#Datatype"/>
  </rdf:Description>
  <rdf:Description rdf:about="http://w3id.org/arto#Photograph">
    <rdfs:label>Photograph</rdfs:label>
    <rdfs:comment>A specific type of artwork created using photography or similar media. </rdfs:comment>
    <rdfs:subClassOf rdf:resource="http://w3id.org/arto#Artwork"/>
    <rdf:type rdf:resource="http://www.w3.org/2002/07/owl#Class"/>
  </rdf:Description>
  <rdf:Description rdf:nodeID="A2">
    <rdf:rest rdf:resource="http://www.w3.org/1999/02/22-rdf-syntax-ns#nil"/>
    <rdf:first rdf:nodeID="A145"/>
  </rdf:Description>
  <rdf:Description rdf:nodeID="A182">
    <owl:allValuesFrom rdf:resource="http://w3id.org/arto#Agent"/>
    <owl:onProperty rdf:resource="http://purl.org/dc/terms/contributor"/>
    <rdf:type rdf:resource="http://www.w3.org/2002/07/owl#Restriction"/>
  </rdf:Description>
  <rdf:Description rdf:about="http://w3id.org/arto#hasColourValue">
    <rdfs:label>hasColourValue</rdfs:label>
    <skos:example>
                      - RGB value:
                        :c_vermilion a arto:Colour ;
                          arto:hasColourValue [
                            a arto:ColourValue ;
                            arto:colourSpace "RGB" ;
                            qudt:vector (227 66 52)      # R,G,B in 0–255
                          ] .

                      - HSV value:
                        :c_skyBlue a arto:Colour ;
                          arto:hasColourValue [
                            a arto:ColourValue ;
                            arto:colourSpace "HSV" ;
                            qudt:vector (197 0.76 1.00)  # H in degrees; S,V in 0–1
                          ] .

                      - CMYK value:
                        :c_cadmiumYellow a arto:Colour ;
                          arto:hasColourValue [
                            a arto:ColourValue ;
                            arto:colourSpace "CMYK" ;
                            qudt:vector (0.00 0.09 0.90 0.00)  # C,M,Y,K in 0–1
                          ] .

                      - CIE Lab value with white point:
                        :c_ultramarine a arto:Colour ;
                          arto:hasColourValue [
                            a arto:ColourValue ;
                            arto:colourSpace "Lab" ;
                            qudt:vector (32.4 14.8 -38.1) ;
                            arto:whitePoint arto:D65
                          ] .
                      </skos:example>
    <rdfs:comment>Associates a colour with its value, allowing for flexible representation of colour information in artworks. This property supports different colour spaces for example RGB and HSV formats, enabling detailed colour analysis and representation.</rdfs:comment>
    <rdfs:range rdf:resource="http://w3id.org/arto#ColourValue"/>
    <rdfs:domain rdf:resource="http://w3id.org/arto#Colour"/>
    <rdf:type rdf:resource="http://www.w3.org/2002/07/owl#ObjectProperty"/>
  </rdf:Description>
  <rdf:Description rdf:about="http://w3id.org/arto#Location">
    <rdfs:label>Location</rdfs:label>
    <rdfs:comment>Represents locations associated with artworks (creation, display, storage, provenance, or depicted scenes). Location type is recorded as free text, e.g., studio, museum, gallery, exhibition venue, storage, auction house, private collection, findspot, city, region, country, fictional place, or depicted place. GeoSPARQL WKT may be provided when precise geometry is known; otherwise names alone are acceptable. Historical changes (renamings/boundaries) can be handled by creating distinct Location instances and linking them to events or times as needed.</rdfs:comment>
    <rdfs:subClassOf rdf:nodeID="A79"/>
    <rdfs:subClassOf rdf:nodeID="A51"/>
    <rdfs:subClassOf rdf:resource="http://www.cidoc-crm.org/cidoc-crm/E53_Place"/>
    <rdf:type rdf:resource="http://www.w3.org/2002/07/owl#Class"/>
  </rdf:Description>
  <rdf:Description rdf:about="http://purl.org/dc/terms/PhysicalResource">
    <rdfs:label xml:lang="en">Physical Resource</rdfs:label>
    <rdfs:isDefinedBy rdf:resource="http://purl.org/dc/terms/"/>
    <rdfs:comment xml:lang="en">A material thing.</rdfs:comment>
    <dc:issued rdf:datatype="http://www.w3.org/2001/XMLSchema#date">2008-01-14</dc:issued>
    <rdf:type rdf:resource="http://www.w3.org/2002/07/owl#NamedIndividual"/>
    <rdf:type rdf:resource="http://www.w3.org/2002/07/owl#Class"/>
  </rdf:Description>
  <rdf:Description rdf:nodeID="A177">
    <rdf:rest rdf:nodeID="A169"/>
    <rdf:first>Artist</rdf:first>
    <rdf:type rdf:resource="http://www.w3.org/1999/02/22-rdf-syntax-ns#List"/>
  </rdf:Description>
  <rdf:Description rdf:about="http://w3id.org/arto#StyleType">
    <rdfs:label>StyleType</rdfs:label>
    <rdfs:comment>Represents the style of an artwork, such as Impressionism, Cubism, etc. This class allows for the classification of artworks based on their stylistic characteristics.</rdfs:comment>
    <rdfs:subClassOf rdf:nodeID="A72"/>
    <rdf:type rdf:resource="http://www.w3.org/2002/07/owl#Class"/>
  </rdf:Description>
  <rdf:Description rdf:nodeID="A193">
    <owl:allValuesFrom rdf:resource="http://w3id.org/arto#Scene"/>
    <owl:onProperty rdf:resource="http://w3id.org/arto#containsScene"/>
    <rdf:type rdf:resource="http://www.w3.org/2002/07/owl#Restriction"/>
  </rdf:Description>
  <rdf:Description rdf:nodeID="A5">
    <rdf:rest rdf:resource="http://www.w3.org/1999/02/22-rdf-syntax-ns#nil"/>
    <rdf:first rdf:resource="http://w3id.org/arto#Scene"/>
  </rdf:Description>
  <rdf:Description rdf:nodeID="A167">
    <rdf:rest rdf:nodeID="A117"/>
    <rdf:first rdf:resource="http://w3id.org/arto#Object"/>
  </rdf:Description>
  <rdf:Description rdf:nodeID="A194">
    <owl:allValuesFrom rdf:resource="http://www.w3.org/2004/02/skos/core#Concept"/>
    <owl:onProperty rdf:resource="http://w3id.org/arto#state"/>
    <rdf:type rdf:resource="http://www.w3.org/2002/07/owl#Restriction"/>
  </rdf:Description>
  <rdf:Description rdf:about="http://purl.org/dc/terms/LicenseDocument">
    <rdfs:label xml:lang="en">License Document</rdfs:label>
    <rdfs:isDefinedBy rdf:resource="http://purl.org/dc/terms/"/>
    <rdfs:comment xml:lang="en">A legal document giving official permission to do something with a resource.</rdfs:comment>
    <dc:issued rdf:datatype="http://www.w3.org/2001/XMLSchema#date">2008-01-14</dc:issued>
    <rdf:type rdf:resource="http://www.w3.org/2002/07/owl#NamedIndividual"/>
    <rdfs:subClassOf rdf:resource="http://purl.org/dc/terms/RightsStatement"/>
    <rdf:type rdf:resource="http://www.w3.org/2002/07/owl#Class"/>
  </rdf:Description>
  <rdf:Description rdf:nodeID="A132">
    <owl:oneOf rdf:nodeID="A133"/>
    <rdf:type rdf:resource="http://www.w3.org/2000/01/rdf-schema#Datatype"/>
  </rdf:Description>
  <rdf:Description rdf:about="https://schema.org/CreativeWork">
    <rdf:type rdf:resource="http://www.w3.org/2002/07/owl#Class"/>
  </rdf:Description>
  <rdf:Description rdf:about="http://purl.org/dc/terms/LCC">
    <rdfs:seeAlso rdf:resource="http://lcweb.loc.gov/catdir/cpso/lcco/lcco.html"/>
    <rdfs:label xml:lang="en">LCC</rdfs:label>
    <rdfs:isDefinedBy rdf:resource="http://purl.org/dc/terms/"/>
    <rdfs:comment xml:lang="en">The set of conceptual resources specified by the Library of Congress Classification.</rdfs:comment>
    <dc:issued rdf:datatype="http://www.w3.org/2001/XMLSchema#date">2000-07-11</dc:issued>
    <rdf:type rdf:resource="http://purl.org/dc/dcam/VocabularyEncodingScheme"/>
    <rdf:type rdf:resource="http://www.w3.org/2002/07/owl#NamedIndividual"/>
  </rdf:Description>
  <rdf:Description rdf:about="http://w3id.org/arto#isLocationOf">
    <skos:example>
                - Museum address: :met_nyc_location arto:isLocationOf :metropolitan_museum
                - Gallery location: :london_bankside arto:isLocationOf :tate_modern
                - Studio location: :manhattan_location arto:isLocationOf :warhol_factory
                - Exhibition event: :venice_giardini arto:isLocationOf :venice_biennale_2024</skos:example>
    <rdfs:label>isLocationOf</rdfs:label>
    <rdfs:comment>Associates a location with the agent or event that it is related to.</rdfs:comment>
    <rdfs:range rdf:nodeID="A164"/>
    <rdfs:domain rdf:resource="http://w3id.org/arto#Location"/>
    <rdf:type rdf:resource="http://www.w3.org/2002/07/owl#ObjectProperty"/>
  </rdf:Description>
  <rdf:Description rdf:nodeID="A157">
    <rdf:rest rdf:resource="http://www.w3.org/1999/02/22-rdf-syntax-ns#nil"/>
    <rdf:first rdf:resource="http://w3id.org/arto#Scene"/>
  </rdf:Description>
  <rdf:Description rdf:about="http://purl.org/dc/terms/Box">
    <rdfs:seeAlso rdf:resource="https://www.dublincore.org/specifications/dublin-core/dcmi-box/"/>
    <rdfs:label xml:lang="en">DCMI Box</rdfs:label>
    <rdfs:isDefinedBy rdf:resource="http://purl.org/dc/terms/"/>
    <rdfs:comment xml:lang="en">The set of regions in space defined by their geographic coordinates according to the DCMI Box Encoding Scheme.</rdfs:comment>
    <dc:issued rdf:datatype="http://www.w3.org/2001/XMLSchema#date">2000-07-11</dc:issued>
    <rdf:type rdf:resource="http://www.w3.org/2002/07/owl#NamedIndividual"/>
    <rdf:type rdf:resource="http://www.w3.org/2000/01/rdf-schema#Datatype"/>
  </rdf:Description>
  <rdf:Description rdf:about="http://purl.org/dc/elements/1.1/rights">
    <rdf:type rdf:resource="http://www.w3.org/2002/07/owl#AnnotationProperty"/>
  </rdf:Description>
  <rdf:Description rdf:nodeID="A189">
    <owl:hasValue rdf:resource="http://vocab.getty.edu/aat/300264088"/>
    <owl:onProperty rdf:resource="http://www.w3.org/2004/02/skos/core#broaderTransitive"/>
    <rdf:type rdf:resource="http://www.w3.org/2002/07/owl#Restriction"/>
  </rdf:Description>
  <rdf:Description rdf:about="http://purl.org/dc/terms/LCSH">
    <rdfs:label xml:lang="en">LCSH</rdfs:label>
    <rdfs:isDefinedBy rdf:resource="http://purl.org/dc/terms/"/>
    <rdfs:comment xml:lang="en">The set of labeled concepts specified by the Library of Congress Subject Headings.</rdfs:comment>
    <dc:issued rdf:datatype="http://www.w3.org/2001/XMLSchema#date">2000-07-11</dc:issued>
    <rdf:type rdf:resource="http://purl.org/dc/dcam/VocabularyEncodingScheme"/>
    <rdf:type rdf:resource="http://www.w3.org/2002/07/owl#NamedIndividual"/>
  </rdf:Description>
  <rdf:Description rdf:nodeID="A38">
    <owl:allValuesFrom rdf:resource="http://w3id.org/arto#Metric"/>
    <owl:onProperty rdf:resource="http://w3id.org/arto#hasMetric"/>
    <rdf:type rdf:resource="http://www.w3.org/2002/07/owl#Restriction"/>
  </rdf:Description>
  <rdf:Description rdf:nodeID="A190">
    <rdf:rest rdf:resource="http://www.w3.org/1999/02/22-rdf-syntax-ns#nil"/>
    <rdf:first rdf:resource="http://w3id.org/arto#Event"/>
  </rdf:Description>
  <rdf:Description rdf:about="http://w3id.org/arto#Connotation">
    <skos:example>
                     - Symbolic meaning: :dove_symbolism rdf:type arto:Symbolism .
                     - Emotional content: :melancholy_mood rdf:type arto:Emotion ; arto:emotionPerspective "artwork"
                     - Historical reference: :revolution_allegory rdf:type arto:Connotation ;
                       dc:description "French Revolution political symbolism"
                     </skos:example>
    <rdfs:label>Connotation</rdfs:label>
    <rdfs:comment>Represents the implied meanings of artwork, includeing themes, symbolic meanings, and
      emotions conveyed by an artwork.</rdfs:comment>
    <rdfs:subClassOf rdf:nodeID="A162"/>
    <rdfs:subClassOf rdf:resource="http://www.cidoc-crm.org/cidoc-crm/E28_Conceptual_Object"/>
    <rdf:type rdf:resource="http://www.w3.org/2002/07/owl#Class"/>
  </rdf:Description>
  <rdf:Description rdf:nodeID="A198">
    <rdf:rest rdf:nodeID="A123"/>
    <rdf:first rdf:resource="http://w3id.org/arto#Object"/>
  </rdf:Description>
  <rdf:Description rdf:about="http://w3id.org/arto#Metric">
    <rdfs:label>Metric</rdfs:label>
    <skos:example>
               :guernica a arto:Artwork ;
                 arto:hasMetric :guernica_MainColour .

               :guernica_MainColour a arto:MainColour ;
                 arto:hasColour :greyTone_Colour .

               :starryNight a arto:Artwork ;
                 arto:hasMetric :starryNight_Balance .

               :starryNight_Balance a arto:BalanceOfComposition ;
                 arto:value 0.72 .

               :sunflowers a arto:Artwork ;
                 arto:hasMetric :sunflowers_Emotion .

               :sunflowers_Emotion a arto:EmotionIntensity ;
                 arto:level "high" .
            </skos:example>
    <rdfs:comment>Represents a quantifiable measurement or characteristic of an artwork,
      encompassing statistical information about basic elements such as colour statistics, emotion
      intensity, balance of composition, and other visual elements, to facilitate structural
      analysis
      and comparison of artworks.</rdfs:comment>
    <rdf:type rdf:resource="http://www.w3.org/2002/07/owl#Class"/>
  </rdf:Description>
  <rdf:Description rdf:about="http://w3id.org/arto#Space">
    <rdfs:label>Space</rdfs:label>
    <skos:example>
               :handscroll_Space a arto:Space ;
               dc:type "isometric / axonometric" .
                
              :Field_Space a arto:Space ;
                dc:type "flat / shallow space" .
            </skos:example>
    <rdfs:comment>Captures the representation of depth, and spatial organisation within artworks. </rdfs:comment>
    <rdfs:subClassOf rdf:nodeID="A30"/>
    <rdfs:subClassOf rdf:resource="http://w3id.org/arto#VisualElement"/>
    <rdf:type rdf:resource="http://www.w3.org/2002/07/owl#Class"/>
  </rdf:Description>
  <rdf:Description rdf:nodeID="A188">
    <owl:onClass rdf:resource="https://schema.org/QuantitativeValue"/>
    <owl:maxQualifiedCardinality rdf:datatype="http://www.w3.org/2001/XMLSchema#nonNegativeInteger">1</owl:maxQualifiedCardinality>
    <owl:onProperty rdf:resource="https://schema.org/width"/>
    <rdf:type rdf:resource="http://www.w3.org/2002/07/owl#Restriction"/>
  </rdf:Description>
  <rdf:Description rdf:nodeID="A105">
    <rdf:rest rdf:nodeID="A93"/>
    <rdf:first>HSV</rdf:first>
  </rdf:Description>
  <rdf:Description rdf:nodeID="A25">
    <owl:allValuesFrom rdf:resource="http://w3id.org/arto#Connotation"/>
    <owl:onProperty rdf:resource="http://w3id.org/arto#relatedToConnotation"/>
    <rdf:type rdf:resource="http://www.w3.org/2002/07/owl#Restriction"/>
  </rdf:Description>
  <rdf:Description rdf:nodeID="A199">
    <owl:minCardinality rdf:datatype="http://www.w3.org/2001/XMLSchema#nonNegativeInteger">1</owl:minCardinality>
  </rdf:Description>
  <rdf:Description rdf:about="http://purl.org/dc/terms/MESH">
    <rdfs:seeAlso rdf:resource="http://www.nlm.nih.gov/mesh/meshhome.html"/>
    <rdfs:label xml:lang="en">MeSH</rdfs:label>
    <rdfs:isDefinedBy rdf:resource="http://purl.org/dc/terms/"/>
    <rdfs:comment xml:lang="en">The set of labeled concepts specified by the Medical Subject Headings.</rdfs:comment>
    <dc:issued rdf:datatype="http://www.w3.org/2001/XMLSchema#date">2000-07-11</dc:issued>
    <rdf:type rdf:resource="http://purl.org/dc/dcam/VocabularyEncodingScheme"/>
    <rdf:type rdf:resource="http://www.w3.org/2002/07/owl#NamedIndividual"/>
  </rdf:Description>
  <rdf:Description rdf:nodeID="A185">
    <owl:allValuesFrom rdf:resource="http://w3id.org/arto#Event"/>
    <owl:onProperty rdf:resource="http://w3id.org/arto#relatedToEvent"/>
    <rdf:type rdf:resource="http://www.w3.org/2002/07/owl#Restriction"/>
  </rdf:Description>
  <rdf:Description rdf:about="http://w3id.org/arto#Line">
    <rdfs:label>Line</rdfs:label>
    <rdfs:comment>Represents linear visual elements in artworks. Typical line types may include straight, curved, broken, contour, gestural, structural, implied, and hatching or cross-hatching. These categories are indicative and may be aligned with controlled vocabularies such as Getty AAT where applicable.</rdfs:comment>
    <rdfs:subClassOf rdf:nodeID="A200"/>
    <rdfs:subClassOf rdf:nodeID="A141"/>
    <rdfs:subClassOf rdf:nodeID="A54"/>
    <rdfs:subClassOf rdf:nodeID="A61"/>
    <rdfs:subClassOf rdf:resource="http://w3id.org/arto#VisualElement"/>
    <rdf:type rdf:resource="http://www.w3.org/2002/07/owl#Class"/>
  </rdf:Description>
  <rdf:Description rdf:nodeID="A26">
    <owl:someValuesFrom rdf:resource="http://w3id.org/arto#Agent"/>
    <owl:onProperty rdf:resource="https://w3id.org/MON/event.owl#agent"/>
    <rdf:type rdf:resource="http://www.w3.org/2002/07/owl#Restriction"/>
  </rdf:Description>
  <rdf:Description rdf:nodeID="A197">
    <owl:someValuesFrom rdf:resource="http://w3id.org/arto#Connotation"/>
    <owl:onProperty rdf:resource="http://w3id.org/arto#hasConnotation"/>
    <rdf:type rdf:resource="http://www.w3.org/2002/07/owl#Restriction"/>
  </rdf:Description>
  <rdf:Description rdf:about="http://purl.org/dc/terms/isReferencedBy">
    <rdfs:label xml:lang="en">Is Referenced By</rdfs:label>
    <rdfs:isDefinedBy rdf:resource="http://purl.org/dc/terms/"/>
    <rdfs:comment xml:lang="en">A related resource that references, cites, or otherwise points to the described resource.</rdfs:comment>
    <dc:description xml:lang="en">This property is intended to be used with non-literal values. This property is an inverse property of References.</dc:description>
    <dc:issued rdf:datatype="http://www.w3.org/2001/XMLSchema#date">2000-07-11</dc:issued>
    <rdf:type rdf:resource="http://www.w3.org/2002/07/owl#NamedIndividual"/>
    <rdfs:subPropertyOf rdf:resource="http://purl.org/dc/terms/relation"/>
    <rdfs:subPropertyOf rdf:resource="http://purl.org/dc/elements/1.1/relation"/>
    <rdf:type rdf:resource="http://www.w3.org/2002/07/owl#AnnotationProperty"/>
  </rdf:Description>
  <rdf:Description rdf:about="http://w3id.org/arto#relatedToScene">
    <skos:example>
                      - Object context: :bread_loaf arto:relatedToScene :market_scene </skos:example>
    <rdfs:label>relatedToScene</rdfs:label>
    <rdfs:comment>Links objects to the scenes they appear in or are associated with.</rdfs:comment>
    <rdfs:range rdf:resource="http://w3id.org/arto#Scene"/>
    <rdfs:domain rdf:resource="http://w3id.org/arto#Object"/>
    <rdf:type rdf:resource="http://www.w3.org/2002/07/owl#ObjectProperty"/>
  </rdf:Description>
  <rdf:Description rdf:about="http://w3id.org/arto#size">
    <rdfs:label>size</rdfs:label>
    <rdfs:comment>Indicates the relative or absolute dimensions of objects and scenes within artwork composition. Size often correlate with narrative importance, symbolic significance, or perspectival organisation in artistic composition.</rdfs:comment>
    <rdfs:range rdf:resource="http://www.w3.org/2001/XMLSchema#string"/>
    <rdfs:domain rdf:nodeID="A111"/>
    <rdf:type rdf:resource="http://www.w3.org/2002/07/owl#DatatypeProperty"/>
  </rdf:Description>
  <rdf:Description rdf:nodeID="A97">
    <rdf:rest rdf:nodeID="A146"/>
    <rdf:first rdf:resource="http://www.w3.org/2004/02/skos/core#Concept"/>
  </rdf:Description>
  <rdf:Description rdf:nodeID="A192">
    <owl:allValuesFrom rdf:resource="http://w3id.org/arto#Metric"/>
    <owl:onProperty rdf:resource="http://w3id.org/arto#hasMetric"/>
    <rdf:type rdf:resource="http://www.w3.org/2002/07/owl#Restriction"/>
  </rdf:Description>
  <rdf:Description rdf:nodeID="A201">
    <owl:minCardinality rdf:datatype="http://www.w3.org/2001/XMLSchema#nonNegativeInteger">1</owl:minCardinality>
  </rdf:Description>
  <rdf:Description rdf:nodeID="A202">
    <owl:minCardinality rdf:datatype="http://www.w3.org/2001/XMLSchema#nonNegativeInteger">1</owl:minCardinality>
  </rdf:Description>
  <rdf:Description rdf:nodeID="A203">
    <owl:qualifiedCardinality rdf:datatype="http://www.w3.org/2001/XMLSchema#nonNegativeInteger">1</owl:qualifiedCardinality>
  </rdf:Description>
  <rdf:Description rdf:nodeID="A204">
    <rdf:rest rdf:nodeID="A205"/>
    <rdf:first rdf:resource="http://w3id.org/arto#Object"/>
  </rdf:Description>
  <rdf:Description rdf:about="http://purl.org/dc/terms/dateCopyrighted">
    <rdfs:label xml:lang="en">Date Copyrighted</rdfs:label>
    <rdfs:isDefinedBy rdf:resource="http://purl.org/dc/terms/"/>
    <rdfs:comment xml:lang="en">Date of copyright of the resource.</rdfs:comment>
    <dc:description xml:lang="en">Typically a year.  Recommended practice is to describe the date, date/time, or period of time as recommended for the property Date, of which this is a subproperty.</dc:description>
    <dc:issued rdf:datatype="http://www.w3.org/2001/XMLSchema#date">2002-07-13</dc:issued>
    <rdf:type rdf:resource="http://www.w3.org/2002/07/owl#NamedIndividual"/>
    <rdfs:subPropertyOf rdf:resource="http://purl.org/dc/terms/date"/>
    <rdf:type rdf:resource="http://www.w3.org/2002/07/owl#DatatypeProperty"/>
    <rdfs:range rdf:resource="http://www.w3.org/2000/01/rdf-schema#Literal"/>
    <rdfs:subPropertyOf rdf:resource="http://purl.org/dc/elements/1.1/date"/>
    <rdf:type rdf:resource="http://www.w3.org/2002/07/owl#AnnotationProperty"/>
  </rdf:Description>
  <rdf:Description rdf:nodeID="A206">
    <owl:cardinality rdf:datatype="http://www.w3.org/2001/XMLSchema#nonNegativeInteger">1</owl:cardinality>
  </rdf:Description>
  <rdf:Description rdf:about="http://purl.org/dc/terms/LinguisticSystem">
    <rdfs:label xml:lang="en">Linguistic System</rdfs:label>
    <rdfs:isDefinedBy rdf:resource="http://purl.org/dc/terms/"/>
    <rdfs:comment xml:lang="en">A system of signs, symbols, sounds, gestures, or rules used in communication.</rdfs:comment>
    <dc:description xml:lang="en">Written, spoken, sign, and computer languages are linguistic systems.</dc:description>
    <dc:issued rdf:datatype="http://www.w3.org/2001/XMLSchema#date">2008-01-14</dc:issued>
    <rdf:type rdf:resource="http://www.w3.org/2002/07/owl#NamedIndividual"/>
    <rdf:type rdf:resource="http://www.w3.org/2002/07/owl#Class"/>
  </rdf:Description>
  <rdf:Description rdf:about="http://w3id.org/arto#MainColour">
    <rdfs:label>MainColour</rdfs:label>
    <skos:example>
                   - :starryNight_MainColour a arto:MainColour ;
                        arto:hasColour :deepBlue_Colour .

                   - :deepBlue_Colour a arto:Colour ;
                        arto:hasColourValue [
                           a arto:RGBValue ;
                           qudt:vector (18,10,143) ;
                        ] .
                </skos:example>
    <rdfs:comment>Represents the primary or most visually dominant colour of an artwork. 
This value can be derived by computational methods such as colour quantisation, clustering, or histogram analysis. This metric links to a specific Colour instance, which may be described using colour values (RGB, HSV, Lab, etc.) </rdfs:comment>
    <rdfs:subClassOf rdf:resource="http://w3id.org/arto#Metric"/>
    <rdf:type rdf:resource="http://www.w3.org/2002/07/owl#Class"/>
  </rdf:Description>
  <rdf:Description rdf:nodeID="A127">
    <owl:unionOf rdf:nodeID="A198"/>
    <rdf:type rdf:resource="http://www.w3.org/2002/07/owl#Class"/>
  </rdf:Description>
  <rdf:Description rdf:about="http://w3id.org/arto#Emotion">
    <skos:example>
# Artist's intended emotion
:guernica_antiwar_anger  arto:Emotion ;
    arto:expresses mfoem:MFOEM_000009 ;
    arto:emotionPerspective "artist" ;
    dc:description "Picasso's anger against the brutality of war" .

# Artwork's emotional expression  
:starry_night_turbulence rdf:type arto:Emotion ;
    arto:expresses mfoem:MFOEM_000028 ;
    arto:emotionPerspective "artwork" ;
    dc:description "Anxiety expressed through swirling brushstrokes and dynamic composition" .

# Viewer's emotional response
:mona_lisa_mystery rdf:type  arto:Emotion ;
    arto:expresses mfoem:MFOEM_000167 ;
    arto:emotionPerspective "viewer" ;
    dc:description "Viewer's curiosity evoked by the enigmatic smile" .
</skos:example>
    <rdfs:label>Emotion</rdfs:label>
    <rdfs:comment>Represents emotional content or affective responses in artworks.
             Uses MFOEM emotion ontology types and the emotionPerspective property to distinguish 
             between artist's intended emotion, artwork's emotional expression, and viewer's response.
             Emotions are expressed using standardised MFOEM emotion types including basic emotions (happiness, sadness, anger, fear, surprise, disgust) and complex emotions (love, anxiety, hope, despair, serenity). </rdfs:comment>
    <rdfs:subClassOf rdf:nodeID="A131"/>
    <rdfs:subClassOf rdf:nodeID="A55"/>
    <rdfs:subClassOf rdf:resource="http://w3id.org/arto#Connotation"/>
    <rdf:type rdf:resource="http://www.w3.org/2002/07/owl#Class"/>
  </rdf:Description>
  <rdf:Description rdf:about="http://w3id.org/arto#containsObject">
    <skos:example>
                      - Landscape scene: :garden_scene arto:containsObject :fountain, :bench, :flowers
                      - Portrait scene: :interior_scene arto:containsObject :chair, :table, :book
                      - Still life scene: :table_scene arto:containsObject :fruit_bowl, :wine_glass, :cloth</skos:example>
    <rdfs:label>containsObject</rdfs:label>
    <rdfs:comment>Indicates specific objects that are present within a scene of an artwork.</rdfs:comment>
    <rdfs:range rdf:resource="http://w3id.org/arto#Object"/>
    <rdfs:domain rdf:resource="http://w3id.org/arto#Scene"/>
    <owl:inverseOf rdf:resource="http://w3id.org/arto#isObjectOf"/>
    <rdf:type rdf:resource="http://www.w3.org/2002/07/owl#ObjectProperty"/>
  </rdf:Description>
  <rdf:Description rdf:nodeID="A207">
    <owl:cardinality rdf:datatype="http://www.w3.org/2001/XMLSchema#nonNegativeInteger">1</owl:cardinality>
  </rdf:Description>
  <rdf:Description rdf:nodeID="A147">
    <owl:someValuesFrom rdf:resource="http://vocab.getty.edu/aat/300163343"/>
    <owl:onProperty rdf:resource="http://www.w3.org/2004/02/skos/core#broader"/>
    <rdf:type rdf:resource="http://www.w3.org/2002/07/owl#Restriction"/>
  </rdf:Description>
  <rdf:Description rdf:nodeID="A208">
    <rdf:rest rdf:nodeID="A74"/>
    <rdf:first rdf:resource="http://w3id.org/arto#Object"/>
  </rdf:Description>
  <rdf:Description rdf:about="http://purl.org/dc/terms/rights">
    <rdfs:label xml:lang="en">Rights</rdfs:label>
    <rdfs:isDefinedBy rdf:resource="http://purl.org/dc/terms/"/>
    <rdfs:comment xml:lang="en">Information about rights held in and over the resource.</rdfs:comment>
    <dc:description xml:lang="en">Typically, rights information includes a statement about various property rights associated with the resource, including intellectual property rights.  Recommended practice is to refer to a rights statement with a URI.  If this is not possible or feasible, a literal value (name, label, or short text) may be provided.</dc:description>
    <j.0:rangeIncludes rdf:resource="http://purl.org/dc/terms/RightsStatement"/>
    <dc:issued rdf:datatype="http://www.w3.org/2001/XMLSchema#date">2008-01-14</dc:issued>
    <rdf:type rdf:resource="http://www.w3.org/2002/07/owl#NamedIndividual"/>
    <rdfs:subPropertyOf rdf:resource="http://purl.org/dc/elements/1.1/rights"/>
    <rdf:type rdf:resource="http://www.w3.org/2002/07/owl#AnnotationProperty"/>
  </rdf:Description>
  <rdf:Description rdf:nodeID="A209">
    <owl:minCardinality rdf:datatype="http://www.w3.org/2001/XMLSchema#nonNegativeInteger">1</owl:minCardinality>
  </rdf:Description>
  <rdf:Description rdf:about="http://purl.obolibrary.org/obo/MFOEM_000001">
    <rdf:type rdf:resource="http://www.w3.org/2002/07/owl#Class"/>
  </rdf:Description>
  <rdf:Description rdf:about="http://purl.org/dc/terms/mediator">
    <rdfs:label xml:lang="en">Mediator</rdfs:label>
    <rdfs:isDefinedBy rdf:resource="http://purl.org/dc/terms/"/>
    <rdfs:comment xml:lang="en">An entity that mediates access to the resource.</rdfs:comment>
    <dc:description xml:lang="en">In an educational context, a mediator might be a parent, teacher, teaching assistant, or care-giver.</dc:description>
    <j.0:rangeIncludes rdf:resource="http://purl.org/dc/terms/AgentClass"/>
    <dc:issued rdf:datatype="http://www.w3.org/2001/XMLSchema#date">2001-05-21</dc:issued>
    <rdf:type rdf:resource="http://www.w3.org/2002/07/owl#NamedIndividual"/>
    <rdfs:subPropertyOf rdf:resource="http://purl.org/dc/terms/audience"/>
    <rdf:type rdf:resource="http://www.w3.org/2002/07/owl#AnnotationProperty"/>
  </rdf:Description>
  <rdf:Description rdf:about="https://schema.org/QuantitativeValue">
    <rdf:type rdf:resource="http://www.w3.org/2002/07/owl#Class"/>
  </rdf:Description>
  <rdf:Description rdf:nodeID="A195">
    <owl:allValuesFrom rdf:resource="http://w3id.org/arto#MaterialType"/>
    <owl:onProperty rdf:resource="http://w3id.org/arto#material"/>
    <rdf:type rdf:resource="http://www.w3.org/2002/07/owl#Restriction"/>
  </rdf:Description>
  <rdf:Description rdf:nodeID="A210">
    <owl:minCardinality rdf:datatype="http://www.w3.org/2001/XMLSchema#nonNegativeInteger">1</owl:minCardinality>
  </rdf:Description>
  <rdf:Description rdf:nodeID="A196">
    <owl:allValuesFrom rdf:resource="http://w3id.org/arto#Metric"/>
    <owl:onProperty rdf:resource="http://w3id.org/arto#hasMetric"/>
    <rdf:type rdf:resource="http://www.w3.org/2002/07/owl#Restriction"/>
  </rdf:Description>
  <rdf:Description rdf:nodeID="A16">
    <owl:allValuesFrom rdf:resource="http://w3id.org/arto#Location"/>
    <owl:onProperty rdf:resource="http://w3id.org/arto#hasLocation"/>
    <rdf:type rdf:resource="http://www.w3.org/2002/07/owl#Restriction"/>
  </rdf:Description>
  <rdf:Description rdf:nodeID="A170">
    <rdf:rest rdf:resource="http://www.w3.org/1999/02/22-rdf-syntax-ns#nil"/>
    <rdf:first>Viewer</rdf:first>
    <rdf:type rdf:resource="http://www.w3.org/1999/02/22-rdf-syntax-ns#List"/>
  </rdf:Description>
  <rdf:Description rdf:nodeID="A181">
    <owl:allValuesFrom rdf:resource="http://www.w3.org/2001/XMLSchema#string"/>
    <owl:onProperty rdf:resource="http://purl.org/dc/terms/title"/>
    <rdf:type rdf:resource="http://www.w3.org/2002/07/owl#Restriction"/>
  </rdf:Description>
  <rdf:Description rdf:about="http://w3id.org/arto#knows">
    <skos:example>
            - Artist relationships: :vincent_van_gogh arto:knows :paul_gauguin
            - Teacher-student: :gustav_klimt arto:knows :egon_schiele
            - Collaborative artists: :pablo_picasso arto:knows :georges_braque</skos:example>
    <rdfs:label>knows</rdfs:label>
    <rdfs:comment>The person knows persons. This property, equivalent to foaf:knows, enables study of artistic movements, teacher-student relationships, collaborative networks, and cultural exchange patterns essential for understanding art historical development and cross-cultural artistic influence.</rdfs:comment>
    <rdfs:range rdf:resource="http://w3id.org/arto#Person"/>
    <rdfs:domain rdf:resource="http://w3id.org/arto#Person"/>
    <rdf:type rdf:resource="http://www.w3.org/2002/07/owl#ObjectProperty"/>
  </rdf:Description>
  <rdf:Description rdf:about="http://purl.org/dc/terms/NLM">
    <rdfs:seeAlso rdf:resource="http://wwwcf.nlm.nih.gov/class/"/>
    <rdfs:label xml:lang="en">NLM</rdfs:label>
    <rdfs:isDefinedBy rdf:resource="http://purl.org/dc/terms/"/>
    <rdfs:comment xml:lang="en">The set of conceptual resources specified by the National Library of Medicine Classification.</rdfs:comment>
    <dc:issued rdf:datatype="http://www.w3.org/2001/XMLSchema#date">2005-06-13</dc:issued>
    <rdf:type rdf:resource="http://purl.org/dc/dcam/VocabularyEncodingScheme"/>
    <rdf:type rdf:resource="http://www.w3.org/2002/07/owl#NamedIndividual"/>
  </rdf:Description>
  <rdf:Description rdf:nodeID="A17">
    <rdf:rest rdf:resource="http://www.w3.org/1999/02/22-rdf-syntax-ns#nil"/>
    <rdf:first>XYZ</rdf:first>
    <rdf:type rdf:resource="http://www.w3.org/1999/02/22-rdf-syntax-ns#List"/>
  </rdf:Description>
  <rdf:Description rdf:nodeID="A183">
    <owl:allValuesFrom rdf:resource="http://w3id.org/arto#Artist"/>
    <owl:onProperty rdf:resource="http://purl.org/dc/terms/creator"/>
    <rdf:type rdf:resource="http://www.w3.org/2002/07/owl#Restriction"/>
  </rdf:Description>
  <rdf:Description rdf:nodeID="A211">
    <owl:cardinality rdf:datatype="http://www.w3.org/2001/XMLSchema#nonNegativeInteger">1</owl:cardinality>
  </rdf:Description>
  <rdf:Description rdf:about="http://vocab.getty.edu/aat/300131647">
    <rdf:type rdf:resource="http://www.w3.org/2002/07/owl#NamedIndividual"/>
  </rdf:Description>
  <rdf:Description rdf:about="http://purl.org/dc/terms/rightsHolder">
    <rdfs:label xml:lang="en">Rights Holder</rdfs:label>
    <rdfs:isDefinedBy rdf:resource="http://purl.org/dc/terms/"/>
    <rdfs:comment xml:lang="en">A person or organization owning or managing rights over the resource.</rdfs:comment>
    <rdfs:comment xml:lang="en">A person or organisation owning or managing rights over the resource.</rdfs:comment>
    <dc:description xml:lang="en">Recommended practice is to refer to the rights holder with a URI. If this is not possible or feasible, a literal value that identifies the rights holder may be provided.</dc:description>
    <j.0:rangeIncludes rdf:resource="http://purl.org/dc/terms/Agent"/>
    <dc:issued rdf:datatype="http://www.w3.org/2001/XMLSchema#date">2004-06-14</dc:issued>
    <rdf:type rdf:resource="http://www.w3.org/2002/07/owl#NamedIndividual"/>
  </rdf:Description>
  <rdf:Description rdf:about="http://www.w3.org/2002/07/owl#maxQualifiedCardinality">
    <rdf:type rdf:resource="http://www.w3.org/2002/07/owl#AnnotationProperty"/>
  </rdf:Description>
  <rdf:Description rdf:nodeID="A66">
    <owl:allValuesFrom rdf:resource="http://w3id.org/arto#ColourTerm"/>
    <owl:onProperty rdf:resource="http://w3id.org/arto#hasColourTerm"/>
    <rdf:type rdf:resource="http://www.w3.org/2002/07/owl#Restriction"/>
  </rdf:Description>
  <rdf:Description rdf:about="http://purl.org/dc/terms/isReplacedBy">
    <rdfs:label xml:lang="en">Is Replaced By</rdfs:label>
    <rdfs:isDefinedBy rdf:resource="http://purl.org/dc/terms/"/>
    <rdfs:comment xml:lang="en">A related resource that supplants, displaces, or supersedes the described resource.</rdfs:comment>
    <dc:description xml:lang="en">This property is intended to be used with non-literal values. This property is an inverse property of Replaces.</dc:description>
    <dc:issued rdf:datatype="http://www.w3.org/2001/XMLSchema#date">2000-07-11</dc:issued>
    <rdf:type rdf:resource="http://www.w3.org/2002/07/owl#NamedIndividual"/>
    <rdfs:subPropertyOf rdf:resource="http://purl.org/dc/terms/relation"/>
    <rdfs:subPropertyOf rdf:resource="http://purl.org/dc/elements/1.1/relation"/>
    <rdf:type rdf:resource="http://www.w3.org/2002/07/owl#AnnotationProperty"/>
  </rdf:Description>
  <rdf:Description rdf:nodeID="A212">
    <owl:cardinality rdf:datatype="http://www.w3.org/2001/XMLSchema#nonNegativeInteger">1</owl:cardinality>
  </rdf:Description>
  <rdf:Description rdf:nodeID="A213">
    <owl:cardinality rdf:datatype="http://www.w3.org/2001/XMLSchema#nonNegativeInteger">1</owl:cardinality>
  </rdf:Description>
  <rdf:Description rdf:nodeID="A214">
    <owl:minCardinality rdf:datatype="http://www.w3.org/2001/XMLSchema#nonNegativeInteger">1</owl:minCardinality>
  </rdf:Description>
  <rdf:Description rdf:nodeID="A172">
    <rdf:rest rdf:nodeID="A99"/>
    <rdf:first rdf:resource="http://w3id.org/arto#Connotation"/>
  </rdf:Description>
  <rdf:Description rdf:about="http://purl.org/vocab/vann/preferredNamespacePrefix">
    <rdf:type rdf:resource="http://www.w3.org/2002/07/owl#AnnotationProperty"/>
  </rdf:Description>
  <rdf:Description rdf:nodeID="A215">
    <rdf:rest rdf:nodeID="A208"/>
    <rdf:first rdf:resource="http://w3id.org/arto#Artwork"/>
  </rdf:Description>
  <rdf:Description rdf:about="http://www.europeana.eu/schemas/edm/currentLocation">
    <rdf:type rdf:resource="http://www.w3.org/2002/07/owl#ObjectProperty"/>
  </rdf:Description>
  <rdf:Description rdf:about="http://purl.org/dc/dcam/domainIncludes">
    <rdf:type rdf:resource="http://www.w3.org/2002/07/owl#AnnotationProperty"/>
  </rdf:Description>
  <rdf:Description rdf:nodeID="A139">
    <owl:unionOf rdf:nodeID="A215"/>
    <rdf:type rdf:resource="http://www.w3.org/2002/07/owl#Class"/>
  </rdf:Description>
  <rdf:Description rdf:about="http://purl.org/dc/elements/1.1/type">
    <rdf:type rdf:resource="http://www.w3.org/2002/07/owl#AnnotationProperty"/>
  </rdf:Description>
  <rdf:Description rdf:about="http://vocab.getty.edu/aat/300163343">
    <rdf:type rdf:resource="http://www.w3.org/2002/07/owl#Class"/>
  </rdf:Description>
  <rdf:Description rdf:nodeID="A49">
    <rdf:rest rdf:nodeID="A62"/>
    <rdf:first>Lab</rdf:first>
    <rdf:type rdf:resource="http://www.w3.org/1999/02/22-rdf-syntax-ns#List"/>
  </rdf:Description>
  <rdf:Description rdf:nodeID="A187">
    <owl:allValuesFrom rdf:resource="http://w3id.org/arto#TechniqueType"/>
    <owl:onProperty rdf:resource="http://w3id.org/arto#technique"/>
    <rdf:type rdf:resource="http://www.w3.org/2002/07/owl#Restriction"/>
  </rdf:Description>
  <rdf:Description rdf:nodeID="A122">
    <rdf:rest rdf:nodeID="A148"/>
    <rdf:first rdf:resource="http://w3id.org/arto#Object"/>
  </rdf:Description>
  <rdf:Description rdf:nodeID="A152">
    <owl:unionOf rdf:nodeID="A129"/>
    <rdf:type rdf:resource="http://www.w3.org/2002/07/owl#Class"/>
  </rdf:Description>
  <rdf:Description rdf:nodeID="A138">
    <rdf:rest rdf:nodeID="A204"/>
    <rdf:first rdf:resource="http://w3id.org/arto#Connotation"/>
  </rdf:Description>
  <rdf:Description rdf:about="http://purl.org/dc/terms/dateAccepted">
    <rdfs:label xml:lang="en">Date Accepted</rdfs:label>
    <rdfs:isDefinedBy rdf:resource="http://purl.org/dc/terms/"/>
    <rdfs:comment xml:lang="en">Date of acceptance of the resource.</rdfs:comment>
    <dc:description xml:lang="en">Recommended practice is to describe the date, date/time, or period of time as recommended for the property Date, of which this is a subproperty.  Examples of resources to which a date of acceptance may be relevant are a thesis (accepted by a university department) or an article (accepted by a journal).</dc:description>
    <dc:issued rdf:datatype="http://www.w3.org/2001/XMLSchema#date">2002-07-13</dc:issued>
    <rdf:type rdf:resource="http://www.w3.org/2002/07/owl#NamedIndividual"/>
    <rdfs:subPropertyOf rdf:resource="http://purl.org/dc/terms/date"/>
    <rdf:type rdf:resource="http://www.w3.org/2002/07/owl#DatatypeProperty"/>
    <rdfs:range rdf:resource="http://www.w3.org/2000/01/rdf-schema#Literal"/>
    <rdfs:subPropertyOf rdf:resource="http://purl.org/dc/elements/1.1/date"/>
    <rdf:type rdf:resource="http://www.w3.org/2002/07/owl#AnnotationProperty"/>
  </rdf:Description>
  <rdf:Description rdf:about="http://vocab.getty.edu/aat/300264088">
    <rdf:type rdf:resource="http://www.w3.org/2002/07/owl#NamedIndividual"/>
  </rdf:Description>
  <rdf:Description rdf:nodeID="A37">
    <rdf:rest rdf:resource="http://www.w3.org/1999/02/22-rdf-syntax-ns#nil"/>
    <rdf:first rdf:resource="http://w3id.org/arto#Event"/>
  </rdf:Description>
  <rdf:Description rdf:about="http://purl.org/dc/terms/created">
    <rdfs:label xml:lang="en">Date Created</rdfs:label>
    <rdfs:isDefinedBy rdf:resource="http://purl.org/dc/terms/"/>
    <rdfs:comment xml:lang="en">Date of creation of the resource.</rdfs:comment>
    <dc:description xml:lang="en">Recommended practice is to describe the date, date/time, or period of time as recommended for the property Date, of which this is a subproperty.</dc:description>
    <dc:issued rdf:datatype="http://www.w3.org/2001/XMLSchema#date">2000-07-11</dc:issued>
    <rdf:type rdf:resource="http://www.w3.org/2002/07/owl#NamedIndividual"/>
    <rdfs:subPropertyOf rdf:resource="http://purl.org/dc/terms/date"/>
    <rdf:type rdf:resource="http://www.w3.org/2002/07/owl#DatatypeProperty"/>
    <rdfs:range rdf:resource="http://www.w3.org/2000/01/rdf-schema#Literal"/>
    <rdfs:subPropertyOf rdf:resource="http://purl.org/dc/elements/1.1/date"/>
    <rdf:type rdf:resource="http://www.w3.org/2002/07/owl#AnnotationProperty"/>
  </rdf:Description>
  <rdf:Description rdf:about="http://purl.org/dc/terms/AgentClass">
    <rdfs:label xml:lang="en">Agent Class</rdfs:label>
    <rdfs:isDefinedBy rdf:resource="http://purl.org/dc/terms/"/>
    <rdfs:comment xml:lang="en">A group of agents.</rdfs:comment>
    <dc:issued rdf:datatype="http://www.w3.org/2001/XMLSchema#date">2008-01-14</dc:issued>
    <rdf:type rdf:resource="http://www.w3.org/2002/07/owl#NamedIndividual"/>
    <rdfs:subClassOf rdf:resource="http://www.w3.org/2000/01/rdf-schema#Class"/>
    <rdf:type rdf:resource="http://www.w3.org/2002/07/owl#Class"/>
  </rdf:Description>
  <rdf:Description rdf:nodeID="A216">
    <owl:minCardinality rdf:datatype="http://www.w3.org/2001/XMLSchema#nonNegativeInteger">1</owl:minCardinality>
  </rdf:Description>
  <rdf:Description rdf:about="http://vocab.getty.edu/aat/300264091">
    <rdf:type rdf:resource="http://www.w3.org/2002/07/owl#NamedIndividual"/>
  </rdf:Description>
  <rdf:Description rdf:nodeID="A200">
    <owl:allValuesFrom rdf:resource="http://www.w3.org/2001/XMLSchema#float"/>
    <owl:onProperty rdf:resource="http://w3id.org/arto#width"/>
    <rdf:type rdf:resource="http://www.w3.org/2002/07/owl#Restriction"/>
  </rdf:Description>
  <rdf:Description rdf:nodeID="A112">
    <rdf:rest rdf:nodeID="A59"/>
    <rdf:first rdf:resource="http://w3id.org/arto#Object"/>
  </rdf:Description>
  <rdf:Description rdf:about="http://purl.org/dc/terms/source">
    <rdfs:label xml:lang="en">Source</rdfs:label>
    <rdfs:isDefinedBy rdf:resource="http://purl.org/dc/terms/"/>
    <rdfs:comment xml:lang="en">A related resource from which the described resource is derived.</rdfs:comment>
    <dc:description xml:lang="en">This property is intended to be used with non-literal values. The described resource may be derived from the related resource in whole or in part. Best practice is to identify the related resource by means of a URI or a string conforming to a formal identification system.</dc:description>
    <dc:issued rdf:datatype="http://www.w3.org/2001/XMLSchema#date">2008-01-14</dc:issued>
    <rdf:type rdf:resource="http://www.w3.org/2002/07/owl#NamedIndividual"/>
    <rdfs:subPropertyOf rdf:resource="http://purl.org/dc/terms/relation"/>
    <rdfs:subPropertyOf rdf:resource="http://purl.org/dc/elements/1.1/source"/>
    <rdf:type rdf:resource="http://www.w3.org/2002/07/owl#AnnotationProperty"/>
  </rdf:Description>
  <rdf:Description rdf:nodeID="A184">
    <owl:allValuesFrom rdf:resource="http://w3id.org/arto#Scene"/>
    <owl:onProperty rdf:resource="http://w3id.org/arto#containsScene"/>
    <rdf:type rdf:resource="http://www.w3.org/2002/07/owl#Restriction"/>
  </rdf:Description>
  <rdf:Description rdf:about="http://w3id.org/arto#Sponsor">
    <rdfs:label>Sponsor</rdfs:label>
    <rdfs:comment>The person or group who sponsor the artwork.</rdfs:comment>
    <rdfs:subClassOf rdf:resource="http://w3id.org/arto#Person"/>
    <rdf:type rdf:resource="http://www.w3.org/2002/07/owl#Class"/>
  </rdf:Description>
  <rdf:Description rdf:nodeID="A135">
    <rdf:rest rdf:nodeID="A84"/>
    <rdf:first rdf:resource="http://w3id.org/arto#Object"/>
  </rdf:Description>
  <rdf:Description rdf:about="http://purl.org/dc/terms/isFormatOf">
    <rdfs:label xml:lang="en">Is Format Of</rdfs:label>
    <rdfs:isDefinedBy rdf:resource="http://purl.org/dc/terms/"/>
    <rdfs:comment xml:lang="en">A pre-existing related resource that is substantially the same as the described resource, but in another format.</rdfs:comment>
    <dc:description xml:lang="en">This property is intended to be used with non-literal values. This property is an inverse property of Has Format.</dc:description>
    <dc:issued rdf:datatype="http://www.w3.org/2001/XMLSchema#date">2000-07-11</dc:issued>
    <rdf:type rdf:resource="http://www.w3.org/2002/07/owl#NamedIndividual"/>
    <rdfs:subPropertyOf rdf:resource="http://purl.org/dc/terms/relation"/>
    <rdfs:subPropertyOf rdf:resource="http://purl.org/dc/elements/1.1/relation"/>
    <rdf:type rdf:resource="http://www.w3.org/2002/07/owl#AnnotationProperty"/>
  </rdf:Description>
  <rdf:Description rdf:about="http://purl.org/dc/terms/MediaTypeOrExtent">
    <rdfs:label xml:lang="en">Media Type or Extent</rdfs:label>
    <rdfs:isDefinedBy rdf:resource="http://purl.org/dc/terms/"/>
    <rdfs:comment xml:lang="en">A media type or extent.</rdfs:comment>
    <dc:issued rdf:datatype="http://www.w3.org/2001/XMLSchema#date">2008-01-14</dc:issued>
    <rdf:type rdf:resource="http://www.w3.org/2002/07/owl#Class"/>
  </rdf:Description>
  <rdf:Description rdf:nodeID="A205">
    <rdf:rest rdf:nodeID="A3"/>
    <rdf:first rdf:resource="http://w3id.org/arto#Scene"/>
  </rdf:Description>
  <rdf:Description rdf:nodeID="A191">
    <owl:allValuesFrom rdf:resource="http://www.w3.org/2001/XMLSchema#string"/>
    <owl:onProperty rdf:resource="http://w3id.org/arto#descriptor"/>
    <rdf:type rdf:resource="http://www.w3.org/2002/07/owl#Restriction"/>
  </rdf:Description>
  <rdf:Description rdf:about="http://purl.org/dc/terms/FileFormat">
    <rdfs:label xml:lang="en">File Format</rdfs:label>
    <rdfs:isDefinedBy rdf:resource="http://purl.org/dc/terms/"/>
    <rdfs:comment xml:lang="en">A digital resource format.</rdfs:comment>
    <dc:issued rdf:datatype="http://www.w3.org/2001/XMLSchema#date">2008-01-14</dc:issued>
    <rdf:type rdf:resource="http://www.w3.org/2002/07/owl#NamedIndividual"/>
    <rdfs:subClassOf rdf:resource="http://purl.org/dc/terms/MediaType"/>
    <rdf:type rdf:resource="http://www.w3.org/2002/07/owl#Class"/>
  </rdf:Description>
  <rdf:Description rdf:nodeID="A108">
    <rdf:rest rdf:nodeID="A48"/>
    <rdf:first>Greyscale</rdf:first>
    <rdf:type rdf:resource="http://www.w3.org/1999/02/22-rdf-syntax-ns#List"/>
  </rdf:Description>
  <rdf:Description rdf:about="http://xmlns.com/foaf/spec/Organization">
    <rdf:type rdf:resource="http://www.w3.org/2002/07/owl#Class"/>
  </rdf:Description>
  <rdf:Description rdf:about="http://purl.org/dc/terms/educationLevel">
    <rdfs:label xml:lang="en">Audience Education Level</rdfs:label>
    <rdfs:isDefinedBy rdf:resource="http://purl.org/dc/terms/"/>
    <rdfs:comment xml:lang="en">A class of agents, defined in terms of progression through an educational or training context, for which the described resource is intended.</rdfs:comment>
    <j.0:rangeIncludes rdf:resource="http://purl.org/dc/terms/AgentClass"/>
    <dc:issued rdf:datatype="http://www.w3.org/2001/XMLSchema#date">2002-07-13</dc:issued>
    <rdf:type rdf:resource="http://www.w3.org/2002/07/owl#NamedIndividual"/>
    <rdfs:subPropertyOf rdf:resource="http://purl.org/dc/terms/audience"/>
    <rdf:type rdf:resource="http://www.w3.org/2002/07/owl#AnnotationProperty"/>
  </rdf:Description>
  <rdf:Description rdf:nodeID="A186">
    <owl:allValuesFrom rdf:resource="http://w3id.org/arto#StyleType"/>
    <owl:onProperty rdf:resource="http://w3id.org/arto#style"/>
    <rdf:type rdf:resource="http://www.w3.org/2002/07/owl#Restriction"/>
  </rdf:Description>
  <rdf:Description rdf:about="http://purl.org/dc/terms/MethodOfInstruction">
    <rdfs:label xml:lang="en">Method of Instruction</rdfs:label>
    <rdfs:isDefinedBy rdf:resource="http://purl.org/dc/terms/"/>
    <rdfs:comment xml:lang="en">A process that is used to engender knowledge, attitudes, and skills.</rdfs:comment>
    <dc:issued rdf:datatype="http://www.w3.org/2001/XMLSchema#date">2008-01-14</dc:issued>
    <rdf:type rdf:resource="http://www.w3.org/2002/07/owl#NamedIndividual"/>
    <rdf:type rdf:resource="http://www.w3.org/2002/07/owl#Class"/>
  </rdf:Description>
  <rdf:Description rdf:about="http://purl.org/dc/terms/RightsStatement">
    <rdfs:label xml:lang="en">Rights Statement</rdfs:label>
    <rdfs:isDefinedBy rdf:resource="http://purl.org/dc/terms/"/>
    <rdfs:comment xml:lang="en">A statement about the intellectual property rights (IPR) held in or over a resource, a legal document giving official permission to do something with a resource, or a statement about access rights.</rdfs:comment>
    <dc:issued rdf:datatype="http://www.w3.org/2001/XMLSchema#date">2008-01-14</dc:issued>
    <rdf:type rdf:resource="http://www.w3.org/2002/07/owl#NamedIndividual"/>
    <rdf:type rdf:resource="http://www.w3.org/2002/07/owl#Class"/>
  </rdf:Description>
  <rdf:Description rdf:nodeID="A217">
    <owl:maxCardinality rdf:datatype="http://www.w3.org/2001/XMLSchema#nonNegativeInteger">1</owl:maxCardinality>
  </rdf:Description>
</rdf:RDF>
