<<<<<<<< HEAD:0.1/arto.rdf
<?xml version="1.0" encoding="UTF-8"?>
<!DOCTYPE rdf:RDF [
  <!ENTITY lcc-cr "https://www.omg.org/spec/LCC/Countries/CountryRepresentation/">
]>
<rdf:RDF xml:base="https://w3id.org/arto"
  xmlns:rdf="http://www.w3.org/1999/02/22-rdf-syntax-ns#"
  xmlns:rdfs="http://www.w3.org/2000/01/rdf-schema#"
  xmlns:ns="http://creativecommons.org/ns#"
  xmlns:owl="http://www.w3.org/2002/07/owl#"
  xmlns:skos="http://www.w3.org/2004/02/skos/core#"
  xmlns:dct="http://purl.org/dc/terms/"
  xmlns:lcc-cr="https://www.omg.org/spec/LCC/Countries/CountryRepresentation/"
  xmlns:arto="http://w3id.org/arto#"
  xmlns:vann="http://purl.org/vocab/vann/"
  xmlns:rdf-star="http://www.w3.org/2019/rdf-star#"
  xmlns:foaf="http://xmlns.com/foaf/0.1/"
  xmlns:dce="http://purl.org/dc/elements/1.1/"
  >

<!-- 
  <owl:Ontology rdf:about="http://w3id.org/arto">
    <owl:imports rdf:resource="http://www.w3.org/2000/01/rdf-schema" />
  </owl:Ontology> -->


  <owl:Ontology rdf:about="https://w3id.org/arto">
        <owl:versionIRI rdf:resource="https://w3id.org/arto/v0.1"/>
        <ns:attributionURL rdf:resource="https://w3id.org/arto"/>
        <dct:description xml:lang="en">The Artwork Object Ontology (ARTO) is a comprehensive ontology designed for describing and contextualizing artworks. It consists of two main components: the Artwork Descriptive Model and the Artwork Contextual Model. ARTO aims to provide a structured and detailed representation of artworks, facilitating tasks such as artwork captioning and information retrieval.</dct:description>
        <dct:issued>2024-04-10</dct:issued>
        <dct:license rdf:resource="https://github.com/SocialMachineLab/ArtworkOntology/blob/main/License"/>
        <dct:rights xml:lang="en">Copyright Â© 2024 Can Yang</dct:rights>
        <dct:title xml:lang="en">Artwork Object Ontology</dct:title>
        <dct:creator xml:lang="en">Can Yang</dct:creator>
        <dct:creator xml:lang="en">Bernardo Pereira Nunes</dct:creator>
        <dct:creator xml:lang="en">Sergio Rodriguez Mendez</dct:creator>
        <vann:preferredNamespacePrefix>arto</vann:preferredNamespacePrefix>
        <vann:preferredNamespacePrefix>https://w3id.org/arto#</vann:preferredNamespacePrefix>
        <rdfs:label xml:lang="en">Artwork Object Ontology</rdfs:label>
        <owl:versionInfo rdf:datatype="http://www.w3.org/2001/XMLSchema#decimal">0.1</owl:versionInfo>
    </owl:Ontology>
    
  <!--
    ///////////////////////////////////////////////////////////////////////////////////////
    //
    // Classes
    //
    ///////////////////////////////////////////////////////////////////////////////////////
     -->
  <owl:Class
    rdf:about="http://w3id.org/arto#Artwork">
    <rdfs:label>Artwork</rdfs:label>
    <rdfs:comment>A created object or piece of art that is intended to be aesthetically pleasing or
      convey a message.</rdfs:comment>
  </owl:Class>

  <owl:Class rdf:about="http://w3id.org/arto#Painting">
    <rdfs:label>Painting</rdfs:label>
    <!-- https://dbpedia.org/ontology/Painting -->
    <rdfs:subClassOf rdf:resource="http://w3id.org/arto#Artwork" />
    <rdfs:comment>A created object or piece of art that is intended to be aesthetically pleasing or
      convey a message.</rdfs:comment>
  </owl:Class>

  <owl:Class rdf:about="http://w3id.org/arto#Series">
    <rdfs:label>Series</rdfs:label>
    <rdfs:comment>A set of artworks.</rdfs:comment>
    <!-- <owl:equivalentClass rdf:resource="https://schema.org/Series" /> -->
  </owl:Class>


  <owl:Class
    rdf:about="http://w3id.org/arto#Artist">
    <rdfs:label>Artist</rdfs:label>
    <!-- https://dbpedia.org/ontology/Artist -->
    <rdfs:comment>The person or group who create or contribute the artwork.</rdfs:comment>
    <rdfs:subClassOf rdf:resource="http://xmlns.com/foaf/0.1/Person" />
  </owl:Class>

  <owl:Class
    rdf:about="http://w3id.org/arto#Sponsor">
    <rdfs:label>Sponsor</rdfs:label>
    <!-- https://saidfathalla.github.io/SEOontology/Documentation/#Sponsor -->
    <rdfs:comment>The person or group who sponsor the artwork.</rdfs:comment>
    <rdfs:subClassOf rdf:resource="http://xmlns.com/foaf/0.1/Person" />
  </owl:Class>

  <owl:Class
    rdf:about="http://w3id.org/arto#Character">
    <rdfs:label>Character</rdfs:label>
    <!-- https://dbpedia.org/ontology/FictionalCharacter -->
    <rdfs:comment>The person or group appeared in the artwork.</rdfs:comment>
    <rdfs:subClassOf rdf:resource="http://xmlns.com/foaf/0.1/Person" />
  </owl:Class>


  <owl:Class
    rdf:about="http://purl.org/dc/terms/Location">
    <rdfs:label>Location</rdfs:label>
    <rdfs:comment>The Location.</rdfs:comment>
  </owl:Class>

  <owl:Class
    rdf:about="https://www.w3.org/TR/owl-time/#time:TemporalEntity">
    <rdfs:label>Time</rdfs:label>
    <rdfs:comment>A temporal interval or instant.</rdfs:comment>
  </owl:Class>

  <owl:Class
    rdf:about="https://www.w3.org/TR/owl-time/#time:Instant">
    <rdfs:label>Instant</rdfs:label>
    <rdfs:comment>A temporal entity with zero extent or duration</rdfs:comment>
    <rdfs:subClassOf rdf:resource="https://www.w3.org/TR/owl-time/#time:TemporalEntity" />
  </owl:Class>


  <owl:Class
    rdf:about="https://www.w3.org/TR/owl-time/#time:Interval">
    <rdfs:label>Interval</rdfs:label>
    <rdfs:comment>A temporal entity with an extent or duration</rdfs:comment>
    <rdfs:subClassOf rdf:resource="https://www.w3.org/TR/owl-time/#time:TemporalEntity" />
  </owl:Class>


  <owl:Class
    rdf:about="http://purl.org/NET/c4dm/event.owl#Event">
    <rdfs:label>Event</rdfs:label>
    <rdfs:comment>
      An arbitrary classification of a space/time region, by a
      cognitive agent. An event may have actively participating agents,
      passive factors, products, and a location in space/time.</rdfs:comment>
  </owl:Class>

  <owl:Class
    rdf:about="http://xmlns.com/foaf/0.1/Agent">
    <rdfs:label>Agent</rdfs:label>
    <rdfs:comment>Represents an Agent.This class comprises people, either individually or in groups,
      who have the potential to perform intentional actions for which they can be held responsible.</rdfs:comment>
  </owl:Class>


  <owl:Class
    rdf:about="http://xmlns.com/foaf/0.1/Organization">
    <rdfs:label>Organization</rdfs:label>
    <rdfs:comment>The Organization class represents a kind of Agent corresponding to instititutions
      such as galleries, museums etc.</rdfs:comment>
    <rdfs:subClassOf rdf:resource="http://xmlns.com/foaf/0.1/Agent" />
    <owl:disjointWith rdf:resource="http://xmlns.com/foaf/0.1/Person" />
  </owl:Class>


  <owl:Class
    rdf:about="http://xmlns.com/foaf/0.1/Person">
    <rdfs:label>Person</rdfs:label>
    <rdfs:comment>Represents a person associated with an artwork.</rdfs:comment>
    <rdfs:subClassOf rdf:resource="http://xmlns.com/foaf/0.1/Agent" />
  </owl:Class>


  <owl:Class
    rdf:about="http://w3id.org/arto#Element">
    <rdfs:label>Element</rdfs:label>
    <rdfs:comment>Represents the visual element associated with an artwork.</rdfs:comment>
  </owl:Class>


  <owl:Class
    rdf:about="http://w3id.org/arto#Color">
    <rdfs:label>Color</rdfs:label>
    <rdfs:comment>Represents the color used in an artwork.</rdfs:comment>
    <rdfs:subClassOf rdf:resource="http://w3id.org/arto#Element" />
  </owl:Class>


  <owl:Class
    rdf:about="http://w3id.org/arto#Line">
    <rdfs:label>Line</rdfs:label>
    <rdfs:comment>Represents the line used in an artwork.</rdfs:comment>
    <rdfs:subClassOf rdf:resource="http://w3id.org/arto#Element" />
  </owl:Class>


  <owl:Class
    rdf:about="http://w3id.org/arto#Space">
    <rdfs:label>Space</rdfs:label>
    <rdfs:comment>Represents the space used in an artwork.</rdfs:comment>
    <rdfs:subClassOf rdf:resource="http://w3id.org/arto#Element" />
  </owl:Class>

  <owl:Class
    rdf:about="http://w3id.org/arto#Composition">
    <rdfs:label>Composition</rdfs:label>
    <rdfs:comment>Represents the composition used in an artwork.</rdfs:comment>
    <rdfs:subClassOf rdf:resource="http://w3id.org/arto#Element" />
  </owl:Class>

  <owl:Class
    rdf:about="http://w3id.org/arto#Object">
    <rdfs:label>Object</rdfs:label>
    <rdfs:comment>Represents the physical or conceptual object within an artwork.</rdfs:comment>
  </owl:Class>


  <owl:Class
    rdf:about="http://w3id.org/arto#Scene">
    <rdfs:label>Scene</rdfs:label>
    <rdfs:comment>A scene can be viewed as a portion of the artwork composed of a group of objects
      that convey a specific meaning or sentiment.</rdfs:comment>
  </owl:Class>


  <owl:Class
    rdf:about="http://w3id.org/arto#Connotation">
    <rdfs:label>Cnnotation</rdfs:label>
    <rdfs:comment>Represents the interpretations of artwork, includeing themes, meanings, and
      emotions conveyed by an artwork.</rdfs:comment>
  </owl:Class>


  <owl:Class
    rdf:about="http://w3id.org/arto#Meaning">
    <rdfs:label>Meaning</rdfs:label>
    <rdfs:comment>Represents the underlying message, symbolism, or significance conveyed by an
      artwork.</rdfs:comment>
    <rdfs:subClassOf rdf:resource="http://w3id.org/arto#Connotation" />
  </owl:Class>


  <owl:Class
    rdf:about="http://w3id.org/arto#Emotion">
    <rdfs:label>Emotion</rdfs:label>
    <rdfs:comment>Represents the emotional response or affective state evoked by an artwork in the
      artist or viewers, such as joy, sadness, anger, or fear.</rdfs:comment>
    <rdfs:subClassOf rdf:resource="http://w3id.org/arto#Connotation" />
  </owl:Class>


  <owl:Class
    rdf:about="http://w3id.org/arto#Theme">
    <rdfs:label>Theme</rdfs:label>
    <rdfs:comment>Represents a central idea, subject, or concept explored in an artwork, which can
      be explicit or implicit, and may reflect broader cultural, social, or political issues.</rdfs:comment>
    <rdfs:subClassOf rdf:resource="http://w3id.org/arto#Connotation" />
  </owl:Class>

  <owl:Class
    rdf:about="http://w3id.org/arto#Metric">
    <rdfs:label>Metric</rdfs:label>
    <rdfs:comment>Represents a quantifiable measurement or characteristic of an artwork,
      encompassing statistical information about basic elements such as color statistics, emotion
      intensity, balance of composition, and other visual elements, to facilitate structural
      analysis
      and comparison of artworks.</rdfs:comment>
  </owl:Class>

  <owl:Class
    rdf:about="http://w3id.org/arto#MainColor">
    <rdfs:label>MainColor</rdfs:label>
    <rdfs:comment>Represents the dominant or most prominent color in an artwork, which can be
      determined through visual analysis or color quantization techniques.</rdfs:comment>
    <rdfs:subClassOf rdf:resource="http://w3id.org/arto#Metric" />
  </owl:Class>


  <owl:Class
    rdf:about="http://w3id.org/arto#ColorHistogram">
    <rdfs:label>ColorHistogram</rdfs:label>
    <rdfs:comment>Represents the distribution of colors in an artwork, typically expressed as a
      histogram or a quantitative representation of the frequency or proportion of each color
      present in
      the artwork.</rdfs:comment>
    <rdfs:subClassOf rdf:resource="http://w3id.org/arto#Metric" />
  </owl:Class>

  <owl:Class
    rdf:about="http://w3id.org/arto#Relevance">
    <rdfs:label>Relevance</rdfs:label>
    <rdfs:comment>Represents the degree to which a particular element or aspect of an artwork is
      related to its overall theme or meaning.</rdfs:comment>
    <rdfs:subClassOf rdf:resource="http://w3id.org/arto#Metric" />
  </owl:Class>

  <owl:Class
    rdf:about="http://w3id.org/arto#EmotionIntensity">
    <rdfs:label>EmotionIntensity</rdfs:label>
    <rdfs:comment>Represents the strength or degree of emotional response evoked by an artwork.</rdfs:comment>
    <rdfs:subClassOf rdf:resource="http://w3id.org/arto#Metric" />
  </owl:Class>

  <owl:Class
    rdf:about="http://w3id.org/arto#BalanceOfComposition">
    <rdfs:label>BalanceOfComposition</rdfs:label>
    <rdfs:comment>Represents the degree of visual equilibrium or harmony in the arrangement of
      elements within an artwork, considering factors such as symmetry, asymmetry, and distribution
      of
      visual elements.</rdfs:comment>
    <rdfs:subClassOf rdf:resource="http://w3id.org/arto#Metric" />
  </owl:Class>
  <!--
    ///////////////////////////////////////////////////////////////////////////////////////
    //
    // Object properties
    //
    ///////////////////////////////////////////////////////////////////////////////////////
     -->

  <owl:ObjectProperty
    rdf:about="https://motools.sourceforge.net/event/event.html#time">
    <rdfs:label>hasTime</rdfs:label>
    <rdfs:comment>Relates the event to the date. Could be a time interval or a time point</rdfs:comment>
    <rdfs:domain>
      <owl:Class>
        <owl:unionOf rdf:parseType="Collection">
          <rdf:Description rdf:about="http://purl.org/NET/c4dm/event.owl#Event" />
          <rdf:Description rdf:about="http://purl.org/dc/terms/Location" />
        </owl:unionOf>
      </owl:Class>
    </rdfs:domain>
    <rdfs:range rdf:resource="https://www.w3.org/TR/owl-time/#time:TemporalEntity" />
  </owl:ObjectProperty>


  <owl:ObjectProperty
    rdf:about="http://www.europeana.eu/schemas/edm/happenedAt">
    <rdfs:label>hasLocation</rdfs:label>
    <rdfs:comment>Relates the event or provenance to the location where it happened.</rdfs:comment>
    <rdfs:domain rdf:resource="http://purl.org/NET/c4dm/event.owl#Event" />
    <rdfs:range rdf:resource="http://purl.org/dc/terms/Location" />
  </owl:ObjectProperty>

  <owl:ObjectProperty
    rdf:about="https://dbpedia.org/ontology/residence">
    <rdfs:label>residence</rdfs:label>
    <rdfs:comment>Relates a person to the location they lived in.</rdfs:comment>
    <rdfs:domain rdf:resource="http://xmlns.com/foaf/0.1/Person" />
    <rdfs:range rdf:resource="http://purl.org/dc/terms/Location" />
  </owl:ObjectProperty>


  <owl:ObjectProperty
    rdf:about="http://purl.org/dc/terms/created">
    <rdfs:label>created</rdfs:label>
    <rdfs:comment>Relates an artwork to its creation date.</rdfs:comment>
    <rdfs:domain rdf:resource="http://w3id.org/arto#Artwork" />
    <rdfs:range rdf:resource="https://www.w3.org/TR/owl-time/#time:TemporalEntity" />
  </owl:ObjectProperty>


  <owl:ObjectProperty
    rdf:about="https://www.geonames.org/ontology#locatedIn">
    <rdfs:label>locatedIn</rdfs:label>
    <rdfs:comment>It . available options are: country, state, city, district,
      street, building etc. </rdfs:comment>
    <rdfs:comment>Indicates the location where an organization is situated.</rdfs:comment>

    <rdfs:domain rdf:resource="http://xmlns.com/foaf/0.1/Organization" />
    <!-- <rdfs:domain rdf:resource="http://purl.org/dc/terms/Location"/> -->
    <rdfs:range rdf:resource="http://purl.org/dc/terms/Location" />
  </owl:ObjectProperty>


  <owl:ObjectProperty
    rdf:about="http://purl.org/dc/terms/isPartOf">
    <rdfs:label>isPartOf</rdfs:label>
    <rdfs:comment>Relates an artwork to the serie of the artwork.</rdfs:comment>
    <rdfs:domain rdf:resource="http://w3id.org/arto#Artwork" />
    <rdfs:range rdf:resource="http://w3id.org/arto#Series" />
  </owl:ObjectProperty>

  <owl:ObjectProperty
    rdf:about="http://www.europeana.eu/schemas/edm/currentLocation">
    <rdfs:label>currentLocation</rdfs:label>
    <rdfs:comment>Relates an artwork to its current physical location.</rdfs:comment>
    <rdfs:domain rdf:resource="http://w3id.org/arto#Artwork" />
    <rdfs:range rdf:resource="http://purl.org/dc/terms/Location" />
  </owl:ObjectProperty>


  <owl:ObjectProperty
    rdf:about="http://w3id.org/arto#relatedToEvent">
    <rdfs:label>relatedToEvent</rdfs:label>
    <rdfs:comment>Relates an artwork to an event included in the artwork.</rdfs:comment>
    <rdfs:domain>
      <owl:Class>
        <owl:unionOf rdf:parseType="Collection">
          <rdf:Description rdf:about="http://w3id.org/arto#Artwork" />
          <rdf:Description rdf:about="http://w3id.org/arto#Connotation" />
        </owl:unionOf>
      </owl:Class>
    </rdfs:domain>
    <rdfs:range rdf:resource="http://purl.org/NET/c4dm/event.owl#Event" />
  </owl:ObjectProperty>


  <owl:ObjectProperty
    rdf:about="http://w3id.org/arto#hasEvent">
    <rdfs:label>hasEvent</rdfs:label>
    <rdfs:comment>Relates an artwork to an event happened to this artwork.</rdfs:comment>
    <rdfs:domain rdf:resource="http://w3id.org/arto#Artwork" />
    <rdfs:range rdf:resource="http://purl.org/NET/c4dm/event.owl#Event" />
  </owl:ObjectProperty>

  <owl:ObjectProperty
    rdf:about="http://purl.org/dc/elements/1.1/creator">
    <rdfs:label>creator</rdfs:label>
    <rdfs:comment>Relates an artwork to the artist(s) who created or contributed to it.</rdfs:comment>
    <!-- <rdfs:domain rdf:resource="http://example.com/artwork#Artwork"/>
    <rdfs:domain rdf:resource="https://schema.org/Series"/> -->
    <rdfs:domain>
      <owl:Class>
        <owl:unionOf rdf:parseType="Collection">
          <rdf:Description rdf:about="http://w3id.org/arto#Artwork" />
          <rdf:Description rdf:about="http://w3id.org/arto#Series" />
        </owl:unionOf>
      </owl:Class>
    </rdfs:domain>
    <rdfs:range rdf:resource="http://w3id.org/arto#Artist" />
  </owl:ObjectProperty>

  <owl:ObjectProperty
    rdf:about="http://purl.org/NET/c4dm/event.owl#agent">
    <rdfs:label>agent</rdfs:label>
    <rdfs:comment>Relates an artwork or event to a agent associated with it.</rdfs:comment>
    <rdfs:domain rdf:resource="http://purl.org/NET/c4dm/event.owl#Event" />
    <rdfs:range rdf:resource="http://xmlns.com/foaf/0.1/Agent" />
  </owl:ObjectProperty>


  <owl:ObjectProperty
    rdf:about="http://purl.org/dc/terms/contributor">
    <rdfs:label>contributor</rdfs:label>
    <rdfs:comment>The Contributor of the Artwork.</rdfs:comment>
    <rdfs:domain rdf:resource="http://w3id.org/arto#Artwork" />
    <rdfs:range rdf:resource="http://xmlns.com/foaf/0.1/Person" />
  </owl:ObjectProperty>


  <owl:ObjectProperty
    rdf:about="http://xmlns.com/foaf/0.1/knows">
    <rdfs:label>knows</rdfs:label>
    <rdfs:comment>The person knows persons.</rdfs:comment>
    <rdfs:domain rdf:resource="http://xmlns.com/foaf/0.1/Person" />
    <rdfs:range rdf:resource="http://xmlns.com/foaf/0.1/Person" />
  </owl:ObjectProperty>

  <!-- <owl:ObjectProperty
    rdf:about="http://w3id.org/arto#contain">
    <rdfs:label>contain</rdfs:label>
    <rdfs:comment>It could contains any objects.</rdfs:comment>
    <rdfs:domain rdf:resource="http://w3id.org/arto#Artwork" />
    <rdfs:range rdf:resource="http://www.w3.org/2002/07/owl#Thing" />
  </owl:ObjectProperty> -->


  <owl:ObjectProperty
    rdf:about="http://w3id.org/arto#relatedTo">
    <!-- http://www.ontologydesignpatterns.org/ont/dul/DUL.owl#isSettingFor -->
    <rdfs:label>relatedTo</rdfs:label>
    <rdfs:comment>The Objects could related to Objects.</rdfs:comment>
    <rdfs:domain rdf:resource="http://w3id.org/arto#Object" />
    <rdfs:range rdf:resource="http://w3id.org/arto#Object" />
  </owl:ObjectProperty>

  <owl:ObjectProperty
    rdf:about="http://w3id.org/arto#containsElements">
    <!-- http://www.ontologydesignpatterns.org/ont/dul/DUL.owl#isSettingFor -->
    <rdfs:label>containsElements</rdfs:label>
    <rdfs:comment>The objects contains elements.</rdfs:comment>
    <rdfs:domain rdf:resource="http://w3id.org/arto#Object" />
    <rdfs:range rdf:resource="http://w3id.org/arto#Element" />
  </owl:ObjectProperty>

  <owl:ObjectProperty
    rdf:about="http://w3id.org/arto#containsObjects">
    <!-- http://www.ontologydesignpatterns.org/ont/dul/DUL.owl#isSettingFor -->
    <rdfs:label>containsObjects</rdfs:label>
    <rdfs:comment>The Scene contains Objects.</rdfs:comment>
    <rdfs:domain rdf:resource="http://w3id.org/arto#Scene" />
    <rdfs:range rdf:resource="http://w3id.org/arto#Object" />
  </owl:ObjectProperty>


  <owl:ObjectProperty
    rdf:about="http://w3id.org/arto#relatedToScene">
    <!-- http://www.ontologydesignpatterns.org/ont/dul/DUL.owl#isSettingFor -->
    <rdfs:label>relatedToSecne</rdfs:label>
    <rdfs:comment>The Scenes that objects related.</rdfs:comment>
    <rdfs:range rdf:resource="http://w3id.org/arto#Scene" />
    <rdfs:domain rdf:resource="http://w3id.org/arto#Object" />
  </owl:ObjectProperty>

  <owl:ObjectProperty
    rdf:about="http://w3id.org/arto#hasConnotation">
    <!-- http://www.ontologydesignpatterns.org/ont/dul/DUL.owl#isSettingFor -->
    <rdfs:label>hasConnotation</rdfs:label>
    <rdfs:comment>Relate artwork and the connotations.</rdfs:comment>
    <rdfs:range rdf:resource="http://w3id.org/arto#Connotation" />
    <rdfs:domain rdf:resource="http://w3id.org/arto#Artwork" />
  </owl:ObjectProperty>

  <!-- <owl:ObjectProperty
  rdf:about="http://w3id.org/arto#relatedToEvent">
  <rdfs:label>relatedToEvent</rdfs:label>
  <rdfs:comment>Relate Event and the connotations.</rdfs:comment>
  <rdfs:range rdf:resource="http://w3id.org/arto#Connotation" />
  <rdfs:domain rdf:resource="http://purl.org/NET/c4dm/event.owl#Event" />
</owl:ObjectProperty> -->

  <owl:ObjectProperty
    rdf:about="http://w3id.org/arto#containsScenes">
    <!-- http://www.ontologydesignpatterns.org/ont/dul/DUL.owl#isSettingFor -->
    <rdfs:label>containsObjects</rdfs:label>
    <rdfs:comment>The Artwork and Scene could contains Scenes.</rdfs:comment>
    <rdfs:domain>
      <owl:Class>
        <owl:unionOf rdf:parseType="Collection">
          <rdf:Description rdf:about="http://w3id.org/arto#Artwork" />
          <rdf:Description rdf:about="http://w3id.org/arto#Scene" />
        </owl:unionOf>
      </owl:Class>
    </rdfs:domain>
    <rdfs:range rdf:resource="http://w3id.org/arto#Scene" />
  </owl:ObjectProperty>


  <owl:ObjectProperty
    rdf:about="http://w3id.org/arto#hasMetric">
    <rdfs:label>hasMetric</rdfs:label>
    <rdfs:comment>The metric of the connotation, scene, Object or the element in the artwork.</rdfs:comment>
    <rdfs:domain>
      <owl:Class>
        <owl:unionOf rdf:parseType="Collection">
          <rdf:Description rdf:about="http://w3id.org/arto#Connotation" />
          <rdf:Description rdf:about="http://w3id.org/arto#Element" />
          <rdf:Description rdf:about="http://w3id.org/arto#Scene" />
          <rdf:Description rdf:about="http://w3id.org/arto#Object" />
        </owl:unionOf>
      </owl:Class>
    </rdfs:domain>
    <rdfs:range rdf:resource="http://w3id.org/arto#Metric" />
  </owl:ObjectProperty>

  <owl:ObjectProperty
    rdf:about="http://w3id.org/arto#express">
    <rdfs:label>express</rdfs:label>
    <rdfs:comment>The connotation expressed in the Scenes or the Objects or Elements in the artwork.</rdfs:comment>
    <rdfs:domain>
      <owl:Class>
        <owl:unionOf rdf:parseType="Collection">
          <rdf:Description rdf:about="http://w3id.org/arto#Element" />
          <rdf:Description rdf:about="http://w3id.org/arto#Scene" />
          <rdf:Description rdf:about="http://w3id.org/arto#Object" />
        </owl:unionOf>
      </owl:Class>
    </rdfs:domain>
    <rdfs:range rdf:resource="http://w3id.org/arto#Connotation" />
  </owl:ObjectProperty>

  <!--
    ///////////////////////////////////////////////////////////////////////////////////////
    //
    // Datatype properties
    //
    ///////////////////////////////////////////////////////////////////////////////////////
     -->


  <owl:DatatypeProperty
    rdf:about="http://w3id.org/arto#source">
    <rdfs:label>source</rdfs:label>
    <rdfs:comment>Relates the source of the meaning in artworks.</rdfs:comment>
    <rdfs:domain rdf:resource="http://w3id.org/arto#Meaning" />
    <rdfs:range rdf:resource="http://www.w3.org/2001/XMLSchema#string" />
  </owl:DatatypeProperty>

  <owl:DatatypeProperty
    rdf:about="http://w3id.org/arto#emotionType">
    <rdfs:label>emotionType</rdfs:label>
    <rdfs:comment>Point out the emotion type.</rdfs:comment>
    <rdfs:domain rdf:resource="http://w3id.org/arto#Emotion" />
    <rdfs:range rdf:resource="http://www.w3.org/2001/XMLSchema#string" />
  </owl:DatatypeProperty>

  <owl:DatatypeProperty
    rdf:about="http://w3id.org/arto#coordinates">
    <rdfs:label>coordinates</rdfs:label>
    <rdfs:comment>The coordinates of the Scene or the Object in the artwork.</rdfs:comment>
    <rdfs:domain>
      <owl:Class>
        <owl:unionOf rdf:parseType="Collection">
          <rdf:Description rdf:about="http://w3id.org/arto#Scene" />
          <rdf:Description rdf:about="http://w3id.org/arto#Object" />
        </owl:unionOf>
      </owl:Class>
    </rdfs:domain>
    <rdfs:range rdf:resource="http://www.w3.org/2001/XMLSchema#string" />
  </owl:DatatypeProperty>


  <owl:DatatypeProperty
    rdf:about="http://w3id.org/arto#size">
    <rdfs:label>size</rdfs:label>
    <rdfs:comment>The size of the Scene or the Object in the artwork.</rdfs:comment>
    <rdfs:domain>
      <owl:Class>
        <owl:unionOf rdf:parseType="Collection">
          <rdf:Description rdf:about="http://w3id.org/arto#Scene" />
          <rdf:Description rdf:about="http://w3id.org/arto#Object" />
        </owl:unionOf>
      </owl:Class>
    </rdfs:domain>
    <rdfs:range rdf:resource="http://www.w3.org/2001/XMLSchema#string" />
  </owl:DatatypeProperty>


  <owl:DatatypeProperty
    rdf:about="http://w3id.org/arto#material">
    <rdfs:label>material</rdfs:label>
    <rdfs:comment>The material of the Object.</rdfs:comment>
    <rdfs:domain rdf:resource="http://w3id.org/arto#Object" />
    <rdfs:range rdf:resource="http://www.w3.org/2001/XMLSchema#string" />
  </owl:DatatypeProperty>

  <owl:DatatypeProperty
    rdf:about="http://w3id.org/arto#hasState">
    <rdfs:label>hasState</rdfs:label>
    <rdfs:comment>The state of the Object.</rdfs:comment>
    <rdfs:domain rdf:resource="http://w3id.org/arto#Object" />
    <rdfs:range rdf:resource="http://www.w3.org/2001/XMLSchema#string" />
  </owl:DatatypeProperty>


  <owl:DatatypeProperty
    rdf:about="http://w3id.org/arto#RGBValue">
    <rdfs:label>RGBValue</rdfs:label>
    <rdfs:comment>The RGBValue of the Color.</rdfs:comment>
    <rdfs:domain rdf:resource="http://w3id.org/arto#Color" />
    <rdfs:range rdf:resource="http://www.w3.org/2001/XMLSchema#int" />
  </owl:DatatypeProperty>

  <owl:DatatypeProperty
    rdf:about="http://w3id.org/arto#HSVValue">
    <rdfs:label>HSVValue</rdfs:label>
    <rdfs:comment>The HSVValue of the Color.</rdfs:comment>
    <rdfs:domain rdf:resource="http://w3id.org/arto#Color" />
    <rdfs:range rdf:resource="http://www.w3.org/2001/XMLSchema#int" />
  </owl:DatatypeProperty>

  <owl:DatatypeProperty
    rdf:about="http://w3id.org/arto#length">
    <rdfs:label>length</rdfs:label>
    <rdfs:comment>The length of the line.</rdfs:comment>
    <rdfs:domain rdf:resource="http://w3id.org/arto#Line" />
    <rdfs:range rdf:resource="http://www.w3.org/2001/XMLSchema#float" />
  </owl:DatatypeProperty>

  <!-- <owl:DatatypeProperty
    rdf:about="http://w3id.org/arto#width">
    <rdfs:label>width</rdfs:label>
    <rdfs:comment>The width of the line.</rdfs:comment>
    <rdfs:domain rdf:resource="http://w3id.org/arto#Line" />
    <rdfs:range rdf:resource="http://www.w3.org/2001/XMLSchema#float" />
  </owl:DatatypeProperty> -->


  <owl:DatatypeProperty
    rdf:about="http://w3id.org/arto#lineType">
    <rdfs:label>lineType</rdfs:label>
    <rdfs:comment>The type of the line.</rdfs:comment>
    <rdfs:domain rdf:resource="http://w3id.org/arto#Line" />
    <rdfs:range rdf:resource="http://www.w3.org/2001/XMLSchema#float" />
  </owl:DatatypeProperty>


  <owl:DatatypeProperty
    rdf:about="http://w3id.org/arto#direction">
    <rdfs:label>direction</rdfs:label>
    <rdfs:comment>The direction of the line.</rdfs:comment>
    <rdfs:domain rdf:resource="http://w3id.org/arto#Line" />
    <rdfs:range rdf:resource="http://www.w3.org/2001/XMLSchema#string" />
  </owl:DatatypeProperty>

  <owl:DatatypeProperty
    rdf:about="http://w3id.org/arto#spaceType">
    <rdfs:label>spaceType</rdfs:label>
    <rdfs:comment>The type of the space.</rdfs:comment>
    <rdfs:domain rdf:resource="http://w3id.org/arto#Space" />
    <rdfs:range rdf:resource="http://www.w3.org/2001/XMLSchema#float" />
  </owl:DatatypeProperty>


  <owl:DatatypeProperty
    rdf:about="http://w3id.org/arto#compositionType">
    <rdfs:label>compositionType</rdfs:label>
    <rdfs:comment>The type of the composition.</rdfs:comment>
    <rdfs:domain rdf:resource="http://w3id.org/arto#Composition" />
    <rdfs:range rdf:resource="http://www.w3.org/2001/XMLSchema#float" />
  </owl:DatatypeProperty>


  <owl:DatatypeProperty
    rdf:about="http://www.europeana.eu/schemas/edm/isShownBy">

    <rdfs:label>imageResource</rdfs:label>
    <rdfs:comment>An unambiguous URI reference to the digital object on the provider's web site in
      the best available resolution/quality. </rdfs:comment>
    <rdfs:domain rdf:resource="http://w3id.org/arto#Artwork" />
    <rdfs:range rdf:resource="http://www.w3.org/2001/XMLSchema#string" />
  </owl:DatatypeProperty>


  <owl:DatatypeProperty
    rdf:about="http://purl.org/dc/terms/description">
    <rdfs:label>description</rdfs:label>
    <rdfs:comment>Relates an artwork to its description.</rdfs:comment>
    <rdfs:domain rdf:resource="http://w3id.org/arto#Artwork" />
    <rdfs:range rdf:resource="http://www.w3.org/2001/XMLSchema#string" />
  </owl:DatatypeProperty>


  <owl:DatatypeProperty
    rdf:about="http://purl.org/dc/elements/1.1/title">
    <rdfs:label>title</rdfs:label>
    <rdfs:comment>Relates an artwork to its title.</rdfs:comment>
    <rdfs:domain rdf:resource="http://w3id.org/arto#Artwork" />
    <rdfs:range rdf:resource="http://www.w3.org/2001/XMLSchema#string" />
  </owl:DatatypeProperty>

  <owl:DatatypeProperty
    rdf:about="https://dbpedia.org/property/style">
    <rdfs:label>style</rdfs:label>
    <rdfs:comment>Relates an artwork to its artistic style or movement.</rdfs:comment>
    <rdfs:domain rdf:resource="http://w3id.org/arto#Artwork" />
    <rdfs:range rdf:resource="http://www.w3.org/2001/XMLSchema#string" />
  </owl:DatatypeProperty>

  <owl:DatatypeProperty
    rdf:about="https://schema.org/genre">
    <rdfs:label>genre</rdfs:label>
    <rdfs:comment>Relates an artwork to its genre.</rdfs:comment>
    <rdfs:domain rdf:resource="http://w3id.org/arto#Artwork" />
    <rdfs:range rdf:resource="http://www.w3.org/2001/XMLSchema#string" />
  </owl:DatatypeProperty>

  <owl:DatatypeProperty
    rdf:about="http://w3id.org/arto#timeType">
    <rdfs:label>timeType</rdfs:label>
    <rdfs:comment>The type of the time entity.</rdfs:comment>
    <rdfs:domain rdf:resource="https://www.w3.org/TR/owl-time/#time:TemporalEntity" />
    <rdfs:range rdf:resource="http://www.w3.org/2001/XMLSchema#string" />
  </owl:DatatypeProperty>


  <owl:DatatypeProperty
    rdf:about="http://purl.org/dc/terms/medium">
    <rdfs:label>medium</rdfs:label>
    <rdfs:comment>Relates an artwork to the medium(s) used in creating it.</rdfs:comment>
    <rdfs:domain rdf:resource="http://w3id.org/arto#Artwork" />
    <!-- <rdfs:range rdf:resource="http://purl.org/dc/terms/PhysicalMedium"/> -->
    <rdfs:range rdf:resource="http://www.w3.org/2001/XMLSchema#string" />
  </owl:DatatypeProperty>


  <owl:DatatypeProperty
    rdf:about="https://semanticweb.cs.vu.nl/2009/11/sem/semdoc.html#sem:eventType">
    <!-- https://dbpedia.org/ontology/type -->
    <rdfs:label>eventType</rdfs:label>
    <rdfs:comment> the type of the event</rdfs:comment>
    <rdfs:domain rdf:resource="http://purl.org/NET/c4dm/event.owl#Event" />
    <!-- <rdfs:range rdf:resource="https://www.w3.org/TR/owl-time/#time:"/> -->
    <rdfs:range rdf:resource="http://www.w3.org/2001/XMLSchema#string" />
  </owl:DatatypeProperty>


  <owl:DatatypeProperty
    rdf:about="http://www.ebu.ch/metadata/ontologies/ebucore/ebucore#height">
    <rdfs:label>height</rdfs:label>
    <rdfs:comment>Relates an artwork to its physical height.</rdfs:comment>
    <rdfs:domain rdf:resource="http://w3id.org/arto#Artwork" />

    <rdfs:range rdf:resource="http://www.w3.org/2001/XMLSchema#string" />
  </owl:DatatypeProperty>

  <owl:DatatypeProperty
    rdf:about="http://www.ebu.ch/metadata/ontologies/ebucore/ebucore#width">
    <rdfs:label>width</rdfs:label>
    <rdfs:comment>Relates an artwork to its physical width.</rdfs:comment>
    <rdfs:domain>
      <owl:Class>
        <owl:unionOf rdf:parseType="Collection">
          <rdf:Description rdf:about="http://w3id.org/arto#Artwork" />
          <rdf:Description rdf:about="http://w3id.org/arto#Line" />
        </owl:unionOf>
      </owl:Class>
    </rdfs:domain>
    <!-- <rdfs:domain rdf:resource="http://w3id.org/arto#Artwork" /> -->
    <rdfs:range rdf:resource="http://www.w3.org/2001/XMLSchema#string" />
  </owl:DatatypeProperty>


  <owl:DatatypeProperty
    rdf:about="https://dbpedia.org/ontology/nationality">
    <rdfs:label>nationality</rdfs:label>
    <rdfs:comment>Relates an person to the Nationality.</rdfs:comment>
    <rdfs:domain rdf:resource="http://xmlns.com/foaf/0.1/Person" />
    <!-- <rdfs:range rdf:resource="http://xmlns.com/foaf/0.1/Person"/> -->
    <rdfs:range rdf:resource="http://www.w3.org/2001/XMLSchema#string" />

  </owl:DatatypeProperty>


  <!-- <owl:DatatypeProperty
    rdf:about="http://www.europeana.eu/schemas/edm/componentColor">
    <rdfs:label>componentColor</rdfs:label>
    <rdfs:comment>The component Color of the Artwork.</rdfs:comment>
    <rdfs:domain rdf:resource="http://w3id.org/arto#Artwork" />
    <rdfs:range rdf:resource="http://www.w3.org/2001/XMLSchema#string" />
  </owl:DatatypeProperty> -->


  <!-- <owl:DatatypeProperty
    rdf:about="http://www.europeana.eu/schemas/edm/hasColorSpace">
    <rdfs:label>hasColorSpace</rdfs:label>
    <rdfs:comment>The Color Space of the Artwork.</rdfs:comment>
    <rdfs:domain rdf:resource="http://w3id.org/arto#Artwork" />
    <rdfs:range rdf:resource="http://www.w3.org/2001/XMLSchema#string" />
  </owl:DatatypeProperty> -->


  <owl:DatatypeProperty
    rdf:about="http://purl.org/dc/elements/1.1/format">
    <rdfs:label>format</rdfs:label>
    <rdfs:comment>The F gormat of the Artwork.</rdfs:comment>
    <rdfs:domain rdf:resource="http://w3id.org/arto#Artwork" />
    <rdfs:range rdf:resource="http://www.w3.org/2001/XMLSchema#string" />
  </owl:DatatypeProperty>


  <owl:DatatypeProperty
    rdf:about="http://www.w3.org/2003/01/geo/wgs84_pos#long">
    <rdfs:domain rdf:resource="http://purl.org/dc/terms/Location" />
    <rdfs:label>longitude</rdfs:label>
    <rdfs:comment>The WGS84 longitude of a SpatialThing (decimal degrees).</rdfs:comment>
    <rdfs:range rdf:resource="http://www.w3.org/2001/XMLSchema#string" />
  </owl:DatatypeProperty>

  <owl:DatatypeProperty
    rdf:about="http://www.w3.org/2003/01/geo/wgs84_pos#lat">
    <rdfs:domain rdf:resource="http://purl.org/dc/terms/Location" />
    <rdfs:label>latitude</rdfs:label>
    <rdfs:comment>The WGS84 latitude of a SpatialThing (decimal degrees).</rdfs:comment>
    <rdfs:range rdf:resource="http://www.w3.org/2001/XMLSchema#string" />
  </owl:DatatypeProperty>

  <owl:DatatypeProperty
    rdf:about="http://purl.org/dc/terms/locationType">
    <!-- https://dbpedia.org/ontology/regionType -->
    <rdfs:domain rdf:resource="http://purl.org/dc/terms/Location" />
    <rdfs:label>locationType</rdfs:label>
    <rdfs:comment>The type of the location. available options are: country, state, city, district,
      street, building etc. </rdfs:comment>
    <rdfs:range rdf:resource="http://www.w3.org/2001/XMLSchema#string" />
  </owl:DatatypeProperty>


========
<?xml version="1.0" encoding="UTF-8"?>
<!DOCTYPE rdf:RDF [
  <!ENTITY lcc-cr "https://www.omg.org/spec/LCC/Countries/CountryRepresentation/">
]>
<rdf:RDF xml:base="https://w3id.org/arto"
  xmlns:rdf="http://www.w3.org/1999/02/22-rdf-syntax-ns#"
  xmlns:rdfs="http://www.w3.org/2000/01/rdf-schema#"
  xmlns:ns="http://creativecommons.org/ns#"
  xmlns:owl="http://www.w3.org/2002/07/owl#"
  xmlns:skos="http://www.w3.org/2004/02/skos/core#"
  xmlns:dct="http://purl.org/dc/terms/"
  xmlns:lcc-cr="https://www.omg.org/spec/LCC/Countries/CountryRepresentation/"
  xmlns:arto="http://w3id.org/arto#"
  xmlns:vann="http://purl.org/vocab/vann/"
  xmlns:rdf-star="http://www.w3.org/2019/rdf-star#">

<!-- 
  <owl:Ontology rdf:about="http://w3id.org/arto">
    <owl:imports rdf:resource="http://www.w3.org/2000/01/rdf-schema" />
  </owl:Ontology> -->


  <owl:Ontology rdf:about="https://w3id.org/arto">
        <owl:versionIRI rdf:resource="https://w3id.org/arto/v0.1"/>
        <ns:attributionURL rdf:resource="https://w3id.org/arto"/>
        <dct:description xml:lang="en">The Artwork Object Ontology (ARTO) is a comprehensive ontology designed for describing and contextualizing artworks. It consists of two main components: the Artwork Descriptive Model and the Artwork Contextual Model. ARTO aims to provide a structured and detailed representation of artworks, facilitating tasks such as artwork captioning and information retrieval.</dct:description>
        <dct:issued>2024-04-10</dct:issued>
        <dct:license rdf:resource="https://github.com/SocialMachineLab/ArtworkOntology/blob/main/License"/>
        <dct:rights xml:lang="en">Copyright Â© 2024 Can Yang</dct:rights>
        <dct:title xml:lang="en">Artwork Object Ontology</dct:title>
        <vann:preferredNamespacePrefix>arto</vann:preferredNamespacePrefix>
        <vann:preferredNamespacePrefix>https://w3id.org/arto#</vann:preferredNamespacePrefix>
        <rdfs:label xml:lang="en">Artwork Object Ontology</rdfs:label>
        <owl:versionInfo rdf:datatype="http://www.w3.org/2001/XMLSchema#decimal">1.0</owl:versionInfo>
    </owl:Ontology>
    
  <!--
    ///////////////////////////////////////////////////////////////////////////////////////
    //
    // Classes
    //
    ///////////////////////////////////////////////////////////////////////////////////////
     -->
  <owl:Class
    rdf:about="http://w3id.org/arto#Artwork">
    <rdfs:label>Artwork</rdfs:label>
    <rdfs:comment>A created object or piece of art that is intended to be aesthetically pleasing or
      convey a message.</rdfs:comment>
  </owl:Class>

  <owl:Class rdf:about="http://w3id.org/arto#Painting">
    <rdfs:label>Painting</rdfs:label>
    <!-- https://dbpedia.org/ontology/Painting -->
    <rdfs:subClassOf rdf:resource="http://w3id.org/arto#Artwork" />
    <rdfs:comment>A created object or piece of art that is intended to be aesthetically pleasing or
      convey a message.</rdfs:comment>
  </owl:Class>

  <owl:Class rdf:about="http://w3id.org/arto#Series">
    <rdfs:label>Series</rdfs:label>
    <rdfs:comment>A set of artworks.</rdfs:comment>
    <!-- <owl:equivalentClass rdf:resource="https://schema.org/Series" /> -->
  </owl:Class>


  <owl:Class
    rdf:about="http://w3id.org/arto#Artist">
    <rdfs:label>Artist</rdfs:label>
    <!-- https://dbpedia.org/ontology/Artist -->
    <rdfs:comment>The person or group who create or contribute the artwork.</rdfs:comment>
    <rdfs:subClassOf rdf:resource="http://xmlns.com/foaf/0.1/Person" />
  </owl:Class>

  <owl:Class
    rdf:about="http://w3id.org/arto#Sponsor">
    <rdfs:label>Sponsor</rdfs:label>
    <!-- https://saidfathalla.github.io/SEOontology/Documentation/#Sponsor -->
    <rdfs:comment>The person or group who sponsor the artwork.</rdfs:comment>
    <rdfs:subClassOf rdf:resource="http://xmlns.com/foaf/0.1/Person" />
  </owl:Class>

  <owl:Class
    rdf:about="http://w3id.org/arto#Character">
    <rdfs:label>Character</rdfs:label>
    <!-- https://dbpedia.org/ontology/FictionalCharacter -->
    <rdfs:comment>The person or group appeared in the artwork.</rdfs:comment>
    <rdfs:subClassOf rdf:resource="http://xmlns.com/foaf/0.1/Person" />
  </owl:Class>


  <owl:Class
    rdf:about="http://purl.org/dc/terms/Location">
    <rdfs:label>Location</rdfs:label>
    <rdfs:comment>The Location.</rdfs:comment>
  </owl:Class>

  <owl:Class
    rdf:about="https://www.w3.org/TR/owl-time/#time:TemporalEntity">
    <rdfs:label>Time</rdfs:label>
    <rdfs:comment>A temporal interval or instant.</rdfs:comment>
  </owl:Class>

  <owl:Class
    rdf:about="https://www.w3.org/TR/owl-time/#time:Instant">
    <rdfs:label>Instant</rdfs:label>
    <rdfs:comment>A temporal entity with zero extent or duration</rdfs:comment>
    <rdfs:subClassOf rdf:resource="https://www.w3.org/TR/owl-time/#time:TemporalEntity" />
  </owl:Class>


  <owl:Class
    rdf:about="https://www.w3.org/TR/owl-time/#time:Interval">
    <rdfs:label>Interval</rdfs:label>
    <rdfs:comment>A temporal entity with an extent or duration</rdfs:comment>
    <rdfs:subClassOf rdf:resource="https://www.w3.org/TR/owl-time/#time:TemporalEntity" />
  </owl:Class>


  <owl:Class
    rdf:about="http://purl.org/NET/c4dm/event.owl#Event">
    <rdfs:label>Event</rdfs:label>
    <rdfs:comment>
      An arbitrary classification of a space/time region, by a
      cognitive agent. An event may have actively participating agents,
      passive factors, products, and a location in space/time.</rdfs:comment>
  </owl:Class>

  <owl:Class
    rdf:about="http://xmlns.com/foaf/0.1/Agent">
    <rdfs:label>Agent</rdfs:label>
    <rdfs:comment>Represents an Agent.This class comprises people, either individually or in groups,
      who have the potential to perform intentional actions for which they can be held responsible.</rdfs:comment>
  </owl:Class>


  <owl:Class
    rdf:about="http://xmlns.com/foaf/0.1/Organization">
    <rdfs:label>Organization</rdfs:label>
    <rdfs:comment>The Organization class represents a kind of Agent corresponding to instititutions
      such as galleries, museums etc.</rdfs:comment>
    <rdfs:subClassOf rdf:resource="http://xmlns.com/foaf/0.1/Agent" />
    <owl:disjointWith rdf:resource="http://xmlns.com/foaf/0.1/Person" />
  </owl:Class>


  <owl:Class
    rdf:about="http://xmlns.com/foaf/0.1/Person">
    <rdfs:label>Person</rdfs:label>
    <rdfs:comment>Represents a person associated with an artwork.</rdfs:comment>
    <rdfs:subClassOf rdf:resource="http://xmlns.com/foaf/0.1/Agent" />
  </owl:Class>


  <owl:Class
    rdf:about="http://w3id.org/arto#Element">
    <rdfs:label>Element</rdfs:label>
    <rdfs:comment>Represents the visual element associated with an artwork.</rdfs:comment>
  </owl:Class>


  <owl:Class
    rdf:about="http://w3id.org/arto#Color">
    <rdfs:label>Color</rdfs:label>
    <rdfs:comment>Represents the color used in an artwork.</rdfs:comment>
    <rdfs:subClassOf rdf:resource="http://w3id.org/arto#Element" />
  </owl:Class>


  <owl:Class
    rdf:about="http://w3id.org/arto#Line">
    <rdfs:label>Line</rdfs:label>
    <rdfs:comment>Represents the line used in an artwork.</rdfs:comment>
    <rdfs:subClassOf rdf:resource="http://w3id.org/arto#Element" />
  </owl:Class>


  <owl:Class
    rdf:about="http://w3id.org/arto#Space">
    <rdfs:label>Space</rdfs:label>
    <rdfs:comment>Represents the space used in an artwork.</rdfs:comment>
    <rdfs:subClassOf rdf:resource="http://w3id.org/arto#Element" />
  </owl:Class>

  <owl:Class
    rdf:about="http://w3id.org/arto#Composition">
    <rdfs:label>Composition</rdfs:label>
    <rdfs:comment>Represents the composition used in an artwork.</rdfs:comment>
    <rdfs:subClassOf rdf:resource="http://w3id.org/arto#Element" />
  </owl:Class>

  <owl:Class
    rdf:about="http://w3id.org/arto#Object">
    <rdfs:label>Object</rdfs:label>
    <rdfs:comment>Represents the physical or conceptual object within an artwork.</rdfs:comment>
  </owl:Class>


  <owl:Class
    rdf:about="http://w3id.org/arto#Scene">
    <rdfs:label>Scene</rdfs:label>
    <rdfs:comment>A scene can be viewed as a portion of the artwork composed of a group of objects
      that convey a specific meaning or sentiment.</rdfs:comment>
  </owl:Class>


  <owl:Class
    rdf:about="http://w3id.org/arto#Connotation">
    <rdfs:label>Cnnotation</rdfs:label>
    <rdfs:comment>Represents the interpretations of artwork, includeing themes, meanings, and
      emotions conveyed by an artwork.</rdfs:comment>
  </owl:Class>


  <owl:Class
    rdf:about="http://w3id.org/arto#Meaning">
    <rdfs:label>Meaning</rdfs:label>
    <rdfs:comment>Represents the underlying message, symbolism, or significance conveyed by an
      artwork.</rdfs:comment>
    <rdfs:subClassOf rdf:resource="http://w3id.org/arto#Connotation" />
  </owl:Class>


  <owl:Class
    rdf:about="http://w3id.org/arto#Emotion">
    <rdfs:label>Emotion</rdfs:label>
    <rdfs:comment>Represents the emotional response or affective state evoked by an artwork in the
      artist or viewers, such as joy, sadness, anger, or fear.</rdfs:comment>
    <rdfs:subClassOf rdf:resource="http://w3id.org/arto#Connotation" />
  </owl:Class>


  <owl:Class
    rdf:about="http://w3id.org/arto#Theme">
    <rdfs:label>Theme</rdfs:label>
    <rdfs:comment>Represents a central idea, subject, or concept explored in an artwork, which can
      be explicit or implicit, and may reflect broader cultural, social, or political issues.</rdfs:comment>
    <rdfs:subClassOf rdf:resource="http://w3id.org/arto#Connotation" />
  </owl:Class>

  <owl:Class
    rdf:about="http://w3id.org/arto#Metric">
    <rdfs:label>Metric</rdfs:label>
    <rdfs:comment>Represents a quantifiable measurement or characteristic of an artwork,
      encompassing statistical information about basic elements such as color statistics, emotion
      intensity, balance of composition, and other visual elements, to facilitate structural
      analysis
      and comparison of artworks.</rdfs:comment>
  </owl:Class>

  <owl:Class
    rdf:about="http://w3id.org/arto#MainColor">
    <rdfs:label>MainColor</rdfs:label>
    <rdfs:comment>Represents the dominant or most prominent color in an artwork, which can be
      determined through visual analysis or color quantization techniques.</rdfs:comment>
    <rdfs:subClassOf rdf:resource="http://w3id.org/arto#Metric" />
  </owl:Class>


  <owl:Class
    rdf:about="http://w3id.org/arto#ColorHistogram">
    <rdfs:label>ColorHistogram</rdfs:label>
    <rdfs:comment>Represents the distribution of colors in an artwork, typically expressed as a
      histogram or a quantitative representation of the frequency or proportion of each color
      present in
      the artwork.</rdfs:comment>
    <rdfs:subClassOf rdf:resource="http://w3id.org/arto#Metric" />
  </owl:Class>

  <owl:Class
    rdf:about="http://w3id.org/arto#Relevance">
    <rdfs:label>Relevance</rdfs:label>
    <rdfs:comment>Represents the degree to which a particular element or aspect of an artwork is
      related to its overall theme or meaning.</rdfs:comment>
    <rdfs:subClassOf rdf:resource="http://w3id.org/arto#Metric" />
  </owl:Class>

  <owl:Class
    rdf:about="http://w3id.org/arto#EmotionIntensity">
    <rdfs:label>EmotionIntensity</rdfs:label>
    <rdfs:comment>Represents the strength or degree of emotional response evoked by an artwork.</rdfs:comment>
    <rdfs:subClassOf rdf:resource="http://w3id.org/arto#Metric" />
  </owl:Class>

  <owl:Class
    rdf:about="http://w3id.org/arto#BalanceOfComposition">
    <rdfs:label>BalanceOfComposition</rdfs:label>
    <rdfs:comment>Represents the degree of visual equilibrium or harmony in the arrangement of
      elements within an artwork, considering factors such as symmetry, asymmetry, and distribution
      of
      visual elements.</rdfs:comment>
    <rdfs:subClassOf rdf:resource="http://w3id.org/arto#Metric" />
  </owl:Class>
  <!--
    ///////////////////////////////////////////////////////////////////////////////////////
    //
    // Object properties
    //
    ///////////////////////////////////////////////////////////////////////////////////////
     -->

  <owl:ObjectProperty
    rdf:about="https://motools.sourceforge.net/event/event.html#time">
    <rdfs:label>hasTime</rdfs:label>
    <rdfs:comment>Relates the event to the date. Could be a time interval or a time point</rdfs:comment>
    <rdfs:domain>
      <owl:Class>
        <owl:unionOf rdf:parseType="Collection">
          <rdf:Description rdf:about="http://purl.org/NET/c4dm/event.owl#Event" />
          <rdf:Description rdf:about="http://purl.org/dc/terms/Location" />
        </owl:unionOf>
      </owl:Class>
    </rdfs:domain>
    <rdfs:range rdf:resource="https://www.w3.org/TR/owl-time/#time:TemporalEntity" />
  </owl:ObjectProperty>


  <owl:ObjectProperty
    rdf:about="http://www.europeana.eu/schemas/edm/happenedAt">
    <rdfs:label>hasLocation</rdfs:label>
    <rdfs:comment>Relates the event or provenance to the location where it happened.</rdfs:comment>
    <rdfs:domain rdf:resource="http://purl.org/NET/c4dm/event.owl#Event" />
    <rdfs:range rdf:resource="http://purl.org/dc/terms/Location" />
  </owl:ObjectProperty>

  <owl:ObjectProperty
    rdf:about="https://dbpedia.org/ontology/residence">
    <rdfs:label>residence</rdfs:label>
    <rdfs:comment>Relates a person to the location they lived in.</rdfs:comment>
    <rdfs:domain rdf:resource="http://xmlns.com/foaf/0.1/Person" />
    <rdfs:range rdf:resource="http://purl.org/dc/terms/Location" />
  </owl:ObjectProperty>


  <owl:ObjectProperty
    rdf:about="http://purl.org/dc/terms/created">
    <rdfs:label>created</rdfs:label>
    <rdfs:comment>Relates an artwork to its creation date.</rdfs:comment>
    <rdfs:domain rdf:resource="http://w3id.org/arto#Artwork" />
    <rdfs:range rdf:resource="https://www.w3.org/TR/owl-time/#time:TemporalEntity" />
  </owl:ObjectProperty>


  <owl:ObjectProperty
    rdf:about="https://www.geonames.org/ontology#locatedIn">
    <rdfs:label>locatedIn</rdfs:label>
    <rdfs:comment>It . available options are: country, state, city, district,
      street, building etc. </rdfs:comment>
    <rdfs:comment>Indicates the location where an organization is situated.</rdfs:comment>

    <rdfs:domain rdf:resource="http://xmlns.com/foaf/0.1/Organization" />
    <!-- <rdfs:domain rdf:resource="http://purl.org/dc/terms/Location"/> -->
    <rdfs:range rdf:resource="http://purl.org/dc/terms/Location" />
  </owl:ObjectProperty>


  <owl:ObjectProperty
    rdf:about="http://purl.org/dc/terms/isPartOf">
    <rdfs:label>isPartOf</rdfs:label>
    <rdfs:comment>Relates an artwork to the serie of the artwork.</rdfs:comment>
    <rdfs:domain rdf:resource="http://w3id.org/arto#Artwork" />
    <rdfs:range rdf:resource="http://w3id.org/arto#Series" />
  </owl:ObjectProperty>

  <owl:ObjectProperty
    rdf:about="http://www.europeana.eu/schemas/edm/currentLocation">
    <rdfs:label>currentLocation</rdfs:label>
    <rdfs:comment>Relates an artwork to its current physical location.</rdfs:comment>
    <rdfs:domain rdf:resource="http://w3id.org/arto#Artwork" />
    <rdfs:range rdf:resource="http://purl.org/dc/terms/Location" />
  </owl:ObjectProperty>


  <owl:ObjectProperty
    rdf:about="http://w3id.org/arto#relatedToEvent">
    <rdfs:label>relatedToEvent</rdfs:label>
    <rdfs:comment>Relates an artwork to an event included in the artwork.</rdfs:comment>
    <rdfs:domain>
      <owl:Class>
        <owl:unionOf rdf:parseType="Collection">
          <rdf:Description rdf:about="http://w3id.org/arto#Artwork" />
          <rdf:Description rdf:about="http://w3id.org/arto#Connotation" />
        </owl:unionOf>
      </owl:Class>
    </rdfs:domain>
    <rdfs:range rdf:resource="http://purl.org/NET/c4dm/event.owl#Event" />
  </owl:ObjectProperty>


  <owl:ObjectProperty
    rdf:about="http://w3id.org/arto#hasEvent">
    <rdfs:label>hasEvent</rdfs:label>
    <rdfs:comment>Relates an artwork to an event happened to this artwork.</rdfs:comment>
    <rdfs:domain rdf:resource="http://w3id.org/arto#Artwork" />
    <rdfs:range rdf:resource="http://purl.org/NET/c4dm/event.owl#Event" />
  </owl:ObjectProperty>

  <owl:ObjectProperty
    rdf:about="http://purl.org/dc/elements/1.1/creator">
    <rdfs:label>creator</rdfs:label>
    <rdfs:comment>Relates an artwork to the artist(s) who created or contributed to it.</rdfs:comment>
    <!-- <rdfs:domain rdf:resource="http://example.com/artwork#Artwork"/>
    <rdfs:domain rdf:resource="https://schema.org/Series"/> -->
    <rdfs:domain>
      <owl:Class>
        <owl:unionOf rdf:parseType="Collection">
          <rdf:Description rdf:about="http://w3id.org/arto#Artwork" />
          <rdf:Description rdf:about="http://w3id.org/arto#Series" />
        </owl:unionOf>
      </owl:Class>
    </rdfs:domain>
    <rdfs:range rdf:resource="http://w3id.org/arto#Artist" />
  </owl:ObjectProperty>

  <owl:ObjectProperty
    rdf:about="http://purl.org/NET/c4dm/event.owl#agent">
    <rdfs:label>agent</rdfs:label>
    <rdfs:comment>Relates an artwork or event to a agent associated with it.</rdfs:comment>
    <rdfs:domain rdf:resource="http://purl.org/NET/c4dm/event.owl#Event" />
    <rdfs:range rdf:resource="http://xmlns.com/foaf/0.1/Agent" />
  </owl:ObjectProperty>


  <owl:ObjectProperty
    rdf:about="http://purl.org/dc/terms/contributor">
    <rdfs:label>contributor</rdfs:label>
    <rdfs:comment>The Contributor of the Artwork.</rdfs:comment>
    <rdfs:domain rdf:resource="http://w3id.org/arto#Artwork" />
    <rdfs:range rdf:resource="http://xmlns.com/foaf/0.1/Person" />
  </owl:ObjectProperty>


  <owl:ObjectProperty
    rdf:about="http://xmlns.com/foaf/0.1/knows">
    <rdfs:label>knows</rdfs:label>
    <rdfs:comment>The person knows persons.</rdfs:comment>
    <rdfs:domain rdf:resource="http://xmlns.com/foaf/0.1/Person" />
    <rdfs:range rdf:resource="http://xmlns.com/foaf/0.1/Person" />
  </owl:ObjectProperty>

  <!-- <owl:ObjectProperty
    rdf:about="http://w3id.org/arto#contain">
    <rdfs:label>contain</rdfs:label>
    <rdfs:comment>It could contains any objects.</rdfs:comment>
    <rdfs:domain rdf:resource="http://w3id.org/arto#Artwork" />
    <rdfs:range rdf:resource="http://www.w3.org/2002/07/owl#Thing" />
  </owl:ObjectProperty> -->


  <owl:ObjectProperty
    rdf:about="http://w3id.org/arto#relatedTo">
    <!-- http://www.ontologydesignpatterns.org/ont/dul/DUL.owl#isSettingFor -->
    <rdfs:label>relatedTo</rdfs:label>
    <rdfs:comment>The Objects could related to Objects.</rdfs:comment>
    <rdfs:domain rdf:resource="http://w3id.org/arto#Object" />
    <rdfs:range rdf:resource="http://w3id.org/arto#Object" />
  </owl:ObjectProperty>

  <owl:ObjectProperty
    rdf:about="http://w3id.org/arto#containsElements">
    <!-- http://www.ontologydesignpatterns.org/ont/dul/DUL.owl#isSettingFor -->
    <rdfs:label>containsElements</rdfs:label>
    <rdfs:comment>The objects contains elements.</rdfs:comment>
    <rdfs:domain rdf:resource="http://w3id.org/arto#Object" />
    <rdfs:range rdf:resource="http://w3id.org/arto#Element" />
  </owl:ObjectProperty>

  <owl:ObjectProperty
    rdf:about="http://w3id.org/arto#containsObjects">
    <!-- http://www.ontologydesignpatterns.org/ont/dul/DUL.owl#isSettingFor -->
    <rdfs:label>containsObjects</rdfs:label>
    <rdfs:comment>The Scene contains Objects.</rdfs:comment>
    <rdfs:domain rdf:resource="http://w3id.org/arto#Scene" />
    <rdfs:range rdf:resource="http://w3id.org/arto#Object" />
  </owl:ObjectProperty>


  <owl:ObjectProperty
    rdf:about="http://w3id.org/arto#relatedToScene">
    <!-- http://www.ontologydesignpatterns.org/ont/dul/DUL.owl#isSettingFor -->
    <rdfs:label>relatedToSecne</rdfs:label>
    <rdfs:comment>The Scenes that objects related.</rdfs:comment>
    <rdfs:range rdf:resource="http://w3id.org/arto#Scene" />
    <rdfs:domain rdf:resource="http://w3id.org/arto#Object" />
  </owl:ObjectProperty>

  <owl:ObjectProperty
    rdf:about="http://w3id.org/arto#hasConnotation">
    <!-- http://www.ontologydesignpatterns.org/ont/dul/DUL.owl#isSettingFor -->
    <rdfs:label>hasConnotation</rdfs:label>
    <rdfs:comment>Relate artwork and the connotations.</rdfs:comment>
    <rdfs:range rdf:resource="http://w3id.org/arto#Connotation" />
    <rdfs:domain rdf:resource="http://w3id.org/arto#Artwork" />
  </owl:ObjectProperty>

  <!-- <owl:ObjectProperty
  rdf:about="http://w3id.org/arto#relatedToEvent">
  <rdfs:label>relatedToEvent</rdfs:label>
  <rdfs:comment>Relate Event and the connotations.</rdfs:comment>
  <rdfs:range rdf:resource="http://w3id.org/arto#Connotation" />
  <rdfs:domain rdf:resource="http://purl.org/NET/c4dm/event.owl#Event" />
</owl:ObjectProperty> -->

  <owl:ObjectProperty
    rdf:about="http://w3id.org/arto#containsScenes">
    <!-- http://www.ontologydesignpatterns.org/ont/dul/DUL.owl#isSettingFor -->
    <rdfs:label>containsObjects</rdfs:label>
    <rdfs:comment>The Artwork and Scene could contains Scenes.</rdfs:comment>
    <rdfs:domain>
      <owl:Class>
        <owl:unionOf rdf:parseType="Collection">
          <rdf:Description rdf:about="http://w3id.org/arto#Artwork" />
          <rdf:Description rdf:about="http://w3id.org/arto#Scene" />
        </owl:unionOf>
      </owl:Class>
    </rdfs:domain>
    <rdfs:range rdf:resource="http://w3id.org/arto#Scene" />
  </owl:ObjectProperty>


  <owl:ObjectProperty
    rdf:about="http://w3id.org/arto#hasMetric">
    <rdfs:label>hasMetric</rdfs:label>
    <rdfs:comment>The metric of the connotation, scene, Object or the element in the artwork.</rdfs:comment>
    <rdfs:domain>
      <owl:Class>
        <owl:unionOf rdf:parseType="Collection">
          <rdf:Description rdf:about="http://w3id.org/arto#Connotation" />
          <rdf:Description rdf:about="http://w3id.org/arto#Element" />
          <rdf:Description rdf:about="http://w3id.org/arto#Scene" />
          <rdf:Description rdf:about="http://w3id.org/arto#Object" />
        </owl:unionOf>
      </owl:Class>
    </rdfs:domain>
    <rdfs:range rdf:resource="http://w3id.org/arto#Metric" />
  </owl:ObjectProperty>

  <owl:ObjectProperty
    rdf:about="http://w3id.org/arto#express">
    <rdfs:label>express</rdfs:label>
    <rdfs:comment>The connotation expressed in the Scenes or the Objects or Elements in the artwork.</rdfs:comment>
    <rdfs:domain>
      <owl:Class>
        <owl:unionOf rdf:parseType="Collection">
          <rdf:Description rdf:about="http://w3id.org/arto#Element" />
          <rdf:Description rdf:about="http://w3id.org/arto#Scene" />
          <rdf:Description rdf:about="http://w3id.org/arto#Object" />
        </owl:unionOf>
      </owl:Class>
    </rdfs:domain>
    <rdfs:range rdf:resource="http://w3id.org/arto#Connotation" />
  </owl:ObjectProperty>

  <!--
    ///////////////////////////////////////////////////////////////////////////////////////
    //
    // Datatype properties
    //
    ///////////////////////////////////////////////////////////////////////////////////////
     -->


  <owl:DatatypeProperty
    rdf:about="http://w3id.org/arto#source">
    <rdfs:label>source</rdfs:label>
    <rdfs:comment>Relates the source of the meaning in artworks.</rdfs:comment>
    <rdfs:domain rdf:resource="http://w3id.org/arto#Meaning" />
    <rdfs:range rdf:resource="http://www.w3.org/2001/XMLSchema#string" />
  </owl:DatatypeProperty>

  <owl:DatatypeProperty
    rdf:about="http://w3id.org/arto#emotionType">
    <rdfs:label>emotionType</rdfs:label>
    <rdfs:comment>Point out the emotion type.</rdfs:comment>
    <rdfs:domain rdf:resource="http://w3id.org/arto#Emotion" />
    <rdfs:range rdf:resource="http://www.w3.org/2001/XMLSchema#string" />
  </owl:DatatypeProperty>

  <owl:DatatypeProperty
    rdf:about="http://w3id.org/arto#coordinates">
    <rdfs:label>coordinates</rdfs:label>
    <rdfs:comment>The coordinates of the Scene or the Object in the artwork.</rdfs:comment>
    <rdfs:domain>
      <owl:Class>
        <owl:unionOf rdf:parseType="Collection">
          <rdf:Description rdf:about="http://w3id.org/arto#Scene" />
          <rdf:Description rdf:about="http://w3id.org/arto#Object" />
        </owl:unionOf>
      </owl:Class>
    </rdfs:domain>
    <rdfs:range rdf:resource="http://www.w3.org/2001/XMLSchema#string" />
  </owl:DatatypeProperty>


  <owl:DatatypeProperty
    rdf:about="http://w3id.org/arto#size">
    <rdfs:label>size</rdfs:label>
    <rdfs:comment>The size of the Scene or the Object in the artwork.</rdfs:comment>
    <rdfs:domain>
      <owl:Class>
        <owl:unionOf rdf:parseType="Collection">
          <rdf:Description rdf:about="http://w3id.org/arto#Scene" />
          <rdf:Description rdf:about="http://w3id.org/arto#Object" />
        </owl:unionOf>
      </owl:Class>
    </rdfs:domain>
    <rdfs:range rdf:resource="http://www.w3.org/2001/XMLSchema#string" />
  </owl:DatatypeProperty>


  <owl:DatatypeProperty
    rdf:about="http://w3id.org/arto#material">
    <rdfs:label>material</rdfs:label>
    <rdfs:comment>The material of the Object.</rdfs:comment>
    <rdfs:domain rdf:resource="http://w3id.org/arto#Object" />
    <rdfs:range rdf:resource="http://www.w3.org/2001/XMLSchema#string" />
  </owl:DatatypeProperty>

  <owl:DatatypeProperty
    rdf:about="http://w3id.org/arto#hasState">
    <rdfs:label>hasState</rdfs:label>
    <rdfs:comment>The state of the Object.</rdfs:comment>
    <rdfs:domain rdf:resource="http://w3id.org/arto#Object" />
    <rdfs:range rdf:resource="http://www.w3.org/2001/XMLSchema#string" />
  </owl:DatatypeProperty>


  <owl:DatatypeProperty
    rdf:about="http://w3id.org/arto#RGBValue">
    <rdfs:label>RGBValue</rdfs:label>
    <rdfs:comment>The RGBValue of the Color.</rdfs:comment>
    <rdfs:domain rdf:resource="http://w3id.org/arto#Color" />
    <rdfs:range rdf:resource="http://www.w3.org/2001/XMLSchema#int" />
  </owl:DatatypeProperty>

  <owl:DatatypeProperty
    rdf:about="http://w3id.org/arto#HSVValue">
    <rdfs:label>HSVValue</rdfs:label>
    <rdfs:comment>The HSVValue of the Color.</rdfs:comment>
    <rdfs:domain rdf:resource="http://w3id.org/arto#Color" />
    <rdfs:range rdf:resource="http://www.w3.org/2001/XMLSchema#int" />
  </owl:DatatypeProperty>

  <owl:DatatypeProperty
    rdf:about="http://w3id.org/arto#length">
    <rdfs:label>length</rdfs:label>
    <rdfs:comment>The length of the line.</rdfs:comment>
    <rdfs:domain rdf:resource="http://w3id.org/arto#Line" />
    <rdfs:range rdf:resource="http://www.w3.org/2001/XMLSchema#float" />
  </owl:DatatypeProperty>

  <!-- <owl:DatatypeProperty
    rdf:about="http://w3id.org/arto#width">
    <rdfs:label>width</rdfs:label>
    <rdfs:comment>The width of the line.</rdfs:comment>
    <rdfs:domain rdf:resource="http://w3id.org/arto#Line" />
    <rdfs:range rdf:resource="http://www.w3.org/2001/XMLSchema#float" />
  </owl:DatatypeProperty> -->


  <owl:DatatypeProperty
    rdf:about="http://w3id.org/arto#lineType">
    <rdfs:label>lineType</rdfs:label>
    <rdfs:comment>The type of the line.</rdfs:comment>
    <rdfs:domain rdf:resource="http://w3id.org/arto#Line" />
    <rdfs:range rdf:resource="http://www.w3.org/2001/XMLSchema#float" />
  </owl:DatatypeProperty>


  <owl:DatatypeProperty
    rdf:about="http://w3id.org/arto#direction">
    <rdfs:label>direction</rdfs:label>
    <rdfs:comment>The direction of the line.</rdfs:comment>
    <rdfs:domain rdf:resource="http://w3id.org/arto#Line" />
    <rdfs:range rdf:resource="http://www.w3.org/2001/XMLSchema#string" />
  </owl:DatatypeProperty>

  <owl:DatatypeProperty
    rdf:about="http://w3id.org/arto#spaceType">
    <rdfs:label>spaceType</rdfs:label>
    <rdfs:comment>The type of the space.</rdfs:comment>
    <rdfs:domain rdf:resource="http://w3id.org/arto#Space" />
    <rdfs:range rdf:resource="http://www.w3.org/2001/XMLSchema#float" />
  </owl:DatatypeProperty>


  <owl:DatatypeProperty
    rdf:about="http://w3id.org/arto#compositionType">
    <rdfs:label>compositionType</rdfs:label>
    <rdfs:comment>The type of the composition.</rdfs:comment>
    <rdfs:domain rdf:resource="http://w3id.org/arto#Composition" />
    <rdfs:range rdf:resource="http://www.w3.org/2001/XMLSchema#float" />
  </owl:DatatypeProperty>


  <owl:DatatypeProperty
    rdf:about="http://www.europeana.eu/schemas/edm/isShownBy">

    <rdfs:label>imageResource</rdfs:label>
    <rdfs:comment>An unambiguous URI reference to the digital object on the provider's web site in
      the best available resolution/quality. </rdfs:comment>
    <rdfs:domain rdf:resource="http://w3id.org/arto#Artwork" />
    <rdfs:range rdf:resource="http://www.w3.org/2001/XMLSchema#string" />
  </owl:DatatypeProperty>


  <owl:DatatypeProperty
    rdf:about="http://purl.org/dc/terms/description">
    <rdfs:label>description</rdfs:label>
    <rdfs:comment>Relates an artwork to its description.</rdfs:comment>
    <rdfs:domain rdf:resource="http://w3id.org/arto#Artwork" />
    <rdfs:range rdf:resource="http://www.w3.org/2001/XMLSchema#string" />
  </owl:DatatypeProperty>


  <owl:DatatypeProperty
    rdf:about="http://purl.org/dc/elements/1.1/title">
    <rdfs:label>title</rdfs:label>
    <rdfs:comment>Relates an artwork to its title.</rdfs:comment>
    <rdfs:domain rdf:resource="http://w3id.org/arto#Artwork" />
    <rdfs:range rdf:resource="http://www.w3.org/2001/XMLSchema#string" />
  </owl:DatatypeProperty>

  <owl:DatatypeProperty
    rdf:about="https://dbpedia.org/property/style">
    <rdfs:label>style</rdfs:label>
    <rdfs:comment>Relates an artwork to its artistic style or movement.</rdfs:comment>
    <rdfs:domain rdf:resource="http://w3id.org/arto#Artwork" />
    <rdfs:range rdf:resource="http://www.w3.org/2001/XMLSchema#string" />
  </owl:DatatypeProperty>

  <owl:DatatypeProperty
    rdf:about="https://schema.org/genre">
    <rdfs:label>genre</rdfs:label>
    <rdfs:comment>Relates an artwork to its genre.</rdfs:comment>
    <rdfs:domain rdf:resource="http://w3id.org/arto#Artwork" />
    <rdfs:range rdf:resource="http://www.w3.org/2001/XMLSchema#string" />
  </owl:DatatypeProperty>

  <owl:DatatypeProperty
    rdf:about="http://w3id.org/arto#timeType">
    <rdfs:label>timeType</rdfs:label>
    <rdfs:comment>The type of the time entity.</rdfs:comment>
    <rdfs:domain rdf:resource="https://www.w3.org/TR/owl-time/#time:TemporalEntity" />
    <rdfs:range rdf:resource="http://www.w3.org/2001/XMLSchema#string" />
  </owl:DatatypeProperty>


  <owl:DatatypeProperty
    rdf:about="http://purl.org/dc/terms/medium">
    <rdfs:label>medium</rdfs:label>
    <rdfs:comment>Relates an artwork to the medium(s) used in creating it.</rdfs:comment>
    <rdfs:domain rdf:resource="http://w3id.org/arto#Artwork" />
    <!-- <rdfs:range rdf:resource="http://purl.org/dc/terms/PhysicalMedium"/> -->
    <rdfs:range rdf:resource="http://www.w3.org/2001/XMLSchema#string" />
  </owl:DatatypeProperty>


  <owl:DatatypeProperty
    rdf:about="https://semanticweb.cs.vu.nl/2009/11/sem/semdoc.html#sem:eventType">
    <!-- https://dbpedia.org/ontology/type -->
    <rdfs:label>eventType</rdfs:label>
    <rdfs:comment> the type of the event</rdfs:comment>
    <rdfs:domain rdf:resource="http://purl.org/NET/c4dm/event.owl#Event" />
    <!-- <rdfs:range rdf:resource="https://www.w3.org/TR/owl-time/#time:"/> -->
    <rdfs:range rdf:resource="http://www.w3.org/2001/XMLSchema#string" />
  </owl:DatatypeProperty>


  <owl:DatatypeProperty
    rdf:about="http://www.ebu.ch/metadata/ontologies/ebucore/ebucore#height">
    <rdfs:label>height</rdfs:label>
    <rdfs:comment>Relates an artwork to its physical height.</rdfs:comment>
    <rdfs:domain rdf:resource="http://w3id.org/arto#Artwork" />

    <rdfs:range rdf:resource="http://www.w3.org/2001/XMLSchema#string" />
  </owl:DatatypeProperty>

  <owl:DatatypeProperty
    rdf:about="http://www.ebu.ch/metadata/ontologies/ebucore/ebucore#width">
    <rdfs:label>width</rdfs:label>
    <rdfs:comment>Relates an artwork to its physical width.</rdfs:comment>
    <rdfs:domain>
      <owl:Class>
        <owl:unionOf rdf:parseType="Collection">
          <rdf:Description rdf:about="http://w3id.org/arto#Artwork" />
          <rdf:Description rdf:about="http://w3id.org/arto#Line" />
        </owl:unionOf>
      </owl:Class>
    </rdfs:domain>
    <!-- <rdfs:domain rdf:resource="http://w3id.org/arto#Artwork" /> -->
    <rdfs:range rdf:resource="http://www.w3.org/2001/XMLSchema#string" />
  </owl:DatatypeProperty>


  <owl:DatatypeProperty
    rdf:about="https://dbpedia.org/ontology/nationality">
    <rdfs:label>nationality</rdfs:label>
    <rdfs:comment>Relates an person to the Nationality.</rdfs:comment>
    <rdfs:domain rdf:resource="http://xmlns.com/foaf/0.1/Person" />
    <!-- <rdfs:range rdf:resource="http://xmlns.com/foaf/0.1/Person"/> -->
    <rdfs:range rdf:resource="http://www.w3.org/2001/XMLSchema#string" />

  </owl:DatatypeProperty>


  <!-- <owl:DatatypeProperty
    rdf:about="http://www.europeana.eu/schemas/edm/componentColor">
    <rdfs:label>componentColor</rdfs:label>
    <rdfs:comment>The component Color of the Artwork.</rdfs:comment>
    <rdfs:domain rdf:resource="http://w3id.org/arto#Artwork" />
    <rdfs:range rdf:resource="http://www.w3.org/2001/XMLSchema#string" />
  </owl:DatatypeProperty> -->


  <!-- <owl:DatatypeProperty
    rdf:about="http://www.europeana.eu/schemas/edm/hasColorSpace">
    <rdfs:label>hasColorSpace</rdfs:label>
    <rdfs:comment>The Color Space of the Artwork.</rdfs:comment>
    <rdfs:domain rdf:resource="http://w3id.org/arto#Artwork" />
    <rdfs:range rdf:resource="http://www.w3.org/2001/XMLSchema#string" />
  </owl:DatatypeProperty> -->


  <owl:DatatypeProperty
    rdf:about="http://purl.org/dc/elements/1.1/format">
    <rdfs:label>format</rdfs:label>
    <rdfs:comment>The F gormat of the Artwork.</rdfs:comment>
    <rdfs:domain rdf:resource="http://w3id.org/arto#Artwork" />
    <rdfs:range rdf:resource="http://www.w3.org/2001/XMLSchema#string" />
  </owl:DatatypeProperty>


  <owl:DatatypeProperty
    rdf:about="http://www.w3.org/2003/01/geo/wgs84_pos#long">
    <rdfs:domain rdf:resource="http://purl.org/dc/terms/Location" />
    <rdfs:label>longitude</rdfs:label>
    <rdfs:comment>The WGS84 longitude of a SpatialThing (decimal degrees).</rdfs:comment>
    <rdfs:range rdf:resource="http://www.w3.org/2001/XMLSchema#string" />
  </owl:DatatypeProperty>

  <owl:DatatypeProperty
    rdf:about="http://www.w3.org/2003/01/geo/wgs84_pos#lat">
    <rdfs:domain rdf:resource="http://purl.org/dc/terms/Location" />
    <rdfs:label>latitude</rdfs:label>
    <rdfs:comment>The WGS84 latitude of a SpatialThing (decimal degrees).</rdfs:comment>
    <rdfs:range rdf:resource="http://www.w3.org/2001/XMLSchema#string" />
  </owl:DatatypeProperty>

  <owl:DatatypeProperty
    rdf:about="http://purl.org/dc/terms/locationType">
    <!-- https://dbpedia.org/ontology/regionType -->
    <rdfs:domain rdf:resource="http://purl.org/dc/terms/Location" />
    <rdfs:label>locationType</rdfs:label>
    <rdfs:comment>The type of the location. available options are: country, state, city, district,
      street, building etc. </rdfs:comment>
    <rdfs:range rdf:resource="http://www.w3.org/2001/XMLSchema#string" />
  </owl:DatatypeProperty>


>>>>>>>> c62016e83f10e0cc61c604eed265a64346c4bbbb:v0.1/arto.rdf
</rdf:RDF>