<?xml version="1.0" encoding="utf-8" ?>
<rdf:RDF xmlns:rdf="http://www.w3.org/1999/02/22-rdf-syntax-ns#"
         xmlns:owl="http://www.w3.org/2002/07/owl#"
         xmlns:cc="http://creativecommons.org/ns#"
         xmlns:dc="http://purl.org/dc/terms/"
         xmlns:ns0="http://purl.org/vocab/vann/"
         xmlns:rdfs="http://www.w3.org/2000/01/rdf-schema#"
         xmlns:skos="http://www.w3.org/2004/02/skos/core#"
         xmlns:foaf="http://xmlns.com/foaf/spec/">

  <owl:Ontology rdf:about="http://w3id.org/arto">
    <rdf:type rdf:resource="http://www.w3.org/2002/07/owl#NamedIndividual"/>
    <owl:versionIRI rdf:resource="http://w3id.org/arto/v0.1"/>
    <cc:attributionURL rdf:resource="http://w3id.org/arto"/>

    <dc:description xml:lang="en">The Artwork Object Ontology (ARTO) is a comprehensive ontology designed for describing and contextualizing artworks. It consists of two main components: the Artwork Descriptive Model and the Artwork Contextual Model. ARTO aims to provide a structured and detailed representation of artworks, facilitating tasks such as artwork captioning and information retrieval.</dc:description>
    <dc:issued>2024-04-10</dc:issued>
    <dc:license rdf:resource="https://github.com/SocialMachineLab/ArtworkOntology/blob/main/License"/>
    <dc:modified>2024-12-05</dc:modified>
    <dc:title xml:lang="en">Artwork Object Ontology</dc:title>
    <ns0:preferredNamespacePrefix>arto</ns0:preferredNamespacePrefix>
    <rdfs:label xml:lang="en">Artwork Object Ontology (ARTO)</rdfs:label>
    <owl:versionInfo>0.1</owl:versionInfo>
    <owl:imports rdf:resource="http://www.cidoc-crm.org/cidoc-crm/"/>
    <owl:imports rdf:resource="http://xmlns.com/foaf/0.1/"/>
    <owl:imports rdf:resource="http://purl.org/dc/terms/"/>
    <owl:imports rdf:resource="http://www.w3.org/2004/02/skos/core"/>
    <owl:imports rdf:resource="https://schema.org/"/>
  </owl:Ontology>

  <owl:AnnotationProperty rdf:about="http://creativecommons.org/ns#attributionURL">
  </owl:AnnotationProperty>

  <owl:AnnotationProperty rdf:about="http://purl.org/dc/terms/issued">
  </owl:AnnotationProperty>

  <owl:AnnotationProperty rdf:about="http://purl.org/dc/terms/license">
  </owl:AnnotationProperty>

  <owl:AnnotationProperty rdf:about="http://purl.org/dc/terms/modified">
  </owl:AnnotationProperty>

  <owl:AnnotationProperty rdf:about="http://purl.org/dc/terms/rights">
  </owl:AnnotationProperty>

  <owl:AnnotationProperty rdf:about="http://purl.org/dc/terms/title">
  </owl:AnnotationProperty>

  <owl:AnnotationProperty rdf:about="http://purl.org/vocab/vann/preferredNamespacePrefix">
  </owl:AnnotationProperty>

  <owl:AnnotationProperty rdf:about="http://www.w3.org/2002/07/owl#cardinality">
  </owl:AnnotationProperty>

  <owl:AnnotationProperty rdf:about="http://www.w3.org/2002/07/owl#maxCardinality">
  </owl:AnnotationProperty>

  <owl:AnnotationProperty rdf:about="http://www.w3.org/2002/07/owl#minCardinality">
  </owl:AnnotationProperty>

  <owl:AnnotationProperty rdf:about="http://www.w3.org/2004/02/skos/core#closeMatch">
  </owl:AnnotationProperty>

  <owl:ObjectProperty rdf:about="http://purl.org/NET/c4dm/event.owl#agent">
  </owl:ObjectProperty>

  <owl:ObjectProperty rdf:about="http://purl.org/dc/terms/contributor">
  </owl:ObjectProperty>

  <owl:ObjectProperty rdf:about="http://purl.org/dc/terms/creator">
  </owl:ObjectProperty>

  <owl:ObjectProperty rdf:about="http://purl.org/dc/terms/hasPart">
  </owl:ObjectProperty>

  <owl:ObjectProperty rdf:about="http://purl.org/dc/terms/isPartOf">
  </owl:ObjectProperty>

  <owl:ObjectProperty rdf:about="http://w3id.org/arto#containsElement">
    <rdfs:subPropertyOf rdf:resource="http://purl.org/dc/terms/hasPart"/>
    <rdfs:domain>
      <owl:Class>
        <owl:unionOf>
          <rdf:Description>
            <rdf:first rdf:resource="http://w3id.org/arto#Object"/>
            <rdf:rest>
              <rdf:Description>
                <rdf:first rdf:resource="http://w3id.org/arto#Scene"/>
                <rdf:rest rdf:resource="http://www.w3.org/1999/02/22-rdf-syntax-ns#nil"/>
              </rdf:Description>
            </rdf:rest>

          </rdf:Description>
        </owl:unionOf>

      </owl:Class>
    </rdfs:domain>

    <rdfs:range rdf:resource="http://w3id.org/arto#VisualElement"/>
    <rdfs:comment>Specifies the visual elements (such as color, line, composition) contained within an object in the artwork.</rdfs:comment>
    <skos:example>
                      - color elements: :sky_object arto:containsElement :blue_gradient_color
                      - Line elements: :mountain_object arto:containsElement :diagonal_line
                      - Compositional elements: :tree_object arto:containsElement :vertical_composition</skos:example>
    <rdfs:label>containsElement</rdfs:label>
  </owl:ObjectProperty>

  <owl:ObjectProperty rdf:about="http://w3id.org/arto#isElementOf">
    <rdfs:subPropertyOf rdf:resource="http://purl.org/dc/terms/isPartOf"/>
    <rdfs:domain rdf:resource="http://w3id.org/arto#VisualElement"/>
    <rdfs:range>
      <owl:Class>
        <owl:unionOf>
          <rdf:Description>
            <rdf:first rdf:resource="http://w3id.org/arto#Object"/>
            <rdf:rest>
              <rdf:Description>
                <rdf:first rdf:resource="http://w3id.org/arto#Scene"/>
                <rdf:rest rdf:resource="http://www.w3.org/1999/02/22-rdf-syntax-ns#nil"/>
              </rdf:Description>
            </rdf:rest>

          </rdf:Description>
        </owl:unionOf>

      </owl:Class>
    </rdfs:range>

    <rdfs:comment>Specifies the object that contains the visual element in the artwork.</rdfs:comment>
    <skos:example>
                  - color elements: :blue_gradient_color arto:isElementOf :sky_object
                  - Line elements: :diagonal_line arto:isElementOf :mountain_object
                  - Compositional elements: :vertical_composition arto:isElementOf :tree_object</skos:example>
    <rdfs:label>isElementOf</rdfs:label>
  </owl:ObjectProperty>

  <owl:ObjectProperty rdf:about="http://w3id.org/arto#containsObject">
    <rdfs:subPropertyOf rdf:resource="http://purl.org/dc/terms/hasPart"/>
    <rdfs:domain rdf:resource="http://w3id.org/arto#Scene"/>
    <rdfs:range rdf:resource="http://w3id.org/arto#Object"/>
    <rdfs:comment>Indicates specific objects that are present within a scene of an artwork.</rdfs:comment>
    <skos:example>
                      - Landscape scene: :garden_scene arto:containsObject :fountain, :bench, :flowers
                      - Portrait scene: :interior_scene arto:containsObject :chair, :table, :book
                      - Still life scene: :table_scene arto:containsObject :fruit_bowl, :wine_glass, :cloth</skos:example>
    <rdfs:label>containsObject</rdfs:label>
  </owl:ObjectProperty>

  <owl:ObjectProperty rdf:about="http://w3id.org/arto#isObjectOf">
    <rdfs:subPropertyOf rdf:resource="http://purl.org/dc/terms/isPartOf"/>
    <rdfs:domain rdf:resource="http://w3id.org/arto#Object"/>
    <rdfs:range rdf:resource="http://w3id.org/arto#Scene"/>
    <owl:inverseOf rdf:resource="http://w3id.org/arto#containsObject"/>
    <rdfs:comment>Indicates the scene that contains the object in the artwork.</rdfs:comment>
    <skos:example>
                - Landscape scene: :fountain arto:isObjectOf :garden_scene
                - Portrait scene: :chair arto:isObjectOf :interior_scene
                - Still life scene: :fruit_bowl arto:isObjectOf :table_scene</skos:example>
    <rdfs:label>isObjectOf</rdfs:label>
  </owl:ObjectProperty>

  <owl:ObjectProperty rdf:about="http://w3id.org/arto#containsScene">
    <rdfs:subPropertyOf rdf:resource="http://purl.org/dc/terms/hasPart"/>
    <rdfs:domain>
      <owl:Class>
        <owl:unionOf>
          <rdf:Description>
            <rdf:first rdf:resource="http://w3id.org/arto#Artwork"/>
            <rdf:rest>
              <rdf:Description>
                <rdf:first rdf:resource="http://w3id.org/arto#Scene"/>
                <rdf:rest rdf:resource="http://www.w3.org/1999/02/22-rdf-syntax-ns#nil"/>
              </rdf:Description>
            </rdf:rest>

          </rdf:Description>
        </owl:unionOf>

      </owl:Class>
    </rdfs:domain>

    <rdfs:range rdf:resource="http://w3id.org/arto#Scene"/>
    <rdfs:comment>Identifies distinct scenes within an artwork or within another scene, allowing for hierarchical scene composition.</rdfs:comment>
    <skos:example>
                      - Nested scenes: :market_scene arto:containsScene :vendor_scene, :customer_scene
                      - Background scenes: :landscape_painting arto:containsScene :mountain_scene, :valley_scene</skos:example>
    <rdfs:label>containsScene</rdfs:label>
  </owl:ObjectProperty>

  <owl:ObjectProperty rdf:about="http://w3id.org/arto#isSceneOf">
    <rdfs:subPropertyOf rdf:resource="http://purl.org/dc/terms/isPartOf"/>
    <rdfs:domain rdf:resource="http://w3id.org/arto#Scene"/>
    <rdfs:range>
      <owl:Class>
        <owl:unionOf>
          <rdf:Description>
            <rdf:first rdf:resource="http://w3id.org/arto#Artwork"/>
            <rdf:rest>
              <rdf:Description>
                <rdf:first rdf:resource="http://w3id.org/arto#Scene"/>
                <rdf:rest rdf:resource="http://www.w3.org/1999/02/22-rdf-syntax-ns#nil"/>
              </rdf:Description>
            </rdf:rest>

          </rdf:Description>
        </owl:unionOf>

      </owl:Class>
    </rdfs:range>

    <owl:inverseOf rdf:resource="http://w3id.org/arto#containsScene"/>
    <rdfs:comment>Specifies the artwork or scene that contains the scene in the artwork.</rdfs:comment>
    <skos:example>
                - Nested scenes: :vendor_scene arto:isSceneOf :market_scene
                - Background scenes: :mountain_scene arto:isSceneOf :landscape_painting</skos:example>
    <rdfs:label>isSceneOf</rdfs:label>
  </owl:ObjectProperty>

  <owl:ObjectProperty rdf:about="http://w3id.org/arto#currentLocation">
    <rdfs:domain rdf:resource="http://w3id.org/arto#Artwork"/>
    <rdfs:range rdf:resource="http://w3id.org/arto#Location"/>
    <rdfs:comment>Specifies the current physical location where an artwork is housed or displayed.</rdfs:comment>
    <skos:example>
                      - Museum location: :mona_lisa arto:currentLocation :louvre_museum
                      - Gallery location: :starry_night arto:currentLocation :moma_gallery_room_24
                      </skos:example>
    <rdfs:label>currentLocation</rdfs:label>
    <owl:cardinality rdf:datatype="http://www.w3.org/2001/XMLSchema#integer">1</owl:cardinality>
    <skos:closeMatch rdf:resource="http://www.europeana.eu/schemas/edm/currentLocation"/>
  </owl:ObjectProperty>

  <owl:ObjectProperty rdf:about="http://w3id.org/arto#expresses">
    <rdfs:domain>
      <owl:Class>
        <owl:unionOf>
          <rdf:Description>
            <rdf:first rdf:resource="http://w3id.org/arto#Object"/>
            <rdf:rest>
              <rdf:Description>
                <rdf:first rdf:resource="http://w3id.org/arto#Scene"/>
                <rdf:rest>
                  <rdf:Description>
                    <rdf:first rdf:resource="http://w3id.org/arto#VisualElement"/>
                    <rdf:rest>
                      <rdf:Description>
                        <rdf:first rdf:resource="http://w3id.org/arto#Artwork"/>
                        <rdf:rest rdf:resource="http://www.w3.org/1999/02/22-rdf-syntax-ns#nil"/>
                      </rdf:Description>
                    </rdf:rest>

                  </rdf:Description>
                </rdf:rest>

              </rdf:Description>
            </rdf:rest>

          </rdf:Description>
        </owl:unionOf>

      </owl:Class>
    </rdfs:domain>

    <rdfs:range rdf:resource="http://w3id.org/arto#Connotation"/>
    <owl:inverseOf>
      <owl:ObjectProperty rdf:about="http://w3id.org/arto#isExpressedBy">
        <rdfs:domain rdf:resource="http://w3id.org/arto#Connotation"/>
        <rdfs:range>
          <owl:Class>
            <owl:unionOf>
              <rdf:Description>
                <rdf:first rdf:resource="http://w3id.org/arto#Object"/>
                <rdf:rest>
                  <rdf:Description>
                    <rdf:first rdf:resource="http://w3id.org/arto#Scene"/>
                    <rdf:rest>
                      <rdf:Description>
                        <rdf:first rdf:resource="http://w3id.org/arto#VisualElement"/>
                        <rdf:rest>
                          <rdf:Description>
                            <rdf:first rdf:resource="http://w3id.org/arto#Artwork"/>
                            <rdf:rest rdf:resource="http://www.w3.org/1999/02/22-rdf-syntax-ns#nil"/>
                          </rdf:Description>
                        </rdf:rest>

                      </rdf:Description>
                    </rdf:rest>

                  </rdf:Description>
                </rdf:rest>

              </rdf:Description>
            </owl:unionOf>

          </owl:Class>
        </rdfs:range>

        <owl:inverseOf rdf:resource="http://w3id.org/arto#expresses"/>
        <rdfs:comment>Associates a connotation with the visual elements, objects, scenes or artwork that express it.</rdfs:comment>
        <skos:example>
                    - Emotional expression: :anger_emotion arto:isExpressedBy :red_color
                    - Symbolic meaning: :peace_meaning arto:isExpressedBy :dove_object
                    - Scene mood: :turbulence_emotion arto:isExpressedBy :storm_scene
                    - Artwork meaning: :anti_war_theme arto:isExpressedBy :guernica</skos:example>
        <rdfs:label>isExpressedBy</rdfs:label>
      </owl:ObjectProperty>
    </owl:inverseOf>

    <rdfs:comment>Links visual elements, objects, scenes, or artworks to their symbolic meanings or emotional connotations.</rdfs:comment>
    <skos:example>
              - Emotional expression: :red_color arto:expresses :anger_emotion
              - Symbolic meaning: :dove_object arto:expresses :peace_meaning
              - Scene mood: :storm_scene arto:expresses :turbulence_emotion
              - Artwork meaning: :guernica arto:expresses :anti_war_theme</skos:example>
    <rdfs:label>express</rdfs:label>
    <skos:closeMatch rdf:resource="https://w3id.org/icon/ontology/recognizedConcept"/>
  </owl:ObjectProperty>

  <owl:ObjectProperty rdf:about="http://w3id.org/arto#hasLocation">
    <rdfs:domain>
      <owl:Class>
        <owl:unionOf>
          <rdf:Description>
            <rdf:first rdf:resource="http://w3id.org/arto#Agent"/>
            <rdf:rest>
              <rdf:Description>
                <rdf:first rdf:resource="http://w3id.org/arto#Event"/>
                <rdf:rest rdf:resource="http://www.w3.org/1999/02/22-rdf-syntax-ns#nil"/>
              </rdf:Description>
            </rdf:rest>

          </rdf:Description>
        </owl:unionOf>

      </owl:Class>
    </rdfs:domain>

    <rdfs:range rdf:resource="http://w3id.org/arto#Location"/>
    <owl:inverseOf>
      <owl:ObjectProperty rdf:about="http://w3id.org/arto#isLocationOf">
        <rdfs:domain rdf:resource="http://w3id.org/arto#Location"/>
        <rdfs:range>
          <owl:Class>
            <owl:unionOf>
              <rdf:Description>
                <rdf:first rdf:resource="http://w3id.org/arto#Agent"/>
                <rdf:rest>
                  <rdf:Description>
                    <rdf:first rdf:resource="http://w3id.org/arto#Event"/>
                    <rdf:rest rdf:resource="http://www.w3.org/1999/02/22-rdf-syntax-ns#nil"/>
                  </rdf:Description>
                </rdf:rest>

              </rdf:Description>
            </owl:unionOf>

          </owl:Class>
        </rdfs:range>

        <owl:inverseOf rdf:resource="http://w3id.org/arto#hasLocation"/>
        <rdfs:comment>Associates a location with the organization or event that it is related to.</rdfs:comment>
        <skos:example>
                - Museum address: :met_nyc_location arto:isLocationOf :metropolitan_museum
                - Gallery location: :london_bankside arto:isLocationOf :tate_modern
                - Studio location: :manhattan_location arto:isLocationOf :warhol_factory
                - Exhibition event: :venice_giardini arto:isLocationOf :venice_biennale_2024</skos:example>
        <rdfs:label>isLocationOf</rdfs:label>
      </owl:ObjectProperty>
    </owl:inverseOf>

    <rdfs:comment>Specifies the physical location of an organization or event related to the artwork.</rdfs:comment>
    <skos:example>
                - Museum address: :metropolitan_museum arto:hasLocation :met_nyc_location
                - Gallery location: :tate_modern arto:hasLocation :london_bankside
                - Studio location: :warhol_factory arto:hasLocation :manhattan_location
                - Exhibition event: :venice_biennale_2024 arto:hasLocation :venice_giardini</skos:example>
    <rdfs:label>hasLocation</rdfs:label>
  </owl:ObjectProperty>

  <owl:ObjectProperty rdf:about="http://w3id.org/arto#hasMetric">
    <rdfs:domain>
      <owl:Class>
        <owl:unionOf>
          <rdf:Description>
            <rdf:first rdf:resource="http://w3id.org/arto#Connotation"/>
            <rdf:rest>
              <rdf:Description>
                <rdf:first rdf:resource="http://w3id.org/arto#Object"/>
                <rdf:rest>
                  <rdf:Description>
                    <rdf:first rdf:resource="http://w3id.org/arto#Scene"/>
                    <rdf:rest>
                      <rdf:Description>
                        <rdf:first rdf:resource="http://w3id.org/arto#VisualElement"/>
                        <rdf:rest rdf:resource="http://www.w3.org/1999/02/22-rdf-syntax-ns#nil"/>
                      </rdf:Description>
                    </rdf:rest>

                  </rdf:Description>
                </rdf:rest>

              </rdf:Description>
            </rdf:rest>

          </rdf:Description>
        </owl:unionOf>

      </owl:Class>
    </rdfs:domain>

    <rdfs:range rdf:resource="http://w3id.org/arto#Metric"/>
    <owl:inverseOf>
      <owl:ObjectProperty rdf:about="http://w3id.org/arto#isMetricOf">
        <rdfs:domain rdf:resource="http://w3id.org/arto#Metric"/>
        <rdfs:range>
          <owl:Class>
            <owl:unionOf>
              <rdf:Description>
                <rdf:first rdf:resource="http://w3id.org/arto#Connotation"/>
                <rdf:rest>
                  <rdf:Description>
                    <rdf:first rdf:resource="http://w3id.org/arto#Object"/>
                    <rdf:rest>
                      <rdf:Description>
                        <rdf:first rdf:resource="http://w3id.org/arto#Scene"/>
                        <rdf:rest>
                          <rdf:Description>
                            <rdf:first rdf:resource="http://w3id.org/arto#VisualElement"/>
                            <rdf:rest rdf:resource="http://www.w3.org/1999/02/22-rdf-syntax-ns#nil"/>
                          </rdf:Description>
                        </rdf:rest>

                      </rdf:Description>
                    </rdf:rest>

                  </rdf:Description>
                </rdf:rest>

              </rdf:Description>
            </owl:unionOf>

          </owl:Class>
        </rdfs:range>

        <owl:inverseOf rdf:resource="http://w3id.org/arto#hasMetric"/>
        <rdfs:comment>Associates a metric with the component of an artwork that it is related to.</rdfs:comment>
        <skos:example>
                - Color metrics: :blue_intensity_75_percent arto:isMetricOf :sky_area
                - Composition balance: :symmetry_score_0.8 arto:isMetricOf :landscape_scene
                - Emotional intensity: :fear_intensity_high arto:isMetricOf :expression_scene</skos:example>
        <rdfs:label>isMetricOf</rdfs:label>
      </owl:ObjectProperty>
    </owl:inverseOf>

    <rdfs:comment>Associates components (Connotation, Scene, Object or the Visual Element) of an artwork with quantifiable measurements or characteristics.</rdfs:comment>
    <skos:example>
                - Color metrics: :sky_area arto:hasMetric :blue_intensity_75_percent
                - Composition balance: :landscape_scene arto:hasMetric :symmetry_score_0.8
                - Emotional intensity: :expression_scene arto:hasMetric :fear_intensity_high</skos:example>
    <rdfs:label>hasMetric</rdfs:label>
  </owl:ObjectProperty>

  <owl:ObjectProperty rdf:about="http://w3id.org/arto#hasTime">
    <rdfs:domain>
      <owl:Class>
        <owl:unionOf>
          <rdf:Description>
            <rdf:first rdf:resource="http://w3id.org/arto#Event"/>
            <rdf:rest>
              <rdf:Description>
                <rdf:first rdf:resource="http://w3id.org/arto#Location"/>
                <rdf:rest rdf:resource="http://www.w3.org/1999/02/22-rdf-syntax-ns#nil"/>
              </rdf:Description>
            </rdf:rest>

          </rdf:Description>
        </owl:unionOf>

      </owl:Class>
    </rdfs:domain>

    <rdfs:range rdf:resource="http://w3id.org/arto#Time"/>
    <owl:inverseOf>
      <owl:ObjectProperty rdf:about="http://w3id.org/arto#isTimeOf">
        <rdfs:domain rdf:resource="http://w3id.org/arto#Time"/>
        <rdfs:range>
          <owl:Class>
            <owl:unionOf>
              <rdf:Description>
                <rdf:first rdf:resource="http://w3id.org/arto#Event"/>
                <rdf:rest>
                  <rdf:Description>
                    <rdf:first rdf:resource="http://w3id.org/arto#Location"/>
                    <rdf:rest rdf:resource="http://www.w3.org/1999/02/22-rdf-syntax-ns#nil"/>
                  </rdf:Description>
                </rdf:rest>

              </rdf:Description>
            </owl:unionOf>

          </owl:Class>
        </rdfs:range>

        <owl:inverseOf rdf:resource="http://w3id.org/arto#hasTime"/>
        <rdfs:comment>Associates a time with the event or location that it is related to.</rdfs:comment>
        <skos:example>
              - Event timing: :spring2024 arto:isTimeOf :exhibition2024
              - Location historical period: :belle_epoque arto:isTimeOf :paris_studio
              </skos:example>
        <rdfs:label>isTimeOf</rdfs:label>
      </owl:ObjectProperty>
    </owl:inverseOf>

    <rdfs:comment>Associates an event or location with its temporal information.</rdfs:comment>
    <skos:example>
              - Event timing: :exhibition2024 arto:hasTime :spring2024
              - Location historical period: :paris_studio arto:hasTime :belle_epoque
              </skos:example>
    <rdfs:label>hasTime</rdfs:label>
  </owl:ObjectProperty>

  <owl:ObjectProperty rdf:about="http://w3id.org/arto#knows">
    <rdfs:domain rdf:resource="http://w3id.org/arto#Person"/>
    <rdfs:range rdf:resource="http://w3id.org/arto#Person"/>
    <rdfs:comment>The person knows persons.</rdfs:comment>
    <skos:example>
            - Artist relationships: :vincent_van_gogh arto:knows :paul_gauguin
            - Teacher-student: :gustav_klimt arto:knows :egon_schiele
            - Collaborative artists: :pablo_picasso arto:knows :georges_braque</skos:example>
    <rdfs:label>knows</rdfs:label>
  </owl:ObjectProperty>

  <owl:ObjectProperty rdf:about="http://w3id.org/arto#relatedTo">
    <rdfs:domain rdf:resource="http://w3id.org/arto#Object"/>
    <rdfs:range rdf:resource="http://w3id.org/arto#Object"/>
    <rdfs:comment>Describes spatial or conceptual relationships between objects within an artwork. The specific relationships are specified using the rdfs:subPropertyOf.</rdfs:comment>
    <skos:example>
                - Spatial relation: :cup_object arto:rests_on :table_object ;
                  arto:rests_on rdfs:subPropertyOf arto:relatedTo;
                - Interaction: :mother_figure arto:holds :child_figure ;
                  arto:holds rdfs:subPropertyOf arto:relatedTo;
                - Position: :cloud_object arto:above :mountain_object ;
                  arto:above rdfs:subPropertyOf arto:relatedTo</skos:example>
    <rdfs:label>relatedTo</rdfs:label>
  </owl:ObjectProperty>

  <owl:ObjectProperty rdf:about="http://w3id.org/arto#relatedToEvent">
    <rdfs:domain>
      <owl:Class>
        <owl:unionOf>
          <rdf:Description>
            <rdf:first rdf:resource="http://w3id.org/arto#Artwork"/>
            <rdf:rest>
              <rdf:Description>
                <rdf:first rdf:resource="http://w3id.org/arto#Scene"/>
                <rdf:rest rdf:resource="http://www.w3.org/1999/02/22-rdf-syntax-ns#nil"/>
              </rdf:Description>
            </rdf:rest>

          </rdf:Description>
        </owl:unionOf>

      </owl:Class>
    </rdfs:domain>

    <rdfs:range rdf:resource="http://w3id.org/arto#Event"/>
    <owl:inverseOf>
      <owl:ObjectProperty rdf:about="http://w3id.org/arto#isEventOf">
        <rdfs:domain rdf:resource="http://w3id.org/arto#Event"/>
        <rdfs:range>
          <owl:Class>
            <owl:unionOf>
              <rdf:Description>
                <rdf:first rdf:resource="http://w3id.org/arto#Artwork"/>
                <rdf:rest>
                  <rdf:Description>
                    <rdf:first rdf:resource="http://w3id.org/arto#Scene"/>
                    <rdf:rest rdf:resource="http://www.w3.org/1999/02/22-rdf-syntax-ns#nil"/>
                  </rdf:Description>
                </rdf:rest>

              </rdf:Description>
            </owl:unionOf>

          </owl:Class>
        </rdfs:range>

        <owl:inverseOf rdf:resource="http://w3id.org/arto#relatedToEvent"/>
        <rdfs:comment>Associates an event with the artwork or scene that it is related to.</rdfs:comment>
        <skos:example>
                - Historical event: :french_revolution_1830 arto:isEventOf :liberty_leading_the_people
                - Biblical event: :biblical_last_supper arto:isEventOf :last_supper
                </skos:example>
        <rdfs:label>isEventOf</rdfs:label>
      </owl:ObjectProperty>
    </owl:inverseOf>

    <rdfs:comment>Connects an artwork or its connotation to historical, mythological, or contemporary events depicted or referenced in the work.</rdfs:comment>
    <skos:example>
                      - Historical event: :liberty_leading_the_people arto:relatedToEvent :french_revolution_1830
                      - Biblical event: :last_supper arto:relatedToEvent :biblical_last_supper
                      </skos:example>
    <rdfs:label>relatedToEvent</rdfs:label>
  </owl:ObjectProperty>

  <owl:ObjectProperty rdf:about="http://w3id.org/arto#relatedToConnotation">
    <rdfs:domain rdf:resource="http://w3id.org/arto#Event"/>
    <rdfs:range rdf:resource="http://w3id.org/arto#Connotation"/>
    <rdfs:comment>Indicates that an event relatedToConnotation some connotations.</rdfs:comment>
    <skos:example>
                  ex:NoahDoveEvent rdf:type arto:Event ;
                  arto:relatedToConnotation ex:PeaceSymbolism ;
                </skos:example>
    <rdfs:label>relatedToConnotation</rdfs:label>
  </owl:ObjectProperty>

  <owl:ObjectProperty rdf:about="http://w3id.org/arto#relatedToScene">
    <rdfs:domain rdf:resource="http://w3id.org/arto#Object"/>
    <rdfs:range rdf:resource="http://w3id.org/arto#Scene"/>
    <rdfs:comment>Links objects to the scenes they appear in or are associated with.</rdfs:comment>
    <skos:example>
                      - Object context: :bread_loaf arto:relatedToScene :market_scene </skos:example>
    <rdfs:label>relatedToScene</rdfs:label>
  </owl:ObjectProperty>

  <owl:ObjectProperty rdf:about="http://w3id.org/arto#state">
    <rdfs:domain rdf:resource="http://w3id.org/arto#Object"/>
    <rdfs:range>
      <owl:Class>
        <owl:unionOf>
          <rdf:Description>
            <rdf:first rdf:resource="http://www.w3.org/2004/02/skos/core#Concept"/>
            <rdf:rest>
              <rdf:Description>
                <rdf:first rdf:resource="http://www.w3.org/2001/XMLSchema#string"/>
                <rdf:rest rdf:resource="http://www.w3.org/1999/02/22-rdf-syntax-ns#nil"/>
              </rdf:Description>
            </rdf:rest>

          </rdf:Description>
        </owl:unionOf>

      </owl:Class>
    </rdfs:range>

    <rdfs:comment>Describes the current condition, position, or status of objects within an artwork, which may be an AAT concept or free text.</rdfs:comment>
    <rdfs:label>state</rdfs:label>
  </owl:ObjectProperty>

  <owl:ObjectProperty rdf:about="http://w3id.org/arto#style">
    <rdfs:domain rdf:resource="http://w3id.org/arto#Artwork"/>
    <rdfs:range>
      <owl:Class rdf:about="http://w3id.org/arto#ArtStyleType">
        <rdfs:subClassOf rdf:resource="http://www.w3.org/2004/02/skos/core#Concept"/>
        <owl:equivalentClass>
          <rdf:Description>
            <owl:unionOf>
              <rdf:Description>
                <rdf:first>
                  <rdf:Description>
                    <owl:hasValue rdf:resource="http://vocab.getty.edu/aat/300015646"/>
                  </rdf:Description>
                </rdf:first>

                <rdf:rest>
                  <rdf:Description>
                    <rdf:first rdf:resource="http://www.w3.org/2004/02/skos/core#Concept"/>
                    <rdf:rest rdf:resource="http://www.w3.org/1999/02/22-rdf-syntax-ns#nil"/>
                  </rdf:Description>
                </rdf:rest>

              </rdf:Description>
            </owl:unionOf>

          </rdf:Description>
        </owl:equivalentClass>

      </owl:Class>
    </rdfs:range>

    <rdfs:comment>The style of the artwork.</rdfs:comment>
    <rdfs:label>style</rdfs:label>
  </owl:ObjectProperty>

  <owl:DatatypeProperty rdf:about="http://purl.org/dc/terms/medium">
  </owl:DatatypeProperty>

  <owl:DatatypeProperty rdf:about="http://w3id.org/arto#HSVValue">
    <rdfs:domain rdf:resource="http://w3id.org/arto#Color"/>
    <rdfs:range rdf:resource="http://www.w3.org/2001/XMLSchema#int"/>
    <rdfs:comment>HSV color value in format 'H,S,V' where H is the hue and the range is 0-360, S is the saturation and the range is 0-100, and V is the value and the range is 0-100</rdfs:comment>
    <rdfs:label>HSVValue</rdfs:label>
  </owl:DatatypeProperty>

  <owl:DatatypeProperty rdf:about="http://w3id.org/arto#RGBValue">
    <rdfs:domain rdf:resource="http://w3id.org/arto#Color"/>
    <rdfs:range rdf:resource="http://www.w3.org/2001/XMLSchema#int"/>
    <rdfs:comment>RGB color value in format 'R,G,B' where R,G,B are integers 0-255</rdfs:comment>
    <rdfs:label>RGBValue</rdfs:label>
  </owl:DatatypeProperty>

  <owl:DatatypeProperty rdf:about="http://w3id.org/arto#coordinates">
    <rdfs:domain>
      <owl:Class>
        <owl:unionOf>
          <rdf:Description>
            <rdf:first rdf:resource="http://w3id.org/arto#Object"/>
            <rdf:rest>
              <rdf:Description>
                <rdf:first rdf:resource="http://w3id.org/arto#Scene"/>
                <rdf:rest rdf:resource="http://www.w3.org/1999/02/22-rdf-syntax-ns#nil"/>
              </rdf:Description>
            </rdf:rest>

          </rdf:Description>
        </owl:unionOf>

      </owl:Class>
    </rdfs:domain>

    <rdfs:range rdf:resource="http://www.w3.org/2001/XMLSchema#string"/>
    <rdfs:comment>The coordinates of the Scene or the Object in the artwork.</rdfs:comment>
    <rdfs:label>coordinates</rdfs:label>
  </owl:DatatypeProperty>

  <owl:DatatypeProperty rdf:about="http://w3id.org/arto#descriptor">
    <rdfs:domain>
      <owl:Class>
        <owl:unionOf>
          <rdf:Description>
            <rdf:first rdf:resource="http://w3id.org/arto#Object"/>
            <rdf:rest>
              <rdf:Description>
                <rdf:first rdf:resource="http://w3id.org/arto#Scene"/>
                <rdf:rest>
                  <rdf:Description>
                    <rdf:first rdf:resource="http://w3id.org/arto#VisualElement"/>
                    <rdf:rest rdf:resource="http://www.w3.org/1999/02/22-rdf-syntax-ns#nil"/>
                  </rdf:Description>
                </rdf:rest>

              </rdf:Description>
            </rdf:rest>

          </rdf:Description>
        </owl:unionOf>

      </owl:Class>
    </rdfs:domain>

    <rdfs:range rdf:resource="http://www.w3.org/2001/XMLSchema#string"/>
    <rdfs:comment>Describes the visual characteristics or properties of an object in an artwork. The specific descriptors are specified using the rdfs:subPropertyOf.</rdfs:comment>
    <skos:example>
                Portrait1 :clothing :RedDress ;
                :clothing rdfs:subPropertyOf arto:descriptor</skos:example>
    <rdfs:label>descriptor</rdfs:label>
  </owl:DatatypeProperty>

  <owl:DatatypeProperty rdf:about="http://w3id.org/arto#direction">
    <rdfs:domain rdf:resource="http://w3id.org/arto#Line"/>
    <rdfs:range rdf:resource="http://www.w3.org/2001/XMLSchema#string"/>
    <rdfs:comment>Describes the orientation of linear elements in an artwork.</rdfs:comment>
    <rdfs:label>direction</rdfs:label>
  </owl:DatatypeProperty>

  <owl:DatatypeProperty rdf:about="http://w3id.org/arto#length">
    <rdfs:domain rdf:resource="http://w3id.org/arto#Line"/>
    <rdfs:range rdf:resource="http://www.w3.org/2001/XMLSchema#float"/>
    <rdfs:comment>The length of the line.</rdfs:comment>
    <rdfs:label>length</rdfs:label>
  </owl:DatatypeProperty>

  <owl:DatatypeProperty rdf:about="http://w3id.org/arto#material">
    <rdfs:domain rdf:resource="http://w3id.org/arto#Object"/>
    <rdfs:range>
      <owl:Class rdf:about="http://w3id.org/arto#MaterialType">
        <rdfs:subClassOf rdf:resource="http://www.w3.org/2004/02/skos/core#Concept"/>
        <owl:equivalentClass>
          <rdf:Description>
            <owl:unionOf>
              <rdf:Description>
                <rdf:first>
                  <rdf:Description>
                    <owl:hasValue rdf:resource="http://vocab.getty.edu/aat/300264091"/>
                  </rdf:Description>
                </rdf:first>

                <rdf:rest>
                  <rdf:Description>
                    <rdf:first rdf:resource="http://www.w3.org/2004/02/skos/core#Concept"/>
                    <rdf:rest rdf:resource="http://www.w3.org/1999/02/22-rdf-syntax-ns#nil"/>
                  </rdf:Description>
                </rdf:rest>

              </rdf:Description>
            </owl:unionOf>

          </rdf:Description>
        </owl:equivalentClass>

      </owl:Class>
    </rdfs:range>

    <rdfs:comment>The material of the Object.</rdfs:comment>
    <rdfs:label>material</rdfs:label>
  </owl:DatatypeProperty>

  <owl:DatatypeProperty rdf:about="http://w3id.org/arto#size">
    <rdfs:domain>
      <owl:Class>
        <owl:unionOf>
          <rdf:Description>
            <rdf:first rdf:resource="http://w3id.org/arto#Object"/>
            <rdf:rest>
              <rdf:Description>
                <rdf:first rdf:resource="http://w3id.org/arto#Scene"/>
                <rdf:rest rdf:resource="http://www.w3.org/1999/02/22-rdf-syntax-ns#nil"/>
              </rdf:Description>
            </rdf:rest>

          </rdf:Description>
        </owl:unionOf>

      </owl:Class>
    </rdfs:domain>

    <rdfs:range rdf:resource="http://www.w3.org/2001/XMLSchema#string"/>
    <rdfs:comment>The size of the Scene or the Object in the artwork.</rdfs:comment>
    <rdfs:label>size</rdfs:label>
  </owl:DatatypeProperty>

  <owl:DatatypeProperty rdf:about="http://w3id.org/arto#source">
    <rdfs:domain rdf:resource="http://w3id.org/arto#Symbolism"/>
    <rdfs:range rdf:resource="http://www.w3.org/2001/XMLSchema#string"/>
    <rdfs:comment>Relates the source of the symbolism in artworks.</rdfs:comment>
    <rdfs:label>source</rdfs:label>
  </owl:DatatypeProperty>

  <owl:Class rdf:about="http://w3id.org/arto#Agent">
    <rdfs:subClassOf>
      <owl:Class rdf:about="http://xmlns.com/foaf/spec/Agent">
      </owl:Class>
    </rdfs:subClassOf>

    <rdfs:subClassOf>
      <owl:Restriction>
        <owl:onProperty rdf:resource="http://w3id.org/arto#hasLocation"/>
        <owl:allValuesFrom rdf:resource="http://w3id.org/arto#Location"/>
      </owl:Restriction>
    </rdfs:subClassOf>

    <rdfs:comment>Represents an Agent.This class comprises people, either individually or in groups,
      who have the potential to perform intentional actions for which they can be held responsible.</rdfs:comment>
    <rdfs:label>Agent</rdfs:label>
  </owl:Class>

  <owl:Class rdf:about="http://w3id.org/arto#Artist">
    <rdfs:subClassOf rdf:resource="http://w3id.org/arto#Person"/>
    <rdfs:comment>The person or group who create or contribute the artwork.</rdfs:comment>
    <rdfs:label>Artist</rdfs:label>
  </owl:Class>

  <owl:Class rdf:about="http://w3id.org/arto#Artwork">
    <rdfs:subClassOf>
      <owl:Class rdf:about="https://schema.org/CreativeWork">
      </owl:Class>
    </rdfs:subClassOf>

    <rdfs:subClassOf>
      <owl:Restriction>
        <owl:onProperty rdf:resource="http://purl.org/dc/terms/contributor"/>
        <owl:allValuesFrom rdf:resource="http://w3id.org/arto#Agent"/>
      </owl:Restriction>
    </rdfs:subClassOf>

    <rdfs:subClassOf>
      <owl:Restriction>
        <owl:onProperty rdf:resource="http://purl.org/dc/terms/creator"/>
        <owl:allValuesFrom rdf:resource="http://w3id.org/arto#Artist"/>
        <owl:minCardinality rdf:datatype="http://www.w3.org/2001/XMLSchema#nonNegativeInteger">1</owl:minCardinality>
      </owl:Restriction>
    </rdfs:subClassOf>

    <rdfs:subClassOf>
      <owl:Restriction>
        <owl:onProperty rdf:resource="http://purl.org/dc/terms/isPartOf"/>
        <owl:allValuesFrom rdf:resource="http://w3id.org/arto#Series"/>
      </owl:Restriction>
    </rdfs:subClassOf>

    <rdfs:subClassOf>
      <owl:Restriction>
        <owl:onProperty rdf:resource="http://purl.org/dc/terms/description"/>
        <owl:allValuesFrom rdf:resource="http://www.w3.org/2001/XMLSchema#string"/>
        <owl:minCardinality rdf:datatype="http://www.w3.org/2001/XMLSchema#nonNegativeInteger">1</owl:minCardinality>
      </owl:Restriction>
    </rdfs:subClassOf>

    <rdfs:subClassOf>
      <owl:Restriction>
        <owl:onProperty rdf:resource="http://purl.org/dc/terms/medium"/>
        <owl:allValuesFrom rdf:resource="http://www.w3.org/2001/XMLSchema#string"/>
        <owl:minCardinality rdf:datatype="http://www.w3.org/2001/XMLSchema#nonNegativeInteger">1</owl:minCardinality>
      </owl:Restriction>
    </rdfs:subClassOf>

    <rdfs:subClassOf>
      <owl:Restriction>
        <owl:onProperty rdf:resource="http://w3id.org/arto#expresses"/>
        <owl:allValuesFrom rdf:resource="http://w3id.org/arto#Connotation"/>
      </owl:Restriction>
    </rdfs:subClassOf>

    <rdfs:subClassOf>
      <owl:Restriction>
        <owl:onProperty rdf:resource="https://dbpedia.org/property/technique"/>
        <owl:allValuesFrom rdf:resource="http://www.w3.org/2001/XMLSchema#string"/>
      </owl:Restriction>
    </rdfs:subClassOf>

    <rdfs:subClassOf>
      <owl:Restriction>
        <owl:onProperty rdf:resource="http://purl.org/dc/terms/title"/>
        <owl:allValuesFrom rdf:resource="http://www.w3.org/2001/XMLSchema#string"/>
        <owl:minCardinality rdf:datatype="http://www.w3.org/2001/XMLSchema#nonNegativeInteger">1</owl:minCardinality>
      </owl:Restriction>
    </rdfs:subClassOf>

    <rdfs:subClassOf>
      <owl:Restriction>
        <owl:onProperty rdf:resource="https://schema.org/height"/>
        <owl:allValuesFrom rdf:resource="http://www.w3.org/2001/XMLSchema#string"/>
        <owl:cardinality rdf:datatype="http://www.w3.org/2001/XMLSchema#nonNegativeInteger">1</owl:cardinality>
      </owl:Restriction>
    </rdfs:subClassOf>

    <rdfs:subClassOf>
      <owl:Restriction>
        <owl:onProperty rdf:resource="https://schema.org/width"/>
        <owl:allValuesFrom rdf:resource="http://www.w3.org/2001/XMLSchema#string"/>
        <owl:cardinality rdf:datatype="http://www.w3.org/2001/XMLSchema#nonNegativeInteger">1</owl:cardinality>
      </owl:Restriction>
    </rdfs:subClassOf>

    <rdfs:subClassOf>
      <owl:Restriction>
        <owl:onProperty rdf:resource="http://www.europeana.eu/schemas/edm/isShownBy"/>
        <owl:allValuesFrom rdf:resource="http://www.w3.org/2001/XMLSchema#anyURI"/>
        <owl:minCardinality rdf:datatype="http://www.w3.org/2001/XMLSchema#nonNegativeInteger">1</owl:minCardinality>
      </owl:Restriction>
    </rdfs:subClassOf>

    <rdfs:subClassOf>
      <owl:Restriction>
        <owl:onProperty rdf:resource="http://w3id.org/arto#style"/>
        <owl:allValuesFrom rdf:resource="http://www.w3.org/2001/XMLSchema#string"/>
        <owl:minCardinality rdf:datatype="http://www.w3.org/2001/XMLSchema#nonNegativeInteger">1</owl:minCardinality>
      </owl:Restriction>
    </rdfs:subClassOf>

    <rdfs:subClassOf>
      <owl:Restriction>
        <owl:onProperty rdf:resource="https://schema.org/genre"/>
        <owl:allValuesFrom rdf:resource="http://www.w3.org/2001/XMLSchema#string"/>
        <owl:minCardinality rdf:datatype="http://www.w3.org/2001/XMLSchema#nonNegativeInteger">1</owl:minCardinality>
      </owl:Restriction>
    </rdfs:subClassOf>

    <rdfs:subClassOf>
      <owl:Restriction>
        <owl:onProperty rdf:resource="http://w3id.org/arto#currentLocation"/>
        <owl:allValuesFrom rdf:resource="http://w3id.org/arto#Location"/>
        <owl:cardinality rdf:datatype="http://www.w3.org/2001/XMLSchema#nonNegativeInteger">1</owl:cardinality>
      </owl:Restriction>
    </rdfs:subClassOf>

    <rdfs:subClassOf>
      <owl:Restriction>
        <owl:onProperty rdf:resource="http://w3id.org/arto#relatedToEvent"/>
        <owl:allValuesFrom rdf:resource="http://w3id.org/arto#Event"/>
      </owl:Restriction>
    </rdfs:subClassOf>

    <rdfs:subClassOf>
      <owl:Restriction>
        <owl:onProperty rdf:resource="http://w3id.org/arto#expresses"/>
        <owl:allValuesFrom rdf:resource="http://w3id.org/arto#Connotation"/>
      </owl:Restriction>
    </rdfs:subClassOf>

    <rdfs:subClassOf>
      <owl:Restriction>
        <owl:onProperty rdf:resource="http://w3id.org/arto#containsScene"/>
        <owl:allValuesFrom rdf:resource="http://w3id.org/arto#Scene"/>
        <owl:minCardinality rdf:datatype="http://www.w3.org/2001/XMLSchema#nonNegativeInteger">1</owl:minCardinality>
      </owl:Restriction>
    </rdfs:subClassOf>

    <rdfs:comment>A created object or piece of art that is intended to be aesthetically pleasing or
                convey a message.
                </rdfs:comment>
    <rdfs:label>Artwork</rdfs:label>
    <skos:closeMatch rdf:resource="http://www.cidoc-crm.org/cidoc-crm/E22_Human_Made_Object"/>
    <skos:closeMatch rdf:resource="https://w3id.org/icon/ontology/Artwork"/>
  </owl:Class>

  <owl:Class rdf:about="http://w3id.org/arto#Series">
    <rdfs:subClassOf>
      <owl:Class rdf:about="https://schema.org/CreativeWorkSeries">
      </owl:Class>
    </rdfs:subClassOf>

    <rdfs:subClassOf>
      <owl:Restriction>
        <owl:onProperty rdf:resource="http://purl.org/dc/terms/creator"/>
        <owl:allValuesFrom rdf:resource="http://w3id.org/arto#Artist"/>
        <owl:minCardinality rdf:datatype="http://www.w3.org/2001/XMLSchema#nonNegativeInteger">1</owl:minCardinality>
      </owl:Restriction>
    </rdfs:subClassOf>

    <rdfs:comment>A collection of related artworks that share common characteristics, themes, or purposes, including:
        - Thematic series
        - Chronological series
        - Technique-based series
        - Subject-based series
        - Experimental series
        - Documentary series</rdfs:comment>
    <rdfs:label>Series</rdfs:label>
    <skos:closeMatch rdf:resource="http://www.cidoc-crm.org/cidoc-crm/E78_Collection"/>
  </owl:Class>
  

  <owl:Class rdf:about="http://w3id.org/arto#BalanceOfComposition">
    <rdfs:subClassOf rdf:resource="http://w3id.org/arto#Metric"/>
    <rdfs:comment>Represents the degree of visual equilibrium or harmony in the arrangement of
      elements within an artwork, considering factors such as symmetry, asymmetry, and distribution
      of
      visual elements.</rdfs:comment>
    <rdfs:label>BalanceOfComposition</rdfs:label>
  </owl:Class>

  <owl:Class rdf:about="http://w3id.org/arto#Character">
    <rdfs:subClassOf rdf:resource="http://w3id.org/arto#Person"/>
    <rdfs:comment>Represents persons, figures, or beings depicted within an artwork.</rdfs:comment>
    <rdfs:label>Character</rdfs:label>
  </owl:Class>

  <owl:Class rdf:about="http://w3id.org/arto#Color">
    <rdfs:subClassOf rdf:resource="http://w3id.org/arto#VisualElement"/>
    <rdfs:subClassOf>
      <owl:Restriction>
        <owl:onProperty rdf:resource="http://w3id.org/arto#RGBValue"/>
        <owl:allValuesFrom rdf:resource="http://www.w3.org/2001/XMLSchema#string"/>
        <owl:cardinality rdf:datatype="http://www.w3.org/2001/XMLSchema#nonNegativeInteger">1</owl:cardinality>
      </owl:Restriction>
    </rdfs:subClassOf>

    <rdfs:subClassOf>
      <owl:Restriction>
        <owl:onProperty rdf:resource="http://w3id.org/arto#HSVValue"/>
        <owl:allValuesFrom rdf:resource="http://www.w3.org/2001/XMLSchema#string"/>
        <owl:cardinality rdf:datatype="http://www.w3.org/2001/XMLSchema#nonNegativeInteger">1</owl:cardinality>
      </owl:Restriction>
    </rdfs:subClassOf>

    <skos:closeMatch rdf:resource="http://vocab.getty.edu/aat/300131647"/>
    <rdfs:comment>The use of color in the artwork.</rdfs:comment>
    <rdfs:label>Color</rdfs:label>
  </owl:Class>

  <owl:Class rdf:about="http://w3id.org/arto#ColorHistogram">
    <rdfs:subClassOf rdf:resource="http://w3id.org/arto#Metric"/>
    <rdfs:comment>Represents the distribution of colors in an artwork, typically expressed as a
      histogram or a quantitative representation of the frequency or proportion of each color
      present in
      the artwork.</rdfs:comment>
    <rdfs:label>ColorHistogram</rdfs:label>
  </owl:Class>

  <owl:Class rdf:about="http://w3id.org/arto#Composition">
    <rdfs:subClassOf rdf:resource="http://w3id.org/arto#VisualElement"/>
    <rdfs:subClassOf>
      <owl:Restriction>
        <owl:onProperty rdf:resource="http://purl.org/dc/terms/type"/>
        <owl:allValuesFrom rdf:resource="http://www.w3.org/2001/XMLSchema#string"/>
        <owl:cardinality rdf:datatype="http://www.w3.org/2001/XMLSchema#nonNegativeInteger">1</owl:cardinality>
      </owl:Restriction>
    </rdfs:subClassOf>

    <skos:closeMatch rdf:resource="http://vocab.getty.edu/aat/300056255"/>
    <rdfs:comment>The arrangement and organization of visual elements.</rdfs:comment>
    <rdfs:label>Composition</rdfs:label>
  </owl:Class>

  <owl:Class rdf:about="http://w3id.org/arto#Connotation">
    <rdfs:subClassOf>
      <owl:Class rdf:about="http://www.cidoc-crm.org/cidoc-crm/E28_Conceptual_Object">
      </owl:Class>
    </rdfs:subClassOf>

    <rdfs:subClassOf>
      <owl:Restriction>
        <owl:onProperty rdf:resource="http://w3id.org/arto#hasMetric"/>
        <owl:allValuesFrom rdf:resource="http://w3id.org/arto#Metric"/>
      </owl:Restriction>
    </rdfs:subClassOf>

    <rdfs:comment>Represents the implied meanings of artwork, includeing themes, symbolic meanings, and
      emotions conveyed by an artwork.</rdfs:comment>
    <rdfs:label>Connotation</rdfs:label>
  </owl:Class>

  <owl:Class rdf:about="http://w3id.org/arto#Emotion">
    <rdfs:subClassOf rdf:resource="http://w3id.org/arto#Connotation"/>
    <rdfs:subClassOf>
      <owl:Restriction>
        <owl:onProperty rdf:resource="http://purl.org/dc/terms/type"/>
        <owl:allValuesFrom rdf:resource="http://www.w3.org/2001/XMLSchema#string"/>
        <owl:cardinality rdf:datatype="http://www.w3.org/2001/XMLSchema#nonNegativeInteger">1</owl:cardinality>
      </owl:Restriction>
    </rdfs:subClassOf>

    <skos:closeMatch rdf:resource="http://vocab.getty.edu/aat/300055150"/>
    <rdfs:comment>Represents the emotional response or affective state evoked by an artwork in the
      artist or viewers, such as joy, sadness, anger, or fear.</rdfs:comment>
    <rdfs:label>Emotion</rdfs:label>
  </owl:Class>

  <owl:Class rdf:about="http://w3id.org/arto#EmotionIntensity">
    <rdfs:subClassOf rdf:resource="http://w3id.org/arto#Metric"/>
    <rdfs:comment>Represents the strength or degree of emotional response evoked by an artwork.</rdfs:comment>
    <rdfs:label>EmotionIntensity</rdfs:label>
  </owl:Class>

  <owl:Class rdf:about="http://w3id.org/arto#Event">
    <rdfs:subClassOf rdf:resource="http://purl.org/NET/c4dm/event.owl#Event"/>
    <rdfs:subClassOf>
      <owl:Restriction>
        <owl:onProperty rdf:resource="http://purl.org/NET/c4dm/event.owl#agent"/>
        <owl:allValuesFrom rdf:resource="http://w3id.org/arto#Agent"/>
        <owl:minCardinality rdf:datatype="http://www.w3.org/2001/XMLSchema#nonNegativeInteger">1</owl:minCardinality>
      </owl:Restriction>
    </rdfs:subClassOf>

    <rdfs:subClassOf>
      <owl:Restriction>
        <owl:onProperty rdf:resource="http://purl.org/dc/terms/type"/>
        <owl:allValuesFrom rdf:resource="http://www.w3.org/2001/XMLSchema#string"/>
        <owl:cardinality rdf:datatype="http://www.w3.org/2001/XMLSchema#nonNegativeInteger">1</owl:cardinality>
      </owl:Restriction>
    </rdfs:subClassOf>

    <rdfs:subClassOf>
      <owl:Restriction>
        <owl:onProperty rdf:resource="http://w3id.org/arto#hasTime"/>
        <owl:allValuesFrom rdf:resource="http://w3id.org/arto#Time"/>
        <owl:minCardinality rdf:datatype="http://www.w3.org/2001/XMLSchema#nonNegativeInteger">1</owl:minCardinality>
      </owl:Restriction>
    </rdfs:subClassOf>

    <rdfs:subClassOf>
      <owl:Restriction>
        <owl:onProperty rdf:resource="http://w3id.org/arto#hasLocation"/>
        <owl:allValuesFrom rdf:resource="http://w3id.org/arto#Location"/>
        <owl:minCardinality rdf:datatype="http://www.w3.org/2001/XMLSchema#nonNegativeInteger">1</owl:minCardinality>
      </owl:Restriction>
    </rdfs:subClassOf>

    <rdfs:subClassOf>
      <owl:Restriction>
        <owl:onProperty rdf:resource="http://w3id.org/arto#relatedToConnotation"/>
        <owl:allValuesFrom rdf:resource="http://w3id.org/arto#Connotation"/>
      </owl:Restriction>
    </rdfs:subClassOf>

    <rdfs:comment>
      An arbitrary classification of a space/time region, by a
      cognitive agent. An event may have actively participating agents,
      passive factors, products, and a location in space/time.</rdfs:comment>
    <rdfs:label>Event</rdfs:label>
    <skos:closeMatch rdf:resource="http://www.cidoc-crm.org/cidoc-crm/E5_Event"/>
  </owl:Class>

  <owl:Class rdf:about="http://w3id.org/arto#Line">
    <rdfs:subClassOf rdf:resource="http://w3id.org/arto#VisualElement"/>
    <rdfs:subClassOf>
      <owl:Restriction>
        <owl:onProperty rdf:resource="https://schema.org/width"/>
        <owl:allValuesFrom rdf:resource="http://www.w3.org/2001/XMLSchema#string"/>
        <owl:cardinality rdf:datatype="http://www.w3.org/2001/XMLSchema#nonNegativeInteger">1</owl:cardinality>
      </owl:Restriction>
    </rdfs:subClassOf>

    <rdfs:subClassOf>
      <owl:Restriction>
        <owl:onProperty rdf:resource="http://w3id.org/arto#direction"/>
        <owl:allValuesFrom rdf:resource="http://www.w3.org/2001/XMLSchema#string"/>
        <owl:cardinality rdf:datatype="http://www.w3.org/2001/XMLSchema#nonNegativeInteger">1</owl:cardinality>
      </owl:Restriction>
    </rdfs:subClassOf>

    <rdfs:subClassOf>
      <owl:Restriction>
        <owl:onProperty rdf:resource="http://w3id.org/arto#length"/>
        <owl:allValuesFrom rdf:resource="http://www.w3.org/2001/XMLSchema#float"/>
        <owl:cardinality rdf:datatype="http://www.w3.org/2001/XMLSchema#nonNegativeInteger">1</owl:cardinality>
      </owl:Restriction>
    </rdfs:subClassOf>

    <rdfs:subClassOf>
      <owl:Restriction>
        <owl:onProperty rdf:resource="http://purl.org/dc/terms/type"/>
        <owl:allValuesFrom rdf:resource="http://www.w3.org/2001/XMLSchema#string"/>
        <owl:cardinality rdf:datatype="http://www.w3.org/2001/XMLSchema#nonNegativeInteger">1</owl:cardinality>
      </owl:Restriction>
    </rdfs:subClassOf>

    <rdfs:comment>Represents linear elements in artwork, including their characteristics and functions:
            - Types of lines (straight, curved, implied)
            - Line qualities (thick, thin, broken, continuous)
            - Directional lines
            - Contour lines
            - Gestural lines
            - Structural lines</rdfs:comment>
    <rdfs:label>Line</rdfs:label>
  </owl:Class>

  <owl:Class rdf:about="http://w3id.org/arto#Location">
    <rdfs:subClassOf rdf:resource="https://schema.org/Place"/>
    <rdfs:subClassOf>
      <owl:Restriction>
        <owl:onProperty rdf:resource="http://www.opengis.net/ont/geosparql#asWKT"/>
        <owl:allValuesFrom rdf:resource="http://www.opengis.net/ont/geosparql#wktLiteral"/>
      </owl:Restriction>
    </rdfs:subClassOf>

    <rdfs:subClassOf>
      <owl:Restriction>
        <owl:onProperty rdf:resource="http://w3id.org/arto#hasTime"/>
        <owl:allValuesFrom rdf:resource="http://w3id.org/arto#Time"/>
      </owl:Restriction>
    </rdfs:subClassOf>

    <rdfs:subClassOf>
      <owl:Restriction>
        <owl:onProperty rdf:resource="http://purl.org/dc/terms/type"/>
        <owl:allValuesFrom rdf:resource="http://www.w3.org/2001/XMLSchema#string"/>
        <owl:cardinality rdf:datatype="http://www.w3.org/2001/XMLSchema#nonNegativeInteger">1</owl:cardinality>
      </owl:Restriction>
    </rdfs:subClassOf>

    <rdfs:comment>Represents a physical or virtual space associated with an artwork.</rdfs:comment>
    <rdfs:label>Location</rdfs:label>
    <skos:closeMatch rdf:resource="http://www.cidoc-crm.org/cidoc-crm/E53_Place"/>
  </owl:Class>

  <owl:Class rdf:about="http://w3id.org/arto#MainColor">
    <rdfs:subClassOf rdf:resource="http://w3id.org/arto#Metric"/>
    <rdfs:comment>Represents the dominant or most prominent color in an artwork, which can be
      determined through visual analysis or color quantization techniques.</rdfs:comment>
    <rdfs:label>MainColor</rdfs:label>
  </owl:Class>

  <owl:Class rdf:about="http://w3id.org/arto#Symbolism">
    <rdfs:subClassOf rdf:resource="http://w3id.org/arto#Connotation"/>
    <rdfs:subClassOf>
      <owl:Restriction>
        <owl:onProperty rdf:resource="http://w3id.org/arto#source"/>
        <owl:allValuesFrom rdf:resource="http://www.w3.org/2001/XMLSchema#string"/>
      </owl:Restriction>
    </rdfs:subClassOf>

    <rdfs:comment>Represents the symbolism conveyed by the object, scene or the visual elements.</rdfs:comment>
    <rdfs:label>Symbolism</rdfs:label>
    <skos:closeMatch rdf:resource="https://w3id.org/icon/ontology/Symbol"/>
  </owl:Class>

  <owl:Class rdf:about="http://w3id.org/arto#Metric">
    <rdfs:comment>Represents a quantifiable measurement or characteristic of an artwork,
      encompassing statistical information about basic elements such as color statistics, emotion
      intensity, balance of composition, and other visual elements, to facilitate structural
      analysis
      and comparison of artworks.</rdfs:comment>
    <rdfs:label>Metric</rdfs:label>
  </owl:Class>

  <owl:Class rdf:about="http://w3id.org/arto#Object">
    <rdfs:subClassOf>
      <owl:Restriction>
        <owl:onProperty rdf:resource="http://w3id.org/arto#expresses"/>
        <owl:someValuesFrom rdf:resource="http://w3id.org/arto#Symbolism"/>
      </owl:Restriction>
    </rdfs:subClassOf>

    <rdfs:subClassOf>
      <owl:Restriction>
        <owl:onProperty rdf:resource="http://w3id.org/arto#relatedToScene"/>
        <owl:allValuesFrom rdf:resource="http://w3id.org/arto#Scene"/>
        <owl:minCardinality rdf:datatype="http://www.w3.org/2001/XMLSchema#nonNegativeInteger">1</owl:minCardinality>
      </owl:Restriction>
    </rdfs:subClassOf>

    <rdfs:subClassOf>
      <owl:Restriction>
        <owl:onProperty rdf:resource="http://w3id.org/arto#relatedTo"/>
        <owl:allValuesFrom rdf:resource="http://w3id.org/arto#Object"/>
      </owl:Restriction>
    </rdfs:subClassOf>

    <rdfs:subClassOf>
      <owl:Restriction>
        <owl:onProperty rdf:resource="http://w3id.org/arto#hasMetric"/>
        <owl:allValuesFrom rdf:resource="http://w3id.org/arto#Metric"/>
      </owl:Restriction>
    </rdfs:subClassOf>

    <rdfs:subClassOf>
      <owl:Restriction>
        <owl:onProperty rdf:resource="http://w3id.org/arto#state"/>
        <owl:allValuesFrom rdf:resource="http://www.w3.org/2001/XMLSchema#string"/>
      </owl:Restriction>
    </rdfs:subClassOf>

    <rdfs:subClassOf>
      <owl:Restriction>
        <owl:onProperty rdf:resource="http://w3id.org/arto#material"/>
        <owl:allValuesFrom rdf:resource="http://www.w3.org/2001/XMLSchema#string"/>
      </owl:Restriction>
    </rdfs:subClassOf>

    <rdfs:subClassOf>
      <owl:Restriction>
        <owl:onProperty rdf:resource="http://w3id.org/arto#coordinates"/>
        <owl:allValuesFrom rdf:resource="http://www.w3.org/2001/XMLSchema#string"/>
        <owl:cardinality rdf:datatype="http://www.w3.org/2001/XMLSchema#nonNegativeInteger">1</owl:cardinality>
      </owl:Restriction>
    </rdfs:subClassOf>

    <rdfs:subClassOf>
      <owl:Restriction>
        <owl:onProperty rdf:resource="http://w3id.org/arto#size"/>
        <owl:allValuesFrom rdf:resource="http://www.w3.org/2001/XMLSchema#string"/>
        <owl:cardinality rdf:datatype="http://www.w3.org/2001/XMLSchema#nonNegativeInteger">1</owl:cardinality>
      </owl:Restriction>
    </rdfs:subClassOf>

    <rdfs:subClassOf>
      <owl:Restriction>
        <owl:onProperty rdf:resource="http://w3id.org/arto#descriptor"/>
        <owl:allValuesFrom rdf:resource="http://www.w3.org/2001/XMLSchema#string"/>
      </owl:Restriction>
    </rdfs:subClassOf>

    <rdfs:comment>Represents the physical or conceptual object within an artwork.</rdfs:comment>
    <rdfs:label>Object</rdfs:label>
    <skos:relatedMatch rdf:resource="https://w3id.org/icon/ontology/ArtisticMotif"/>
  </owl:Class>

  <owl:Class rdf:about="http://w3id.org/arto#Organization">
    <rdfs:subClassOf rdf:resource="http://w3id.org/arto#Agent"/>
    <rdfs:subClassOf>
      <owl:Class rdf:about="http://xmlns.com/foaf/spec/Organization">
      </owl:Class>
    </rdfs:subClassOf>

    <owl:disjointWith rdf:resource="http://w3id.org/arto#Person"/>
    <rdfs:comment>The Organization class represents a kind of Agent corresponding to instititutions
      such as galleries, museums etc.</rdfs:comment>
    <rdfs:label>Organization</rdfs:label>
  </owl:Class>

  <owl:Class rdf:about="http://w3id.org/arto#Painting">
    <rdfs:subClassOf rdf:resource="http://w3id.org/arto#Artwork"/>
    <rdfs:comment>A specific type of artwork created using paint or similar media. </rdfs:comment>
    <rdfs:label>Painting</rdfs:label>
  </owl:Class>

  <owl:Class rdf:about="http://w3id.org/arto#Person">
    <rdfs:subClassOf rdf:resource="http://w3id.org/arto#Agent"/>
    <rdfs:subClassOf>
      <owl:Class rdf:about="http://xmlns.com/foaf/spec/Person">
      </owl:Class>
    </rdfs:subClassOf>

    <rdfs:subClassOf>
      <owl:Restriction>
        <owl:onProperty rdf:resource="https://dbpedia.org/property/residence"/>
        <owl:allValuesFrom rdf:resource="http://w3id.org/arto#Location"/>
      </owl:Restriction>
    </rdfs:subClassOf>

    <rdfs:subClassOf>
      <owl:Restriction>
        <owl:onProperty rdf:resource="http://w3id.org/arto#knows"/>
        <owl:allValuesFrom rdf:resource="http://w3id.org/arto#Person"/>
      </owl:Restriction>
    </rdfs:subClassOf>

    <rdfs:comment>Individual human beings involved with artwork may include artists, curators, critics, collectors, conservators, researchers, and other roles.</rdfs:comment>
    <rdfs:label>Person</rdfs:label>
  </owl:Class>

  <owl:Class rdf:about="http://w3id.org/arto#Photograph">
    <rdfs:subClassOf rdf:resource="http://w3id.org/arto#Artwork"/>
    <rdfs:comment>A specific type of artwork created using photography or similar media. </rdfs:comment>
    <rdfs:label>Photograph</rdfs:label>
  </owl:Class>

  <owl:Class rdf:about="http://w3id.org/arto#Relevance">
    <rdfs:subClassOf rdf:resource="http://w3id.org/arto#Metric"/>
    <rdfs:comment>Measures and describes the significance or importance of elements within an artwork, including:
                  - Thematic relevance
                  - Visual importance
                  - Symbolic significance
                  - Narrative relevance
                  - Historical relevance
                  - Compositional importance</rdfs:comment>
    <rdfs:label>Relevance</rdfs:label>
  </owl:Class>

  <owl:Class rdf:about="http://w3id.org/arto#Scene">
    <rdfs:subClassOf>
      <owl:Restriction>
        <owl:onProperty rdf:resource="http://w3id.org/arto#containsObject"/>
        <owl:allValuesFrom rdf:resource="http://w3id.org/arto#Object"/>
      </owl:Restriction>
    </rdfs:subClassOf>

    <rdfs:subClassOf>
      <owl:Restriction>
        <owl:onProperty rdf:resource="http://w3id.org/arto#containsScene"/>
        <owl:allValuesFrom rdf:resource="http://w3id.org/arto#Scene"/>
      </owl:Restriction>
    </rdfs:subClassOf>

    <rdfs:subClassOf>
      <owl:Restriction>
        <owl:onProperty rdf:resource="http://w3id.org/arto#hasMetric"/>
        <owl:allValuesFrom rdf:resource="http://w3id.org/arto#Metric"/>
      </owl:Restriction>
    </rdfs:subClassOf>

    <rdfs:subClassOf>
      <owl:Restriction>
        <owl:onProperty rdf:resource="http://w3id.org/arto#expresses"/>
        <owl:allValuesFrom rdf:resource="http://w3id.org/arto#Connotation"/>
      </owl:Restriction>
    </rdfs:subClassOf>

    <rdfs:subClassOf>
      <owl:Restriction>
        <owl:onProperty rdf:resource="http://w3id.org/arto#coordinates"/>
        <owl:allValuesFrom rdf:resource="http://www.w3.org/2001/XMLSchema#string"/>
        <owl:cardinality rdf:datatype="http://www.w3.org/2001/XMLSchema#nonNegativeInteger">1</owl:cardinality>
      </owl:Restriction>
    </rdfs:subClassOf>

    <rdfs:subClassOf>
      <owl:Restriction>
        <owl:onProperty rdf:resource="http://w3id.org/arto#size"/>
        <owl:allValuesFrom rdf:resource="http://www.w3.org/2001/XMLSchema#string"/>
        <owl:cardinality rdf:datatype="http://www.w3.org/2001/XMLSchema#nonNegativeInteger">1</owl:cardinality>
      </owl:Restriction>
    </rdfs:subClassOf>

    <rdfs:subClassOf>
      <owl:Restriction>
        <owl:onProperty rdf:resource="http://w3id.org/arto#descriptor"/>
        <owl:allValuesFrom rdf:resource="http://www.w3.org/2001/XMLSchema#string"/>
      </owl:Restriction>
    </rdfs:subClassOf>

    <rdfs:subClassOf>
      <owl:Restriction>
        <owl:onProperty rdf:resource="http://w3id.org/arto#relatedToEvent"/>
        <owl:allValuesFrom rdf:resource="http://w3id.org/arto#Event"/>
      </owl:Restriction>
    </rdfs:subClassOf>

    <rdfs:comment>Represents a distinct portion or area of an artwork that forms a coherent visual or narrative unit. </rdfs:comment>
    <rdfs:label>Scene</rdfs:label>
    <skos:closeMatch rdf:resource="https://w3id.org/icon/ontology/Image"/>
  </owl:Class>

  <owl:Class rdf:about="http://w3id.org/arto#Sculpture">
    <rdfs:subClassOf rdf:resource="http://w3id.org/arto#Artwork"/>
    <rdfs:comment>A specific type of artwork created using sculptural techniques, such as carving,
      modelling, or casting.</rdfs:comment>
    <rdfs:label>Sculpture</rdfs:label>
  </owl:Class>

  <owl:Class rdf:about="http://w3id.org/arto#Space">
    <rdfs:subClassOf rdf:resource="http://w3id.org/arto#VisualElement"/>
    <rdfs:subClassOf>
      <owl:Restriction>
        <owl:onProperty rdf:resource="http://purl.org/dc/terms/type"/>
        <owl:allValuesFrom rdf:resource="http://www.w3.org/2001/XMLSchema#string"/>
      </owl:Restriction>
    </rdfs:subClassOf>

    <rdfs:comment>Represents the spatial elements and relationships within an artwork.</rdfs:comment>
    <rdfs:label>Space</rdfs:label>
  </owl:Class>

  <owl:Class rdf:about="http://w3id.org/arto#Sponsor">
    <rdfs:subClassOf rdf:resource="http://w3id.org/arto#Person"/>
    <rdfs:comment>The person or group who sponsor the artwork.</rdfs:comment>
    <rdfs:label>Sponsor</rdfs:label>
  </owl:Class>

  <owl:Class rdf:about="http://w3id.org/arto#Theme">
    <rdfs:subClassOf rdf:resource="http://w3id.org/arto#Connotation"/>
    <rdfs:comment>Represents a central idea, subject, or concept explored in an artwork, which can
      be explicit or implicit, and may reflect broader cultural, social, or political issues.</rdfs:comment>
    <rdfs:label>Theme</rdfs:label>
  </owl:Class>

  <owl:Class rdf:about="http://w3id.org/arto#Time">
    <owl:equivalentClass>
      <owl:Class rdf:about="http://www.w3.org/2006/time#TemporalEntity">
      </owl:Class>
    </owl:equivalentClass>

    <rdfs:subClassOf>
      <owl:Restriction>
        <owl:onProperty rdf:resource="https://schema.org/endDate"/>
        <owl:allValuesFrom rdf:resource="http://www.w3.org/2001/XMLSchema#dateTime"/>
        <owl:cardinality rdf:datatype="http://www.w3.org/2001/XMLSchema#nonNegativeInteger">1</owl:cardinality>
      </owl:Restriction>
    </rdfs:subClassOf>

    <rdfs:subClassOf>
      <owl:Restriction>
        <owl:onProperty rdf:resource="https://schema.org/startDate"/>
        <owl:allValuesFrom rdf:resource="http://www.w3.org/2001/XMLSchema#dateTime"/>
        <owl:cardinality rdf:datatype="http://www.w3.org/2001/XMLSchema#nonNegativeInteger">1</owl:cardinality>
      </owl:Restriction>
    </rdfs:subClassOf>

    <rdfs:subClassOf>
      <owl:Restriction>
        <owl:onProperty rdf:resource="http://purl.org/dc/terms/type"/>
        <owl:allValuesFrom rdf:resource="http://www.w3.org/2001/XMLSchema#string"/>
        <owl:cardinality rdf:datatype="http://www.w3.org/2001/XMLSchema#nonNegativeInteger">1</owl:cardinality>
      </owl:Restriction>
    </rdfs:subClassOf>

    <rdfs:comment>Represents temporal aspects related to artwork, including:
            - Creation periods
            - Historical periods
            - Exhibition periods
            - Conservation periods
            - Depicted time periods
            - Time-based elements
            </rdfs:comment>
    <skos:example>
            - :renaissance_period rdf:type arto:Time ;
                sdo:startDate &quot;1400&quot; ;
                sdo:endDate &quot;1600&quot; .
                
            </skos:example>
    <rdfs:label>Time</rdfs:label>
  </owl:Class>

  <owl:Class rdf:about="http://w3id.org/arto#VisualElement">
    <rdfs:subClassOf>
      <owl:Class rdf:about="http://www.cidoc-crm.org/cidoc-crm/E26_Physical_Feature">
      </owl:Class>
    </rdfs:subClassOf>

    <rdfs:subClassOf>
      <owl:Restriction>
        <owl:onProperty rdf:resource="http://w3id.org/arto#hasMetric"/>
        <owl:allValuesFrom rdf:resource="http://w3id.org/arto#Metric"/>
      </owl:Restriction>
    </rdfs:subClassOf>

    <rdfs:subClassOf>
      <owl:Restriction>
        <owl:onProperty rdf:resource="http://w3id.org/arto#expresses"/>
        <owl:allValuesFrom rdf:resource="http://w3id.org/arto#Connotation"/>
      </owl:Restriction>
    </rdfs:subClassOf>

    <rdfs:subClassOf>
      <owl:Restriction>
        <owl:onProperty rdf:resource="http://w3id.org/arto#descriptor"/>
        <owl:allValuesFrom rdf:resource="http://www.w3.org/2001/XMLSchema#string"/>
      </owl:Restriction>
    </rdfs:subClassOf>

    <rdfs:comment>Represents the fundamental visual components of an artwork, including: lines and shapes, colors and textures, forms and patterns, space and perspective, light and shadow, etc.</rdfs:comment>
    <rdfs:label>Element</rdfs:label>
  </owl:Class>

  <owl:Class rdf:about="http://www.w3.org/2001/XMLSchema#dateTime">
  </owl:Class>

  <rdf:Description rdf:nodeID="genid135">
    <owl:minCardinality rdf:datatype="http://www.w3.org/2001/XMLSchema#nonNegativeInteger">1</owl:minCardinality>
  </rdf:Description>

  <rdf:Description rdf:nodeID="genid136">
    <owl:minCardinality rdf:datatype="http://www.w3.org/2001/XMLSchema#nonNegativeInteger">1</owl:minCardinality>
  </rdf:Description>

  <rdf:Description rdf:nodeID="genid137">
    <owl:minCardinality rdf:datatype="http://www.w3.org/2001/XMLSchema#nonNegativeInteger">1</owl:minCardinality>
  </rdf:Description>

  <rdf:Description rdf:nodeID="genid138">
    <owl:cardinality rdf:datatype="http://www.w3.org/2001/XMLSchema#nonNegativeInteger">1</owl:cardinality>
  </rdf:Description>

  <rdf:Description rdf:nodeID="genid139">
    <owl:maxCardinality rdf:datatype="http://www.w3.org/2001/XMLSchema#nonNegativeInteger">1</owl:maxCardinality>
  </rdf:Description>

  <rdf:Description rdf:nodeID="genid140">
    <owl:cardinality rdf:datatype="http://www.w3.org/2001/XMLSchema#nonNegativeInteger">1</owl:cardinality>
  </rdf:Description>

  <rdf:Description rdf:nodeID="genid141">
    <owl:cardinality rdf:datatype="http://www.w3.org/2001/XMLSchema#nonNegativeInteger">1</owl:cardinality>
  </rdf:Description>

  <rdf:Description rdf:nodeID="genid142">
    <owl:minCardinality rdf:datatype="http://www.w3.org/2001/XMLSchema#nonNegativeInteger">1</owl:minCardinality>
  </rdf:Description>

  <rdf:Description rdf:nodeID="genid143">
    <owl:cardinality rdf:datatype="http://www.w3.org/2001/XMLSchema#nonNegativeInteger">1</owl:cardinality>
  </rdf:Description>

  <rdf:Description rdf:nodeID="genid144">
    <owl:cardinality rdf:datatype="http://www.w3.org/2001/XMLSchema#nonNegativeInteger">1</owl:cardinality>
  </rdf:Description>

  <rdf:Description rdf:nodeID="genid145">
    <owl:cardinality rdf:datatype="http://www.w3.org/2001/XMLSchema#nonNegativeInteger">1</owl:cardinality>
  </rdf:Description>

</rdf:RDF>