@prefix : <http://w3id.org/arto#> .
@prefix cc: <http://creativecommons.org/ns#> .
@prefix crm: <http://www.cidoc-crm.org/cidoc-crm/> .
@prefix dc: <http://purl.org/dc/terms/> .
@prefix gn: <https://www.geonames.org/ontology#> .
@prefix dbo: <https://dbpedia.org/ontology/> .
@prefix dbp: <https://dbpedia.org/property/> .
@prefix edm: <http://www.europeana.eu/schemas/edm/> .
@prefix geo: <http://www.w3.org/2003/01/geo/wgs84_pos#> .
@prefix owl: <http://www.w3.org/2002/07/owl#> .
@prefix rdf: <http://www.w3.org/1999/02/22-rdf-syntax-ns#> .
@prefix sdo: <https://schema.org/> .
@prefix sem: <http://semanticweb.cs.vu.nl/2009/11/sem/> .
@prefix skos: <http://www.w3.org/2004/02/skos/core#> .
@prefix xml: <http://www.w3.org/XML/1998/namespace> .
@prefix xsd: <http://www.w3.org/2001/XMLSchema#> .
@prefix arto: <http://w3id.org/arto#> .
@prefix foaf: <http://xmlns.com/foaf/0.1/> .
@prefix rdfs: <http://www.w3.org/2000/01/rdf-schema#> .
@prefix vann: <http://purl.org/vocab/vann/> .
@prefix event: <http://purl.org/NET/c4dm/event.owl#> .
@prefix ebucore: <http://www.ebu.ch/metadata/ontologies/ebucore/ebucore#> .
@base <http://w3id.org/arto> .

<http://w3id.org/arto> rdf:type owl:Ontology ;
                         owl:versionIRI <http://w3id.org/arto/v0.1> ;
                         cc:attributionURL <httpå‘¢://w3id.org/arto> ;
                         dc:issued "2024-04-10" ;
                         dc:license <https://github.com/SocialMachineLab/ArtworkOntology/blob/main/License> ;
                         dc:title "Artwork Object Ontology"@en ;
                         vann:preferredNamespacePrefix "arto" ;
                         rdfs:label "Artwork Object Ontology (ARTO)"@en ;
                         owl:versionInfo "0.1"^^xsd:string .

#################################################################
#    Annotation properties
#################################################################

###  http://creativecommons.org/ns#attributionURL
cc:attributionURL rdf:type owl:AnnotationProperty .


###  http://purl.org/dc/terms/issued
dc:issued rdf:type owl:AnnotationProperty .


###  http://purl.org/dc/terms/license
dc:license rdf:type owl:AnnotationProperty .


###  http://purl.org/dc/terms/rights
dc:rights rdf:type owl:AnnotationProperty .


###  http://purl.org/dc/terms/title
dc:title rdf:type owl:AnnotationProperty .


###  http://purl.org/vocab/vann/preferredNamespacePrefix
vann:preferredNamespacePrefix rdf:type owl:AnnotationProperty .


#################################################################
#    Object Properties
#################################################################

###  http://purl.org/NET/c4dm/event.owl#agent
event:agent rdf:type owl:ObjectProperty ;
            rdfs:domain arto:Event ;
            rdfs:range foaf:Agent ;
            rdfs:comment """Relates an event to an agent (person or organization) associated with it.
            Example:
            - An acquisition event by a museum: :acquisition_2023 event:agent :metropolitan_museum""" ;
            rdfs:label "agent" .


###  http://w3id.org/arto#hasTime
arto:hasTime rdf:type owl:ObjectProperty ;
           rdfs:domain [ rdf:type owl:Class ;
                         owl:unionOf ( arto:Event
                                       arto:Location
                                     )
                       ] ;
           rdfs:range arto:Time ;
           rdfs:comment """Associates an event or location with its temporal information.
              Example:
              - Event timing: :exhibition2024 arto:hasTime :spring2024
              - Location historical period: :paris_studio arto:hasTime :belle_epoque
              """ ;
           rdfs:label "hasTime" .


###  http://purl.org/dc/terms/creator
dc:creator rdf:type owl:ObjectProperty ;
             rdfs:domain [ rdf:type owl:Class ;
                           owl:unionOf ( arto:Artwork
                                         arto:Series
                                       )
                         ] ;
             rdfs:range arto:Artist ;
             rdfs:comment """Relates an artwork or series to its primary creator(s). This property identifies the artist(s) who conceptualized and executed the work.
              Examples:
              - Single artist: :starry_night dc:creator :vincent_van_gogh
              - Multiple artists: :fountain dc:creator :marcel_duchamp, :alfred_stieglitz
              - Art series: :water_lilies_series dc:creator :claude_monet""" ;
             rdfs:label "creator" .


###  http://purl.org/dc/terms/contributor
dc:contributor rdf:type owl:ObjectProperty ;
               rdfs:domain arto:Artwork ;
               rdfs:range foaf:Agent ;
               rdfs:comment "The Contributor of the Artwork." ;
               rdfs:comment """Identifies contributors to an artwork who assisted in its creation or development. This may include studio assistants, technical advisors, collaborative participants or others.

                Examples:
                - Studio assistant: :sistine_chapel dc:contributor :workshop_assistant_giovanni
                - Technical advisor: :digital_installation dc:contributor :software_engineer_smith
                - Collaborative input: :performance_piece dc:contributor :sound_designer_jones""" ;
               rdfs:label "contributor" .


###  http://purl.org/dc/terms/created
dc:created rdf:type owl:ObjectProperty ;
           rdfs:domain arto:Artwork ;
           rdfs:range arto:Time ;
           rdfs:comment """Specifies the creation date or period of an artwork, which can be a specific date, year, or time range during which the work was produced.
            Examples:
            - Specific date: :mona_lisa dc:created :1503
            - Period range: :david_sculpture dc:created :1501_1504
            - Approximate date: :cave_painting dc:created :paleolithic_period""" ;
           rdfs:label "created" .


###  http://purl.org/dc/terms/isPartOf
dc:isPartOf rdf:type owl:ObjectProperty ;
            rdfs:domain arto:Artwork ;
            rdfs:range arto:Series ;
            rdfs:comment """Identifies an artwork as being part of a larger series or collection.

              Examples:
              - :water_lily_1919 dc:isPartOf :water_lilies_series
              - :sunflower_painting_1 dc:isPartOf :sunflowers_series""" ;
            rdfs:label "isPartOf" .


###  http://w3id.org/arto#containsElement
arto:containsElement rdf:type owl:ObjectProperty ;
                      rdfs:domain arto:Object ;
                      rdfs:range arto:VisualElement ;
                      rdfs:comment """Specifies the visual elements (such as color, line, composition) contained within an object in the artwork.

                      Examples:
                      - Color elements: :sky_object arto:containsElement :blue_gradient_color
                      - Line elements: :mountain_object arto:containsElement :diagonal_line
                      - Compositional elements: :tree_object arto:containsElement :vertical_composition""" ;
                      rdfs:subClassOf dc:hasPart ;
                      rdfs:label "containsElement" .


###  http://w3id.org/arto#containsObject
arto:containsObject rdf:type owl:ObjectProperty ;
                     rdfs:domain arto:Scene ;
                     rdfs:range arto:Object ;
                     rdfs:comment """Indicates specific objects that are present within a scene of an artwork.

                      Examples:
                      - Landscape scene: :garden_scene arto:containsObject :fountain, :bench, :flowers
                      - Portrait scene: :interior_scene arto:containsObject :chair, :table, :book
                      - Still life scene: :table_scene arto:containsObject :fruit_bowl, :wine_glass, :cloth""" ;
                     rdfs:subClassOf dc:hasPart ;
                     rdfs:label "containsObject" .


###  http://w3id.org/arto#containsScene
arto:containsScene rdf:type owl:ObjectProperty ;
                    rdfs:domain [ rdf:type owl:Class ;
                                  owl:unionOf ( arto:Artwork
                                                arto:Scene
                                              )
                                ] ;
                    rdfs:range arto:Scene ;
                    rdfs:comment """Identifies distinct scenes within an artwork or within another scene, allowing for hierarchical scene composition.
                      Examples:
                      - Nested scenes: :market_scene arto:containsScene :vendor_scene, :customer_scene
                      - Background scenes: :landscape_painting arto:containsScene :mountain_scene, :valley_scene""" ;
                    rdfs:subClassOf dc:hasPart ;
                    rdfs:label "containsScene" .


###  http://w3id.org/arto#express
arto:expresses rdf:type owl:ObjectProperty ;
             rdfs:domain [ rdf:type owl:Class ;
                           owl:unionOf ( arto:VisualElement
                                         arto:Object
                                         arto:Scene
                                       )
                         ] ;
             rdfs:range arto:Connotation ;
             rdfs:comment """Links visual elements, objects, or scenes to their symbolic meanings or emotional connotations.

              Examples:
              - Emotional expression: :red_color arto:expresses :anger_emotion
              - Symbolic meaning: :dove_object arto:expresses :peace_meaning
              - Scene mood: :storm_scene arto:expresses :turbulence_emotion""" ;
             rdfs:label "express" .


###  http://w3id.org/arto#hasConnotation
arto:hasConnotation rdf:type owl:ObjectProperty ;
                    rdfs:domain arto:Artwork ;
                    rdfs:range arto:Connotation ;
                    rdfs:comment """Associates an artwork with its broader meanings, themes, or emotional content.
                      Examples:
                      - Symbolic meaning: :guernica arto:hasConnotation :anti_war_theme """ ;
                    rdfs:label "hasConnotation" .


###  http://w3id.org/arto#hasEvent
arto:hasEvent rdf:type owl:ObjectProperty ;
              rdfs:domain arto:Artwork ;
              rdfs:range arto:Event ;
              rdfs:comment """Relates an artwork to significant events in its history, including creation, restoration, exhibition, or damage events.

                Examples:
                - Restoration: :mona_lisa arto:hasEvent :restoration_1956
                - Exhibition: :night_watch arto:hasEvent :rijksmuseum_exhibition_2024
                - Damage event: :the_kiss arto:hasEvent :vandalism_incident_1977""" ;
              rdfs:label "hasEvent" .


###  http://w3id.org/arto#hasMetric
arto:hasMetric rdf:type owl:ObjectProperty ;
               rdfs:domain [ rdf:type owl:Class ;
                             owl:unionOf ( arto:Connotation
                                           arto:VisualElement
                                           arto:Object
                                           arto:Scene
                                         )
                           ] ;
               rdfs:range arto:Metric ;
               rdfs:comment """Associates components (Connotation, Scene, Object or the Visual Element) of an artwork with quantifiable measurements or characteristics.

                Examples:
                - Color metrics: :sky_area arto:hasMetric :blue_intensity_75_percent
                - Composition balance: :landscape_scene arto:hasMetric :symmetry_score_0.8
                - Emotional intensity: :expression_scene arto:hasMetric :fear_intensity_high""" ;
               rdfs:label "hasMetric" .


###  http://w3id.org/arto#relatedTo
arto:relatedTo rdf:type owl:ObjectProperty ;
               rdfs:domain arto:Object ;
               rdfs:range arto:Object ;
               rdfs:comment """Describes spatial or conceptual relationships between objects within an artwork.
                Examples:
                - Spatial relation: :cup_object arto:relatedTo :table_object ;
                                  arto:relationType "rests_on"
                - Interaction: :mother_figure arto:relatedTo :child_figure ;
                              arto:relationType "holds"
                - Position: :cloud_object arto:relatedTo :mountain_object ;
                          arto:relationType "above" """ ;
               rdfs:label "relatedTo" .


###  http://w3id.org/arto#relatedToEvent
arto:relatedToEvent rdf:type owl:ObjectProperty ;
                    rdfs:domain [ rdf:type owl:Class ;
                                  owl:unionOf ( arto:Artwork
                                                arto:Connotation
                                              )
                                ] ;
                    rdfs:range arto:Event ;
                    rdfs:comment """Connects an artwork or its connotation to historical, mythological, or contemporary events depicted or referenced in the work.
                      Examples:
                      - Historical event: :liberty_leading_the_people arto:relatedToEvent :french_revolution_1830
                      - Biblical event: :last_supper arto:relatedToEvent :biblical_last_supper
                      """ ; 
                    rdfs:label "relatedToEvent" .


###  http://w3id.org/arto#relatedToScene
arto:relatedToScene rdf:type owl:ObjectProperty ;
                    rdfs:domain arto:Object ;
                    rdfs:range arto:Scene ;
                    rdfs:comment """Links objects to the scenes they appear in or are associated with.
                      Examples:
                      - Object context: :bread_loaf arto:relatedToScene :market_scene """ ;
                    rdfs:label "relatedToScene" .


###  http://w3id.org/arto#currentLocation
arto:currentLocation rdf:type owl:ObjectProperty ;
                    rdfs:domain arto:Artwork ;
                    rdfs:range arto:Location ;
                    rdfs:comment """Specifies the current physical location where an artwork is housed or displayed.

                      Examples:
                      - Museum location: :mona_lisa arto:currentLocation :louvre_museum
                      - Gallery location: :starry_night arto:currentLocation :moma_gallery_room_24
                      """ ; 
                    rdfs:label "currentLocation" ;
                    skos:closeMatch edm:currentLocation .


arto:hasLocation rdf:type owl:ObjectProperty ;
               rdfs:domain [ rdf:type owl:Class ;
                            owl:unionOf ( foaf:Organization arto:Event )
                          ] ;
               rdfs:range arto:Location ;
               rdfs:comment """Specifies the physical location of an organization or event related to the artwork.

                Examples:
                - Museum address: :metropolitan_museum arto:hasLocation :met_nyc_location
                - Gallery location: :tate_modern arto:hasLocation :london_bankside
                - Studio location: :warhol_factory arto:hasLocation :manhattan_location
                - Exhibition event: :venice_biennale_2024 arto:hasLocation :venice_giardini""" ;
               rdfs:label "hasLocation" .


###  http://xmlns.com/foaf/0.1/knows
foaf:knows rdf:type owl:ObjectProperty ;
           rdfs:domain foaf:Person ;
           rdfs:range foaf:Person ;
           rdfs:comment """The person knows persons.
            Examples:
            - Artist relationships: :vincent_van_gogh foaf:knows :paul_gauguin
            - Teacher-student: :gustav_klimt foaf:knows :egon_schiele
            - Collaborative artists: :pablo_picasso foaf:knows :georges_braque""" ;
           rdfs:label "knows" .


###  https://dbpedia.org/ontology/residence
dbo:residence rdf:type owl:ObjectProperty ;
              rdfs:domain foaf:Person ;
              rdfs:range arto:Location ;
              rdfs:comment """Indicates where a person (usually an artist) lived during specific periods.

                Examples:
                - Artist home: :claude_monet dbo:residence :giverny_house
                - Studio location: :andy_warhol dbo:residence :the_factory_nyc
                - Multiple residences: :pablo_picasso dbo:residence :paris_montmartre, :barcelona_gothic_quarter""" ;
              rdfs:label "residence" .



#################################################################
#    Data properties
#################################################################

###  http://www.ebu.ch/metadata/ontologies/ebucore/ebucore#dimensions
ebucore:dimensions rdf:type owl:DatatypeProperty ;
            rdfs:domain arto:Artwork ;
            rdfs:range xsd:string ;
            rdfs:comment "The dimension of the Artwork." ;
            rdfs:label "dimension" .


###  http://purl.org/dc/terms/title
dc:title rdf:type owl:DatatypeProperty ;
           rdfs:domain arto:Artwork ;
           rdfs:range xsd:string ;
           rdfs:comment "Relates an artwork to its title." ;
           rdfs:label "title" .


###  http://purl.org/dc/terms/description
dc:description rdf:type owl:DatatypeProperty ;
               rdfs:domain arto:Artwork ;
               rdfs:range xsd:string ;
               rdfs:comment "Relates an artwork to its description." ;
               rdfs:label "description" .


###  http://w3id.org/arto#locationType
arto:locationType rdf:type owl:DatatypeProperty ;
                rdfs:domain arto:Location ;
                rdfs:range xsd:string ;
                rdfs:comment """The type of the location. available options are: country, state, city, district,
      street, building etc. """ ;
                rdfs:label "locationType" .


###  http://purl.org/dc/terms/medium
dc:medium rdf:type owl:DatatypeProperty ;
          rdfs:domain arto:Artwork ;
          rdfs:range xsd:string ;
          rdfs:comment "Relates an artwork to the medium(s) used in creating it." ;
          rdfs:label "medium" .


###  http://semanticweb.cs.vu.nl/2009/11/sem/eventType
sem:eventType rdf:type owl:DatatypeProperty ;
              rdfs:domain arto:Event ;
              rdfs:range xsd:string ;
              rdfs:comment "The type of the event" ;
              rdfs:label "eventType" .


###  http://w3id.org/arto#HSVValue
arto:HSVValue rdf:type owl:DatatypeProperty ;
              rdfs:domain arto:Color ;
              rdfs:range xsd:string ;
              rdfs:comment "HSV color value in format 'H,S,V' where H is the hue and the range is 0-360, S is the saturation and the range is 0-100, and V is the value and the range is 0-100" ;
              rdfs:label "HSVValue" .


###  http://w3id.org/arto#RGBValue
arto:RGBValue rdf:type owl:DatatypeProperty ;
              rdfs:domain arto:Color ;
              rdfs:range xsd:string ;
              rdfs:comment "RGB color value in format 'R,G,B' where R,G,B are integers 0-255" ;
              rdfs:label "RGBValue" .


###  http://w3id.org/arto#compositionType
arto:compositionType rdf:type owl:DatatypeProperty ;
                     rdfs:domain arto:Composition ;
                     rdfs:range xsd:string ;
                     rdfs:comment """The type of the composition.  This includes:
                        - Basic composition types (triangular, circular, linear)
                        - Dynamic vs. static arrangements
                        - Symmetrical vs. asymmetrical balance
                        - Grid-based structures
                        - Rule of thirds applications
                        - Golden ratio compositions
                        - Hierarchical arrangements""" ;
                     rdfs:label "compositionType" .


###  http://w3id.org/arto#coordinates
arto:coordinates rdf:type owl:DatatypeProperty ;
                 rdfs:domain [ rdf:type owl:Class ;
                               owl:unionOf ( arto:Object
                                             arto:Scene
                                           )
                             ] ;
                 rdfs:range xsd:string ;
                 rdfs:comment "The coordinates of the Scene or the Object in the artwork." ;
                 rdfs:label "coordinates" .


###  http://w3id.org/arto#direction
arto:direction rdf:type owl:DatatypeProperty ;
               rdfs:domain arto:Line ;
               rdfs:range xsd:string ;
               rdfs:comment "Describes the orientation of linear elements in an artwork." ;
               rdfs:label "direction" .


###  http://w3id.org/arto#emotionType
arto:emotionType rdf:type owl:DatatypeProperty ;
                 rdfs:domain arto:Emotion ;
                 rdfs:range xsd:string ;
                 rdfs:comment "Point out the emotion type." ;
                 rdfs:label "emotionType" .


###  http://w3id.org/arto#state
arto:state rdf:type owl:DatatypeProperty ;
              rdfs:domain arto:Object ;
              rdfs:range xsd:string ;
              rdfs:comment "Describes the current condition, position, or status of objects within an artwork." ;
              rdfs:label "state" .


###  http://w3id.org/arto#length
arto:length rdf:type owl:DatatypeProperty ;
            rdfs:domain arto:Line ;
            rdfs:range xsd:float ;
            rdfs:comment "The length of the line." ;
            rdfs:label "length" .

###  https://schema.org/startDate
sdo:startDate rdf:type owl:DatatypeProperty ;
            rdfs:domain arto:Time ;
            rdfs:range xsd:dataTime ;
            rdfs:comment "The start date of a time entity." ;
            rdfs:label "startDate" .


###  https://schema.org/endDate
sdo:endDate rdf:type owl:DatatypeProperty ;
            rdfs:domain arto:Time ;
            rdfs:range xsd:dataTime ;
            rdfs:comment "The end date of a time entity." ;
            rdfs:label "endDate" .


###  http://w3id.org/arto#lineType
arto:lineType rdf:type owl:DatatypeProperty ;
              rdfs:domain arto:Line ;
              rdfs:range xsd:string ;
              rdfs:comment "The type of the line." ;
              rdfs:label "lineType" .


###  http://w3id.org/arto#originalTitle
arto:originalTitle rdf:type owl:DatatypeProperty ;
              rdfs:domain arto:Artwork ;
              rdfs:range xsd:string ;
              rdfs:comment "The original title of the artwork, potentially in its original language." ;
              rdfs:label "originalTitle" .



###  http://w3id.org/arto#material
arto:material rdf:type owl:DatatypeProperty ;
              rdfs:domain arto:Object ;
              rdfs:range xsd:string ;
              rdfs:comment "The material of the Object." ;
              rdfs:label "material" .


###  http://w3id.org/arto#size
arto:size rdf:type owl:DatatypeProperty ;
          rdfs:domain [ rdf:type owl:Class ;
                        owl:unionOf ( arto:Object
                                      arto:Scene
                                    )
                      ] ;
          rdfs:range xsd:string ;
          rdfs:comment "The size of the Scene or the Object in the artwork." ;
          rdfs:label "size" .


###  http://w3id.org/arto#source
arto:source rdf:type owl:DatatypeProperty ;
            rdfs:domain arto:Meaning ;
            rdfs:range xsd:string ;
            rdfs:comment "Relates the source of the meaning in artworks." ;
            rdfs:label "source" .


###  http://w3id.org/arto#spaceType
arto:spaceType rdf:type owl:DatatypeProperty ;
               rdfs:domain arto:Space ;
               rdfs:range xsd:string ;
               rdfs:comment "The type of the space." ;
               rdfs:label "spaceType" .


###  http://w3id.org/arto#timeType
arto:timeType rdf:type owl:DatatypeProperty ;
              rdfs:domain <http://www.w3.org/2006/time#TemporalEntity> ;
              rdfs:range xsd:string ;
              rdfs:comment "The type of the time entity." ;
              rdfs:label "timeType" .


###  http://www.ebu.ch/metadata/ontologies/ebucore/ebucore#height
ebucore:height rdf:type owl:DatatypeProperty ;
               rdfs:domain arto:Artwork ;
               rdfs:range xsd:string ;
               rdfs:comment "Relates an artwork to its physical height." ;
               rdfs:label "height" .


###  http://www.ebu.ch/metadata/ontologies/ebucore/ebucore#width
ebucore:width rdf:type owl:DatatypeProperty ;
              rdfs:domain [ rdf:type owl:Class ;
                            owl:unionOf ( arto:Artwork
                                          arto:Line
                                        )
                          ] ;
              rdfs:range xsd:string ;
              rdfs:comment "Relates an artwork to its physical width." ;
              rdfs:label "width" .


###  http://www.europeana.eu/schemas/edm/isShownBy
edm:isShownBy rdf:type owl:DatatypeProperty ;
              rdfs:domain arto:Artwork ;
              rdfs:range xsd:string ;
              rdfs:comment """An unambiguous URI reference to the digital object on the provider's web site in
      the best available resolution/quality. """ ;
              rdfs:label "isShownBy" .


###  http://www.w3.org/2003/01/geo/wgs84_pos#lat
geo:asWKT rdf:type owl:DatatypeProperty ;
        rdfs:domain arto:Location ;
        rdfs:range geo:wktLiteral ;
        rdfs:comment "Representing a geographical point using WKT format" ;
        rdfs:label "asWKT" .

###  https://dbpedia.org/ontology/nationality
dbo:nationality rdf:type owl:DatatypeProperty ;
                rdfs:domain foaf:Person ;
                rdfs:range xsd:string ;
                rdfs:comment "Relates an person to the Nationality." ;
                rdfs:label "nationality" .


###  https://dbpedia.org/property/style
dbp:style rdf:type owl:DatatypeProperty ;
          rdfs:domain arto:Artwork ;
          rdfs:range xsd:string ;
          rdfs:comment "Relates an artwork to its artistic style or movement." ;
          rdfs:label "style" .


###  https://schema.org/genre
sdo:genre rdf:type owl:DatatypeProperty ;
          rdfs:domain arto:Artwork ;
          rdfs:range xsd:string ;
          rdfs:comment "Relates an artwork to its genre." ;
          rdfs:label "genre" .


#################################################################
#    Classes
#################################################################

###  http://w3id.org/arto#Event
arto:Event rdf:type owl:Class ;
            rdfs:comment """
      An arbitrary classification of a space/time region, by a
      cognitive agent. An event may have actively participating agents,
      passive factors, products, and a location in space/time.""" ;
            rdfs:subClassOf event:Event ;
            rdfs:subClassOf sdo:Event ;
            skos:closeMatch crm:E5_Event ;
            rdfs:label "Event" .


###  http://w3id.org/arto#Location
arto:Location rdf:type owl:Class ;
            rdfs:comment "Represents a physical or virtual space associated with an artwork." ;
            rdfs:subClassOf dc:Location ;
            skos:closeMatch crm:E53_Place ;
            skos:closeMatch sdo:Place ;
            rdfs:label "Location" .


###  http://w3id.org/arto#Artist
arto:Artist rdf:type owl:Class ;
            rdfs:subClassOf foaf:Person ;
            rdfs:comment "The person or group who create or contribute the artwork." ;
            rdfs:label "Artist" .
            


###  http://w3id.org/arto#Artwork
arto:Artwork rdf:type owl:Class ;
             rdfs:comment """A created object or piece of art that is intended to be aesthetically pleasing or
                convey a message.
                """ ;
             rdfs:label "Artwork" ;
             skos:closeMatch crm:E22_Human_Made_Object ;
             rdfs:subClassOf sdo:CreativeWork .


###  http://w3id.org/arto#BalanceOfComposition
arto:BalanceOfComposition rdf:type owl:Class ;
                          rdfs:subClassOf arto:Metric ;
                          rdfs:comment """Represents the degree of visual equilibrium or harmony in the arrangement of
      elements within an artwork, considering factors such as symmetry, asymmetry, and distribution
      of
      visual elements.""" ;
                          rdfs:label "BalanceOfComposition" .


###  http://w3id.org/arto#Character
arto:Character rdf:type owl:Class ;
               rdfs:subClassOf foaf:Person ;
               rdfs:comment "Represents persons, figures, or beings depicted within an artwork." ;
               rdfs:label "Character" .
               


###  http://w3id.org/arto#Color
arto:Color rdf:type owl:Class ;
           rdfs:subClassOf arto:VisualElement ;
           rdfs:closeMatch sdo:Color ;
           rdfs:comment "The use of color in the artwork." ;
           rdfs:label "Color" .


###  http://w3id.org/arto#ColorHistogram
arto:ColorHistogram rdf:type owl:Class ;
                    rdfs:subClassOf arto:Metric ;
                    rdfs:comment """Represents the distribution of colors in an artwork, typically expressed as a
      histogram or a quantitative representation of the frequency or proportion of each color
      present in
      the artwork.""" ;
                    rdfs:label "ColorHistogram" .


###  http://w3id.org/arto#Composition
arto:Composition rdf:type owl:Class ;
                 rdfs:subClassOf arto:VisualElement ;
                 rdfs:comment "The arrangement and organization of visual elements." ;
                 rdfs:label "Composition" .


###  http://w3id.org/arto#Connotation
arto:Connotation rdf:type owl:Class ;
                 rdfs:comment """Represents the implied meanings of artwork, includeing themes, symbolic meanings, and
      emotions conveyed by an artwork.""" ;
                 rdfs:subClassOf crm:E28_Conceptual_Object ;
                 rdfs:label "Cnnotation" .


###  http://w3id.org/arto#Element
arto:VisualElement rdf:type owl:Class ;
             rdfs:comment "Represents the fundamental visual components of an artwork, including: lines and shapes, colors and textures, forms and patterns, space and perspective, light and shadow, etc." ;
             rdfs:subClassOf crm:E26_Physical_Feature ;
             rdfs:label "Element" .


###  http://w3id.org/arto#Emotion
arto:Emotion rdf:type owl:Class ;
             rdfs:subClassOf arto:Connotation ;
             rdfs:comment """Represents the emotional response or affective state evoked by an artwork in the
      artist or viewers, such as joy, sadness, anger, or fear.""" ;
             rdfs:label "Emotion" .


###  http://w3id.org/arto#EmotionIntensity
arto:EmotionIntensity rdf:type owl:Class ;
                      rdfs:subClassOf arto:Metric ;
                      rdfs:comment "Represents the strength or degree of emotional response evoked by an artwork." ;
                      rdfs:label "EmotionIntensity" .


###  http://w3id.org/arto#Line
arto:Line rdf:type owl:Class ;
          rdfs:subClassOf arto:VisualElement ;
          rdfs:comment """Represents linear elements in artwork, including their characteristics and functions:
            - Types of lines (straight, curved, implied)
            - Line qualities (thick, thin, broken, continuous)
            - Directional lines
            - Contour lines
            - Gestural lines
            - Structural lines""" ;
          rdfs:label "Line" .


###  http://w3id.org/arto#MainColor
arto:MainColor rdf:type owl:Class ;
               rdfs:subClassOf arto:Metric ;
               rdfs:comment """Represents the dominant or most prominent color in an artwork, which can be
      determined through visual analysis or color quantization techniques.""" ;
               rdfs:label "MainColor" .


###  http://w3id.org/arto#Meaning
arto:Meaning rdf:type owl:Class ;
             rdfs:subClassOf arto:Connotation ;
             rdfs:comment """Represents the underlying message, symbolism, or significance conveyed by an
      artwork.""" ;
             rdfs:label "Meaning" .


###  http://w3id.org/arto#Metric
arto:Metric rdf:type owl:Class ;
            rdfs:comment """Represents a quantifiable measurement or characteristic of an artwork,
      encompassing statistical information about basic elements such as color statistics, emotion
      intensity, balance of composition, and other visual elements, to facilitate structural
      analysis
      and comparison of artworks.""" ;
            rdfs:label "Metric" .


###  http://w3id.org/arto#Object
arto:Object rdf:type owl:Class ;
            rdfs:comment "Represents the physical or conceptual object within an artwork." ;
            rdfs:label "Object" .


###  http://w3id.org/arto#Painting
arto:Painting rdf:type owl:Class ;
              rdfs:subClassOf arto:Artwork ;
              rdfs:comment """A specific type of artwork created using paint or similar media. """ ;
              rdfs:label "Painting" .


###  http://w3id.org/arto#Relevance
arto:Relevance rdf:type owl:Class ;
               rdfs:subClassOf arto:Metric ;
               rdfs:comment """Measures and describes the significance or importance of elements within an artwork, including:
                  - Thematic relevance
                  - Visual importance
                  - Symbolic significance
                  - Narrative relevance
                  - Historical relevance
                  - Compositional importance""" ;
               rdfs:label "Relevance" .


###  http://w3id.org/arto#Scene
arto:Scene rdf:type owl:Class ;
           rdfs:comment """Represents a distinct portion or area of an artwork that forms a coherent visual or narrative unit. """ ;
           rdfs:label "Scene" .


###  http://w3id.org/arto#Series
arto:Series rdf:type owl:Class ;
            rdfs:comment """A collection of related artworks that share common characteristics, themes, or purposes, including:
                - Thematic series
                - Chronological series
                - Technique-based series
                - Subject-based series
                - Experimental series
                - Documentary series""" ;
            rdfs:label "Series" ;
            skos:closeMatch crm:E78_Collection ;
            rdfs:subClassOf sdo:CreativeWorkSeries .



###  http://w3id.org/arto#Space
arto:Space rdf:type owl:Class ;
           rdfs:subClassOf arto:VisualElement ;
           rdfs:comment "Represents the spatial elements and relationships within an artwork." ;
           rdfs:label "Space" .


###  http://w3id.org/arto#Sponsor
arto:Sponsor rdf:type owl:Class ;
             rdfs:subClassOf foaf:Person ;
             rdfs:comment "The person or group who sponsor the artwork." ;
             rdfs:label "Sponsor" .


###  http://w3id.org/arto#Theme
arto:Theme rdf:type owl:Class ;
           rdfs:subClassOf arto:Connotation ;
           rdfs:comment """Represents a central idea, subject, or concept explored in an artwork, which can
      be explicit or implicit, and may reflect broader cultural, social, or political issues.""" ;
           rdfs:label "Theme" .


###  http://w3id.org/arto#Time
arto:Time rdf:type owl:Class ;
          rdfs:comment """Represents temporal aspects related to artwork, including:
            - Creation periods
            - Historical periods
            - Exhibition periods
            - Conservation periods
            - Depicted time periods
            - Time-based elements

            Examples:
            - :renaissance_period rdf:type arto:Time ;
                arto:startDate "1400" ;
                arto:endDate "1600" ;
                arto:culturalPeriod "European_Renaissance"
            """ ;
          owl:equivalentClass <http://www.w3.org/2006/time#TemporalEntity> ;
          rdfs:label "Time" .


###  http://xmlns.com/foaf/0.1/Agent
foaf:Agent rdf:type owl:Class ;
           rdfs:comment """Represents an Agent.This class comprises people, either individually or in groups,
      who have the potential to perform intentional actions for which they can be held responsible.""" ;
           rdfs:label "Agent" .


###  http://xmlns.com/foaf/0.1/Organization
foaf:Organization rdf:type owl:Class ;
                  rdfs:subClassOf foaf:Agent ;
                  owl:disjointWith foaf:Person ;
                  rdfs:comment """The Organization class represents a kind of Agent corresponding to instititutions
      such as galleries, museums etc.""" ;
                  rdfs:label "Organization" .


###  http://xmlns.com/foaf/0.1/Person
foaf:Person rdf:type owl:Class ;
            rdfs:subClassOf foaf:Agent ;
            owl:equivalentClass crm:E21_Person ;
            rdfs:comment """Individual human beings involved with artwork may include artists, curators, critics, collectors, conservators, researchers, and other roles.""" ;
            rdfs:label "Person" .


#################################################################
#    Individuals
#################################################################

###  http://w3id.org/arto
<http://w3id.org/arto> rdf:type owl:NamedIndividual ;
                        dc:description "The Artwork Object Ontology (ARTO) is a comprehensive ontology designed for describing and contextualizing artworks. It consists of two main components: the Artwork Descriptive Model and the Artwork Contextual Model. ARTO aims to provide a structured and detailed representation of artworks, facilitating tasks such as artwork captioning and information retrieval."@en .


###  Generated by the OWL API (version 4.5.9.2019-02-01T07:24:44Z) https://github.com/owlcs/owlapi
